@prefix : <https://w3id.org/gcdfo/salmon#> .
@prefix oa: <http://www.w3.org/ns/oa#> .
@prefix bfo: <http://purl.obolibrary.org/obo/BFO_> .
@prefix dqv: <http://www.w3.org/ns/dqv#> .
@prefix dwc: <http://rs.tdwg.org/dwc/terms/> .
@prefix iao: <http://purl.obolibrary.org/obo/IAO_> .
@prefix iop: <https://w3id.org/iadopt/ont/> .
@prefix odo: <http://purl.dataone.org/odo/> .
@prefix org: <http://www.w3.org/ns/org#> .
@prefix owl: <http://www.w3.org/2002/07/owl#> .
@prefix rdf: <http://www.w3.org/1999/02/22-rdf-syntax-ns#> .
@prefix xml: <http://www.w3.org/XML/1998/namespace> .
@prefix xsd: <http://www.w3.org/2001/XMLSchema#> .
@prefix envo: <http://purl.obolibrary.org/obo/ENVO_> .
@prefix prov: <http://www.w3.org/ns/prov#> .
@prefix qudt: <http://qudt.org/schema/qudt/> .
@prefix rdfs: <http://www.w3.org/2000/01/rdf-schema#> .
@prefix skos: <http://www.w3.org/2004/02/skos/core#> .
@prefix sosa: <http://www.w3.org/ns/sosa/> .
@prefix unit: <http://qudt.org/vocab/unit/> .
@prefix vann: <http://purl.org/vocab/vann/> .
@prefix gcdfo: <https://w3id.org/gcdfo/salmon#> .
@prefix dwciri: <http://rs.tdwg.org/dwc/iri/> .
@prefix schema: <https://schema.org/> .
@prefix dcterms: <http://purl.org/dc/terms/> .
@prefix qudtunit: <http://qudt.org/vocab/unit/> .
@base <https://w3id.org/gcdfo/salmon> .

<https://w3id.org/gcdfo/salmon> rdf:type owl:Ontology ;
                                 owl:versionIRI <https://w3id.org/gcdfo/salmon/0.0.6-alpha> ;
                                 <http://purl.obolibrary.org/obo/IAO_0000115> "Hybrid OWL+SKOS ontology for DFO salmon data. Uses SKOS for controlled vocabularies (methods, criteria) and OWL for formal relationships and events."@en ;
                                 dcterms:contributor "Brett Johnson"@en ,
                                                     "Melissa K. Morrison"@en ;
                                 dcterms:created "2025-09-06"^^xsd:date ;
                                 dcterms:creator "Fishery & Assessment Data Section (FADS) Data Stewardship Unit"@en ;
                                 dcterms:description "OWL + SKOS ontology for DFO salmon data: stocks/CUs/MUs, survey events, escapement measurements, and GSI constructs; aligns to DwC via rdfs:subClassOf; hybrid approach with SKOS for methods and OWL for events."@en ;
                                 dcterms:license <https://creativecommons.org/licenses/by/4.0/> ;
                                 dcterms:modified "2026-02-24"^^xsd:date ;
                                 dcterms:publisher "Fisheries and Oceans Canada (DFO) Pacific Region Science Branch"@en ;
                                 dcterms:title "DFO Salmon Ontology"@en ;
                                 vann:preferredNamespacePrefix "gcdfo" ;
                                 vann:preferredNamespaceUri "https://w3id.org/gcdfo/salmon#" ;
                                 rdfs:seeAlso <https://github.com/dfo-pacific-science/dfo-salmon-ontology> ;
                                 owl:priorVersion <https://w3id.org/gcdfo/salmon/0.0.2> ;
                                 owl:versionInfo "0.0.6-alpha (integrated pre-release review branch)" ;
                                 schema:codeRepository <https://github.com/dfo-pacific-science/dfo-salmon-ontology> .

#################################################################
#    Annotation properties
#################################################################

###  http://purl.obolibrary.org/obo/IAO_0000115
<http://purl.obolibrary.org/obo/IAO_0000115> rdf:type owl:AnnotationProperty ;
                                             rdfs:isDefinedBy <http://purl.obolibrary.org/obo/iao.owl> ;
                                             rdfs:label "definition"@en .


###  http://purl.obolibrary.org/obo/IAO_0000119
<http://purl.obolibrary.org/obo/IAO_0000119> rdf:type owl:AnnotationProperty ;
                                             rdfs:isDefinedBy <http://purl.obolibrary.org/obo/iao.owl> ;
                                             rdfs:label "definition source"@en .


###  http://purl.org/dc/terms/contributor
dcterms:contributor rdf:type owl:AnnotationProperty .


###  http://purl.org/dc/terms/created
dcterms:created rdf:type owl:AnnotationProperty .


###  http://purl.org/dc/terms/creator
dcterms:creator rdf:type owl:AnnotationProperty .


###  http://purl.org/dc/terms/description
dcterms:description rdf:type owl:AnnotationProperty .


###  http://purl.org/dc/terms/identifier
dcterms:identifier rdf:type owl:AnnotationProperty .


###  http://purl.org/dc/terms/isPartOf
dcterms:isPartOf rdf:type owl:AnnotationProperty .


###  http://purl.org/dc/terms/isVersionOf
dcterms:isVersionOf rdf:type owl:AnnotationProperty .


###  http://purl.org/dc/terms/license
dcterms:license rdf:type owl:AnnotationProperty .


###  http://purl.org/dc/terms/modified
dcterms:modified rdf:type owl:AnnotationProperty .


###  http://purl.org/dc/terms/publisher
dcterms:publisher rdf:type owl:AnnotationProperty .


###  http://purl.org/dc/terms/source
dcterms:source rdf:type owl:AnnotationProperty .


###  http://purl.org/dc/terms/title
dcterms:title rdf:type owl:AnnotationProperty .


###  http://purl.org/vocab/vann/preferredNamespacePrefix
vann:preferredNamespacePrefix rdf:type owl:AnnotationProperty .


###  http://purl.org/vocab/vann/preferredNamespaceUri
vann:preferredNamespaceUri rdf:type owl:AnnotationProperty .


###  http://www.w3.org/2004/02/skos/core#altLabel
skos:altLabel rdf:type owl:AnnotationProperty .


###  http://www.w3.org/2004/02/skos/core#broader
skos:broader rdf:type owl:AnnotationProperty .


###  http://www.w3.org/2004/02/skos/core#closeMatch
skos:closeMatch rdf:type owl:AnnotationProperty .


###  http://www.w3.org/2004/02/skos/core#definition
skos:definition rdf:type owl:AnnotationProperty .


###  http://www.w3.org/2004/02/skos/core#exactMatch
skos:exactMatch rdf:type owl:AnnotationProperty .


###  http://www.w3.org/2004/02/skos/core#hasTopConcept
skos:hasTopConcept rdf:type owl:AnnotationProperty .


###  http://www.w3.org/2004/02/skos/core#inScheme
skos:inScheme rdf:type owl:AnnotationProperty .


###  http://www.w3.org/2004/02/skos/core#notation
skos:notation rdf:type owl:AnnotationProperty .


###  http://www.w3.org/2004/02/skos/core#prefLabel
skos:prefLabel rdf:type owl:AnnotationProperty .


###  http://www.w3.org/2004/02/skos/core#scopeNote
skos:scopeNote rdf:type owl:AnnotationProperty .


###  https://schema.org/codeRepository
schema:codeRepository rdf:type owl:AnnotationProperty .


###  https://w3id.org/gcdfo/salmon#theme
gcdfo:theme rdf:type owl:AnnotationProperty ;
            rdfs:comment "Associates OWL classes and SKOS concepts with high-level thematic concept schemes (e.g., Stock Assessment, GSI, Policy)."@en ;
            rdfs:isDefinedBy <https://w3id.org/gcdfo/salmon> ;
            rdfs:label "theme"@en ;
            gcdfo:theme gcdfo:DataModelProvenanceTheme .


#################################################################
#    Datatypes
#################################################################

###  http://www.w3.org/2001/XMLSchema#anyURI
xsd:anyURI rdf:type rdfs:Datatype .


###  http://www.w3.org/2001/XMLSchema#boolean
xsd:boolean rdf:type rdfs:Datatype .


###  http://www.w3.org/2001/XMLSchema#date
xsd:date rdf:type rdfs:Datatype .


###  http://www.w3.org/2001/XMLSchema#dateTime
xsd:dateTime rdf:type rdfs:Datatype .


###  http://www.w3.org/2001/XMLSchema#decimal
xsd:decimal rdf:type rdfs:Datatype .


###  http://www.w3.org/2001/XMLSchema#gYear
xsd:gYear rdf:type rdfs:Datatype .


###  http://www.w3.org/2001/XMLSchema#integer
xsd:integer rdf:type rdfs:Datatype .


###  http://www.w3.org/2001/XMLSchema#string
xsd:string rdf:type rdfs:Datatype .


#################################################################
#    Object Properties
#################################################################

###  http://www.w3.org/ns/dqv#inDimension
dqv:inDimension rdf:type owl:ObjectProperty ;
                <http://purl.obolibrary.org/obo/IAO_0000115> "Represents the dimensions a quality metric, certificate and annotation allow a measurement of."@en ;
                <http://purl.obolibrary.org/obo/IAO_0000119> <https://www.w3.org/TR/vocab-dqv/> ;
                rdfs:comment "Dimensions are meant to systematically organize metrics, quality certificates and quality annotations. The Data Quality Vocabulary defines no specific cardinality constraints for dqv:inDimension, since distinct quality frameworks might have different perspectives over a metric. A metric may therefore be associated to more than one dimension. However, those who define new quality metrics should try to avoid this as much as possible and assign only one dimension to the metrics they define. More than one dimension can be indicated for each quality annotation or certificate."@en ;
                rdfs:isDefinedBy dqv: ;
                rdfs:label "in dimension"@en .


###  http://www.w3.org/ns/prov#generated
prov:generated rdf:type owl:ObjectProperty .


###  http://www.w3.org/ns/prov#used
prov:used rdf:type owl:ObjectProperty .


###  http://www.w3.org/ns/prov#wasDerivedFrom
prov:wasDerivedFrom rdf:type owl:ObjectProperty .


###  https://w3id.org/gcdfo/salmon#conservationUnitOf
gcdfo:conservationUnitOf rdf:type owl:ObjectProperty ;
                         owl:inverseOf gcdfo:hasConservationUnit ;
                         rdfs:domain gcdfo:ConservationUnit ;
                         rdfs:range gcdfo:StockManagementUnit ;
                         <http://purl.obolibrary.org/obo/IAO_0000115> "Relates a Conservation Unit to the Stock Management Unit it belongs to."@en ;
                         rdfs:isDefinedBy <https://w3id.org/gcdfo/salmon> ;
                         rdfs:label "Conservation Unit of"@en ;
                         gcdfo:theme gcdfo:FisheriesManagementTheme ,
                                     gcdfo:PolicyGovernanceTheme ,
                                     gcdfo:WildSalmonPolicyTheme .


###  https://w3id.org/gcdfo/salmon#demeOf
gcdfo:demeOf rdf:type owl:ObjectProperty ;
             owl:inverseOf gcdfo:hasDeme ;
             rdfs:domain gcdfo:Deme ;
             rdfs:range gcdfo:Population ;
             <http://purl.obolibrary.org/obo/IAO_0000115> "Relates a deme to the population it belongs to."@en ;
             rdfs:isDefinedBy <https://w3id.org/gcdfo/salmon> ;
             rdfs:label "deme of"@en ;
             gcdfo:theme gcdfo:GeneticsStockCompositionTheme ,
                         gcdfo:WildSalmonPolicyTheme .


###  https://w3id.org/gcdfo/salmon#hasConservationUnit
gcdfo:hasConservationUnit rdf:type owl:ObjectProperty ;
                          rdfs:domain gcdfo:StockManagementUnit ;
                          rdfs:range gcdfo:ConservationUnit ;
                          <http://purl.obolibrary.org/obo/IAO_0000115> "Relates a Stock Management Unit to one of its constituent Conservation Units."@en ;
                          rdfs:isDefinedBy <https://w3id.org/gcdfo/salmon> ;
                          rdfs:label "has Conservation Unit"@en ;
                          gcdfo:theme gcdfo:FisheriesManagementTheme ,
                                      gcdfo:PolicyGovernanceTheme ,
                                      gcdfo:WildSalmonPolicyTheme .


###  https://w3id.org/gcdfo/salmon#hasDeme
gcdfo:hasDeme rdf:type owl:ObjectProperty ;
              rdfs:domain gcdfo:Population ;
              rdfs:range gcdfo:Deme ;
              <http://purl.obolibrary.org/obo/IAO_0000115> "Relates a population to one of its constituent demes."@en ;
              rdfs:isDefinedBy <https://w3id.org/gcdfo/salmon> ;
              rdfs:label "has deme"@en ;
              gcdfo:theme gcdfo:GeneticsStockCompositionTheme ,
                          gcdfo:WildSalmonPolicyTheme .


###  https://w3id.org/gcdfo/salmon#hasFeatureOfInterest
gcdfo:hasFeatureOfInterest rdf:type owl:ObjectProperty ;
                           rdfs:subPropertyOf prov:used ;
                           rdfs:domain gcdfo:SurveyEvent ;
                           rdfs:range gcdfo:ReportingOrManagementStratum ;
                           <http://purl.obolibrary.org/obo/IAO_0000115> "Relates a survey event to the reporting or management stratum that the event targets for inference or status interpretation."@en ;
                           rdfs:isDefinedBy <https://w3id.org/gcdfo/salmon> ;
                           rdfs:label "has feature of interest"@en ;
                           skos:closeMatch sosa:hasFeatureOfInterest ;
                           gcdfo:theme gcdfo:DataModelProvenanceTheme ,
                                       gcdfo:PolicyGovernanceTheme ,
                                       gcdfo:StockAssessmentTheme .


###  https://w3id.org/gcdfo/salmon#hasObservationResult
gcdfo:hasObservationResult rdf:type owl:ObjectProperty ;
                           rdfs:subPropertyOf prov:generated ;
                           rdfs:domain gcdfo:SurveyEvent ;
                           rdfs:range gcdfo:EscapementMeasurement ;
                           <http://purl.obolibrary.org/obo/IAO_0000115> "Relates a survey event to a measurement datum/result it produces for salmon assessment workflows."@en ;
                           rdfs:isDefinedBy <https://w3id.org/gcdfo/salmon> ;
                           rdfs:label "has observation result"@en ;
                           skos:closeMatch sosa:hasResult ;
                           gcdfo:theme gcdfo:DataModelProvenanceTheme ,
                                       gcdfo:StockAssessmentTheme .


###  https://w3id.org/gcdfo/salmon#hasObservedVariable
gcdfo:hasObservedVariable rdf:type owl:ObjectProperty ;
                          rdfs:domain gcdfo:SurveyEvent ;
                          rdfs:range gcdfo:SalmonDataVariable ;
                          <http://purl.obolibrary.org/obo/IAO_0000115> "Relates a survey event to a salmon data variable specification that defines what was measured or derived."@en ;
                          rdfs:isDefinedBy <https://w3id.org/gcdfo/salmon> ;
                          rdfs:label "has observed variable"@en ;
                          skos:closeMatch sosa:observedProperty ;
                          gcdfo:theme gcdfo:DataModelProvenanceTheme ,
                                      gcdfo:StockAssessmentTheme .


###  https://w3id.org/gcdfo/salmon#hasPopulation
gcdfo:hasPopulation rdf:type owl:ObjectProperty ;
                    owl:inverseOf gcdfo:populationOf ;
                    rdfs:domain gcdfo:ConservationUnit ;
                    rdfs:range gcdfo:Population ;
                    <http://purl.obolibrary.org/obo/IAO_0000115> "Relates a Conservation Unit to one of its constituent populations."@en ;
                    rdfs:isDefinedBy <https://w3id.org/gcdfo/salmon> ;
                    rdfs:label "has population"@en ;
                    gcdfo:theme gcdfo:StockAssessmentTheme ,
                                gcdfo:WildSalmonPolicyTheme .


###  https://w3id.org/gcdfo/salmon#hasTargetOrLimitExploitationRate
gcdfo:hasTargetOrLimitExploitationRate rdf:type owl:ObjectProperty ;
                                       owl:inverseOf gcdfo:isTargetOrLimitForObservedExploitationRate ;
                                       rdfs:domain gcdfo:ObservedExploitationRate ;
                                       rdfs:range gcdfo:TargetOrLimitExploitationRate ;
                                       <http://purl.obolibrary.org/obo/IAO_0000115> "Relates an observed exploitation-rate estimate to the target, threshold, or limit exploitation-rate value used to evaluate it."@en ;
                                       rdfs:isDefinedBy <https://w3id.org/gcdfo/salmon> ;
                                       rdfs:label "has target or limit exploitation rate"@en ;
                                       gcdfo:theme gcdfo:FisheriesManagementTheme ,
                                                   gcdfo:PolicyGovernanceTheme ,
                                                   gcdfo:StockAssessmentTheme .


###  https://w3id.org/gcdfo/salmon#hasYearBasis
gcdfo:hasYearBasis rdf:type owl:ObjectProperty ;
                   rdfs:domain [ rdf:type owl:Class ;
                                 owl:unionOf ( gcdfo:EscapementMeasurement
                                               gcdfo:ExploitationRate
                                               gcdfo:ObservedExploitationRate
                                               gcdfo:SpawnerAbundance
                                               gcdfo:TargetOrLimitExploitationRate
                                               gcdfo:TotalExploitationRate
                                             )
                               ] ;
                   rdfs:range [ rdf:type owl:Class ;
                                owl:unionOf ( gcdfo:BroodYear
                                              gcdfo:CatchYear
                                              gcdfo:ReturnYear
                                            )
                              ] ;
                   <http://purl.obolibrary.org/obo/IAO_0000115> "Links a measurement or rate to the year basis (e.g., brood year, catch year, or return year) it is reported against."@en ;
                   rdfs:isDefinedBy <https://w3id.org/gcdfo/salmon> ;
                   rdfs:label "has year basis"@en ;
                   gcdfo:theme gcdfo:DataModelProvenanceTheme ,
                               gcdfo:StockAssessmentTheme .


###  https://w3id.org/gcdfo/salmon#isSampleOfStratum
gcdfo:isSampleOfStratum rdf:type owl:ObjectProperty ;
                        rdfs:subPropertyOf prov:wasDerivedFrom ;
                        rdfs:domain dwc:MaterialEntity ;
                        rdfs:range gcdfo:ReportingOrManagementStratum ;
                        <http://purl.obolibrary.org/obo/IAO_0000115> "Relates a material sample to the reporting or management stratum it is taken to represent in analysis."@en ;
                        rdfs:isDefinedBy <https://w3id.org/gcdfo/salmon> ;
                        rdfs:label "is sample of stratum"@en ;
                        skos:closeMatch sosa:isSampleOf ;
                        gcdfo:theme gcdfo:DataModelProvenanceTheme ,
                                    gcdfo:PolicyGovernanceTheme ,
                                    gcdfo:StockAssessmentTheme .


###  https://w3id.org/gcdfo/salmon#isTargetOrLimitForObservedExploitationRate
gcdfo:isTargetOrLimitForObservedExploitationRate rdf:type owl:ObjectProperty ;
                                                 rdfs:domain gcdfo:TargetOrLimitExploitationRate ;
                                                 rdfs:range gcdfo:ObservedExploitationRate ;
                                                 <http://purl.obolibrary.org/obo/IAO_0000115> "Relates a target, threshold, or limit exploitation-rate value to the observed exploitation-rate estimate it evaluates."@en ;
                                                 rdfs:isDefinedBy <https://w3id.org/gcdfo/salmon> ;
                                                 rdfs:label "is target or limit for observed exploitation rate"@en ;
                                                 gcdfo:theme gcdfo:FisheriesManagementTheme ,
                                                             gcdfo:PolicyGovernanceTheme ,
                                                             gcdfo:StockAssessmentTheme .


###  https://w3id.org/gcdfo/salmon#populationOf
gcdfo:populationOf rdf:type owl:ObjectProperty ;
                   rdfs:domain gcdfo:Population ;
                   rdfs:range gcdfo:ConservationUnit ;
                   <http://purl.obolibrary.org/obo/IAO_0000115> "Relates a population to the Conservation Unit it belongs to."@en ;
                   rdfs:isDefinedBy <https://w3id.org/gcdfo/salmon> ;
                   rdfs:label "population of"@en ;
                   gcdfo:theme gcdfo:StockAssessmentTheme ,
                               gcdfo:WildSalmonPolicyTheme .


###  https://w3id.org/gcdfo/salmon#usesObservationProcedure
gcdfo:usesObservationProcedure rdf:type owl:ObjectProperty ;
                               rdfs:domain gcdfo:SurveyEvent ;
                               rdfs:range <http://purl.obolibrary.org/obo/IAO_0000104> ;
                               <http://purl.obolibrary.org/obo/IAO_0000115> "Relates a survey event to the procedure/protocol used to execute it."@en ;
                               rdfs:isDefinedBy <https://w3id.org/gcdfo/salmon> ;
                               rdfs:label "uses observation procedure"@en ;
                               skos:closeMatch sosa:usedProcedure ;
                               gcdfo:theme gcdfo:DataModelProvenanceTheme ,
                                           gcdfo:StockAssessmentTheme .


###  https://w3id.org/gcdfo/salmon#variableHasConstraint
gcdfo:variableHasConstraint rdf:type owl:ObjectProperty ;
                            rdfs:subPropertyOf iop:hasConstraint ;
                            rdfs:domain gcdfo:SalmonDataVariable ;
                            rdfs:range iop:Constraint ;
                            <http://purl.obolibrary.org/obo/IAO_0000115> "Relates a salmon data variable to an optional constraint component in I-ADOPT decomposition."@en ;
                            rdfs:isDefinedBy <https://w3id.org/gcdfo/salmon> ;
                            rdfs:label "variable has constraint"@en ;
                            gcdfo:theme gcdfo:DataModelProvenanceTheme ,
                                        gcdfo:StockAssessmentTheme .


###  https://w3id.org/gcdfo/salmon#variableHasContextObject
gcdfo:variableHasContextObject rdf:type owl:ObjectProperty ;
                               rdfs:subPropertyOf iop:hasContextObject ;
                               rdfs:domain gcdfo:SalmonDataVariable ;
                               rdfs:range iop:Entity ;
                               <http://purl.obolibrary.org/obo/IAO_0000115> "Relates a salmon data variable to an optional context object/entity component in I-ADOPT decomposition."@en ;
                               rdfs:isDefinedBy <https://w3id.org/gcdfo/salmon> ;
                               rdfs:label "variable has context object"@en ;
                               gcdfo:theme gcdfo:DataModelProvenanceTheme ,
                                           gcdfo:StockAssessmentTheme .


###  https://w3id.org/gcdfo/salmon#variableHasMatrix
gcdfo:variableHasMatrix rdf:type owl:ObjectProperty ;
                        rdfs:subPropertyOf iop:hasMatrix ;
                        rdfs:domain gcdfo:SalmonDataVariable ;
                        rdfs:range iop:Entity ;
                        <http://purl.obolibrary.org/obo/IAO_0000115> "Relates a salmon data variable to an optional matrix/context entity component in I-ADOPT decomposition."@en ;
                        rdfs:isDefinedBy <https://w3id.org/gcdfo/salmon> ;
                        rdfs:label "variable has matrix"@en ;
                        gcdfo:theme gcdfo:DataModelProvenanceTheme ,
                                    gcdfo:StockAssessmentTheme .


###  https://w3id.org/gcdfo/salmon#variableHasObjectOfInterest
gcdfo:variableHasObjectOfInterest rdf:type owl:ObjectProperty ;
                                  rdfs:subPropertyOf iop:hasObjectOfInterest ;
                                  rdfs:domain gcdfo:SalmonDataVariable ;
                                  rdfs:range iop:Entity ;
                                  <http://purl.obolibrary.org/obo/IAO_0000115> "Relates a salmon data variable to the entity/object-of-interest component in I-ADOPT decomposition."@en ;
                                  rdfs:isDefinedBy <https://w3id.org/gcdfo/salmon> ;
                                  rdfs:label "variable has object of interest"@en ;
                                  gcdfo:theme gcdfo:DataModelProvenanceTheme ,
                                              gcdfo:StockAssessmentTheme .


###  https://w3id.org/gcdfo/salmon#variableHasProperty
gcdfo:variableHasProperty rdf:type owl:ObjectProperty ;
                          rdfs:subPropertyOf iop:hasProperty ;
                          rdfs:domain gcdfo:SalmonDataVariable ;
                          rdfs:range iop:Property ;
                          <http://purl.obolibrary.org/obo/IAO_0000115> "Relates a salmon data variable to the measured/estimated property component in I-ADOPT decomposition."@en ;
                          rdfs:isDefinedBy <https://w3id.org/gcdfo/salmon> ;
                          rdfs:label "variable has property"@en ;
                          gcdfo:theme gcdfo:DataModelProvenanceTheme ,
                                      gcdfo:StockAssessmentTheme .


###  https://w3id.org/gcdfo/salmon#variableHasStatisticalModifier
gcdfo:variableHasStatisticalModifier rdf:type owl:ObjectProperty ;
                                     rdfs:subPropertyOf iop:hasStatisticalModifier ;
                                     rdfs:domain gcdfo:SalmonDataVariable ;
                                     rdfs:range iop:StatisticalModifier ;
                                     <http://purl.obolibrary.org/obo/IAO_0000115> "Relates a salmon data variable to an optional statistical modifier component in I-ADOPT decomposition."@en ;
                                     rdfs:isDefinedBy <https://w3id.org/gcdfo/salmon> ;
                                     rdfs:label "variable has statistical modifier"@en ;
                                     gcdfo:theme gcdfo:DataModelProvenanceTheme ,
                                                 gcdfo:StockAssessmentTheme .


###  https://w3id.org/iadopt/ont/hasConstraint
iop:hasConstraint rdf:type owl:ObjectProperty .


###  https://w3id.org/iadopt/ont/hasContextObject
iop:hasContextObject rdf:type owl:ObjectProperty .


###  https://w3id.org/iadopt/ont/hasMatrix
iop:hasMatrix rdf:type owl:ObjectProperty .


###  https://w3id.org/iadopt/ont/hasObjectOfInterest
iop:hasObjectOfInterest rdf:type owl:ObjectProperty .


###  https://w3id.org/iadopt/ont/hasProperty
iop:hasProperty rdf:type owl:ObjectProperty .


###  https://w3id.org/iadopt/ont/hasStatisticalModifier
iop:hasStatisticalModifier rdf:type owl:ObjectProperty .


#################################################################
#    Classes
#################################################################

###  http://purl.dataone.org/odo/ECSO_00002050
odo:ECSO_00002050 rdf:type owl:Class ;
                  rdfs:subClassOf <http://purl.obolibrary.org/obo/IAO_0000109> ;
                  <http://purl.obolibrary.org/obo/IAO_0000115> "year of measurement"@en ;
                  rdfs:isDefinedBy odo: ;
                  rdfs:label "year of measurement"@en .


###  http://purl.dataone.org/odo/SALMON_00000137
odo:SALMON_00000137 rdf:type owl:Class ;
                    rdfs:subClassOf <http://purl.obolibrary.org/obo/BFO_0000040> ;
                    <http://purl.obolibrary.org/obo/IAO_0000115> "The Food and Agriculture Organization of the United Nations (FAO) defines a fishery as '...an activity leading to harvesting of fish. It may involve capture of wild fish or raising of fish through aquaculture.'"@en ;
                    rdfs:isDefinedBy odo: ;
                    rdfs:label "Fishery type"@en .


###  http://purl.dataone.org/odo/SALMON_00000167
odo:SALMON_00000167 rdf:type owl:Class ;
                    rdfs:subClassOf <http://purl.obolibrary.org/obo/IAO_0000030> ;
                    <http://purl.obolibrary.org/obo/IAO_0000115> "A measurement type taken of some physical, biological, or ecological aspect of a fish or fishes."@en ;
                    rdfs:isDefinedBy odo: ;
                    rdfs:label "Fish measurement type"@en .


###  http://purl.dataone.org/odo/SALMON_00000479
odo:SALMON_00000479 rdf:type owl:Class ;
                    rdfs:subClassOf <http://purl.obolibrary.org/obo/IAO_0000109> ;
                    <http://purl.obolibrary.org/obo/IAO_0000115> "The number of salmon which do not get caught by commercial or recreational fisheries and return to their freshwater spawning habitat."@en ;
                    rdfs:isDefinedBy odo: ;
                    rdfs:label "Salmon escapement count"@en .


###  http://purl.dataone.org/odo/SALMON_00000639
odo:SALMON_00000639 rdf:type owl:Class ;
                    rdfs:subClassOf <http://purl.obolibrary.org/obo/BFO_0000040> ;
                    <http://purl.obolibrary.org/obo/IAO_0000115> "Group of individuals of a species which can be regarded as an entity for management or assessment purposes; a separate breeding population of a species; term used to identify a management unit of fishery species. A distinct genetic population, a population defined by movement pattern, part of a population potentially harvestable, or a quantity of fish from a given area. May be a total or a spawning stock."@en ;
                    rdfs:isDefinedBy odo: ;
                    rdfs:label "Fish stock type"@en .


###  http://purl.obolibrary.org/obo/BFO_0000015
<http://purl.obolibrary.org/obo/BFO_0000015> rdf:type owl:Class ;
                                             <http://purl.obolibrary.org/obo/IAO_0000115> "An occurrent that has temporal parts and for some time t, p s-depends_on some material entity at t."@en ;
                                             rdfs:isDefinedBy <http://purl.obolibrary.org/obo/bfo.owl> ;
                                             rdfs:label "process"@en .


###  http://purl.obolibrary.org/obo/BFO_0000020
<http://purl.obolibrary.org/obo/BFO_0000020> rdf:type owl:Class ;
                                             <http://purl.obolibrary.org/obo/IAO_0000115> "b is a specifically dependent continuant = Def. b is a continuant & there is some independent continuant c which is not a spatial region and which is such that b s-depends_on c at every time t during the course of b’s existence. (axiom label in BFO2 Reference: [050-003])"@en ;
                                             rdfs:isDefinedBy <http://purl.obolibrary.org/obo/bfo.owl> ;
                                             rdfs:label "specifically dependent continuant"@en .


###  http://purl.obolibrary.org/obo/BFO_0000031
<http://purl.obolibrary.org/obo/BFO_0000031> rdf:type owl:Class ;
                                             <http://purl.obolibrary.org/obo/IAO_0000115> "A continuant that is dependent on one or more independent continuants and whose instances can be multiply instantiated."@en ;
                                             rdfs:isDefinedBy <http://purl.obolibrary.org/obo/bfo.owl> ;
                                             rdfs:label "generically dependent continuant"@en .


###  http://purl.obolibrary.org/obo/BFO_0000040
<http://purl.obolibrary.org/obo/BFO_0000040> rdf:type owl:Class ;
                                             <http://purl.obolibrary.org/obo/IAO_0000115> "An independent continuant that is spatially extended whose identity is independent of that of other entities and can be maintained through time."@en ;
                                             rdfs:isDefinedBy <http://purl.obolibrary.org/obo/bfo.owl> ;
                                             rdfs:label "material entity"@en .


###  http://purl.obolibrary.org/obo/ENVO_00000020
<http://purl.obolibrary.org/obo/ENVO_00000020> rdf:type owl:Class ;
                                               rdfs:subClassOf <http://purl.obolibrary.org/obo/ENVO_01000617> ;
                                               <http://purl.obolibrary.org/obo/IAO_0000115> "A body of water or other liquid of considerable size contained in a depression on a landmass."@en ;
                                               rdfs:isDefinedBy <http://purl.obolibrary.org/obo/envo.owl> ;
                                               rdfs:label "lake"@en .


###  http://purl.obolibrary.org/obo/ENVO_00000022
<http://purl.obolibrary.org/obo/ENVO_00000022> rdf:type owl:Class ;
                                               rdfs:subClassOf <http://purl.obolibrary.org/obo/ENVO_01000618> ;
                                               <http://purl.obolibrary.org/obo/IAO_0000115> "A stream which, through permanent or seasonal flow processes, moves from elevated land towards lower elevations through a definite channel and empties either into a sea, lake, or another river or ends on land as bed seepage and evapotranspiration exceed water supply."@en ;
                                               rdfs:isDefinedBy <http://purl.obolibrary.org/obo/envo.owl> ;
                                               rdfs:label "river"@en .


###  http://purl.obolibrary.org/obo/ENVO_00000023
<http://purl.obolibrary.org/obo/ENVO_00000023> rdf:type owl:Class ;
                                               rdfs:subClassOf <http://purl.obolibrary.org/obo/ENVO_01000618> ;
                                               <http://purl.obolibrary.org/obo/IAO_0000115> "A watercourse which is linear and flows across the solid portion of a planetary surface."@en ;
                                               rdfs:comment "A creek is typically smaller than a stream."@en ;
                                               rdfs:isDefinedBy <http://purl.obolibrary.org/obo/envo.owl> ;
                                               rdfs:label "stream"@en ;
                                               skos:altLabel "creek"@en .


###  http://purl.obolibrary.org/obo/ENVO_00000033
<http://purl.obolibrary.org/obo/ENVO_00000033> rdf:type owl:Class ;
                                               rdfs:subClassOf <http://purl.obolibrary.org/obo/ENVO_01000617> ;
                                               <http://purl.obolibrary.org/obo/IAO_0000115> "A body of water, usually of smaller size than a lake."@en ;
                                               rdfs:isDefinedBy <http://purl.obolibrary.org/obo/envo.owl> ;
                                               rdfs:label "pond"@en .


###  http://purl.obolibrary.org/obo/ENVO_00000063
<http://purl.obolibrary.org/obo/ENVO_00000063> rdf:type owl:Class ;
                                               rdfs:subClassOf <http://purl.obolibrary.org/obo/BFO_0000040> ;
                                               rdfs:isDefinedBy <http://purl.obolibrary.org/obo/envo.owl> ;
                                               rdfs:label "water body"@en .


###  http://purl.obolibrary.org/obo/ENVO_00000234
<http://purl.obolibrary.org/obo/ENVO_00000234> rdf:type owl:Class ;
                                               rdfs:subClassOf <http://purl.obolibrary.org/obo/ENVO_00000023> ;
                                               <http://purl.obolibrary.org/obo/IAO_0000115> "A small, slow-moving stream or creek; usually located in low-lying areas."@en ;
                                               rdfs:isDefinedBy <http://purl.obolibrary.org/obo/envo.owl> ;
                                               rdfs:label "bayou"@en ;
                                               skos:altLabel "slough"@en ;
                                               skos:prefLabel "slough"@en .


###  http://purl.obolibrary.org/obo/ENVO_01000617
<http://purl.obolibrary.org/obo/ENVO_01000617> rdf:type owl:Class ;
                                               rdfs:subClassOf <http://purl.obolibrary.org/obo/ENVO_00000063> ;
                                               <http://purl.obolibrary.org/obo/IAO_0000115> "A lentic water body is a water body in which the accumulated water, in its totality, has very little to no directed flow."@en ;
                                               rdfs:isDefinedBy <http://purl.obolibrary.org/obo/envo.owl> ;
                                               rdfs:label "lentic water body"@en .


###  http://purl.obolibrary.org/obo/ENVO_01000618
<http://purl.obolibrary.org/obo/ENVO_01000618> rdf:type owl:Class ;
                                               rdfs:subClassOf <http://purl.obolibrary.org/obo/ENVO_00000063> ;
                                               <http://purl.obolibrary.org/obo/IAO_0000115> "A lotic water body is a water body in which the accumulated water, in its totality, is flowing."@en ;
                                               rdfs:isDefinedBy <http://purl.obolibrary.org/obo/envo.owl> ;
                                               rdfs:label "lotic water body"@en .


###  http://purl.obolibrary.org/obo/IAO_0000030
<http://purl.obolibrary.org/obo/IAO_0000030> rdf:type owl:Class ;
                                             rdfs:subClassOf <http://purl.obolibrary.org/obo/BFO_0000031> ;
                                             <http://purl.obolibrary.org/obo/IAO_0000115> "A generically dependent continuant that is about some thing."@en ;
                                             rdfs:isDefinedBy <http://purl.obolibrary.org/obo/iao.owl> ;
                                             rdfs:label "information content entity"@en .


###  http://purl.obolibrary.org/obo/IAO_0000033
<http://purl.obolibrary.org/obo/IAO_0000033> rdf:type owl:Class ;
                                             rdfs:subClassOf <http://purl.obolibrary.org/obo/IAO_0000030> ;
                                             <http://purl.obolibrary.org/obo/IAO_0000115> "An information content entity whose concretizations indicate to their bearer how to realize them in a process."@en ;
                                             rdfs:isDefinedBy <http://purl.obolibrary.org/obo/iao.owl> ;
                                             rdfs:label "directive information entity"@en .


###  http://purl.obolibrary.org/obo/IAO_0000104
<http://purl.obolibrary.org/obo/IAO_0000104> rdf:type owl:Class ;
                                             rdfs:subClassOf <http://purl.obolibrary.org/obo/IAO_0000030> ;
                                             <http://purl.obolibrary.org/obo/IAO_0000115> "A directive information entity with action specifications and objective specifications as parts, and that may be concretized as a realizable entity that, if realized, is realized in a process in which the bearer tries to achieve the objectives by taking the actions specified."@en ;
                                             rdfs:isDefinedBy <http://purl.obolibrary.org/obo/iao.owl> ;
                                             rdfs:label "plan specification"@en .


###  http://purl.obolibrary.org/obo/IAO_0000109
<http://purl.obolibrary.org/obo/IAO_0000109> rdf:type owl:Class ;
                                             rdfs:subClassOf <http://purl.obolibrary.org/obo/IAO_0000030> ;
                                             <http://purl.obolibrary.org/obo/IAO_0000115> "A measurement datum is an information content entity that is a recording of the output of a measurement such as produced by a device."@en ;
                                             rdfs:isDefinedBy <http://purl.obolibrary.org/obo/iao.owl> ;
                                             rdfs:label "measurement datum"@en .


###  http://purl.obolibrary.org/obo/IAO_0000310
<http://purl.obolibrary.org/obo/IAO_0000310> rdf:type owl:Class ;
                                             rdfs:subClassOf <http://purl.obolibrary.org/obo/IAO_0000030> ;
                                             <http://purl.obolibrary.org/obo/IAO_0000115> "A collection of information content entities intended to be understood together as a whole."@en ;
                                             rdfs:isDefinedBy <http://purl.obolibrary.org/obo/iao.owl> ;
                                             rdfs:label "document"@en .


###  http://rs.tdwg.org/dwc/terms/Event
dwc:Event rdf:type owl:Class ;
          rdfs:subClassOf <http://purl.obolibrary.org/obo/BFO_0000015> ;
          <http://purl.obolibrary.org/obo/IAO_0000115> "An action that occurs at some location during some time."@en ;
          <http://purl.obolibrary.org/obo/IAO_0000119> <https://dwc.tdwg.org/list/> ;
          rdfs:isDefinedBy dwc: ;
          rdfs:label "Event"@en .


###  http://rs.tdwg.org/dwc/terms/Identification
dwc:Identification rdf:type owl:Class ;
                   rdfs:subClassOf <http://purl.obolibrary.org/obo/BFO_0000015> ;
                   <http://purl.obolibrary.org/obo/IAO_0000115> "A taxonomic determination (e.g., the assignment to a dwc:Taxon)."@en ;
                   <http://purl.obolibrary.org/obo/IAO_0000119> <https://dwc.tdwg.org/list/> ;
                   rdfs:isDefinedBy dwc: ;
                   rdfs:label "Identification"@en .


###  http://rs.tdwg.org/dwc/terms/MaterialEntity
dwc:MaterialEntity rdf:type owl:Class ;
                   rdfs:subClassOf <http://purl.obolibrary.org/obo/BFO_0000040> ;
                   <http://purl.obolibrary.org/obo/IAO_0000115> "An entity that can be identified, exists for some period of time, and consists in whole or in part of physical matter while it exists."@en ;
                   <http://purl.obolibrary.org/obo/IAO_0000119> <https://dwc.tdwg.org/list/> ;
                   rdfs:isDefinedBy dwc: ;
                   rdfs:label "Material Entity"@en .


###  http://rs.tdwg.org/dwc/terms/Occurrence
dwc:Occurrence rdf:type owl:Class ;
               rdfs:subClassOf <http://purl.obolibrary.org/obo/BFO_0000015> ;
               <http://purl.obolibrary.org/obo/IAO_0000115> "An existence of a dwc:Organism at a particular place at a particular time."@en ;
               <http://purl.obolibrary.org/obo/IAO_0000119> <https://dwc.tdwg.org/list/> ;
               rdfs:isDefinedBy dwc: ;
               rdfs:label "Occurrence"@en .


###  http://rs.tdwg.org/dwc/terms/Organism
dwc:Organism rdf:type owl:Class ;
             rdfs:subClassOf <http://purl.obolibrary.org/obo/BFO_0000040> ;
             <http://purl.obolibrary.org/obo/IAO_0000115> "A particular organism or defined group of organisms considered to be taxonomically homogeneous."@en ;
             <http://purl.obolibrary.org/obo/IAO_0000119> <https://dwc.tdwg.org/list/> ;
             rdfs:isDefinedBy dwc: ;
             rdfs:label "Organism"@en .


###  http://www.w3.org/2004/02/skos/core#Concept
skos:Concept rdf:type owl:Class .


###  http://www.w3.org/2004/02/skos/core#ConceptScheme
skos:ConceptScheme rdf:type owl:Class .


###  http://www.w3.org/ns/dqv#Dimension
dqv:Dimension rdf:type owl:Class ;
              rdfs:subClassOf skos:Concept ;
              <http://purl.obolibrary.org/obo/IAO_0000115> "Represents criteria relevant for assessing quality. Each quality dimension must have one or more metric to measure it. A dimension is linked with a category using the dqv:inCategory property."@en ;
              <http://purl.obolibrary.org/obo/IAO_0000119> <https://www.w3.org/TR/vocab-dqv/> ;
              rdfs:isDefinedBy dqv: ;
              rdfs:label "Dimension"@en .


###  http://www.w3.org/ns/dqv#QualityAnnotation
dqv:QualityAnnotation rdf:type owl:Class ;
                      rdfs:subClassOf oa:Annotation ;
                      <http://purl.obolibrary.org/obo/IAO_0000115> "Represents quality annotations, including ratings, quality certificates or feedback that can be associated to datasets or distributions. Quality annotations must have one oa:motivatedBy statement with an instance of oa:Motivation (and skos:Concept) that reflects a quality assessment purpose. We define this instance as dqv:qualityAssessment."@en ;
                      <http://purl.obolibrary.org/obo/IAO_0000119> <https://www.w3.org/TR/vocab-dqv/> ;
                      rdfs:isDefinedBy dqv: ;
                      rdfs:label "Quality Annotation"@en .


###  http://www.w3.org/ns/oa#Annotation
oa:Annotation rdf:type owl:Class ;
              rdfs:subClassOf <http://purl.obolibrary.org/obo/IAO_0000030> ;
              <http://purl.obolibrary.org/obo/IAO_0000115> "The class for Web Annotations."@en ;
              <http://purl.obolibrary.org/obo/IAO_0000119> oa:Annotation ;
              rdfs:isDefinedBy oa: ;
              rdfs:label "Annotation"@en .


###  http://www.w3.org/ns/prov#Activity
prov:Activity rdf:type owl:Class .


###  https://w3id.org/gcdfo/salmon#AbundancePercentileMetric
gcdfo:AbundancePercentileMetric rdf:type owl:Class ;
                                rdfs:subClassOf gcdfo:ObservedRateOrAbundance ;
                                <http://purl.obolibrary.org/obo/IAO_0000115> "An abundance percentile metric giving the percentile rank of the current generational average spawner abundance relative to a historical reference distribution."@en ;
                                <http://purl.obolibrary.org/obo/IAO_0000119> "Fisheries and Oceans Canada. 2024. Rapid Status Approximations for Pacific Salmon Derived from Integrated Expert Assessments under DFO’s Wild Salmon Policy. CSAS Pacific Region Science Response 2024/004."@en ;
                                dcterms:source <https://waves-vagues.dfo-mpo.gc.ca/library-bibliotheque/41225260.pdf> ;
                                rdfs:isDefinedBy <https://w3id.org/gcdfo/salmon> ;
                                rdfs:label "Abundance percentile metric"@en ;
                                gcdfo:theme gcdfo:DataModelProvenanceTheme ,
                                            gcdfo:StockAssessmentTheme ,
                                            gcdfo:WildSalmonPolicyTheme .


###  https://w3id.org/gcdfo/salmon#BenchmarkRatioMetric
gcdfo:BenchmarkRatioMetric rdf:type owl:Class ;
                           rdfs:subClassOf gcdfo:ObservedRateOrAbundance ;
                           <http://purl.obolibrary.org/obo/IAO_0000115> "A benchmark-ratio metric equal to the ratio of current generational average spawner abundance to a specified benchmark (lower or upper benchmark), where 1.0 indicates equality to that benchmark."@en ;
                           <http://purl.obolibrary.org/obo/IAO_0000119> "Fisheries and Oceans Canada. 2024. Rapid Status Approximations for Pacific Salmon Derived from Integrated Expert Assessments under DFO’s Wild Salmon Policy. CSAS Pacific Region Science Response 2024/004."@en ;
                           dcterms:source <https://waves-vagues.dfo-mpo.gc.ca/library-bibliotheque/41225260.pdf> ;
                           rdfs:isDefinedBy <https://w3id.org/gcdfo/salmon> ;
                           rdfs:label "Benchmark ratio metric"@en ;
                           gcdfo:theme gcdfo:DataModelProvenanceTheme ,
                                       gcdfo:StockAssessmentTheme ,
                                       gcdfo:WildSalmonPolicyTheme .


###  https://w3id.org/gcdfo/salmon#BroodYear
gcdfo:BroodYear rdf:type owl:Class ;
                rdfs:subClassOf gcdfo:YearBasis ;
                <http://purl.obolibrary.org/obo/IAO_0000115> "The parental year for a group of returning salmon, i.e. the calendar year when the majority of parents of these fish spawned."@en ;
                <http://purl.obolibrary.org/obo/IAO_0000119> "Fisheries and Oceans Canada. Pacific Salmon - Glossary (Pacific Region). https://www.pac.dfo-mpo.gc.ca/fm-gp/salmon-saumon/gloss-eng.html."@en ;
                dcterms:source <https://www.pac.dfo-mpo.gc.ca/fm-gp/salmon-saumon/gloss-eng.html> ;
                rdfs:isDefinedBy <https://w3id.org/gcdfo/salmon> ;
                rdfs:label "Brood year"@en ;
                skos:closeMatch odo:SALMON_00000520 ;
                gcdfo:theme gcdfo:StockAssessmentTheme .


###  https://w3id.org/gcdfo/salmon#CWTMarineSurvivalRate
gcdfo:CWTMarineSurvivalRate rdf:type owl:Class ;
                            rdfs:subClassOf gcdfo:ObservedRateOrAbundance ;
                            <http://purl.obolibrary.org/obo/IAO_0000115> "A marine survival proportion estimated for a coded-wire-tag (CWT) release group, defined as the portion of tagged smolts that survive to be caught in marine fisheries or return to freshwater as adults."@en ;
                            <http://purl.obolibrary.org/obo/IAO_0000119> "Fisheries and Oceans Canada. 2021. Marine Survival Forecast of Southern British Columbia Coho (defines marine survival as (Catch+Escapement)/Release for coded-wire-tag smolt releases)."@en ;
                            dcterms:source <https://waves-vagues.dfo-mpo.gc.ca/Library/40978680.pdf> ;
                            rdfs:isDefinedBy <https://w3id.org/gcdfo/salmon> ;
                            rdfs:label "CWT marine survival rate"@en ;
                            skos:altLabel "Coded-wire-tag marine survival rate"@en ;
                            gcdfo:theme gcdfo:MonitoringFieldWorkTheme ,
                                        gcdfo:StockAssessmentTheme .


###  https://w3id.org/gcdfo/salmon#CatchYear
gcdfo:CatchYear rdf:type owl:Class ;
                rdfs:subClassOf gcdfo:YearBasis ;
                <http://purl.obolibrary.org/obo/IAO_0000115> "The calendar year in which returning salmon are caught in fisheries (as opposed to the brood year in which the cohort was spawned)."@en ;
                rdfs:isDefinedBy <https://w3id.org/gcdfo/salmon> ;
                rdfs:label "Catch year"@en ;
                gcdfo:theme gcdfo:StockAssessmentTheme .


###  https://w3id.org/gcdfo/salmon#ConfidenceCategory
gcdfo:ConfidenceCategory rdf:type owl:Class .


###  https://w3id.org/gcdfo/salmon#ConservationUnit
gcdfo:ConservationUnit rdf:type owl:Class ;
                       rdfs:subClassOf gcdfo:ReportingOrManagementStratum ;
                       <http://purl.obolibrary.org/obo/IAO_0000115> "A group of fish sufficiently isolated from other groups that, if extirpated, is very unlikely to recolonize naturally within an acceptable timeframe."@en ;
                       <http://purl.obolibrary.org/obo/IAO_0000119> "Fisheries and Oceans Canada. 2005. Canada's Policy for Conservation of Wild Pacific Salmon. https://waves-vagues.dfo-mpo.gc.ca/library-bibliotheque/315577.pdf."@en ,
                                                                    "Fisheries and Oceans Canada. Canada's Policy for Conservation of Wild Pacific Salmon - Glossary. https://www.pac.dfo-mpo.gc.ca/fm-gp/salmon-saumon/wsp-pss/policy-politique-eng.html#glossary."@en ;
                       dcterms:isPartOf <urn:ISBN:0662405382> ;
                       dcterms:source <https://waves-vagues.dfo-mpo.gc.ca/library-bibliotheque/315577.pdf> ,
                                      <https://www.pac.dfo-mpo.gc.ca/fm-gp/salmon-saumon/wsp-pss/policy-politique-eng.html#glossary> ;
                       rdfs:isDefinedBy <https://w3id.org/gcdfo/salmon> ;
                       rdfs:label "Conservation Unit"@en ;
                       gcdfo:theme gcdfo:PolicyGovernanceTheme ,
                                   gcdfo:SalmonEnhancementHatcheriesTheme ,
                                   gcdfo:WildSalmonPolicyTheme .


###  https://w3id.org/gcdfo/salmon#Deme
gcdfo:Deme rdf:type owl:Class ;
           rdfs:subClassOf dwc:Organism ;
           <http://purl.obolibrary.org/obo/IAO_0000115> "A local interbreeding group of organisms within a species. In salmon, a deme typically corresponds to a spawning population at a specific site. Demes are the finest biological unit and make up populations."@en ;
           rdfs:isDefinedBy <https://w3id.org/gcdfo/salmon> ;
           rdfs:label "Deme"@en ;
           gcdfo:theme gcdfo:GeneticsStockCompositionTheme ,
                       gcdfo:StockAssessmentTheme ,
                       gcdfo:WildSalmonPolicyTheme .


###  https://w3id.org/gcdfo/salmon#Escapement
gcdfo:Escapement rdf:type owl:Class ;
                 rdfs:subClassOf <http://purl.obolibrary.org/obo/BFO_0000015> ;
                 <http://purl.obolibrary.org/obo/IAO_0000115> "The number of mature salmon that pass through (or escape) fisheries and return to fresh water to spawn."@en ;
                 <http://purl.obolibrary.org/obo/IAO_0000119> "Fisheries and Oceans Canada. 2005. Canada's Policy for Conservation of Wild Pacific Salmon. https://waves-vagues.dfo-mpo.gc.ca/library-bibliotheque/315577.pdf."@en ;
                 dcterms:source <https://waves-vagues.dfo-mpo.gc.ca/library-bibliotheque/315577.pdf> ;
                 rdfs:isDefinedBy <https://w3id.org/gcdfo/salmon> ;
                 rdfs:label "Escapement"@en ;
                 skos:closeMatch odo:SALMON_00000479 ;
                 gcdfo:theme gcdfo:MonitoringFieldWorkTheme ,
                             gcdfo:StockAssessmentTheme .


###  https://w3id.org/gcdfo/salmon#EscapementMeasurement
gcdfo:EscapementMeasurement rdf:type owl:Class ;
                            rdfs:subClassOf <http://purl.obolibrary.org/obo/IAO_0000109> ;
                            <http://purl.obolibrary.org/obo/IAO_0000115> "A measurement or estimate of escapement tied to a stock and a survey event."@en ;
                            rdfs:isDefinedBy <https://w3id.org/gcdfo/salmon> ;
                            rdfs:label "Escapement measurement"@en ;
                            skos:closeMatch sosa:Result ;
                            gcdfo:theme gcdfo:MonitoringFieldWorkTheme ,
                                        gcdfo:StockAssessmentTheme .


###  https://w3id.org/gcdfo/salmon#EscapementSurveyEvent
gcdfo:EscapementSurveyEvent rdf:type owl:Class ;
                            rdfs:subClassOf gcdfo:SurveyEvent ;
                            <http://purl.obolibrary.org/obo/IAO_0000115> "A survey event specifically for estimating escapement."@en ;
                            rdfs:isDefinedBy <https://w3id.org/gcdfo/salmon> ;
                            rdfs:label "Escapement Survey Event"@en ;
                            skos:closeMatch sosa:Sampling ;
                            skos:prefLabel "Escapement Survey Event"@en ;
                            gcdfo:theme gcdfo:MonitoringFieldWorkTheme ,
                                        gcdfo:StockAssessmentTheme .


###  https://w3id.org/gcdfo/salmon#ExploitationRate
gcdfo:ExploitationRate rdf:type owl:Class ;
                       rdfs:subClassOf <http://purl.obolibrary.org/obo/IAO_0000109> ;
                       <http://purl.obolibrary.org/obo/IAO_0000115> "A fishing mortality rate expressed as the proportion of the total return removed by fishing over a specified assessment period."@en ;
                       <http://purl.obolibrary.org/obo/IAO_0000119> "Fisheries and Oceans Canada. Pacific Salmon - Glossary (Pacific Region). https://www.pac.dfo-mpo.gc.ca/fm-gp/salmon-saumon/gloss-eng.html."@en ;
                       dcterms:source <https://www.pac.dfo-mpo.gc.ca/fm-gp/salmon-saumon/gloss-eng.html> ;
                       rdfs:isDefinedBy <https://w3id.org/gcdfo/salmon> ;
                       rdfs:label "Exploitation rate"@en ;
                       gcdfo:theme gcdfo:FisheriesManagementTheme ,
                                   gcdfo:StockAssessmentTheme .


###  https://w3id.org/gcdfo/salmon#FisheriesReferencePointLower
gcdfo:FisheriesReferencePointLower rdf:type owl:Class ;
                                   rdfs:subClassOf gcdfo:LimitReferencePoint ;
                                   <http://purl.obolibrary.org/obo/IAO_0000115> "A lower fisheries-management reference point defined for Stock Management Units (SMUs) and related fishery decision frameworks. It may be informed by Conservation Unit (CU) lower biological benchmarks, but is not identical to CU-level lower biological benchmarks used to delineate Wild Salmon Policy biological status zones."@en ;
                                   <http://purl.obolibrary.org/obo/IAO_0000119> "Fisheries and Oceans Canada. (2022). Methodologies and Guidelines for Defining Limit Reference Points for Pacific Salmon. DFO Can. Sci. Advis. Sec. Sci. Advis. Rep. 2022/030. (Erratum: December 2022)."@en ;
                                   rdfs:isDefinedBy <https://w3id.org/gcdfo/salmon> ;
                                   rdfs:label "Fisheries Reference Point - Lower"@en ;
                                   skos:altLabel "FRP-L"@en ;
                                   gcdfo:theme gcdfo:FisheriesManagementTheme ,
                                               gcdfo:PolicyGovernanceTheme ,
                                               gcdfo:StockAssessmentTheme .


###  https://w3id.org/gcdfo/salmon#GenerationalAverageAbundance
gcdfo:GenerationalAverageAbundance rdf:type owl:Class ;
                                   rdfs:subClassOf gcdfo:ObservedRateOrAbundance ;
                                   <http://purl.obolibrary.org/obo/IAO_0000115> "The generational average of spawner abundance, calculated as a geometric mean across the number of years corresponding to the most common age at return (generation length), optionally after smoothing depending on CU group."@en ;
                                   <http://purl.obolibrary.org/obo/IAO_0000119> "Fisheries and Oceans Canada. 2024. Rapid Status Approximations for Pacific Salmon Derived from Integrated Expert Assessments under DFO’s Wild Salmon Policy. CSAS Pacific Region Science Response 2024/004."@en ;
                                   dcterms:source <https://waves-vagues.dfo-mpo.gc.ca/library-bibliotheque/41225260.pdf> ;
                                   rdfs:isDefinedBy <https://w3id.org/gcdfo/salmon> ;
                                   rdfs:label "Generational average abundance"@en ;
                                   gcdfo:theme gcdfo:DataModelProvenanceTheme ,
                                               gcdfo:StockAssessmentTheme ,
                                               gcdfo:WildSalmonPolicyTheme .


###  https://w3id.org/gcdfo/salmon#InRiverMortalityRate
gcdfo:InRiverMortalityRate rdf:type owl:Class ;
                           rdfs:subClassOf gcdfo:ObservedRateOrAbundance ;
                           <http://purl.obolibrary.org/obo/IAO_0000115> "The proportion of fish in a defined population/cohort that die during freshwater migration in-river on the way to spawning areas during a specified assessment interval, excluding landed catch (fishery removals) where those are accounted separately."@en ;
                           <http://purl.obolibrary.org/obo/IAO_0000119> "Fisheries and Oceans Canada. 2025. Stock-Specific Fraser River Sockeye Salmon Run Size Determination. CSAS Pacific Region Science Advisory Report 2025/021 (en route mortality excluding landed catch). COSEWIC. 2017. Sockeye Salmon (Oncorhynchus nerka) assessment and status report (en-route loss is fish that perished in the river en-route to spawning grounds for reasons other than fishing)."@en ;
                           dcterms:source <https://waves-vagues.dfo-mpo.gc.ca/library-bibliotheque/41294622.pdf> ,
                                          <https://www.canada.ca/en/environment-climate-change/services/species-risk-public-registry/cosewic-assessments-status-reports/sockeye-salmon-2017.html> ;
                           rdfs:isDefinedBy <https://w3id.org/gcdfo/salmon> ;
                           rdfs:label "In-river mortality rate"@en ;
                           gcdfo:theme gcdfo:StockAssessmentTheme .


###  https://w3id.org/gcdfo/salmon#IndicatorRiver
gcdfo:IndicatorRiver rdf:type owl:Class ;
                     rdfs:subClassOf gcdfo:ReportingOrManagementStratum ;
                     <http://purl.obolibrary.org/obo/IAO_0000115> "A reporting and assessment stratum identifying monitored indicator streams that provide representative indices of spawner abundance for nearby streams."@en ;
                     dcterms:source <https://www.salmonexplorer.ca/methods/glossary.html> ;
                     rdfs:isDefinedBy <https://w3id.org/gcdfo/salmon> ;
                     rdfs:label "Indicator river"@en ;
                     skos:altLabel "Indicator stream"@en ;
                     gcdfo:theme gcdfo:MonitoringFieldWorkTheme ,
                                 gcdfo:PolicyGovernanceTheme ,
                                 gcdfo:StockAssessmentTheme .


###  https://w3id.org/gcdfo/salmon#LimitReferencePoint
gcdfo:LimitReferencePoint rdf:type owl:Class ;
                          rdfs:subClassOf gcdfo:ReferencePoint ;
                          <http://purl.obolibrary.org/obo/IAO_0000115> "A fish stock experiencing serious harm may be depleted to the point where it has impaired productivity or reproductive capacity. As a result, the stock would be less resilient to fishing and could not easily rebuild. Serious harm may be irreversible, or only slowly reversible over the long-term, and can be due to fishing, other human-induced impacts, or natural causes. Under the Precautionary Approach policy and the Fish Stocks Provisions (FSPs), breaching the LRP is a trigger for a rebuilding plan."@en ;
                          <http://purl.obolibrary.org/obo/IAO_0000119> "Fisheries and Oceans Canada. Introduction to Stock Assessment - Glossary. https://www.dfo-mpo.gc.ca/science/species-especes/fisheries-halieutiques/assessment-evaluation/glossary-glossaire/index-eng.html."@en ;
                          dcterms:source <https://www.dfo-mpo.gc.ca/science/species-especes/fisheries-halieutiques/assessment-evaluation/glossary-glossaire/index-eng.html> ;
                          rdfs:isDefinedBy <https://w3id.org/gcdfo/salmon> ;
                          rdfs:label "Limit reference point"@en ;
                          skos:altLabel "LRP"@en ;
                          gcdfo:theme gcdfo:FisheriesManagementTheme ,
                                      gcdfo:PolicyGovernanceTheme ,
                                      gcdfo:StockAssessmentTheme .


###  https://w3id.org/gcdfo/salmon#LongTermTrendMetric
gcdfo:LongTermTrendMetric rdf:type owl:Class ;
                          rdfs:subClassOf gcdfo:ObservedRateOrAbundance ;
                          <http://purl.obolibrary.org/obo/IAO_0000115> "A long-term trend metric comparing the current generational average (geometric mean) spawner abundance to the long-term average (geometric mean) spawner abundance for an assessed time series."@en ;
                          <http://purl.obolibrary.org/obo/IAO_0000119> "Fisheries and Oceans Canada. 2024. Rapid Status Approximations for Pacific Salmon Derived from Integrated Expert Assessments under DFO’s Wild Salmon Policy. CSAS Pacific Region Science Response 2024/004."@en ;
                          dcterms:source <https://waves-vagues.dfo-mpo.gc.ca/library-bibliotheque/41225260.pdf> ;
                          rdfs:isDefinedBy <https://w3id.org/gcdfo/salmon> ;
                          rdfs:label "Long-term trend metric"@en ;
                          gcdfo:theme gcdfo:DataModelProvenanceTheme ,
                                      gcdfo:StockAssessmentTheme ,
                                      gcdfo:WildSalmonPolicyTheme .


###  https://w3id.org/gcdfo/salmon#LowerBiologicalBenchmark
gcdfo:LowerBiologicalBenchmark rdf:type owl:Class ;
                               rdfs:subClassOf gcdfo:MetricBenchmark ;
                               <http://purl.obolibrary.org/obo/IAO_0000115> "Lower benchmark value for a Conservation Unit (CU) metric used to delineate Wild Salmon Policy status zones (typically the boundary between Red and Amber zones). This CU-level biological benchmark is distinct from SMU-level fisheries management lower reference points such as FRP-L."@en ;
                               <http://purl.obolibrary.org/obo/IAO_0000119> "Fisheries and Oceans Canada. (2021). Wild Salmon Policy 2018-2022 Implementation Plan. Available at https://waves-vagues.dfo-mpo.gc.ca/library-bibliotheque/40728109.pdf."@en ;
                               dcterms:source <https://waves-vagues.dfo-mpo.gc.ca/library-bibliotheque/40728109.pdf> ;
                               rdfs:isDefinedBy <https://w3id.org/gcdfo/salmon> ;
                               rdfs:label "Lower biological benchmark"@en ;
                               gcdfo:theme gcdfo:PolicyGovernanceTheme ,
                                           gcdfo:StockAssessmentTheme ,
                                           gcdfo:WildSalmonPolicyTheme .


###  https://w3id.org/gcdfo/salmon#MainstemMortalityRate
gcdfo:MainstemMortalityRate rdf:type owl:Class ;
                            rdfs:subClassOf gcdfo:ObservedRateOrAbundance ;
                            <http://purl.obolibrary.org/obo/IAO_0000115> "The proportion of fish that die while migrating through the freshwater mainstem portion of a river system (as operationally delimited by the assessment workflow), over a specified interval or between specified mainstem reference points."@en ;
                            <http://purl.obolibrary.org/obo/IAO_0000119> "LGL Limited. Migration and Survival of Late-run Fraser Sockeye (radio-telemetry methods; fish detected at Mission are classified as survivors, fishery-related mortalities, or in-river mortalities; fixed-station tracking is conducted at strategic locations including mainstem confluences)."@en ;
                            dcterms:source <https://waves-vagues.dfo-mpo.gc.ca/library-bibliotheque/341440.pdf> ;
                            rdfs:isDefinedBy <https://w3id.org/gcdfo/salmon> ;
                            rdfs:label "Mainstem mortality rate"@en ;
                            gcdfo:theme gcdfo:StockAssessmentTheme .


###  https://w3id.org/gcdfo/salmon#MarineSurvivalIndex
gcdfo:MarineSurvivalIndex rdf:type owl:Class ;
                          rdfs:subClassOf gcdfo:ObservedRateOrAbundance ;
                          <http://purl.obolibrary.org/obo/IAO_0000115> "A dimensionless index or covariate representing marine survival conditions or relative marine survival outcomes (not necessarily a survival proportion)."@en ;
                          <http://purl.obolibrary.org/obo/IAO_0000119> "Fisheries and Oceans Canada. 2021. Marine Survival Forecast of Southern British Columbia Coho (uses climate indicators correlated with marine survival; supports index-like predictors for survival conditions)."@en ;
                          dcterms:source <https://waves-vagues.dfo-mpo.gc.ca/Library/40978680.pdf> ;
                          rdfs:isDefinedBy <https://w3id.org/gcdfo/salmon> ;
                          rdfs:label "Marine survival index"@en ;
                          gcdfo:theme gcdfo:HabitatEcosystemClimateTheme ,
                                      gcdfo:StockAssessmentTheme .


###  https://w3id.org/gcdfo/salmon#MetricBenchmark
gcdfo:MetricBenchmark rdf:type owl:Class ;
                      rdfs:subClassOf <http://purl.obolibrary.org/obo/IAO_0000030> ;
                      <http://purl.obolibrary.org/obo/IAO_0000115> "Benchmark value for a metric that helps delineate status zones (for example, the limit reference point for absolute abundance)."@en ;
                      <http://purl.obolibrary.org/obo/IAO_0000119> "Pestal, G., MacDonald, B.L., Grant, S.C.H., and Holt, C.A. 2023. State of the salmon: rapid status assessment approach for Pacific salmon under Canada's Wild Salmon Policy. Canadian Technical Report of Fisheries and Aquatic Sciences 3570."@en ;
                      dcterms:source <https://publications.gc.ca/site/eng/9.928944/publication.html> ;
                      rdfs:isDefinedBy <https://w3id.org/gcdfo/salmon> ;
                      rdfs:label "Metric benchmark"@en ;
                      gcdfo:theme gcdfo:StockAssessmentTheme ,
                                  gcdfo:WildSalmonPolicyTheme .


###  https://w3id.org/gcdfo/salmon#ObservedExploitationRate
gcdfo:ObservedExploitationRate rdf:type owl:Class ;
                               rdfs:subClassOf gcdfo:ExploitationRate ,
                                               gcdfo:ObservedRateOrAbundance ;
                               <http://purl.obolibrary.org/obo/IAO_0000115> "An empirically estimated exploitation rate derived from observed or reconstructed catches/removals and returns/escapement for a specified stock and period."@en ;
                               <http://purl.obolibrary.org/obo/IAO_0000119> "Fisheries and Oceans Canada. Pacific Salmon - Glossary (Pacific Region). https://www.pac.dfo-mpo.gc.ca/fm-gp/salmon-saumon/gloss-eng.html."@en ;
                               dcterms:source <https://www.pac.dfo-mpo.gc.ca/fm-gp/salmon-saumon/gloss-eng.html> ;
                               rdfs:isDefinedBy <https://w3id.org/gcdfo/salmon> ;
                               rdfs:label "Observed exploitation rate"@en ;
                               gcdfo:theme gcdfo:DataModelProvenanceTheme ,
                                           gcdfo:FisheriesManagementTheme ,
                                           gcdfo:StockAssessmentTheme .


###  https://w3id.org/gcdfo/salmon#ObservedRateOrAbundance
gcdfo:ObservedRateOrAbundance rdf:type owl:Class ;
                              rdfs:subClassOf <http://purl.obolibrary.org/obo/IAO_0000109> ;
                              <http://purl.obolibrary.org/obo/IAO_0000115> "A measurement datum representing an empirically observed rate, count, or abundance derived from monitoring or survey data."@en ;
                              rdfs:isDefinedBy <https://w3id.org/gcdfo/salmon> ;
                              rdfs:label "Observed rate or abundance"@en ;
                              gcdfo:theme gcdfo:DataModelProvenanceTheme ,
                                          gcdfo:StockAssessmentTheme .


###  https://w3id.org/gcdfo/salmon#OceanMortalityRate
gcdfo:OceanMortalityRate rdf:type owl:Class ;
                         rdfs:subClassOf gcdfo:ObservedRateOrAbundance ;
                         <http://purl.obolibrary.org/obo/IAO_0000115> "The proportion of fish that die during the ocean (marine) life-history phase for a defined population/cohort and interval; when a marine survival proportion is available, ocean mortality may be represented as its complement under the assessment’s accounting conventions."@en ;
                         <http://purl.obolibrary.org/obo/IAO_0000119> "COSEWIC. 2017. Sockeye Salmon (Oncorhynchus nerka) assessment and status report (marine survival index described and interpreted in a Pacific salmon assessment context)."@en ;
                         dcterms:source <https://www.canada.ca/en/environment-climate-change/services/species-risk-public-registry/cosewic-assessments-status-reports/sockeye-salmon-2017.html> ;
                         rdfs:isDefinedBy <https://w3id.org/gcdfo/salmon> ;
                         rdfs:label "Ocean mortality rate"@en ;
                         gcdfo:theme gcdfo:StockAssessmentTheme .


###  https://w3id.org/gcdfo/salmon#PercentChangeMetric
gcdfo:PercentChangeMetric rdf:type owl:Class ;
                          rdfs:subClassOf gcdfo:ObservedRateOrAbundance ;
                          <http://purl.obolibrary.org/obo/IAO_0000115> "A short-term trend metric quantifying the percent (linear) change in spawner abundance over the most recent three generations."@en ;
                          <http://purl.obolibrary.org/obo/IAO_0000119> "Fisheries and Oceans Canada. 2024. Rapid Status Approximations for Pacific Salmon Derived from Integrated Expert Assessments under DFO’s Wild Salmon Policy. CSAS Pacific Region Science Response 2024/004."@en ;
                          dcterms:source <https://waves-vagues.dfo-mpo.gc.ca/library-bibliotheque/41225260.pdf> ;
                          rdfs:isDefinedBy <https://w3id.org/gcdfo/salmon> ;
                          rdfs:label "Percent change metric"@en ;
                          skos:altLabel "Rapid-status percent change metric"@en ;
                          gcdfo:theme gcdfo:DataModelProvenanceTheme ,
                                      gcdfo:StockAssessmentTheme ,
                                      gcdfo:WildSalmonPolicyTheme .


###  https://w3id.org/gcdfo/salmon#Population
gcdfo:Population rdf:type owl:Class ;
                 rdfs:subClassOf dwc:Organism ;
                 <http://purl.obolibrary.org/obo/IAO_0000115> "A group of organisms of the same species occupying a defined area that interbreed and share a gene pool. In salmon, populations are composed of one or more demes and form the biological basis for Conservation Units."@en ;
                 rdfs:isDefinedBy <https://w3id.org/gcdfo/salmon> ;
                 rdfs:label "Population"@en ;
                 gcdfo:theme gcdfo:GeneticsStockCompositionTheme ,
                             gcdfo:StockAssessmentTheme ,
                             gcdfo:WildSalmonPolicyTheme .


###  https://w3id.org/gcdfo/salmon#ProbabilityDeclineBelowLowerBenchmarkMetric
gcdfo:ProbabilityDeclineBelowLowerBenchmarkMetric rdf:type owl:Class ;
                                                  rdfs:subClassOf gcdfo:ObservedRateOrAbundance ;
                                                  <http://purl.obolibrary.org/obo/IAO_0000115> "A probability metric estimating the risk that spawner abundance will be below the lower benchmark, given uncertainty in benchmark estimates and/or abundance estimates, for a defined forecast or assessment horizon."@en ;
                                                  <http://purl.obolibrary.org/obo/IAO_0000119> "Fisheries and Oceans Canada. 2024. Rapid Status Approximations for Pacific Salmon Derived from Integrated Expert Assessments under DFO’s Wild Salmon Policy. CSAS Pacific Region Science Response 2024/004."@en ;
                                                  dcterms:source <https://waves-vagues.dfo-mpo.gc.ca/library-bibliotheque/41225260.pdf> ;
                                                  rdfs:isDefinedBy <https://w3id.org/gcdfo/salmon> ;
                                                  rdfs:label "Probability of decline below lower benchmark metric"@en ;
                                                  gcdfo:theme gcdfo:DataModelProvenanceTheme ,
                                                              gcdfo:StockAssessmentTheme ,
                                                              gcdfo:WildSalmonPolicyTheme .


###  https://w3id.org/gcdfo/salmon#ProportionHatcheryOriginSpawners
gcdfo:ProportionHatcheryOriginSpawners rdf:type owl:Class ;
                                       rdfs:subClassOf gcdfo:ObservedRateOrAbundance ;
                                       <http://purl.obolibrary.org/obo/IAO_0000115> "The proportion of spawners in a population-year that are hatchery-origin (hatchery-origin spawners divided by total spawners)."@en ;
                                       <http://purl.obolibrary.org/obo/IAO_0000119> "Derived for SPSR term coverage (Issue #33 term request scope); ‘hatchery-origin’ is defined in the Salmon Origin scheme and operational marking is described in the DFO Coded Wire Tag Program page."@en ;
                                       dcterms:source <https://www.pac.dfo-mpo.gc.ca/pacific-smon-pacifique/science/research-recherche/cwt-mmc-eng.html> ;
                                       rdfs:isDefinedBy <https://w3id.org/gcdfo/salmon> ;
                                       rdfs:label "Proportion of hatchery-origin spawners"@en ;
                                       skos:altLabel "pHOS"@en ;
                                       gcdfo:theme gcdfo:SalmonEnhancementHatcheriesTheme ,
                                                   gcdfo:StockAssessmentTheme .


###  https://w3id.org/gcdfo/salmon#RapidStatusScoreMetric
gcdfo:RapidStatusScoreMetric rdf:type owl:Class ;
                             rdfs:subClassOf gcdfo:ObservedRateOrAbundance ;
                             <http://purl.obolibrary.org/obo/IAO_0000115> "A numeric score produced by a rapid-status algorithm used to represent an ordered status outcome and/or decision-rule position."@en ;
                             <http://purl.obolibrary.org/obo/IAO_0000119> "Fisheries and Oceans Canada. 2024. Rapid Status Approximations for Pacific Salmon Derived from Integrated Expert Assessments under DFO’s Wild Salmon Policy. CSAS Pacific Region Science Response 2024/004."@en ;
                             dcterms:source <https://waves-vagues.dfo-mpo.gc.ca/library-bibliotheque/41225260.pdf> ;
                             rdfs:isDefinedBy <https://w3id.org/gcdfo/salmon> ;
                             rdfs:label "Rapid status score metric"@en ;
                             gcdfo:theme gcdfo:DataModelProvenanceTheme ,
                                         gcdfo:StockAssessmentTheme ,
                                         gcdfo:WildSalmonPolicyTheme .


###  https://w3id.org/gcdfo/salmon#ReferencePoint
gcdfo:ReferencePoint rdf:type owl:Class ;
                     rdfs:subClassOf <http://purl.obolibrary.org/obo/IAO_0000030> ;
                     <http://purl.obolibrary.org/obo/IAO_0000115> "Reference points are used as targets to achieve or as limits to avoid."@en ;
                     <http://purl.obolibrary.org/obo/IAO_0000119> "Fisheries and Oceans Canada. Introduction to Stock Assessment - Glossary. https://www.dfo-mpo.gc.ca/science/species-especes/fisheries-halieutiques/assessment-evaluation/glossary-glossaire/index-eng.html."@en ;
                     dcterms:source <https://www.dfo-mpo.gc.ca/science/species-especes/fisheries-halieutiques/assessment-evaluation/glossary-glossaire/index-eng.html> ;
                     rdfs:isDefinedBy <https://w3id.org/gcdfo/salmon> ;
                     rdfs:label "Reference point"@en ;
                     gcdfo:theme gcdfo:FisheriesManagementTheme ,
                                 gcdfo:PolicyGovernanceTheme ,
                                 gcdfo:StockAssessmentTheme .


###  https://w3id.org/gcdfo/salmon#RelativeHatcherySpawnerAbundance
gcdfo:RelativeHatcherySpawnerAbundance rdf:type owl:Class ;
                                       rdfs:subClassOf gcdfo:RelativeSpawnerAbundance ;
                                       <http://purl.obolibrary.org/obo/IAO_0000115> "Hatchery-origin spawner abundance expressed as a relative (dimensionless) abundance metric to a defined reference (commonly benchmarks), for within-series comparison; in rapid-status workflows, relative abundance is computed using the current generational average (geometric mean) divided by CU-specific lower and/or upper benchmarks."@en ;
                                       <http://purl.obolibrary.org/obo/IAO_0000119> "Fisheries and Oceans Canada. 2024. Rapid Status Approximations for Pacific Salmon… CSAS Pacific Region Science Response 2024/004 (relative abundance metric definition and computation). Holt et al. 2009. Indicators of Status and Benchmarks… CSAS Res. Doc. 2009/058 (discusses hatchery/wild considerations for status assessments)."@en ;
                                       dcterms:source <https://waves-vagues.dfo-mpo.gc.ca/library-bibliotheque/339096.pdf> ,
                                                      <https://waves-vagues.dfo-mpo.gc.ca/library-bibliotheque/41225260.pdf> ;
                                       rdfs:isDefinedBy <https://w3id.org/gcdfo/salmon> ;
                                       rdfs:label "Relative hatchery spawner abundance"@en ;
                                       gcdfo:theme gcdfo:SalmonEnhancementHatcheriesTheme ,
                                                   gcdfo:StockAssessmentTheme .


###  https://w3id.org/gcdfo/salmon#RelativeHatcherySpawnerAbundanceChange
gcdfo:RelativeHatcherySpawnerAbundanceChange rdf:type owl:Class ;
                                             rdfs:subClassOf gcdfo:RelativeSpawnerAbundanceChange ;
                                             <http://purl.obolibrary.org/obo/IAO_0000115> "A change metric (delta or percent change, as defined by the workflow) computed from relative hatchery-origin spawner abundance values over time; in rapid-status workflows, percent change is derived from log-transformed series and quantified over the most recent three generations."@en ;
                                             <http://purl.obolibrary.org/obo/IAO_0000119> "Fisheries and Oceans Canada. 2024. Rapid Status Approximations for Pacific Salmon… CSAS Pacific Region Science Response 2024/004 (definition and computation notes for percent change as a short-term trend over three generations)."@en ;
                                             dcterms:source <https://waves-vagues.dfo-mpo.gc.ca/library-bibliotheque/41225260.pdf> ;
                                             rdfs:isDefinedBy <https://w3id.org/gcdfo/salmon> ;
                                             rdfs:label "Relative hatchery spawner abundance change"@en ;
                                             gcdfo:theme gcdfo:SalmonEnhancementHatcheriesTheme ,
                                                         gcdfo:StockAssessmentTheme .


###  https://w3id.org/gcdfo/salmon#RelativeHatcherySpawnerAbundancePercentile
gcdfo:RelativeHatcherySpawnerAbundancePercentile rdf:type owl:Class ;
                                                 rdfs:subClassOf gcdfo:RelativeSpawnerAbundancePercentile ;
                                                 <http://purl.obolibrary.org/obo/IAO_0000115> "The percentile rank of relative hatchery-origin spawner abundance against a defined historical reference distribution."@en ;
                                                 <http://purl.obolibrary.org/obo/IAO_0000119> "Fisheries and Oceans Canada. 2024. Rapid Status Approximations… CSAS Science Response 2024/004 (percentile benchmarks discussion)."@en ;
                                                 dcterms:source <https://waves-vagues.dfo-mpo.gc.ca/library-bibliotheque/41225260.pdf> ;
                                                 rdfs:isDefinedBy <https://w3id.org/gcdfo/salmon> ;
                                                 rdfs:label "Relative hatchery spawner abundance percentile"@en ;
                                                 gcdfo:theme gcdfo:SalmonEnhancementHatcheriesTheme ,
                                                             gcdfo:StockAssessmentTheme .


###  https://w3id.org/gcdfo/salmon#RelativeHatcherySpawnerAbundanceTrend
gcdfo:RelativeHatcherySpawnerAbundanceTrend rdf:type owl:Class ;
                                            rdfs:subClassOf gcdfo:RelativeSpawnerAbundanceTrend ;
                                            <http://purl.obolibrary.org/obo/IAO_0000115> "A trend metric computed from relative hatchery-origin spawner abundance using a defined trend method; in rapid-status workflows, long-term trend is the ratio of current generational average (geometric mean) abundance to long-term average (geometric mean)."@en ;
                                            <http://purl.obolibrary.org/obo/IAO_0000119> "Fisheries and Oceans Canada. 2024. Rapid Status Approximations for Pacific Salmon… CSAS Pacific Region Science Response 2024/004 (long-term trend in abundance metric definition)."@en ;
                                            dcterms:source <https://waves-vagues.dfo-mpo.gc.ca/library-bibliotheque/41225260.pdf> ;
                                            rdfs:isDefinedBy <https://w3id.org/gcdfo/salmon> ;
                                            rdfs:label "Relative hatchery spawner abundance trend"@en ;
                                            gcdfo:theme gcdfo:SalmonEnhancementHatcheriesTheme ,
                                                        gcdfo:StockAssessmentTheme .


###  https://w3id.org/gcdfo/salmon#RelativeSpawnerAbundance
gcdfo:RelativeSpawnerAbundance rdf:type owl:Class ;
                               rdfs:subClassOf gcdfo:SpawnerAbundance ;
                               <http://purl.obolibrary.org/obo/IAO_0000115> "Spawner abundance expressed as a relative (dimensionless) abundance metric to a defined reference (commonly benchmarks), for within-series comparison; in rapid-status workflows, relative abundance is computed using the current generational average (geometric mean) divided by CU-specific lower and/or upper benchmarks."@en ;
                               <http://purl.obolibrary.org/obo/IAO_0000119> "Fisheries and Oceans Canada. 2024. Rapid Status Approximations for Pacific Salmon Derived from Integrated Expert Assessments under Fisheries and Oceans Canada Wild Salmon Policy. CSAS Pacific Region Science Response 2024/004 (relative abundance metric definition and computation)."@en ;
                               dcterms:source <https://waves-vagues.dfo-mpo.gc.ca/library-bibliotheque/41225260.pdf> ;
                               rdfs:isDefinedBy <https://w3id.org/gcdfo/salmon> ;
                               rdfs:label "Relative spawner abundance"@en ;
                               gcdfo:theme gcdfo:StockAssessmentTheme ,
                                           gcdfo:WildSalmonPolicyTheme .


###  https://w3id.org/gcdfo/salmon#RelativeSpawnerAbundanceChange
gcdfo:RelativeSpawnerAbundanceChange rdf:type owl:Class ;
                                     rdfs:subClassOf gcdfo:SpawnerAbundanceChange ;
                                     <http://purl.obolibrary.org/obo/IAO_0000115> "A change metric (delta or percent change, as defined by the workflow) computed from relative spawner abundance values over time; where rapid-status percent-change approaches are used, it represents change in abundance over the most recent three generations after log transformation (and smoothing where applicable)."@en ;
                                     <http://purl.obolibrary.org/obo/IAO_0000119> "Fisheries and Oceans Canada. 2024. Rapid Status Approximations for Pacific Salmon… CSAS Pacific Region Science Response 2024/004 (definition and computation notes for percent change as a short-term trend over three generations)."@en ;
                                     dcterms:source <https://waves-vagues.dfo-mpo.gc.ca/library-bibliotheque/41225260.pdf> ;
                                     rdfs:isDefinedBy <https://w3id.org/gcdfo/salmon> ;
                                     rdfs:label "Relative spawner abundance change"@en ;
                                     gcdfo:theme gcdfo:StockAssessmentTheme ,
                                                 gcdfo:WildSalmonPolicyTheme .


###  https://w3id.org/gcdfo/salmon#RelativeSpawnerAbundancePercentile
gcdfo:RelativeSpawnerAbundancePercentile rdf:type owl:Class ;
                                         rdfs:subClassOf gcdfo:SpawnerAbundancePercentile ;
                                         <http://purl.obolibrary.org/obo/IAO_0000115> "The percentile rank of relative spawner abundance against a defined historical reference distribution."@en ;
                                         <http://purl.obolibrary.org/obo/IAO_0000119> "Fisheries and Oceans Canada. 2024. Rapid Status Approximations… CSAS Science Response 2024/004 (percentile benchmarks discussion)."@en ;
                                         dcterms:source <https://waves-vagues.dfo-mpo.gc.ca/library-bibliotheque/41225260.pdf> ;
                                         rdfs:isDefinedBy <https://w3id.org/gcdfo/salmon> ;
                                         rdfs:label "Relative spawner abundance percentile"@en ;
                                         gcdfo:theme gcdfo:StockAssessmentTheme ,
                                                     gcdfo:WildSalmonPolicyTheme .


###  https://w3id.org/gcdfo/salmon#RelativeSpawnerAbundanceTrend
gcdfo:RelativeSpawnerAbundanceTrend rdf:type owl:Class ;
                                    rdfs:subClassOf gcdfo:SpawnerAbundanceTrend ;
                                    <http://purl.obolibrary.org/obo/IAO_0000115> "A long-term trend metric expressed as the ratio of the current generational average (geometric mean) spawner abundance to the long-term average (geometric mean), yielding a dimensionless measure of relative abundance through time."@en ;
                                    <http://purl.obolibrary.org/obo/IAO_0000119> "Fisheries and Oceans Canada. 2024. Rapid Status Approximations for Pacific Salmon… CSAS Pacific Region Science Response 2024/004 (long-term trend in abundance defined as ratio of current generational average to long-term average)."@en ;
                                    dcterms:source <https://waves-vagues.dfo-mpo.gc.ca/library-bibliotheque/41225260.pdf> ;
                                    rdfs:isDefinedBy <https://w3id.org/gcdfo/salmon> ;
                                    rdfs:label "Relative spawner abundance trend"@en ;
                                    gcdfo:theme gcdfo:StockAssessmentTheme ,
                                                gcdfo:WildSalmonPolicyTheme .


###  https://w3id.org/gcdfo/salmon#RelativeWildSpawnerAbundance
gcdfo:RelativeWildSpawnerAbundance rdf:type owl:Class ;
                                   rdfs:subClassOf gcdfo:RelativeSpawnerAbundance ;
                                   <http://purl.obolibrary.org/obo/IAO_0000115> "Natural-origin (wild) spawner abundance expressed as a relative (dimensionless) abundance metric to a defined reference (commonly benchmarks), for within-series comparison; where WSP-style relative abundance is used, it is computed using current generational averages (geometric mean) relative to CU-specific benchmarks."@en ;
                                   <http://purl.obolibrary.org/obo/IAO_0000119> "Fisheries and Oceans Canada. 2024. Rapid Status Approximations for Pacific Salmon… CSAS Pacific Region Science Response 2024/004 (relative abundance metric definition). Holt et al. 2009. Indicators of Status and Benchmarks for Conservation Units in Canada's Wild Salmon Policy. CSAS Res. Doc. 2009/058 (wild vs hatchery-origin considerations in spawner series context)."@en ;
                                   dcterms:source <https://waves-vagues.dfo-mpo.gc.ca/library-bibliotheque/339096.pdf> ,
                                                  <https://waves-vagues.dfo-mpo.gc.ca/library-bibliotheque/41225260.pdf> ;
                                   rdfs:isDefinedBy <https://w3id.org/gcdfo/salmon> ;
                                   rdfs:label "Relative wild spawner abundance"@en ;
                                   gcdfo:theme gcdfo:StockAssessmentTheme ,
                                               gcdfo:WildSalmonPolicyTheme .


###  https://w3id.org/gcdfo/salmon#RelativeWildSpawnerAbundanceChange
gcdfo:RelativeWildSpawnerAbundanceChange rdf:type owl:Class ;
                                         rdfs:subClassOf gcdfo:RelativeSpawnerAbundanceChange ;
                                         <http://purl.obolibrary.org/obo/IAO_0000115> "A change metric (delta or percent change, as defined by the workflow) computed from relative natural-origin spawner abundance values over time; in rapid-status workflows, percent change is defined over the most recent three generations using log-transformed abundance series."@en ;
                                         <http://purl.obolibrary.org/obo/IAO_0000119> "Fisheries and Oceans Canada. 2024. Rapid Status Approximations for Pacific Salmon… CSAS Pacific Region Science Response 2024/004 (definition and computation notes for percent change over the most recent three generations)."@en ;
                                         dcterms:source <https://waves-vagues.dfo-mpo.gc.ca/library-bibliotheque/41225260.pdf> ;
                                         rdfs:isDefinedBy <https://w3id.org/gcdfo/salmon> ;
                                         rdfs:label "Relative wild spawner abundance change"@en ;
                                         gcdfo:theme gcdfo:StockAssessmentTheme ,
                                                     gcdfo:WildSalmonPolicyTheme .


###  https://w3id.org/gcdfo/salmon#RelativeWildSpawnerAbundancePercentile
gcdfo:RelativeWildSpawnerAbundancePercentile rdf:type owl:Class ;
                                             rdfs:subClassOf gcdfo:RelativeSpawnerAbundancePercentile ;
                                             <http://purl.obolibrary.org/obo/IAO_0000115> "The percentile rank of relative natural-origin spawner abundance against a defined historical reference distribution."@en ;
                                             <http://purl.obolibrary.org/obo/IAO_0000119> "Fisheries and Oceans Canada. 2024. Rapid Status Approximations… CSAS Science Response 2024/004 (percentile benchmarks discussion)."@en ;
                                             dcterms:source <https://waves-vagues.dfo-mpo.gc.ca/library-bibliotheque/41225260.pdf> ;
                                             rdfs:isDefinedBy <https://w3id.org/gcdfo/salmon> ;
                                             rdfs:label "Relative wild spawner abundance percentile"@en ;
                                             gcdfo:theme gcdfo:StockAssessmentTheme ,
                                                         gcdfo:WildSalmonPolicyTheme .


###  https://w3id.org/gcdfo/salmon#RelativeWildSpawnerAbundanceTrend
gcdfo:RelativeWildSpawnerAbundanceTrend rdf:type owl:Class ;
                                        rdfs:subClassOf gcdfo:RelativeSpawnerAbundanceTrend ;
                                        <http://purl.obolibrary.org/obo/IAO_0000115> "A trend metric computed from relative natural-origin spawner abundance using a defined trend method; in rapid-status workflows, long-term trend is the ratio of current generational average (geometric mean) abundance to long-term average (geometric mean)."@en ;
                                        <http://purl.obolibrary.org/obo/IAO_0000119> "Fisheries and Oceans Canada. 2024. Rapid Status Approximations for Pacific Salmon… CSAS Pacific Region Science Response 2024/004 (long-term trend in abundance metric definition)."@en ;
                                        dcterms:source <https://waves-vagues.dfo-mpo.gc.ca/library-bibliotheque/41225260.pdf> ;
                                        rdfs:isDefinedBy <https://w3id.org/gcdfo/salmon> ;
                                        rdfs:label "Relative wild spawner abundance trend"@en ;
                                        gcdfo:theme gcdfo:StockAssessmentTheme ,
                                                    gcdfo:WildSalmonPolicyTheme .


###  https://w3id.org/gcdfo/salmon#ReportingOrManagementStratum
gcdfo:ReportingOrManagementStratum rdf:type owl:Class ;
                                   rdfs:subClassOf <http://purl.obolibrary.org/obo/IAO_0000030> ;
                                   <http://purl.obolibrary.org/obo/IAO_0000115> "An information-defined grouping of fish populations used for reporting, conservation assessment, or management purposes. Examples include Conservation Units (CUs), Stock Management Units (MUs), and Designatable Units (DUs)."@en ;
                                   rdfs:isDefinedBy <https://w3id.org/gcdfo/salmon> ;
                                   rdfs:label "Reporting or management stratum"@en ;
                                   skos:closeMatch sosa:FeatureOfInterest ;
                                   gcdfo:theme gcdfo:PolicyGovernanceTheme ,
                                               gcdfo:StockAssessmentTheme .


###  https://w3id.org/gcdfo/salmon#ReturnYear
gcdfo:ReturnYear rdf:type owl:Class ;
                 rdfs:subClassOf gcdfo:YearBasis ;
                 <http://purl.obolibrary.org/obo/IAO_0000115> "The calendar year in which adult salmon return from the ocean to freshwater systems (a year basis used to contextualize run/return-related measurements)."@en ;
                 <http://purl.obolibrary.org/obo/IAO_0000119> "Fisheries and Oceans Canada. Pacific Salmon Glossary (Pacific Region web page)."@en ;
                 dcterms:source <https://www.pac.dfo-mpo.gc.ca/fm-gp/salmon-saumon/gloss-eng.html> ;
                 rdfs:isDefinedBy <https://w3id.org/gcdfo/salmon> ;
                 rdfs:label "Return year"@en ;
                 gcdfo:theme gcdfo:FisheriesManagementTheme ,
                             gcdfo:StockAssessmentTheme ,
                             gcdfo:WildSalmonPolicyTheme .


###  https://w3id.org/gcdfo/salmon#SalmonDataVariable
gcdfo:SalmonDataVariable rdf:type owl:Class ;
                         rdfs:subClassOf <http://purl.obolibrary.org/obo/IAO_0000030> ;
                         <http://purl.obolibrary.org/obo/IAO_0000115> "A variable specification used to decompose a measured salmon-data quantity into semantic components (object of interest, property, and optional constraints/modifiers), following the I-ADOPT variable pattern for SDP metadata workflows."@en ;
                         rdfs:isDefinedBy <https://w3id.org/gcdfo/salmon> ;
                         rdfs:label "Salmon data variable"@en ;
                         skos:closeMatch sosa:Property ,
                                         iop:Variable ;
                         gcdfo:theme gcdfo:DataModelProvenanceTheme ,
                                     gcdfo:StockAssessmentTheme .


###  https://w3id.org/gcdfo/salmon#SpawnerAbundance
gcdfo:SpawnerAbundance rdf:type owl:Class ;
                       rdfs:subClassOf gcdfo:ObservedRateOrAbundance ;
                       <http://purl.obolibrary.org/obo/IAO_0000115> "The abundance (count) of adult salmon that reach spawning grounds in a given system and time period (often operationalized as escapement/spawning escapement)."@en ;
                       <http://purl.obolibrary.org/obo/IAO_0000119> "Fisheries and Oceans Canada. Pacific Salmon Glossary (defines escapement/spawning escapement as the number of salmon returning to the spawning grounds)."@en ;
                       dcterms:source <https://www.pac.dfo-mpo.gc.ca/fm-gp/salmon-saumon/gloss-eng.html> ;
                       rdfs:isDefinedBy <https://w3id.org/gcdfo/salmon> ;
                       rdfs:label "Spawner abundance"@en ;
                       skos:altLabel "Escapement (count)"@en ;
                       skos:closeMatch odo:SALMON_00000479 ;
                       gcdfo:theme gcdfo:StockAssessmentTheme ,
                                   gcdfo:WildSalmonPolicyTheme .


###  https://w3id.org/gcdfo/salmon#SpawnerAbundanceChange
gcdfo:SpawnerAbundanceChange rdf:type owl:Class ;
                             rdfs:subClassOf gcdfo:ObservedRateOrAbundance ;
                             <http://purl.obolibrary.org/obo/IAO_0000115> "A change metric (delta or percent change, as defined by the workflow) computed from spawner abundance values over time; in rapid-status workflows, percent change is quantified as a linear change in log-transformed abundance over the most recent three generations."@en ;
                             <http://purl.obolibrary.org/obo/IAO_0000119> "Fisheries and Oceans Canada. 2024. Rapid Status Approximations for Pacific Salmon… CSAS Pacific Region Science Response 2024/004 (percent change definition and computation notes). COSEWIC. 2017. Sockeye Salmon assessment and status report (log-linear rate-of-change model and percent-change derivation over three generations)."@en ;
                             dcterms:source <https://waves-vagues.dfo-mpo.gc.ca/library-bibliotheque/41225260.pdf> ,
                                            <https://www.canada.ca/en/environment-climate-change/services/species-risk-public-registry/cosewic-assessments-status-reports/sockeye-salmon-2017.html> ;
                             rdfs:isDefinedBy <https://w3id.org/gcdfo/salmon> ;
                             rdfs:label "Spawner abundance change"@en ;
                             gcdfo:theme gcdfo:StockAssessmentTheme ,
                                         gcdfo:WildSalmonPolicyTheme .


###  https://w3id.org/gcdfo/salmon#SpawnerAbundancePercentile
gcdfo:SpawnerAbundancePercentile rdf:type owl:Class ;
                                 rdfs:subClassOf gcdfo:ObservedRateOrAbundance ;
                                 <http://purl.obolibrary.org/obo/IAO_0000115> "The percentile rank of a spawner abundance value (annual or period-specific) against a defined historical reference distribution."@en ;
                                 <http://purl.obolibrary.org/obo/IAO_0000119> "Fisheries and Oceans Canada. 2024. Rapid Status Approximations… CSAS Science Response 2024/004 (percentile benchmarks discussion)."@en ;
                                 dcterms:source <https://waves-vagues.dfo-mpo.gc.ca/library-bibliotheque/41225260.pdf> ;
                                 rdfs:isDefinedBy <https://w3id.org/gcdfo/salmon> ;
                                 rdfs:label "Spawner abundance percentile"@en ;
                                 gcdfo:theme gcdfo:StockAssessmentTheme ,
                                             gcdfo:WildSalmonPolicyTheme .


###  https://w3id.org/gcdfo/salmon#SpawnerAbundanceTrend
gcdfo:SpawnerAbundanceTrend rdf:type owl:Class ;
                            rdfs:subClassOf gcdfo:ObservedRateOrAbundance ;
                            <http://purl.obolibrary.org/obo/IAO_0000115> "A trend metric computed from spawner abundance over time using a defined trend method (e.g., slope over a specified window)."@en ;
                            <http://purl.obolibrary.org/obo/IAO_0000119> "Derived for SPSR term coverage; distinct from gcdfo:LongTermTrendMetric (current generational average vs long-term average) in CSAS Science Response 2024/004."@en ;
                            dcterms:source <https://waves-vagues.dfo-mpo.gc.ca/library-bibliotheque/41225260.pdf> ;
                            rdfs:isDefinedBy <https://w3id.org/gcdfo/salmon> ;
                            rdfs:label "Spawner abundance trend"@en ;
                            gcdfo:theme gcdfo:StockAssessmentTheme ,
                                        gcdfo:WildSalmonPolicyTheme .


###  https://w3id.org/gcdfo/salmon#Stock
gcdfo:Stock rdf:type owl:Class ;
            rdfs:subClassOf gcdfo:ReportingOrManagementStratum ;
            <http://purl.obolibrary.org/obo/IAO_0000115> "An operationally-defined grouping of salmon used for assessment and management purposes. A stock is a management unit or reporting stratum, not a biological organism."@en ;
            <http://purl.obolibrary.org/obo/IAO_0000119> "Fisheries and Oceans Canada. Introduction to Stock Assessment - Glossary. https://www.dfo-mpo.gc.ca/science/species-especes/fisheries-halieutiques/assessment-evaluation/glossary-glossaire/index-eng.html."@en ;
            dcterms:source <https://www.dfo-mpo.gc.ca/science/species-especes/fisheries-halieutiques/assessment-evaluation/glossary-glossaire/index-eng.html> ;
            rdfs:isDefinedBy <https://w3id.org/gcdfo/salmon> ;
            rdfs:label "Stock"@en ;
            skos:altLabel "Fish stock"@en ;
            gcdfo:theme gcdfo:FisheriesManagementTheme ,
                        gcdfo:PolicyGovernanceTheme ,
                        gcdfo:StockAssessmentTheme .


###  https://w3id.org/gcdfo/salmon#StockAssessment
gcdfo:StockAssessment rdf:type owl:Class ;
                      rdfs:subClassOf <http://purl.obolibrary.org/obo/BFO_0000015> ;
                      <http://purl.obolibrary.org/obo/IAO_0000115> "The scientific process of analyzing data to estimate the abundance and productivity of fish stocks in the past, present, and future. It is the backbone of successful science-based fisheries management"@en ;
                      <http://purl.obolibrary.org/obo/IAO_0000119> "Fisheries and Oceans Canada. Introduction to Stock Assessment. https://www.dfo-mpo.gc.ca/science/species-especes/fisheries-halieutiques/assessment-evaluation/module-1/09-eng.html."@en ;
                      dcterms:source <https://www.dfo-mpo.gc.ca/science/species-especes/fisheries-halieutiques/assessment-evaluation/module-1/09-eng.html> ;
                      rdfs:isDefinedBy <https://w3id.org/gcdfo/salmon> ;
                      rdfs:label "Stock assessment"@en ;
                      gcdfo:theme gcdfo:StockAssessmentTheme .


###  https://w3id.org/gcdfo/salmon#StockManagementUnit
gcdfo:StockManagementUnit rdf:type owl:Class ;
                          rdfs:subClassOf gcdfo:ReportingOrManagementStratum ;
                          <http://purl.obolibrary.org/obo/IAO_0000115> "A collection of stocks that are managed together with a joint stock status."@en ;
                          <http://purl.obolibrary.org/obo/IAO_0000119> "Fisheries and Oceans Canada. Introduction to Stock Assessment - Glossary. https://www.dfo-mpo.gc.ca/science/species-especes/fisheries-halieutiques/assessment-evaluation/glossary-glossaire/index-eng.html."@en ;
                          dcterms:source <https://www.dfo-mpo.gc.ca/science/species-especes/fisheries-halieutiques/assessment-evaluation/glossary-glossaire/index-eng.html> ;
                          rdfs:isDefinedBy <https://w3id.org/gcdfo/salmon> ;
                          rdfs:label "Stock Management Unit"@en ;
                          skos:altLabel "SMU"@en ;
                          gcdfo:theme gcdfo:FisheriesManagementTheme ,
                                      gcdfo:PolicyGovernanceTheme ,
                                      gcdfo:StockAssessmentTheme .


###  https://w3id.org/gcdfo/salmon#SurveyEvent
gcdfo:SurveyEvent rdf:type owl:Class ;
                  rdfs:subClassOf dwc:Event ,
                                  prov:Activity ;
                  <http://purl.obolibrary.org/obo/IAO_0000115> "A field event that collects information about key fish stocks to track their status, and track progress to implement fishery policies and measures for these stocks."@en ;
                  <http://purl.obolibrary.org/obo/IAO_0000119> "Fisheries and Oceans Canada. About the Sustainability Survey for Fisheries. https://www.dfo-mpo.gc.ca/reports-rapports/regs/sff-cpd/survey-sondage/about-propos-en.html."@en ;
                  dcterms:source <https://www.dfo-mpo.gc.ca/reports-rapports/regs/sff-cpd/survey-sondage/about-propos-en.html> ;
                  rdfs:isDefinedBy <https://w3id.org/gcdfo/salmon> ;
                  rdfs:label "Survey event"@en ;
                  skos:closeMatch sosa:Sampling ;
                  gcdfo:theme gcdfo:MonitoringFieldWorkTheme ,
                              gcdfo:StockAssessmentTheme .


###  https://w3id.org/gcdfo/salmon#TargetOrLimitExploitationRate
gcdfo:TargetOrLimitExploitationRate rdf:type owl:Class ;
                                    rdfs:subClassOf gcdfo:ExploitationRate ,
                                                    gcdfo:TargetOrLimitRateOrAbundance ;
                                    <http://purl.obolibrary.org/obo/IAO_0000115> "A policy- or management-defined exploitation-rate value used as a target, threshold, or limit reference in decision rules."@en ;
                                    <http://purl.obolibrary.org/obo/IAO_0000119> "Fisheries and Oceans Canada. Introduction to Stock Assessment - Glossary. https://www.dfo-mpo.gc.ca/science/species-especes/fisheries-halieutiques/assessment-evaluation/glossary-glossaire/index-eng.html."@en ;
                                    dcterms:source <https://www.dfo-mpo.gc.ca/science/species-especes/fisheries-halieutiques/assessment-evaluation/glossary-glossaire/index-eng.html> ;
                                    rdfs:isDefinedBy <https://w3id.org/gcdfo/salmon> ;
                                    rdfs:label "Target or limit exploitation rate"@en ;
                                    gcdfo:theme gcdfo:FisheriesManagementTheme ,
                                                gcdfo:PolicyGovernanceTheme ,
                                                gcdfo:StockAssessmentTheme .


###  https://w3id.org/gcdfo/salmon#TargetOrLimitRateOrAbundance
gcdfo:TargetOrLimitRateOrAbundance rdf:type owl:Class ;
                                   rdfs:subClassOf <http://purl.obolibrary.org/obo/IAO_0000109> ;
                                   <http://purl.obolibrary.org/obo/IAO_0000115> "A value specification representing a policy- or model-defined target or limit, such as TAC or UMSY."@en ;
                                   rdfs:isDefinedBy <https://w3id.org/gcdfo/salmon> ;
                                   rdfs:label "Target or limit rate or abundance"@en ;
                                   gcdfo:theme gcdfo:DataModelProvenanceTheme ,
                                               gcdfo:PolicyGovernanceTheme ,
                                               gcdfo:StockAssessmentTheme .


###  https://w3id.org/gcdfo/salmon#TerminalMortalityRate
gcdfo:TerminalMortalityRate rdf:type owl:Class ;
                            rdfs:subClassOf gcdfo:ObservedRateOrAbundance ;
                            <http://purl.obolibrary.org/obo/IAO_0000115> "The proportion of fish that die after reaching terminal spawning areas (or immediate vicinity) but before successfully spawning, as defined by the assessment workflow (i.e., pre-spawn mortality in terminal areas)."@en ;
                            <http://purl.obolibrary.org/obo/IAO_0000119> "COSEWIC. 2017. Sockeye Salmon (Oncorhynchus nerka) assessment and status report (pre-spawn mortality includes fish that made it to spawning grounds but did not successfully spawn). LGL Limited. Migration and Survival of Late-run Fraser Sockeye (operational identification of pre-spawn mortalities from spawning-area detections)."@en ;
                            dcterms:source <https://waves-vagues.dfo-mpo.gc.ca/library-bibliotheque/341440.pdf> ,
                                           <https://www.canada.ca/en/environment-climate-change/services/species-risk-public-registry/cosewic-assessments-status-reports/sockeye-salmon-2017.html> ;
                            rdfs:isDefinedBy <https://w3id.org/gcdfo/salmon> ;
                            rdfs:label "Terminal mortality rate"@en ;
                            gcdfo:theme gcdfo:StockAssessmentTheme .


###  https://w3id.org/gcdfo/salmon#TotalExploitationRate
gcdfo:TotalExploitationRate rdf:type owl:Class ;
                            rdfs:subClassOf gcdfo:ObservedExploitationRate ;
                            <http://purl.obolibrary.org/obo/IAO_0000115> "The overall proportion of the total return of adult salmon removed by all fisheries over a defined period, aggregating across gear or fishery components."@en ;
                            rdfs:isDefinedBy <https://w3id.org/gcdfo/salmon> ;
                            rdfs:label "Total exploitation rate"@en ;
                            gcdfo:theme gcdfo:FisheriesManagementTheme ,
                                        gcdfo:StockAssessmentTheme .


###  https://w3id.org/gcdfo/salmon#TotalMortalityRate
gcdfo:TotalMortalityRate rdf:type owl:Class ;
                         rdfs:subClassOf gcdfo:ObservedRateOrAbundance ;
                         <http://purl.obolibrary.org/obo/IAO_0000115> "The overall proportion of fish in a defined cohort that die over the full assessment interval across all included phases and mortality sources, consistent with the workflow’s accounting (e.g., catch vs escapement vs migration losses where relevant)."@en ;
                         <http://purl.obolibrary.org/obo/IAO_0000119> "Fisheries and Oceans Canada. 2025. Stock-Specific Fraser River Sockeye Salmon Run Size Determination. CSAS Pacific Region Science Advisory Report 2025/021 (run size components include catch, spawning escapement, and en route mortality; other Pacific salmon run sizes typically sum catch + escapement). COSEWIC. 2017. Sockeye Salmon assessment and status report (uses catch, escapement, and en-route loss as distinct accounting components)."@en ;
                         dcterms:source <https://waves-vagues.dfo-mpo.gc.ca/library-bibliotheque/41294622.pdf> ,
                                        <https://www.canada.ca/en/environment-climate-change/services/species-risk-public-registry/cosewic-assessments-status-reports/sockeye-salmon-2017.html> ;
                         rdfs:isDefinedBy <https://w3id.org/gcdfo/salmon> ;
                         rdfs:label "Total mortality rate"@en ;
                         gcdfo:theme gcdfo:StockAssessmentTheme .


###  https://w3id.org/gcdfo/salmon#UpperBiologicalBenchmark
gcdfo:UpperBiologicalBenchmark rdf:type owl:Class ;
                               rdfs:subClassOf gcdfo:MetricBenchmark ;
                               <http://purl.obolibrary.org/obo/IAO_0000115> "Upper benchmark value for a metric used to delineate Wild Salmon Policy status zones (typically the boundary between Amber and Green zones)."@en ;
                               <http://purl.obolibrary.org/obo/IAO_0000119> "Fisheries and Oceans Canada. Wild Salmon Policy 2018-2022 Implementation Plan. https://waves-vagues.dfo-mpo.gc.ca/library-bibliotheque/40728109.pdf."@en ;
                               dcterms:source <https://waves-vagues.dfo-mpo.gc.ca/library-bibliotheque/40728109.pdf> ;
                               rdfs:isDefinedBy <https://w3id.org/gcdfo/salmon> ;
                               rdfs:label "Upper biological benchmark"@en ;
                               gcdfo:theme gcdfo:PolicyGovernanceTheme ,
                                           gcdfo:StockAssessmentTheme ,
                                           gcdfo:WildSalmonPolicyTheme .


###  https://w3id.org/gcdfo/salmon#UpperStockReferencePoint
gcdfo:UpperStockReferencePoint rdf:type owl:Class ;
                               rdfs:subClassOf gcdfo:ReferencePoint ;
                               <http://purl.obolibrary.org/obo/IAO_0000115> "A threshold below which fishing must be reduced to avoid reaching the LRP. The USR must be set at an appropriate distance above the LRP to provide sufficient opportunity for managers to recognize a declining stock status and sufficient time for management actions to take effect. "@en ;
                               <http://purl.obolibrary.org/obo/IAO_0000119> "Fisheries and Oceans Canada. Introduction to Stock Assessment - Glossary. https://www.dfo-mpo.gc.ca/science/species-especes/fisheries-halieutiques/assessment-evaluation/glossary-glossaire/index-eng.html."@en ;
                               dcterms:source <https://www.dfo-mpo.gc.ca/science/species-especes/fisheries-halieutiques/assessment-evaluation/glossary-glossaire/index-eng.html> ;
                               rdfs:isDefinedBy <https://w3id.org/gcdfo/salmon> ;
                               rdfs:label "Upper stock reference"@en ;
                               skos:altLabel "USR"@en ;
                               gcdfo:theme gcdfo:FisheriesManagementTheme ,
                                           gcdfo:PolicyGovernanceTheme ,
                                           gcdfo:StockAssessmentTheme .


###  https://w3id.org/gcdfo/salmon#WSPBiologicalStatusZone
gcdfo:WSPBiologicalStatusZone rdf:type owl:Class .


###  https://w3id.org/gcdfo/salmon#WSPRapidStatus
gcdfo:WSPRapidStatus rdf:type owl:Class ;
                     rdfs:subClassOf <http://purl.obolibrary.org/obo/IAO_0000030> ;
                     <http://purl.obolibrary.org/obo/IAO_0000115> "The WSP rapid status assessment approach builds on previously completed WSP integrated status assessments. The WSP rapid status approach ensures statuses are scientifically objective, consistent, and comparable across BC/Yukon CUs. This approach is also relatively easy to implement, applicable to data rich and data poor CUs, and can be updated annually."@en ;
                     <http://purl.obolibrary.org/obo/IAO_0000119> "Pestal, G., MacDonald, B.L., Grant, S.C.H., and Holt, C.A. 2023. State of the salmon: rapid status assessment approach for Pacific salmon under Canada's Wild Salmon Policy. Canadian Technical Report of Fisheries and Aquatic Sciences 3570."@en ;
                     dcterms:source <https://publications.gc.ca/site/eng/9.928944/publication.html> ;
                     rdfs:isDefinedBy <https://w3id.org/gcdfo/salmon> ;
                     rdfs:label "WSP rapid status"@en ;
                     gcdfo:theme gcdfo:PolicyGovernanceTheme ,
                                 gcdfo:StockAssessmentTheme ,
                                 gcdfo:WildSalmonPolicyTheme .


###  https://w3id.org/gcdfo/salmon#WSPRapidStatusAlgorithmThreshold
gcdfo:WSPRapidStatusAlgorithmThreshold rdf:type owl:Class ;
                                       rdfs:subClassOf <http://purl.obolibrary.org/obo/IAO_0000030> ;
                                       <http://purl.obolibrary.org/obo/IAO_0000115> "Threshold value used by the rapid-status algorithm that may differ from expert-defined benchmarks to incorporate precautionary buffers."@en ;
                                       <http://purl.obolibrary.org/obo/IAO_0000119> "Fisheries and Oceans Canada. 2024. Rapid Status Approximations for Pacific Salmon Derived from Integrated Expert Assessments under Fisheries and Oceans Canada Wild Salmon Policy. DFO Canadian Science Advisory Secretariat Science Response 2024/004."@en ;
                                       dcterms:source <https://www.dfo-mpo.gc.ca/csas-sccs/Publications/ScR-RS/2024/2024_004-eng.html> ;
                                       rdfs:isDefinedBy <https://w3id.org/gcdfo/salmon> ;
                                       rdfs:label "Rapid-status algorithm threshold"@en ;
                                       gcdfo:theme gcdfo:StockAssessmentTheme ,
                                                   gcdfo:WildSalmonPolicyTheme .


###  https://w3id.org/gcdfo/salmon#YearBasis
gcdfo:YearBasis rdf:type owl:Class ;
                rdfs:subClassOf <http://purl.obolibrary.org/obo/IAO_0000030> ;
                <http://purl.obolibrary.org/obo/IAO_0000115> "A year-based temporal reference used to contextualize measurements or rates (e.g., brood year, catch year, or return year)."@en ;
                rdfs:isDefinedBy <https://w3id.org/gcdfo/salmon> ;
                rdfs:label "Year basis"@en ;
                gcdfo:theme gcdfo:StockAssessmentTheme .


###  https://w3id.org/iadopt/ont/Constraint
iop:Constraint rdf:type owl:Class .


###  https://w3id.org/iadopt/ont/Entity
iop:Entity rdf:type owl:Class .


###  https://w3id.org/iadopt/ont/Property
iop:Property rdf:type owl:Class .


###  https://w3id.org/iadopt/ont/StatisticalModifier
iop:StatisticalModifier rdf:type owl:Class .


#################################################################
#    Individuals
#################################################################

###  https://w3id.org/gcdfo/salmon#AbundanceDataType
gcdfo:AbundanceDataType rdf:type owl:NamedIndividual ,
                                 skos:Concept ;
                        <http://purl.obolibrary.org/obo/IAO_0000115> "A categorical attribute indicating whether an abundance time series is recorded as absolute abundance or as a relative index (used by rapid-status workflows)."@en ;
                        <http://purl.obolibrary.org/obo/IAO_0000119> "Fisheries and Oceans Canada. 2024. Rapid Status Approximations for Pacific Salmon Derived from Integrated Expert Assessments under DFO’s Wild Salmon Policy. CSAS Pacific Region Science Response 2024/004."@en ;
                        dcterms:source <https://waves-vagues.dfo-mpo.gc.ca/library-bibliotheque/41225260.pdf> ;
                        rdfs:isDefinedBy <https://w3id.org/gcdfo/salmon> ;
                        skos:broader gcdfo:MeasurementContext ;
                        skos:definition "A categorical attribute indicating whether an abundance time series is recorded as absolute abundance or as a relative index (used by rapid-status workflows)."@en ;
                        skos:inScheme gcdfo:MeasurementContextScheme ;
                        skos:prefLabel "Abundance data type"@en ;
                        skos:scopeNote "In SPSR rapid-status workflows, this field distinguishes absolute abundance vs relative index inputs (often abbreviated in code as 'Abs_Abd' and 'RelIdx')."@en ;
                        gcdfo:theme gcdfo:DataModelProvenanceTheme ,
                                    gcdfo:StockAssessmentTheme ,
                                    gcdfo:WildSalmonPolicyTheme .


###  https://w3id.org/gcdfo/salmon#AerialSurveyCount
gcdfo:AerialSurveyCount rdf:type owl:NamedIndividual ,
                                 skos:Concept ;
                        rdfs:comment "Legacy methods: Helicopter, Fixed Wing Aircraft, Aerial, Drone, UAS, UAV"@en ;
                        rdfs:isDefinedBy <https://w3id.org/gcdfo/salmon> ;
                        skos:broader gcdfo:EnumerationMethod ;
                        skos:definition "Overflights (helicopter, fixed wing, or drone) with documented flight lines, coverage, visibility, and sensor settings. Imagery may be reviewed post-flight."@en ;
                        skos:inScheme gcdfo:EnumerationMethodScheme ;
                        skos:prefLabel "Aerial Survey Count"@en ;
                        gcdfo:theme gcdfo:MonitoringFieldWorkTheme ,
                                    gcdfo:StockAssessmentTheme .


###  https://w3id.org/gcdfo/salmon#Age1YearClass
gcdfo:Age1YearClass rdf:type owl:NamedIndividual ,
                             skos:Concept ;
                    rdfs:isDefinedBy <https://w3id.org/gcdfo/salmon> ;
                    skos:broader gcdfo:AgeClassValue ;
                    skos:definition "Age class value 1 year."@en ;
                    skos:inScheme gcdfo:AgeClassValueScheme ;
                    skos:notation 1 ;
                    skos:prefLabel "Age 1 year class"@en ;
                    gcdfo:theme gcdfo:StockAssessmentTheme .


###  https://w3id.org/gcdfo/salmon#Age2YearClass
gcdfo:Age2YearClass rdf:type owl:NamedIndividual ,
                             skos:Concept ;
                    rdfs:isDefinedBy <https://w3id.org/gcdfo/salmon> ;
                    skos:broader gcdfo:AgeClassValue ;
                    skos:definition "Age class value 2 years."@en ;
                    skos:inScheme gcdfo:AgeClassValueScheme ;
                    skos:notation 2 ;
                    skos:prefLabel "Age 2 year class"@en ;
                    gcdfo:theme gcdfo:StockAssessmentTheme .


###  https://w3id.org/gcdfo/salmon#Age3YearClass
gcdfo:Age3YearClass rdf:type owl:NamedIndividual ,
                             skos:Concept ;
                    rdfs:isDefinedBy <https://w3id.org/gcdfo/salmon> ;
                    skos:broader gcdfo:AgeClassValue ;
                    skos:definition "Age class value 3 years."@en ;
                    skos:inScheme gcdfo:AgeClassValueScheme ;
                    skos:notation 3 ;
                    skos:prefLabel "Age 3 year class"@en ;
                    gcdfo:theme gcdfo:StockAssessmentTheme .


###  https://w3id.org/gcdfo/salmon#Age4YearClass
gcdfo:Age4YearClass rdf:type owl:NamedIndividual ,
                             skos:Concept ;
                    rdfs:isDefinedBy <https://w3id.org/gcdfo/salmon> ;
                    skos:broader gcdfo:AgeClassValue ;
                    skos:definition "Age class value 4 years."@en ;
                    skos:inScheme gcdfo:AgeClassValueScheme ;
                    skos:notation 4 ;
                    skos:prefLabel "Age 4 year class"@en ;
                    gcdfo:theme gcdfo:StockAssessmentTheme .


###  https://w3id.org/gcdfo/salmon#Age5YearClass
gcdfo:Age5YearClass rdf:type owl:NamedIndividual ,
                             skos:Concept ;
                    rdfs:isDefinedBy <https://w3id.org/gcdfo/salmon> ;
                    skos:broader gcdfo:AgeClassValue ;
                    skos:definition "Age class value 5 years."@en ;
                    skos:inScheme gcdfo:AgeClassValueScheme ;
                    skos:notation 5 ;
                    skos:prefLabel "Age 5 year class"@en ;
                    gcdfo:theme gcdfo:StockAssessmentTheme .


###  https://w3id.org/gcdfo/salmon#Age6YearClass
gcdfo:Age6YearClass rdf:type owl:NamedIndividual ,
                             skos:Concept ;
                    rdfs:isDefinedBy <https://w3id.org/gcdfo/salmon> ;
                    skos:broader gcdfo:AgeClassValue ;
                    skos:definition "Age class value 6 years."@en ;
                    skos:inScheme gcdfo:AgeClassValueScheme ;
                    skos:notation 6 ;
                    skos:prefLabel "Age 6 year class"@en ;
                    gcdfo:theme gcdfo:StockAssessmentTheme .


###  https://w3id.org/gcdfo/salmon#Age7YearClass
gcdfo:Age7YearClass rdf:type owl:NamedIndividual ,
                             skos:Concept ;
                    rdfs:isDefinedBy <https://w3id.org/gcdfo/salmon> ;
                    skos:broader gcdfo:AgeClassValue ;
                    skos:definition "Age class value 7 years."@en ;
                    skos:inScheme gcdfo:AgeClassValueScheme ;
                    skos:notation 7 ;
                    skos:prefLabel "Age 7 year class"@en ;
                    gcdfo:theme gcdfo:StockAssessmentTheme .


###  https://w3id.org/gcdfo/salmon#AgeAtMaturityBasis
gcdfo:AgeAtMaturityBasis rdf:type owl:NamedIndividual ,
                                  skos:Concept ;
                         rdfs:isDefinedBy <https://w3id.org/gcdfo/salmon> ;
                         skos:broader gcdfo:AgeBasis ;
                         skos:definition "Age measured at maturity."@en ;
                         skos:inScheme gcdfo:AgeBasisScheme ;
                         skos:prefLabel "Age at maturity basis"@en ;
                         gcdfo:theme gcdfo:DataModelProvenanceTheme ,
                                     gcdfo:StockAssessmentTheme .


###  https://w3id.org/gcdfo/salmon#AgeAtReturnBasis
gcdfo:AgeAtReturnBasis rdf:type owl:NamedIndividual ,
                                skos:Concept ;
                       rdfs:isDefinedBy <https://w3id.org/gcdfo/salmon> ;
                       skos:broader gcdfo:AgeBasis ;
                       skos:definition "Age measured at return migration (adult return timing)."@en ;
                       skos:inScheme gcdfo:AgeBasisScheme ;
                       skos:prefLabel "Age at return basis"@en ;
                       gcdfo:theme gcdfo:DataModelProvenanceTheme ,
                                   gcdfo:StockAssessmentTheme .


###  https://w3id.org/gcdfo/salmon#AgeAtSamplingBasis
gcdfo:AgeAtSamplingBasis rdf:type owl:NamedIndividual ,
                                  skos:Concept ;
                         rdfs:isDefinedBy <https://w3id.org/gcdfo/salmon> ;
                         skos:broader gcdfo:AgeBasis ;
                         skos:definition "Age measured at the time of sampling or observation."@en ;
                         skos:inScheme gcdfo:AgeBasisScheme ;
                         skos:prefLabel "Age at sampling basis"@en ;
                         gcdfo:theme gcdfo:DataModelProvenanceTheme ,
                                     gcdfo:StockAssessmentTheme .


###  https://w3id.org/gcdfo/salmon#AgeBasis
gcdfo:AgeBasis rdf:type owl:NamedIndividual ,
                        skos:Concept ;
               rdfs:isDefinedBy <https://w3id.org/gcdfo/salmon> ;
               skos:definition "The reference event or life-history point that an age value is measured against."@en ;
               skos:inScheme gcdfo:AgeBasisScheme ;
               skos:prefLabel "Age basis"@en ;
               gcdfo:theme gcdfo:DataModelProvenanceTheme ,
                           gcdfo:StockAssessmentTheme .


###  https://w3id.org/gcdfo/salmon#AgeBasisScheme
gcdfo:AgeBasisScheme rdf:type owl:NamedIndividual ,
                              skos:ConceptScheme ;
                     rdfs:isDefinedBy <https://w3id.org/gcdfo/salmon> ;
                     skos:definition "Controlled vocabulary for the reference event used by an age value (for example, age at return)."@en ;
                     skos:hasTopConcept gcdfo:AgeBasis ;
                     skos:prefLabel "Age basis scheme"@en ;
                     gcdfo:theme gcdfo:DataModelProvenanceTheme ,
                                 gcdfo:StockAssessmentTheme .


###  https://w3id.org/gcdfo/salmon#AgeClassValue
gcdfo:AgeClassValue rdf:type owl:NamedIndividual ,
                             skos:Concept ;
                    rdfs:isDefinedBy <https://w3id.org/gcdfo/salmon> ;
                    skos:definition "An integer-like age class value used as a compositional constraint in salmon measurements."@en ;
                    skos:inScheme gcdfo:AgeClassValueScheme ;
                    skos:prefLabel "Age class value"@en ;
                    gcdfo:theme gcdfo:StockAssessmentTheme .


###  https://w3id.org/gcdfo/salmon#AgeClassValueScheme
gcdfo:AgeClassValueScheme rdf:type owl:NamedIndividual ,
                                   skos:ConceptScheme ;
                          rdfs:isDefinedBy <https://w3id.org/gcdfo/salmon> ;
                          skos:definition "Controlled vocabulary for integer-like age class values used as constraints on salmon measurements."@en ;
                          skos:hasTopConcept gcdfo:AgeClassValue ;
                          skos:prefLabel "Age class value scheme"@en ;
                          gcdfo:theme gcdfo:StockAssessmentTheme .


###  https://w3id.org/gcdfo/salmon#AgeDimension
gcdfo:AgeDimension rdf:type owl:NamedIndividual ,
                            skos:Concept ;
                   rdfs:isDefinedBy <https://w3id.org/gcdfo/salmon> ;
                   skos:definition "The age component represented by a value (total age, freshwater years, or ocean years)."@en ;
                   skos:inScheme gcdfo:AgeDimensionScheme ;
                   skos:prefLabel "Age dimension"@en ;
                   gcdfo:theme gcdfo:StockAssessmentTheme .


###  https://w3id.org/gcdfo/salmon#AgeDimensionScheme
gcdfo:AgeDimensionScheme rdf:type owl:NamedIndividual ,
                                  skos:ConceptScheme ;
                         rdfs:isDefinedBy <https://w3id.org/gcdfo/salmon> ;
                         skos:definition "Controlled vocabulary for which age component is represented (total age, freshwater years, or ocean years)."@en ;
                         skos:hasTopConcept gcdfo:AgeDimension ;
                         skos:prefLabel "Age dimension scheme"@en ;
                         gcdfo:theme gcdfo:StockAssessmentTheme .


###  https://w3id.org/gcdfo/salmon#AgeNotation
gcdfo:AgeNotation rdf:type owl:NamedIndividual ,
                           skos:Concept ;
                  rdfs:isDefinedBy <https://w3id.org/gcdfo/salmon> ;
                  skos:definition "A notation system used to encode salmon age values in stock assessment data."@en ;
                  skos:inScheme gcdfo:AgeNotationScheme ;
                  skos:prefLabel "Age notation"@en ;
                  gcdfo:theme gcdfo:DataModelProvenanceTheme ,
                              gcdfo:StockAssessmentTheme .


###  https://w3id.org/gcdfo/salmon#AgeNotationScheme
gcdfo:AgeNotationScheme rdf:type owl:NamedIndividual ,
                                 skos:ConceptScheme ;
                        rdfs:isDefinedBy <https://w3id.org/gcdfo/salmon> ;
                        skos:definition "Controlled vocabulary for salmon age notation systems (for example, Gilbert-Rich and European notation)."@en ;
                        skos:hasTopConcept gcdfo:AgeNotation ;
                        skos:prefLabel "Age notation scheme"@en ;
                        gcdfo:theme gcdfo:DataModelProvenanceTheme ,
                                    gcdfo:StockAssessmentTheme .


###  https://w3id.org/gcdfo/salmon#AmberZone
gcdfo:AmberZone rdf:type owl:NamedIndividual ,
                         skos:Concept ,
                         gcdfo:WSPBiologicalStatusZone ;
                <http://purl.obolibrary.org/obo/IAO_0000119> "Fisheries and Oceans Canada. Wild Salmon Policy 2018-2022 Implementation Plan. https://waves-vagues.dfo-mpo.gc.ca/library-bibliotheque/40728109.pdf."@en ;
                dcterms:source <https://waves-vagues.dfo-mpo.gc.ca/library-bibliotheque/40728109.pdf> ;
                rdfs:isDefinedBy <https://w3id.org/gcdfo/salmon> ;
                skos:definition "Amber status implies caution in the management of the Conservation Unit. While a CU in the Amber zone should be at a low risk of loss, there will be a degree of lost production. Decisions about the conservation of CUs in the Amber zone will involve broader consideration of biological, social, and economic issues. "@en ;
                skos:inScheme gcdfo:WSPBiologicalStatusZoneScheme ;
                skos:prefLabel "Amber zone"@en ;
                gcdfo:theme gcdfo:StockAssessmentTheme ,
                            gcdfo:WildSalmonPolicyTheme .


###  https://w3id.org/gcdfo/salmon#AreaUnderTheCurve
gcdfo:AreaUnderTheCurve rdf:type owl:NamedIndividual ,
                                 skos:Concept ;
                        rdfs:isDefinedBy <https://w3id.org/gcdfo/salmon> ;
                        skos:altLabel "AUC"@en ;
                        skos:broader gcdfo:EstimateMethod ;
                        skos:definition "Integrates serial counts over time using a survey-life parameter; may apply observer efficiency."@en ;
                        skos:inScheme gcdfo:EstimateMethodScheme ;
                        skos:prefLabel "Area Under the Curve"@en ;
                        gcdfo:theme gcdfo:MonitoringFieldWorkTheme ,
                                    gcdfo:StockAssessmentTheme .


###  https://w3id.org/gcdfo/salmon#BenchmarkLevelScheme
gcdfo:BenchmarkLevelScheme rdf:type owl:NamedIndividual ,
                                    skos:ConceptScheme ;
                           rdfs:isDefinedBy <https://w3id.org/gcdfo/salmon> ;
                           skos:definition "Controlled vocabulary for generic benchmark-level qualifiers usable as I-ADOPT constraint values attached to benchmark variables or values."@en ;
                           skos:prefLabel "Benchmark Level Scheme"@en ;
                           gcdfo:theme gcdfo:StockAssessmentTheme ,
                                       gcdfo:WildSalmonPolicyTheme .


###  https://w3id.org/gcdfo/salmon#BiologicalBenchmarkAndIndicatorScheme
gcdfo:BiologicalBenchmarkAndIndicatorScheme rdf:type owl:NamedIndividual ,
                                                     skos:ConceptScheme ;
                                            rdfs:isDefinedBy <https://w3id.org/gcdfo/salmon> ;
                                            skos:definition "Controlled vocabulary for key biological benchmarks, performance indicators, and reference points used in salmon stock assessment and management (e.g., SMSY, Sgen, spawner abundance)."@en ;
                                            skos:hasTopConcept gcdfo:TargetOrLimitRateOrAbundance ;
                                            skos:prefLabel "Biological Benchmark and Indicator Scheme"@en ;
                                            gcdfo:theme gcdfo:StockAssessmentTheme ,
                                                        gcdfo:WildSalmonPolicyTheme .


###  https://w3id.org/gcdfo/salmon#BreachBypass
gcdfo:BreachBypass rdf:type owl:NamedIndividual ,
                            skos:Concept ;
                   rdfs:comment "Limits to Type 2 maximum"@en ;
                   rdfs:isDefinedBy <https://w3id.org/gcdfo/salmon> ;
                   skos:broader gcdfo:DowngradeCriteria ;
                   skos:definition "Bypass or breach risks not monitored and verified negligible"@en ;
                   skos:inScheme gcdfo:DowngradeCriteriaScheme ;
                   skos:prefLabel "Bypass/Breach Risk"@en ;
                   gcdfo:theme gcdfo:DataModelProvenanceTheme ,
                               gcdfo:StockAssessmentTheme .


###  https://w3id.org/gcdfo/salmon#COSEWICStatusScheme
gcdfo:COSEWICStatusScheme rdf:type owl:NamedIndividual ,
                                   skos:ConceptScheme ;
                          rdfs:isDefinedBy <https://w3id.org/gcdfo/salmon> ;
                          skos:definition "Controlled vocabulary for COSEWIC statuses"@en ;
                          skos:hasTopConcept gcdfo:COSEWICStatusCategory ;
                          skos:prefLabel "COSEWIC Status Scheme"@en ;
                          gcdfo:theme gcdfo:PolicyGovernanceTheme ,
                                      gcdfo:SpeciesAtRiskRecoveryTheme ,
                                      gcdfo:StockAssessmentTheme .


###  https://w3id.org/gcdfo/salmon#CalibratedTimeSeries
gcdfo:CalibratedTimeSeries rdf:type owl:NamedIndividual ,
                                    skos:Concept ;
                           rdfs:comment "Document calibration source years, transferability, diagnostics. Type-2 when calibration robust and applicable; else Type-3."@en ;
                           rdfs:isDefinedBy <https://w3id.org/gcdfo/salmon> ;
                           skos:broader gcdfo:EstimateMethod ;
                           skos:definition "Regression/state-space model calibrated to a Type-1/2 series converts a lower-precision index to abundance."@en ;
                           skos:inScheme gcdfo:EstimateMethodScheme ;
                           skos:prefLabel "Calibrated Time Series"@en ;
                           gcdfo:theme gcdfo:MonitoringFieldWorkTheme ,
                                       gcdfo:StockAssessmentTheme .


###  https://w3id.org/gcdfo/salmon#CatchContext
gcdfo:CatchContext rdf:type owl:NamedIndividual ,
                            skos:Concept ;
                   rdfs:isDefinedBy <https://w3id.org/gcdfo/salmon> ;
                   skos:broader gcdfo:MeasurementContext ;
                   skos:definition "Measurement context indicating values refer to fishery catch."@en ;
                   skos:inScheme gcdfo:MeasurementContextScheme ;
                   skos:prefLabel "Catch context"@en ;
                   gcdfo:theme gcdfo:StockAssessmentTheme .


###  https://w3id.org/gcdfo/salmon#Classification
gcdfo:Classification rdf:type owl:NamedIndividual ,
                              skos:Concept ;
                     rdfs:comment "Limits to Type 3 maximum"@en ;
                     rdfs:isDefinedBy <https://w3id.org/gcdfo/salmon> ;
                     skos:broader gcdfo:DowngradeCriteria ;
                     skos:definition "Classification/attribution not documented"@en ;
                     skos:inScheme gcdfo:DowngradeCriteriaScheme ;
                     skos:prefLabel "Classification"@en ;
                     gcdfo:theme gcdfo:DataModelProvenanceTheme ,
                                 gcdfo:StockAssessmentTheme .


###  https://w3id.org/gcdfo/salmon#ConfidenceCategory
gcdfo:ConfidenceCategory rdf:type owl:NamedIndividual ,
                                  skos:Concept .


###  https://w3id.org/gcdfo/salmon#CrossSectionCoverage
gcdfo:CrossSectionCoverage rdf:type owl:NamedIndividual ,
                                    skos:Concept ;
                           rdfs:comment "Limits to Type 2 maximum"@en ;
                           rdfs:isDefinedBy <https://w3id.org/gcdfo/salmon> ;
                           skos:broader gcdfo:DowngradeCriteria ;
                           skos:definition "Incomplete cross-section coverage"@en ;
                           skos:inScheme gcdfo:DowngradeCriteriaScheme ;
                           skos:prefLabel "Cross-section Coverage"@en ;
                           gcdfo:theme gcdfo:DataModelProvenanceTheme ,
                                       gcdfo:StockAssessmentTheme .


###  https://w3id.org/gcdfo/salmon#DataModelProvenanceTheme
gcdfo:DataModelProvenanceTheme rdf:type owl:NamedIndividual ,
                                        skos:Concept ;
                               rdfs:isDefinedBy <https://w3id.org/gcdfo/salmon> ;
                               skos:definition "Data models, analytical workflows, provenance, quality dimensions, and metadata supporting salmon science."@en ;
                               skos:inScheme gcdfo:ThemeScheme ;
                               skos:prefLabel "Data, Models, and Provenance"@en ;
                               gcdfo:theme gcdfo:DataModelProvenanceTheme .


###  https://w3id.org/gcdfo/salmon#DataQualityRatingContext
gcdfo:DataQualityRatingContext rdf:type owl:NamedIndividual ,
                                        skos:Concept ;
                               rdfs:isDefinedBy <https://w3id.org/gcdfo/salmon> ;
                               skos:broader gcdfo:MeasurementContext ;
                               skos:definition "Measurement context indicating categorical or ordinal quality ratings."@en ;
                               skos:inScheme gcdfo:MeasurementContextScheme ;
                               skos:prefLabel "Data quality rating context"@en ;
                               gcdfo:theme gcdfo:DataModelProvenanceTheme .


###  https://w3id.org/gcdfo/salmon#Detectability
gcdfo:Detectability rdf:type owl:NamedIndividual ,
                             skos:Concept ;
                    rdfs:comment "Limits to Type 3 maximum"@en ;
                    rdfs:isDefinedBy <https://w3id.org/gcdfo/salmon> ;
                    skos:broader gcdfo:DowngradeCriteria ;
                    skos:definition "Detectability factors not validated"@en ;
                    skos:inScheme gcdfo:DowngradeCriteriaScheme ;
                    skos:prefLabel "Detectability"@en ;
                    gcdfo:theme gcdfo:DataModelProvenanceTheme ,
                                gcdfo:StockAssessmentTheme .


###  https://w3id.org/gcdfo/salmon#DeviceConfiguration
gcdfo:DeviceConfiguration rdf:type owl:NamedIndividual ,
                                   skos:Concept ;
                          rdfs:comment "Limits to Type 2 maximum"@en ;
                          rdfs:isDefinedBy <https://w3id.org/gcdfo/salmon> ;
                          skos:broader gcdfo:DowngradeCriteria ;
                          skos:definition "Device not within operational specifications"@en ;
                          skos:inScheme gcdfo:DowngradeCriteriaScheme ;
                          skos:prefLabel "Device Configuration"@en ;
                          gcdfo:theme gcdfo:DataModelProvenanceTheme ,
                                      gcdfo:StockAssessmentTheme .


###  https://w3id.org/gcdfo/salmon#Documentation
gcdfo:Documentation rdf:type owl:NamedIndividual ,
                             skos:Concept ;
                    rdfs:comment "Downgrades Type 1/2 by one level"@en ;
                    rdfs:isDefinedBy <https://w3id.org/gcdfo/salmon> ;
                    skos:broader gcdfo:DowngradeCriteria ;
                    skos:definition "Missing SIL/SEN logs or QA/methods report"@en ;
                    skos:inScheme gcdfo:DowngradeCriteriaScheme ;
                    skos:prefLabel "Documentation"@en ;
                    gcdfo:theme gcdfo:DataModelProvenanceTheme ,
                                gcdfo:StockAssessmentTheme .


###  https://w3id.org/gcdfo/salmon#DowngradeCriteria
gcdfo:DowngradeCriteria rdf:type owl:NamedIndividual ,
                                 skos:Concept ;
                        rdfs:isDefinedBy <https://w3id.org/gcdfo/salmon> ;
                        skos:definition "Criteria that may result in downgrading an escapement estimate type classification"@en ;
                        skos:inScheme gcdfo:DowngradeCriteriaScheme ;
                        skos:prefLabel "Downgrade Criteria"@en ;
                        gcdfo:theme gcdfo:DataModelProvenanceTheme ,
                                    gcdfo:StockAssessmentTheme .


###  https://w3id.org/gcdfo/salmon#DowngradeCriteriaScheme
gcdfo:DowngradeCriteriaScheme rdf:type owl:NamedIndividual ,
                                       skos:ConceptScheme ;
                              rdfs:isDefinedBy <https://w3id.org/gcdfo/salmon> ;
                              skos:definition "Controlled vocabulary for estimate type downgrade criteria"@en ;
                              skos:hasTopConcept gcdfo:DowngradeCriteria ;
                              skos:prefLabel "Downgrade Criteria Scheme"@en ;
                              gcdfo:theme gcdfo:StockAssessmentTheme .


###  https://w3id.org/gcdfo/salmon#EffortStandardization
gcdfo:EffortStandardization rdf:type owl:NamedIndividual ,
                                     skos:Concept ;
                            rdfs:comment "Limits to Type 4 maximum"@en ;
                            rdfs:isDefinedBy <https://w3id.org/gcdfo/salmon> ;
                            skos:broader gcdfo:DowngradeCriteria ;
                            skos:definition "Effort not standardized"@en ;
                            skos:inScheme gcdfo:DowngradeCriteriaScheme ;
                            skos:prefLabel "Effort Standardization"@en ;
                            gcdfo:theme gcdfo:DataModelProvenanceTheme ,
                                        gcdfo:StockAssessmentTheme .


###  https://w3id.org/gcdfo/salmon#ElectrofishingCount
gcdfo:ElectrofishingCount rdf:type owl:NamedIndividual ,
                                   skos:Concept ;
                          rdfs:comment "Legacy methods: Electrofishing, Electroshocking"@en ;
                          rdfs:isDefinedBy <https://w3id.org/gcdfo/salmon> ;
                          skos:broader gcdfo:EnumerationMethod ;
                          skos:definition "Effort-standardized electrofishing passes used to generate catch-per-unit-effort (CPUE) indices."@en ;
                          skos:inScheme gcdfo:EnumerationMethodScheme ;
                          skos:prefLabel "Electrofishing Count"@en ;
                          gcdfo:theme gcdfo:MonitoringFieldWorkTheme ,
                                      gcdfo:StockAssessmentTheme .


###  https://w3id.org/gcdfo/salmon#EnumerationMethod
gcdfo:EnumerationMethod rdf:type owl:NamedIndividual ,
                                 skos:Concept ;
                        rdfs:isDefinedBy <https://w3id.org/gcdfo/salmon> ;
                        skos:definition "A method used to enumerate or count salmon in the field"@en ;
                        skos:inScheme gcdfo:EnumerationMethodScheme ;
                        skos:prefLabel "Enumeration Method"@en ;
                        gcdfo:theme gcdfo:MonitoringFieldWorkTheme ,
                                    gcdfo:StockAssessmentTheme .


###  https://w3id.org/gcdfo/salmon#EnumerationMethodScheme
gcdfo:EnumerationMethodScheme rdf:type owl:NamedIndividual ,
                                       skos:ConceptScheme ;
                              rdfs:isDefinedBy <https://w3id.org/gcdfo/salmon> ;
                              skos:definition "Controlled vocabulary for salmon enumeration methods"@en ;
                              skos:hasTopConcept gcdfo:EnumerationMethod ;
                              skos:prefLabel "Escapement Enumeration Method Scheme"@en ;
                              gcdfo:theme gcdfo:StockAssessmentTheme .


###  https://w3id.org/gcdfo/salmon#EnvironmentalConditions
gcdfo:EnvironmentalConditions rdf:type owl:NamedIndividual ,
                                       skos:Concept ;
                              rdfs:comment "Limits to Type 2 maximum"@en ;
                              rdfs:isDefinedBy <https://w3id.org/gcdfo/salmon> ;
                              skos:broader gcdfo:DowngradeCriteria ;
                              skos:definition "Environmental conditions outside specifications"@en ;
                              skos:inScheme gcdfo:DowngradeCriteriaScheme ;
                              skos:prefLabel "Environmental Conditions"@en ;
                              gcdfo:theme gcdfo:DataModelProvenanceTheme ,
                                          gcdfo:StockAssessmentTheme .


###  https://w3id.org/gcdfo/salmon#EstimateMethod
gcdfo:EstimateMethod rdf:type owl:NamedIndividual ,
                              skos:Concept ;
                     rdfs:isDefinedBy <https://w3id.org/gcdfo/salmon> ;
                     skos:definition "A method used to analyze and estimate salmon abundance from enumeration data"@en ;
                     skos:inScheme gcdfo:EstimateMethodScheme ;
                     skos:prefLabel "Estimate Method"@en ;
                     gcdfo:theme gcdfo:MonitoringFieldWorkTheme ,
                                 gcdfo:StockAssessmentTheme .


###  https://w3id.org/gcdfo/salmon#EstimateMethodScheme
gcdfo:EstimateMethodScheme rdf:type owl:NamedIndividual ,
                                    skos:ConceptScheme ;
                           rdfs:isDefinedBy <https://w3id.org/gcdfo/salmon> ;
                           skos:definition "Controlled vocabulary for salmon estimate methods"@en ;
                           skos:hasTopConcept gcdfo:EstimateMethod ;
                           skos:prefLabel "Escapement Estimate Method Scheme"@en ;
                           gcdfo:theme gcdfo:StockAssessmentTheme .


###  https://w3id.org/gcdfo/salmon#EstimateType
gcdfo:EstimateType rdf:type owl:NamedIndividual ,
                            skos:Concept ;
                   rdfs:isDefinedBy <https://w3id.org/gcdfo/salmon> ;
                   skos:definition "Classification of escapement estimate quality based on Hyatt 1997 framework"@en ;
                   skos:inScheme gcdfo:EstimateTypeScheme ;
                   skos:prefLabel "Estimate Type"@en ;
                   gcdfo:theme gcdfo:DataModelProvenanceTheme ,
                               gcdfo:StockAssessmentTheme .


###  https://w3id.org/gcdfo/salmon#EstimateTypeScheme
gcdfo:EstimateTypeScheme rdf:type owl:NamedIndividual ,
                                  skos:ConceptScheme ;
                         rdfs:isDefinedBy <https://w3id.org/gcdfo/salmon> ;
                         skos:definition "Controlled vocabulary for Hyatt 1997 estimate types"@en ;
                         skos:hasTopConcept gcdfo:EstimateType ;
                         skos:prefLabel "Escapement Estimate Type Scheme"@en ;
                         gcdfo:theme gcdfo:StockAssessmentTheme .


###  https://w3id.org/gcdfo/salmon#EuropeanAgeNotation
gcdfo:EuropeanAgeNotation rdf:type owl:NamedIndividual ,
                                   skos:Concept ;
                          dcterms:source <https://www.pac.dfo-mpo.gc.ca/fm-gp/fraser/docs/archiv-reports-rapports/indigenous-autochtone/2010FrasRvrChkInformDoc.htm> ;
                          rdfs:isDefinedBy <https://w3id.org/gcdfo/salmon> ;
                          skos:broader gcdfo:AgeNotation ;
                          skos:definition "Salmon age notation that records freshwater years followed by ocean years (for example, 1.2)."@en ;
                          skos:inScheme gcdfo:AgeNotationScheme ;
                          skos:notation "European" ;
                          skos:prefLabel "European age notation"@en ;
                          gcdfo:theme gcdfo:DataModelProvenanceTheme ,
                                      gcdfo:StockAssessmentTheme .


###  https://w3id.org/gcdfo/salmon#ExpansionFactor
gcdfo:ExpansionFactor rdf:type owl:NamedIndividual ,
                               skos:Concept ;
                      <http://purl.obolibrary.org/obo/IAO_0000115> "A multiplicative factor used to expand observed counts or detections from a sampled subset (e.g., indicator sites, PIT detections) to an estimated total abundance or escapement."@en ;
                      <http://purl.obolibrary.org/obo/IAO_0000119> "Fisheries and Oceans Canada. 2021. Marine Survival Forecast of Southern British Columbia Coho (describes applying expansion factors to PIT detections to estimate total escapement)."@en ;
                      dcterms:source <https://waves-vagues.dfo-mpo.gc.ca/Library/40978680.pdf> ;
                      rdfs:isDefinedBy <https://w3id.org/gcdfo/salmon> ;
                      skos:broader gcdfo:ExpansionMathematicalOperations ;
                      skos:definition "A multiplicative factor used to expand observed counts or detections from a sampled subset (e.g., indicator sites, PIT detections) to an estimated total abundance or escapement."@en ;
                      skos:inScheme gcdfo:EstimateMethodScheme ;
                      skos:prefLabel "Expansion factor"@en ;
                      gcdfo:theme gcdfo:DataModelProvenanceTheme ,
                                  gcdfo:StockAssessmentTheme .


###  https://w3id.org/gcdfo/salmon#ExpansionMathematicalOperations
gcdfo:ExpansionMathematicalOperations rdf:type owl:NamedIndividual ,
                                               skos:Concept ;
                                      rdfs:comment "Legacy methods: Lake Expansion, Redd Expansion, Peak×Factor, (Peak+CumDead)×Factor, Addition/Subtraction, Multiplication/Division. Inherits base method's Type; weak provenance = downgrade one Type."@en ;
                                      rdfs:isDefinedBy <https://w3id.org/gcdfo/salmon> ;
                                      skos:broader gcdfo:EstimateMethod ;
                                      skos:definition "Applies expansion factors or arithmetic transforms to a base count/index."@en ;
                                      skos:inScheme gcdfo:EstimateMethodScheme ;
                                      skos:prefLabel "Expansion/Mathematical Operations"@en ;
                                      gcdfo:theme gcdfo:MonitoringFieldWorkTheme ,
                                                  gcdfo:StockAssessmentTheme .


###  https://w3id.org/gcdfo/salmon#FishStockProvisions
gcdfo:FishStockProvisions rdf:type owl:NamedIndividual ,
                                   skos:Concept ;
                          rdfs:isDefinedBy <https://w3id.org/gcdfo/salmon> ;
                          skos:altLabel "FSP"@en ;
                          skos:broader gcdfo:PolicyFramework ;
                          skos:definition "Legal provisions in Canada's Fisheries Act and regulations related to maintaining and rebuilding fish stocks, including obligations triggered when reference points are breached."@en ;
                          skos:inScheme gcdfo:PolicyFrameworkScheme ;
                          skos:prefLabel "Fish Stocks Provisions"@en ;
                          gcdfo:theme gcdfo:FisheriesManagementTheme ,
                                      gcdfo:PolicyGovernanceTheme ,
                                      gcdfo:StockAssessmentTheme .


###  https://w3id.org/gcdfo/salmon#FisheriesManagementTheme
gcdfo:FisheriesManagementTheme rdf:type owl:NamedIndividual ,
                                        skos:Concept ;
                               rdfs:isDefinedBy <https://w3id.org/gcdfo/salmon> ;
                               skos:definition "Fishery openings, harvest control rules, catch/effort measures, and exploitation monitoring for salmon fisheries."@en ;
                               skos:inScheme gcdfo:ThemeScheme ;
                               skos:prefLabel "Fisheries Management"@en ;
                               gcdfo:theme gcdfo:DataModelProvenanceTheme .


###  https://w3id.org/gcdfo/salmon#FixedSiteCensusElectronic
gcdfo:FixedSiteCensusElectronic rdf:type owl:NamedIndividual ,
                                         skos:Concept ;
                                rdfs:comment "Legacy methods: Electronic/Optical counter, Resistivity Counter, Video/Camera counter"@en ;
                                rdfs:isDefinedBy <https://w3id.org/gcdfo/salmon> ;
                                skos:broader gcdfo:EnumerationMethod ;
                                skos:definition "Automated counting at a constrained opening using electronic/optical counters, resistivity counters, or video/camera systems. QA review of automated events, cross-section coverage, and uptime/coverage are documented."@en ;
                                skos:inScheme gcdfo:EnumerationMethodScheme ;
                                skos:prefLabel "Fixed Site Census (Electronic)"@en ;
                                gcdfo:theme gcdfo:MonitoringFieldWorkTheme ,
                                            gcdfo:StockAssessmentTheme .


###  https://w3id.org/gcdfo/salmon#FixedSiteCensusManual
gcdfo:FixedSiteCensusManual rdf:type owl:NamedIndividual ,
                                     skos:Concept ;
                            rdfs:comment "Legacy methods: Fence, Weir, Fixed Site Census (manual)"@en ;
                            rdfs:isDefinedBy <https://w3id.org/gcdfo/salmon> ;
                            skos:broader gcdfo:EnumerationMethod ;
                            skos:definition "Salmon are guided through a controlled opening in a fence/weir where trained observers visually tally each passage event on a continuous or daily schedule. Counting chambers/windows and SIL/SEN daily logs document coverage; bypass routes are monitored and closed where possible."@en ;
                            skos:inScheme gcdfo:EnumerationMethodScheme ;
                            skos:prefLabel "Fixed Site Census (Manual)"@en ;
                            gcdfo:theme gcdfo:MonitoringFieldWorkTheme ,
                                        gcdfo:StockAssessmentTheme .


###  https://w3id.org/gcdfo/salmon#FixedStationTally
gcdfo:FixedStationTally rdf:type owl:NamedIndividual ,
                                 skos:Concept ;
                        rdfs:isDefinedBy <https://w3id.org/gcdfo/salmon> ;
                        skos:broader gcdfo:EstimateMethod ;
                        skos:definition "Seasonal total = roll‑up of daily/continuous counts from a fixed (non‑sonar) station; simple arithmetic with documented coverage."@en ;
                        skos:inScheme gcdfo:EstimateMethodScheme ;
                        skos:prefLabel "Fixed‑Station Tally"@en ;
                        gcdfo:theme gcdfo:MonitoringFieldWorkTheme ,
                                    gcdfo:StockAssessmentTheme .


###  https://w3id.org/gcdfo/salmon#FreshwaterAgeDimension
gcdfo:FreshwaterAgeDimension rdf:type owl:NamedIndividual ,
                                      skos:Concept ;
                             rdfs:isDefinedBy <https://w3id.org/gcdfo/salmon> ;
                             skos:broader gcdfo:AgeDimension ;
                             skos:definition "Age value represents years spent in freshwater."@en ;
                             skos:inScheme gcdfo:AgeDimensionScheme ;
                             skos:prefLabel "Freshwater age dimension"@en ;
                             gcdfo:theme gcdfo:StockAssessmentTheme .


###  https://w3id.org/gcdfo/salmon#GeneticsStockCompositionTheme
gcdfo:GeneticsStockCompositionTheme rdf:type owl:NamedIndividual ,
                                             skos:Concept ;
                                    rdfs:isDefinedBy <https://w3id.org/gcdfo/salmon> ;
                                    skos:definition "Genetic markers, assays, and analyses used to infer stock composition, parentage, and population structure."@en ;
                                    skos:inScheme gcdfo:ThemeScheme ;
                                    skos:prefLabel "Genetics and Stock Composition"@en ;
                                    gcdfo:theme gcdfo:DataModelProvenanceTheme .


###  https://w3id.org/gcdfo/salmon#GilbertRichAgeNotation
gcdfo:GilbertRichAgeNotation rdf:type owl:NamedIndividual ,
                                      skos:Concept ;
                             dcterms:source <https://www.pac.dfo-mpo.gc.ca/fm-gp/fraser/docs/archiv-reports-rapports/indigenous-autochtone/2010FrasRvrChkInformDoc.htm> ;
                             rdfs:isDefinedBy <https://w3id.org/gcdfo/salmon> ;
                             skos:altLabel "GR age notation"@en ;
                             skos:broader gcdfo:AgeNotation ;
                             skos:definition "Salmon age notation where total age is annotated with freshwater years as a subscript-like suffix (for example, 4_2 for total age 4 with 2 freshwater years)."@en ;
                             skos:inScheme gcdfo:AgeNotationScheme ;
                             skos:notation "Gilbert-Rich" ;
                             skos:prefLabel "Gilbert-Rich age notation"@en ;
                             gcdfo:theme gcdfo:DataModelProvenanceTheme ,
                                         gcdfo:StockAssessmentTheme .


###  https://w3id.org/gcdfo/salmon#GreenZone
gcdfo:GreenZone rdf:type owl:NamedIndividual ,
                         skos:Concept ,
                         gcdfo:WSPBiologicalStatusZone ;
                <http://purl.obolibrary.org/obo/IAO_0000119> "Fisheries and Oceans Canada. Wild Salmon Policy 2018-2022 Implementation Plan. https://waves-vagues.dfo-mpo.gc.ca/library-bibliotheque/40728109.pdf."@en ;
                dcterms:source <https://waves-vagues.dfo-mpo.gc.ca/library-bibliotheque/40728109.pdf> ;
                rdfs:isDefinedBy <https://w3id.org/gcdfo/salmon> ;
                skos:definition "Social and economic considerations will tend to be the primary drivers for the management of Conservation Units in the Green zone, though ecosystem or other non-consumptive use values could also be considered."@en ;
                skos:inScheme gcdfo:WSPBiologicalStatusZoneScheme ;
                skos:prefLabel "Green zone"@en ;
                gcdfo:theme gcdfo:PolicyGovernanceTheme ,
                            gcdfo:WildSalmonPolicyTheme .


###  https://w3id.org/gcdfo/salmon#HabitatEcosystemClimateTheme
gcdfo:HabitatEcosystemClimateTheme rdf:type owl:NamedIndividual ,
                                            skos:Concept ;
                                   rdfs:isDefinedBy <https://w3id.org/gcdfo/salmon> ;
                                   skos:definition "Habitat attributes, ecosystem conditions, and climate or environmental stressors affecting salmon."@en ;
                                   skos:inScheme gcdfo:ThemeScheme ;
                                   skos:prefLabel "Habitat, Ecosystem, and Climate Pressures"@en ;
                                   gcdfo:theme gcdfo:DataModelProvenanceTheme .


###  https://w3id.org/gcdfo/salmon#HatcheryOrigin
gcdfo:HatcheryOrigin rdf:type owl:NamedIndividual ,
                              skos:Concept ;
                     <http://purl.obolibrary.org/obo/IAO_0000119> "Fisheries and Oceans Canada. 2018. Review of genetically based targets for enhanced contributions to Canadian Pacific Chinook Salmon populations. DFO Canadian Science Advisory Secretariat Science Advisory Report 2018/001 (Erratum: October 2023)."@en ;
                     dcterms:source <https://www.dfo-mpo.gc.ca/csas-sccs/Publications/SAR-AS/2018/2018_001-eng.html> ;
                     rdfs:isDefinedBy <https://w3id.org/gcdfo/salmon> ;
                     skos:broader gcdfo:SalmonOrigin ;
                     skos:definition "Individuals that were born or reared in a hatchery facility."@en ;
                     skos:inScheme gcdfo:SalmonOriginScheme ;
                     skos:prefLabel "Hatchery-origin"@en ;
                     gcdfo:theme gcdfo:GeneticsStockCompositionTheme ,
                                 gcdfo:SalmonEnhancementHatcheriesTheme ,
                                 gcdfo:StockAssessmentTheme .


###  https://w3id.org/gcdfo/salmon#HydroacousticModelling
gcdfo:HydroacousticModelling rdf:type owl:NamedIndividual ,
                                      skos:Concept ;
                             rdfs:comment "Legacy methods: Hydroacoustics, Sonar (ARIS/DIDSON). Not Type-1 under Hyatt; interpolation and classification error are central downgrades."@en ;
                             rdfs:isDefinedBy <https://w3id.org/gcdfo/salmon> ;
                             skos:broader gcdfo:EstimateMethod ;
                             skos:definition "Model pipeline converts sonar detections to passage totals; sets range/angle/blind zones; species/size attribution rules documented."@en ;
                             skos:inScheme gcdfo:EstimateMethodScheme ;
                             skos:prefLabel "Hydroacoustic Modelling"@en ;
                             gcdfo:theme gcdfo:MonitoringFieldWorkTheme ,
                                         gcdfo:StockAssessmentTheme .


###  https://w3id.org/gcdfo/salmon#HydroacousticSonarCount
gcdfo:HydroacousticSonarCount rdf:type owl:NamedIndividual ,
                                       skos:Concept ;
                              rdfs:comment "Legacy methods: Sonar-ARIS, Sonar-DIDSON, Hydroacoustic"@en ;
                              rdfs:isDefinedBy <https://w3id.org/gcdfo/salmon> ;
                              skos:broader gcdfo:EnumerationMethod ;
                              skos:definition "Sonar detections (ARIS, DIDSON, or other hydroacoustic systems) with documented coverage, visibility/noise conditions, and uptime. Raw detections require processing through a modelling/classification pipeline."@en ;
                              skos:inScheme gcdfo:EnumerationMethodScheme ;
                              skos:prefLabel "Hydroacoustic Sonar Count"@en ;
                              gcdfo:theme gcdfo:MonitoringFieldWorkTheme ,
                                          gcdfo:StockAssessmentTheme .


###  https://w3id.org/gcdfo/salmon#InRiverPhase
gcdfo:InRiverPhase rdf:type owl:NamedIndividual ,
                            skos:Concept ;
                   rdfs:isDefinedBy <https://w3id.org/gcdfo/salmon> ;
                   skos:altLabel "Freshwater phase"@en ;
                   skos:broader gcdfo:LifePhase ;
                   skos:definition "Freshwater in-river phase (migration and/or residence) outside the marine environment."@en ;
                   skos:inScheme gcdfo:LifePhaseScheme ;
                   skos:prefLabel "In-river phase"@en ;
                   gcdfo:theme gcdfo:StockAssessmentTheme .


###  https://w3id.org/gcdfo/salmon#InfillMethod
gcdfo:InfillMethod rdf:type owl:NamedIndividual ,
                            skos:Concept ;
                   rdfs:comment "Limits to Type 2 maximum"@en ;
                   rdfs:isDefinedBy <https://w3id.org/gcdfo/salmon> ;
                   skos:broader gcdfo:DowngradeCriteria ;
                   skos:definition "Interpolation used for missing data; defensibility must be documented"@en ;
                   skos:inScheme gcdfo:DowngradeCriteriaScheme ;
                   skos:prefLabel "Infill Method"@en ;
                   gcdfo:theme gcdfo:DataModelProvenanceTheme ,
                               gcdfo:StockAssessmentTheme .


###  https://w3id.org/gcdfo/salmon#LifePhase
gcdfo:LifePhase rdf:type owl:NamedIndividual ,
                         skos:Concept ;
                rdfs:isDefinedBy <https://w3id.org/gcdfo/salmon> ;
                skos:definition "A phase or segment used to stratify salmon measurements by where or when they apply (e.g., ocean phase, terminal phase)."@en ;
                skos:inScheme gcdfo:LifePhaseScheme ;
                skos:prefLabel "Life phase"@en ;
                gcdfo:theme gcdfo:StockAssessmentTheme .


###  https://w3id.org/gcdfo/salmon#LifePhaseScheme
gcdfo:LifePhaseScheme rdf:type owl:NamedIndividual ,
                               skos:ConceptScheme ;
                      rdfs:isDefinedBy <https://w3id.org/gcdfo/salmon> ;
                      skos:definition "Controlled vocabulary for life-phase or fishery/migration segment qualifiers used to stratify measurements (e.g., ocean, terminal, mainstem)."@en ;
                      skos:hasTopConcept gcdfo:LifePhase ;
                      skos:prefLabel "Life phase scheme"@en ;
                      gcdfo:theme gcdfo:StockAssessmentTheme .


###  https://w3id.org/gcdfo/salmon#LowerBenchmark
gcdfo:LowerBenchmark rdf:type owl:NamedIndividual ,
                              skos:Concept ;
                     rdfs:isDefinedBy <https://w3id.org/gcdfo/salmon> ;
                     skos:definition "A lower-threshold benchmark value, typically delineating the boundary between Red and Amber status zones."@en ;
                     skos:inScheme gcdfo:BenchmarkLevelScheme ;
                     skos:prefLabel "Lower benchmark"@en ;
                     gcdfo:theme gcdfo:StockAssessmentTheme ,
                                 gcdfo:WildSalmonPolicyTheme .


###  https://w3id.org/gcdfo/salmon#MainstemPhase
gcdfo:MainstemPhase rdf:type owl:NamedIndividual ,
                             skos:Concept ;
                    rdfs:isDefinedBy <https://w3id.org/gcdfo/salmon> ;
                    skos:broader gcdfo:LifePhase ;
                    skos:definition "Freshwater mainstem migration phase in a river system (often corresponding to mainstem in-river fisheries or monitoring segments)."@en ;
                    skos:inScheme gcdfo:LifePhaseScheme ;
                    skos:prefLabel "Mainstem phase"@en ;
                    gcdfo:theme gcdfo:StockAssessmentTheme .


###  https://w3id.org/gcdfo/salmon#ManagementReferenceContext
gcdfo:ManagementReferenceContext rdf:type owl:NamedIndividual ,
                                          skos:Concept ;
                                 rdfs:isDefinedBy <https://w3id.org/gcdfo/salmon> ;
                                 skos:broader gcdfo:MeasurementContext ;
                                 skos:definition "Measurement context indicating values are management benchmarks or reference-oriented metrics."@en ;
                                 skos:inScheme gcdfo:MeasurementContextScheme ;
                                 skos:prefLabel "Management reference context"@en ;
                                 gcdfo:theme gcdfo:PolicyGovernanceTheme ,
                                             gcdfo:StockAssessmentTheme .


###  https://w3id.org/gcdfo/salmon#MarkRecaptureAnalysis
gcdfo:MarkRecaptureAnalysis rdf:type owl:NamedIndividual ,
                                     skos:Concept ;
                            rdfs:comment "Legacy methods: Petersen, Jolly-Seber, Open model, Bayesian MR. Store uncertainty (e.g., CV) when available; note tag loss/recovery protocols."@en ;
                            rdfs:isDefinedBy <https://w3id.org/gcdfo/salmon> ;
                            skos:broader gcdfo:EstimateMethod ;
                            skos:definition "Capture-recapture estimators (Petersen, Jolly-Seber, open/Bayesian models) applied to field marks/recoveries."@en ;
                            skos:inScheme gcdfo:EstimateMethodScheme ;
                            skos:prefLabel "Mark-Recapture Analysis"@en ;
                            gcdfo:theme gcdfo:MonitoringFieldWorkTheme ,
                                        gcdfo:StockAssessmentTheme .


###  https://w3id.org/gcdfo/salmon#MarkRecaptureAssumptions
gcdfo:MarkRecaptureAssumptions rdf:type owl:NamedIndividual ,
                                        skos:Concept ;
                               rdfs:comment "Limits to Type 3 maximum"@en ;
                               rdfs:isDefinedBy <https://w3id.org/gcdfo/salmon> ;
                               skos:broader gcdfo:DowngradeCriteria ;
                               skos:definition "MR assumptions not evaluated"@en ;
                               skos:inScheme gcdfo:DowngradeCriteriaScheme ;
                               skos:prefLabel "Mark-Recapture Assumptions"@en ;
                               gcdfo:theme gcdfo:DataModelProvenanceTheme ,
                                           gcdfo:StockAssessmentTheme .


###  https://w3id.org/gcdfo/salmon#MarkRecaptureFieldProgram
gcdfo:MarkRecaptureFieldProgram rdf:type owl:NamedIndividual ,
                                         skos:Concept ;
                                rdfs:comment "Legacy methods: Tag Recovery"@en ;
                                rdfs:isDefinedBy <https://w3id.org/gcdfo/salmon> ;
                                skos:broader gcdfo:EnumerationMethod ;
                                skos:definition "Field program involving marking and subsequent recapture/recovery of tagged fish with documented assumptions and recovery coverage."@en ;
                                skos:inScheme gcdfo:EnumerationMethodScheme ;
                                skos:prefLabel "Mark-Recapture Field Program"@en ;
                                gcdfo:theme gcdfo:MonitoringFieldWorkTheme ,
                                            gcdfo:StockAssessmentTheme .


###  https://w3id.org/gcdfo/salmon#MeasurementContext
gcdfo:MeasurementContext rdf:type owl:NamedIndividual ,
                                  skos:Concept ;
                         rdfs:isDefinedBy <https://w3id.org/gcdfo/salmon> ;
                         skos:definition "A context qualifier used to disambiguate the interpretation of a measurement column."@en ;
                         skos:inScheme gcdfo:MeasurementContextScheme ;
                         skos:prefLabel "Measurement context"@en ;
                         gcdfo:theme gcdfo:DataModelProvenanceTheme ,
                                     gcdfo:StockAssessmentTheme .


###  https://w3id.org/gcdfo/salmon#MeasurementContextScheme
gcdfo:MeasurementContextScheme rdf:type owl:NamedIndividual ,
                                        skos:ConceptScheme ;
                               rdfs:isDefinedBy <https://w3id.org/gcdfo/salmon> ;
                               skos:definition "Controlled vocabulary for compositional measurement context qualifiers (for example, catch context, run context)."@en ;
                               skos:hasTopConcept gcdfo:MeasurementContext ;
                               skos:prefLabel "Measurement context scheme"@en ;
                               gcdfo:theme gcdfo:DataModelProvenanceTheme ,
                                           gcdfo:StockAssessmentTheme .


###  https://w3id.org/gcdfo/salmon#MethodUnknown
gcdfo:MethodUnknown rdf:type owl:NamedIndividual ,
                             skos:Concept ;
                    rdfs:comment "Limits to Type 5 maximum"@en ;
                    rdfs:isDefinedBy <https://w3id.org/gcdfo/salmon> ;
                    skos:broader gcdfo:DowngradeCriteria ;
                    skos:definition "Survey/analytical methods not adequately identified/consistent"@en ;
                    skos:inScheme gcdfo:DowngradeCriteriaScheme ;
                    skos:prefLabel "Method Unknown/Inconsistent"@en ;
                    gcdfo:theme gcdfo:DataModelProvenanceTheme ,
                                gcdfo:StockAssessmentTheme .


###  https://w3id.org/gcdfo/salmon#MonitoringFieldWorkTheme
gcdfo:MonitoringFieldWorkTheme rdf:type owl:NamedIndividual ,
                                        skos:Concept ;
                               rdfs:isDefinedBy <https://w3id.org/gcdfo/salmon> ;
                               skos:definition "Field observations, sampling protocols, survey events, gear, and measurement methods used to collect salmon data."@en ;
                               skos:inScheme gcdfo:ThemeScheme ;
                               skos:prefLabel "Monitoring and Field Work"@en ;
                               gcdfo:theme gcdfo:DataModelProvenanceTheme .


###  https://w3id.org/gcdfo/salmon#NaturalOrigin
gcdfo:NaturalOrigin rdf:type owl:NamedIndividual ,
                             skos:Concept ;
                    <http://purl.obolibrary.org/obo/IAO_0000119> "Fisheries and Oceans Canada. 2018. Review of genetically based targets for enhanced contributions to Canadian Pacific Chinook Salmon populations. DFO Canadian Science Advisory Secretariat Science Advisory Report 2018/001 (Erratum: October 2023)."@en ;
                    dcterms:source <https://www.dfo-mpo.gc.ca/csas-sccs/Publications/SAR-AS/2018/2018_001-eng.html> ;
                    rdfs:isDefinedBy <https://w3id.org/gcdfo/salmon> ;
                    skos:broader gcdfo:SalmonOrigin ;
                    skos:definition "Individuals that are born and reared in the wild (natural environment)."@en ;
                    skos:inScheme gcdfo:SalmonOriginScheme ;
                    skos:prefLabel "Natural-origin"@en ;
                    gcdfo:theme gcdfo:GeneticsStockCompositionTheme ,
                                gcdfo:StockAssessmentTheme ,
                                gcdfo:WildSalmonPolicyTheme .


###  https://w3id.org/gcdfo/salmon#NumberOfVisits
gcdfo:NumberOfVisits rdf:type owl:NamedIndividual ,
                              skos:Concept ;
                     rdfs:comment "Limits to Type 4 maximum"@en ;
                     rdfs:isDefinedBy <https://w3id.org/gcdfo/salmon> ;
                     skos:broader gcdfo:DowngradeCriteria ;
                     skos:definition "Insufficient number of survey visits"@en ;
                     skos:inScheme gcdfo:DowngradeCriteriaScheme ;
                     skos:prefLabel "Number of Visits"@en ;
                     gcdfo:theme gcdfo:DataModelProvenanceTheme ,
                                 gcdfo:StockAssessmentTheme .


###  https://w3id.org/gcdfo/salmon#OceanAgeDimension
gcdfo:OceanAgeDimension rdf:type owl:NamedIndividual ,
                                 skos:Concept ;
                        rdfs:isDefinedBy <https://w3id.org/gcdfo/salmon> ;
                        skos:altLabel "Marine age dimension"@en ;
                        skos:broader gcdfo:AgeDimension ;
                        skos:definition "Age value represents years spent in the marine environment."@en ;
                        skos:inScheme gcdfo:AgeDimensionScheme ;
                        skos:prefLabel "Ocean age dimension"@en ;
                        gcdfo:theme gcdfo:StockAssessmentTheme .


###  https://w3id.org/gcdfo/salmon#OceanPhase
gcdfo:OceanPhase rdf:type owl:NamedIndividual ,
                          skos:Concept ;
                 rdfs:isDefinedBy <https://w3id.org/gcdfo/salmon> ;
                 skos:altLabel "Marine phase"@en ;
                 skos:broader gcdfo:LifePhase ;
                 skos:definition "Phase of the salmon life cycle or assessment period occurring in the marine environment."@en ;
                 skos:inScheme gcdfo:LifePhaseScheme ;
                 skos:prefLabel "Ocean phase"@en ;
                 gcdfo:theme gcdfo:StockAssessmentTheme .


###  https://w3id.org/gcdfo/salmon#PeakCountAnalysis
gcdfo:PeakCountAnalysis rdf:type owl:NamedIndividual ,
                                 skos:Concept ;
                        rdfs:comment "Legacy methods: Peak Live, Peak Live + Dead, Peak + Cumulative Dead, Cumulative New"@en ;
                        rdfs:isDefinedBy <https://w3id.org/gcdfo/salmon> ;
                        skos:broader gcdfo:EstimateMethod ;
                        skos:definition "Uses the peak survey (live ± dead variants) as the season estimate/index."@en ;
                        skos:inScheme gcdfo:EstimateMethodScheme ;
                        skos:prefLabel "Peak Count Analysis"@en ;
                        gcdfo:theme gcdfo:MonitoringFieldWorkTheme ,
                                    gcdfo:StockAssessmentTheme .


###  https://w3id.org/gcdfo/salmon#PolicyFramework
gcdfo:PolicyFramework rdf:type owl:NamedIndividual ,
                               skos:Concept ;
                      rdfs:isDefinedBy <https://w3id.org/gcdfo/salmon> ;
                      skos:definition "A policy, legal, or governance framework that defines how salmon status metrics, benchmarks, or reference points are set and interpreted."@en ;
                      skos:inScheme gcdfo:PolicyFrameworkScheme ;
                      skos:prefLabel "Policy framework"@en ;
                      gcdfo:theme gcdfo:PolicyGovernanceTheme ,
                                  gcdfo:StockAssessmentTheme ,
                                  gcdfo:WildSalmonPolicyTheme .


###  https://w3id.org/gcdfo/salmon#PolicyFrameworkScheme
gcdfo:PolicyFrameworkScheme rdf:type owl:NamedIndividual ,
                                     skos:ConceptScheme ;
                            rdfs:isDefinedBy <https://w3id.org/gcdfo/salmon> ;
                            skos:definition "Controlled vocabulary for policy and governance frameworks referenced by salmon assessment metrics and benchmarks (e.g., WSP, PA)."@en ;
                            skos:hasTopConcept gcdfo:PolicyFramework ;
                            skos:prefLabel "Policy framework scheme"@en ;
                            gcdfo:theme gcdfo:PolicyGovernanceTheme ,
                                        gcdfo:StockAssessmentTheme ,
                                        gcdfo:WildSalmonPolicyTheme .


###  https://w3id.org/gcdfo/salmon#PolicyGovernanceTheme
gcdfo:PolicyGovernanceTheme rdf:type owl:NamedIndividual ,
                                     skos:Concept ;
                            rdfs:isDefinedBy <https://w3id.org/gcdfo/salmon> ;
                            skos:definition "DFO policy frameworks, governance, regulations, and organizational structure relevant to salmon management."@en ;
                            skos:inScheme gcdfo:ThemeScheme ;
                            skos:prefLabel "Policy, Governance, and Organizational Structure"@en ;
                            gcdfo:theme gcdfo:DataModelProvenanceTheme .


###  https://w3id.org/gcdfo/salmon#PrecautionaryApproach
gcdfo:PrecautionaryApproach rdf:type owl:NamedIndividual ,
                                     skos:Concept ;
                            rdfs:isDefinedBy <https://w3id.org/gcdfo/salmon> ;
                            skos:altLabel "PA"@en ;
                            skos:broader gcdfo:PolicyFramework ;
                            skos:definition "DFO policy framework for applying precaution in fisheries decision-making, including use of reference points and stock status zones."@en ;
                            skos:inScheme gcdfo:PolicyFrameworkScheme ;
                            skos:prefLabel "Precautionary Approach"@en ;
                            gcdfo:theme gcdfo:FisheriesManagementTheme ,
                                        gcdfo:PolicyGovernanceTheme ,
                                        gcdfo:StockAssessmentTheme .


###  https://w3id.org/gcdfo/salmon#PrecisionAccuracy
gcdfo:PrecisionAccuracy rdf:type owl:NamedIndividual ,
                                 skos:Concept ;
                        rdfs:comment "Downgrades by one level"@en ;
                        rdfs:isDefinedBy <https://w3id.org/gcdfo/salmon> ;
                        skos:broader gcdfo:DowngradeCriteria ;
                        skos:definition "Precision/accuracy weaker than expected for type"@en ;
                        skos:inScheme gcdfo:DowngradeCriteriaScheme ;
                        skos:prefLabel "Precision/Accuracy"@en ;
                        gcdfo:theme gcdfo:DataModelProvenanceTheme ,
                                    gcdfo:StockAssessmentTheme .


###  https://w3id.org/gcdfo/salmon#RapidStatusConfidenceHigh
gcdfo:RapidStatusConfidenceHigh rdf:type owl:NamedIndividual ,
                                         skos:Concept ,
                                         gcdfo:ConfidenceCategory ;
                                <http://purl.obolibrary.org/obo/IAO_0000115> "Rapid status confidence category indicating that high-quality abundance metrics support the result."@en ;
                                rdfs:isDefinedBy <https://w3id.org/gcdfo/salmon> ;
                                rdfs:label "High rapid-status confidence"@en ;
                                skos:inScheme gcdfo:RapidStatusConfidenceScheme ;
                                skos:prefLabel "High confidence"@en ;
                                gcdfo:theme gcdfo:StockAssessmentTheme ,
                                            gcdfo:WildSalmonPolicyTheme .


###  https://w3id.org/gcdfo/salmon#RapidStatusConfidenceLow
gcdfo:RapidStatusConfidenceLow rdf:type owl:NamedIndividual ,
                                        skos:Concept ,
                                        gcdfo:ConfidenceCategory ;
                               <http://purl.obolibrary.org/obo/IAO_0000115> "Rapid status confidence category indicating limited supporting data (for example, derived from trend metrics alone)."@en ;
                               rdfs:isDefinedBy <https://w3id.org/gcdfo/salmon> ;
                               rdfs:label "Low rapid-status confidence"@en ;
                               skos:inScheme gcdfo:RapidStatusConfidenceScheme ;
                               skos:prefLabel "Low confidence"@en ;
                               gcdfo:theme gcdfo:StockAssessmentTheme ,
                                           gcdfo:WildSalmonPolicyTheme .


###  https://w3id.org/gcdfo/salmon#RapidStatusConfidenceMedium
gcdfo:RapidStatusConfidenceMedium rdf:type owl:NamedIndividual ,
                                           skos:Concept ,
                                           gcdfo:ConfidenceCategory ;
                                  <http://purl.obolibrary.org/obo/IAO_0000115> "Rapid status confidence category indicating mixed evidence or reliance on trend metrics supplemented by some abundance information."@en ;
                                  rdfs:isDefinedBy <https://w3id.org/gcdfo/salmon> ;
                                  rdfs:label "Medium rapid-status confidence"@en ;
                                  skos:inScheme gcdfo:RapidStatusConfidenceScheme ;
                                  skos:prefLabel "Medium confidence"@en ;
                                  gcdfo:theme gcdfo:StockAssessmentTheme ,
                                              gcdfo:WildSalmonPolicyTheme .


###  https://w3id.org/gcdfo/salmon#RapidStatusConfidenceScheme
gcdfo:RapidStatusConfidenceScheme rdf:type owl:NamedIndividual ,
                                           skos:ConceptScheme ;
                                  rdfs:isDefinedBy <https://w3id.org/gcdfo/salmon> ;
                                  skos:definition "Controlled vocabulary for categorical confidence ratings attached to rapid status assessments."@en ;
                                  skos:hasTopConcept gcdfo:ConfidenceCategory ;
                                  skos:prefLabel "Rapid status confidence scheme"@en ;
                                  gcdfo:theme gcdfo:StockAssessmentTheme ,
                                              gcdfo:WildSalmonPolicyTheme .


###  https://w3id.org/gcdfo/salmon#ReachCoverage
gcdfo:ReachCoverage rdf:type owl:NamedIndividual ,
                             skos:Concept ;
                    rdfs:comment "Limits to Type 3 maximum"@en ;
                    rdfs:isDefinedBy <https://w3id.org/gcdfo/salmon> ;
                    skos:broader gcdfo:DowngradeCriteria ;
                    skos:definition "Insufficient reach coverage"@en ;
                    skos:inScheme gcdfo:DowngradeCriteriaScheme ;
                    skos:prefLabel "Reach Coverage"@en ;
                    gcdfo:theme gcdfo:DataModelProvenanceTheme ,
                                gcdfo:StockAssessmentTheme .


###  https://w3id.org/gcdfo/salmon#RecruitStageContext
gcdfo:RecruitStageContext rdf:type owl:NamedIndividual ,
                                   skos:Concept ;
                          rdfs:isDefinedBy <https://w3id.org/gcdfo/salmon> ;
                          skos:broader gcdfo:MeasurementContext ;
                          skos:definition "Measurement context indicating values refer to recruits."@en ;
                          skos:inScheme gcdfo:MeasurementContextScheme ;
                          skos:prefLabel "Recruit stage context"@en ;
                          gcdfo:theme gcdfo:StockAssessmentTheme .


###  https://w3id.org/gcdfo/salmon#RedZone
gcdfo:RedZone rdf:type owl:NamedIndividual ,
                       skos:Concept ,
                       gcdfo:WSPBiologicalStatusZone ;
              <http://purl.obolibrary.org/obo/IAO_0000119> "Fisheries and Oceans Canada. Wild Salmon Policy 2018-2022 Implementation Plan. https://waves-vagues.dfo-mpo.gc.ca/library-bibliotheque/40728109.pdf."@en ;
              dcterms:source <https://waves-vagues.dfo-mpo.gc.ca/library-bibliotheque/40728109.pdf> ;
              rdfs:isDefinedBy <https://w3id.org/gcdfo/salmon> ;
              skos:definition "A Conservation Unit in the Red zone is undesirable because of the risk of extirpation, and the loss of ecological benefits and salmon production. Changes in status will trigger management actions that will vary depending on species, geographic regions, and cause of the decline."@en ;
              skos:inScheme gcdfo:WSPBiologicalStatusZoneScheme ;
              skos:prefLabel "Red zone"@en ;
              gcdfo:theme gcdfo:StockAssessmentTheme ,
                          gcdfo:WildSalmonPolicyTheme .


###  https://w3id.org/gcdfo/salmon#ReddCount
gcdfo:ReddCount rdf:type owl:NamedIndividual ,
                         skos:Concept ;
                rdfs:comment "Legacy methods: Redd Counts"@en ;
                rdfs:isDefinedBy <https://w3id.org/gcdfo/salmon> ;
                skos:broader gcdfo:EnumerationMethod ;
                skos:definition "Redd counts with documentation of detectability, timing, and reach coverage. Conversion to spawner estimates requires spawners-per-redd factors handled in analysis."@en ;
                skos:inScheme gcdfo:EnumerationMethodScheme ;
                skos:prefLabel "Redd Count"@en ;
                gcdfo:theme gcdfo:MonitoringFieldWorkTheme ,
                            gcdfo:StockAssessmentTheme .


###  https://w3id.org/gcdfo/salmon#ReddExpansionAnalysis
gcdfo:ReddExpansionAnalysis rdf:type owl:NamedIndividual ,
                                     skos:Concept ;
                            rdfs:comment "Requires validated spawners-per-redd factor and documentation of detectability assumptions."@en ;
                            rdfs:isDefinedBy <https://w3id.org/gcdfo/salmon> ;
                            skos:broader gcdfo:EstimateMethod ;
                            skos:definition "Converts redd counts to spawner estimates using spawners-per-redd expansion factors."@en ;
                            skos:inScheme gcdfo:EstimateMethodScheme ;
                            skos:prefLabel "Redd Expansion Analysis"@en ;
                            gcdfo:theme gcdfo:MonitoringFieldWorkTheme ,
                                        gcdfo:StockAssessmentTheme .


###  https://w3id.org/gcdfo/salmon#ReviewQA
gcdfo:ReviewQA rdf:type owl:NamedIndividual ,
                        skos:Concept ;
               rdfs:comment "Limits to Type 2 maximum"@en ;
               rdfs:isDefinedBy <https://w3id.org/gcdfo/salmon> ;
               skos:broader gcdfo:DowngradeCriteria ;
               skos:definition "Insufficient QA review of automated events"@en ;
               skos:inScheme gcdfo:DowngradeCriteriaScheme ;
               skos:prefLabel "Review/QA"@en ;
               gcdfo:theme gcdfo:DataModelProvenanceTheme ,
                           gcdfo:StockAssessmentTheme .


###  https://w3id.org/gcdfo/salmon#RunContext
gcdfo:RunContext rdf:type owl:NamedIndividual ,
                          skos:Concept ;
                 rdfs:isDefinedBy <https://w3id.org/gcdfo/salmon> ;
                 skos:broader gcdfo:MeasurementContext ;
                 skos:definition "Measurement context indicating values refer to run size or returning run composition."@en ;
                 skos:inScheme gcdfo:MeasurementContextScheme ;
                 skos:prefLabel "Run context"@en ;
                 gcdfo:theme gcdfo:StockAssessmentTheme .


###  https://w3id.org/gcdfo/salmon#RunCoverage
gcdfo:RunCoverage rdf:type owl:NamedIndividual ,
                           skos:Concept ;
                  rdfs:comment "Limits to Type 2 maximum"@en ;
                  rdfs:isDefinedBy <https://w3id.org/gcdfo/salmon> ;
                  skos:broader gcdfo:DowngradeCriteria ;
                  skos:definition "Run-window coverage < 95% of season days"@en ;
                  skos:inScheme gcdfo:DowngradeCriteriaScheme ;
                  skos:prefLabel "Run Coverage"@en ;
                  gcdfo:theme gcdfo:DataModelProvenanceTheme ,
                              gcdfo:StockAssessmentTheme .


###  https://w3id.org/gcdfo/salmon#SalmonEnhancementHatcheriesTheme
gcdfo:SalmonEnhancementHatcheriesTheme rdf:type owl:NamedIndividual ,
                                                skos:Concept ;
                                       rdfs:isDefinedBy <https://w3id.org/gcdfo/salmon> ;
                                       skos:definition "Hatchery production, broodstock management, releases, and enhancement program practices for salmon."@en ;
                                       skos:inScheme gcdfo:ThemeScheme ;
                                       skos:prefLabel "Salmon Enhancement and Hatcheries"@en ;
                                       gcdfo:theme gcdfo:DataModelProvenanceTheme .


###  https://w3id.org/gcdfo/salmon#SalmonOrigin
gcdfo:SalmonOrigin rdf:type owl:NamedIndividual ,
                            skos:Concept ;
                   rdfs:isDefinedBy <https://w3id.org/gcdfo/salmon> ;
                   skos:definition "Origin category describing whether salmon are naturally produced, hatchery produced, or mixed-origin."@en ;
                   skos:inScheme gcdfo:SalmonOriginScheme ;
                   skos:prefLabel "Salmon origin"@en ;
                   gcdfo:theme gcdfo:SalmonEnhancementHatcheriesTheme ,
                               gcdfo:StockAssessmentTheme .


###  https://w3id.org/gcdfo/salmon#SalmonOriginScheme
gcdfo:SalmonOriginScheme rdf:type owl:NamedIndividual ,
                                  skos:ConceptScheme ;
                         rdfs:isDefinedBy <https://w3id.org/gcdfo/salmon> ;
                         skos:definition "Controlled vocabulary for describing the origin of individual salmon (e.g., natural-origin, hatchery-origin, mixed-origin)."@en ;
                         skos:hasTopConcept gcdfo:SalmonOrigin ;
                         skos:prefLabel "Salmon Origin Scheme"@en ;
                         gcdfo:theme gcdfo:GeneticsStockCompositionTheme ,
                                     gcdfo:SalmonEnhancementHatcheriesTheme ,
                                     gcdfo:StockAssessmentTheme .


###  https://w3id.org/gcdfo/salmon#SpawnerStageContext
gcdfo:SpawnerStageContext rdf:type owl:NamedIndividual ,
                                   skos:Concept ;
                          rdfs:isDefinedBy <https://w3id.org/gcdfo/salmon> ;
                          skos:broader gcdfo:MeasurementContext ;
                          skos:definition "Measurement context indicating values refer to spawners or spawning-stage fish."@en ;
                          skos:inScheme gcdfo:MeasurementContextScheme ;
                          skos:prefLabel "Spawner stage context"@en ;
                          gcdfo:theme gcdfo:StockAssessmentTheme .


###  https://w3id.org/gcdfo/salmon#SpeciesAtRiskRecoveryTheme
gcdfo:SpeciesAtRiskRecoveryTheme rdf:type owl:NamedIndividual ,
                                          skos:Concept ;
                                 rdfs:isDefinedBy <https://w3id.org/gcdfo/salmon> ;
                                 skos:definition "COSEWIC/SARA recovery planning, critical habitat, threats, and status assessments for species of conservation concern."@en ;
                                 skos:inScheme gcdfo:ThemeScheme ;
                                 skos:prefLabel "Species at Risk and Recovery"@en ;
                                 gcdfo:theme gcdfo:DataModelProvenanceTheme .


###  https://w3id.org/gcdfo/salmon#StockAssessmentTheme
gcdfo:StockAssessmentTheme rdf:type owl:NamedIndividual ,
                                    skos:Concept ;
                           rdfs:isDefinedBy <https://w3id.org/gcdfo/salmon> ;
                           skos:definition "Stock assessment models, benchmarks, status determinations, and performance metrics for salmon units."@en ;
                           skos:inScheme gcdfo:ThemeScheme ;
                           skos:prefLabel "Stock Assessment"@en ;
                           gcdfo:theme gcdfo:DataModelProvenanceTheme .


###  https://w3id.org/gcdfo/salmon#StockStatusZoneScheme
gcdfo:StockStatusZoneScheme rdf:type owl:NamedIndividual ,
                                     skos:ConceptScheme ;
                            rdfs:isDefinedBy <https://w3id.org/gcdfo/salmon> ;
                            skos:altLabel "Stock Status Zone Scheme"@en ;
                            skos:definition "Legacy alias scheme for stock status zones. Use :WSPBiologicalStatusZoneScheme as the canonical scheme for Red/Amber/Green Wild Salmon Policy biological status zones."@en ;
                            skos:exactMatch gcdfo:WSPBiologicalStatusZoneScheme ;
                            skos:hasTopConcept gcdfo:WSPBiologicalStatusZone ;
                            skos:prefLabel "Stock Status Zone Scheme (legacy alias)"@en ;
                            gcdfo:theme gcdfo:FisheriesManagementTheme ,
                                        gcdfo:StockAssessmentTheme ,
                                        gcdfo:WildSalmonPolicyTheme .


###  https://w3id.org/gcdfo/salmon#SurvivalOrMortalityContext
gcdfo:SurvivalOrMortalityContext rdf:type owl:NamedIndividual ,
                                          skos:Concept ;
                                 rdfs:isDefinedBy <https://w3id.org/gcdfo/salmon> ;
                                 skos:broader gcdfo:MeasurementContext ;
                                 skos:definition "Measurement context indicating values represent survival, mortality, or related rates."@en ;
                                 skos:inScheme gcdfo:MeasurementContextScheme ;
                                 skos:prefLabel "Survival or mortality context"@en ;
                                 gcdfo:theme gcdfo:StockAssessmentTheme .


###  https://w3id.org/gcdfo/salmon#TerminalPhase
gcdfo:TerminalPhase rdf:type owl:NamedIndividual ,
                             skos:Concept ;
                    rdfs:isDefinedBy <https://w3id.org/gcdfo/salmon> ;
                    skos:broader gcdfo:LifePhase ;
                    skos:definition "Phase occurring in terminal areas near river mouths or spawning areas (often including terminal fisheries and local migration to spawning sites)."@en ;
                    skos:inScheme gcdfo:LifePhaseScheme ;
                    skos:prefLabel "Terminal phase"@en ;
                    gcdfo:theme gcdfo:StockAssessmentTheme .


###  https://w3id.org/gcdfo/salmon#ThemeScheme
gcdfo:ThemeScheme rdf:type owl:NamedIndividual ,
                           skos:ConceptScheme ;
                  rdfs:isDefinedBy <https://w3id.org/gcdfo/salmon> ;
                  skos:definition "High-level thematic concept scheme for organizing DFO Salmon Ontology classes and concepts."@en ;
                  skos:prefLabel "Theme Scheme"@en ;
                  gcdfo:theme gcdfo:DataModelProvenanceTheme .


###  https://w3id.org/gcdfo/salmon#Timing
gcdfo:Timing rdf:type owl:NamedIndividual ,
                      skos:Concept ;
             rdfs:comment "Limits to Type 3 maximum"@en ;
             rdfs:isDefinedBy <https://w3id.org/gcdfo/salmon> ;
             skos:broader gcdfo:DowngradeCriteria ;
             skos:definition "Poor timing of surveys"@en ;
             skos:inScheme gcdfo:DowngradeCriteriaScheme ;
             skos:prefLabel "Timing"@en ;
             gcdfo:theme gcdfo:DataModelProvenanceTheme ,
                         gcdfo:StockAssessmentTheme .


###  https://w3id.org/gcdfo/salmon#TotalAgeDimension
gcdfo:TotalAgeDimension rdf:type owl:NamedIndividual ,
                                 skos:Concept ;
                        rdfs:isDefinedBy <https://w3id.org/gcdfo/salmon> ;
                        skos:broader gcdfo:AgeDimension ;
                        skos:definition "Age value represents total age in years."@en ;
                        skos:inScheme gcdfo:AgeDimensionScheme ;
                        skos:prefLabel "Total age dimension"@en ;
                        gcdfo:theme gcdfo:StockAssessmentTheme .


###  https://w3id.org/gcdfo/salmon#TrapCount
gcdfo:TrapCount rdf:type owl:NamedIndividual ,
                         skos:Concept ;
                rdfs:comment "Legacy methods: Trap, Hatchery Passage Counting"@en ;
                rdfs:isDefinedBy <https://w3id.org/gcdfo/salmon> ;
                skos:broader gcdfo:EnumerationMethod ;
                skos:definition "Trap-based counts from non-spanning traps with documented emptying schedule, efficiency measurements, and coverage information."@en ;
                skos:inScheme gcdfo:EnumerationMethodScheme ;
                skos:prefLabel "Trap Count"@en ;
                gcdfo:theme gcdfo:MonitoringFieldWorkTheme ,
                            gcdfo:StockAssessmentTheme .


###  https://w3id.org/gcdfo/salmon#TrapEfficiency
gcdfo:TrapEfficiency rdf:type owl:NamedIndividual ,
                              skos:Concept ;
                     rdfs:comment "Limits to Type 3 maximum"@en ;
                     rdfs:isDefinedBy <https://w3id.org/gcdfo/salmon> ;
                     skos:broader gcdfo:DowngradeCriteria ;
                     skos:definition "Trap efficiency not measured/validated"@en ;
                     skos:inScheme gcdfo:DowngradeCriteriaScheme ;
                     skos:prefLabel "Trap Efficiency"@en ;
                     gcdfo:theme gcdfo:DataModelProvenanceTheme ,
                                 gcdfo:StockAssessmentTheme .


###  https://w3id.org/gcdfo/salmon#TrapModelAnalysis
gcdfo:TrapModelAnalysis rdf:type owl:NamedIndividual ,
                                 skos:Concept ;
                        rdfs:comment "Requires documented trap efficiency measurements and cross-section coverage factors."@en ;
                        rdfs:isDefinedBy <https://w3id.org/gcdfo/salmon> ;
                        skos:broader gcdfo:EstimateMethod ;
                        skos:definition "Trap-based counts adjusted with efficiency/coverage models to estimate total passage."@en ;
                        skos:inScheme gcdfo:EstimateMethodScheme ;
                        skos:prefLabel "Trap Model Analysis"@en ;
                        gcdfo:theme gcdfo:MonitoringFieldWorkTheme ,
                                    gcdfo:StockAssessmentTheme .


###  https://w3id.org/gcdfo/salmon#Type1
gcdfo:Type1 rdf:type owl:NamedIndividual ,
                     skos:Concept ;
            rdfs:isDefinedBy <https://w3id.org/gcdfo/salmon> ;
            skos:broader gcdfo:EstimateType ;
            skos:definition "Total, seasonal counts through fence or fishway; virtually no bypass. Simple, often single step analysis. Reliable resolution of between year differences >10% (in absolute units)."@en ;
            skos:inScheme gcdfo:EstimateTypeScheme ;
            skos:prefLabel "Type-1, True Abundance, high resolution"@en ;
            gcdfo:theme gcdfo:DataModelProvenanceTheme ,
                        gcdfo:StockAssessmentTheme .


###  https://w3id.org/gcdfo/salmon#Type2
gcdfo:Type2 rdf:type owl:NamedIndividual ,
                     skos:Concept ;
            rdfs:isDefinedBy <https://w3id.org/gcdfo/salmon> ;
            skos:broader gcdfo:EstimateType ;
            skos:definition "Indirect estimate of total spawner abundance with qualified accuracy and known precision (i.e., a variance estimate—an explicit quantitative measure of uncertainty around the estimate). Derived from high-effort, standardized methods (e.g., mark-recapture, serial counts for area under the curve) with documented analytical conversions (including interpolation/calibration as needed). Reported in absolute units (estimate ± variance). Reliable resolution of between-year differences >25% (in absolute units)."@en ;
            skos:inScheme gcdfo:EstimateTypeScheme ;
            skos:prefLabel "Type-2, True Abundance, medium resolution"@en ;
            gcdfo:theme gcdfo:DataModelProvenanceTheme ,
                        gcdfo:StockAssessmentTheme .


###  https://w3id.org/gcdfo/salmon#Type3
gcdfo:Type3 rdf:type owl:NamedIndividual ,
                     skos:Concept ;
            rdfs:isDefinedBy <https://w3id.org/gcdfo/salmon> ;
            skos:broader gcdfo:EstimateType ;
            skos:definition "Relative abundance index (i.e., not an absolute count) derived from moderate to high effort surveys (typically 3 or more site visits) using standardized methods applied consistently between and within years (e.g., equal-effort surveys executed by walk, swim, overflight). Accuracy and precision are not fully quantified (i.e., no explicit variance estimate), but are assumed stable enough for within-series comparisons. Reliable resolution of between-year differences >25% (in relative units)."@en ;
            skos:inScheme gcdfo:EstimateTypeScheme ;
            skos:prefLabel "Type-3, Relative Abundance, high resolution"@en ;
            gcdfo:theme gcdfo:DataModelProvenanceTheme ,
                        gcdfo:StockAssessmentTheme .


###  https://w3id.org/gcdfo/salmon#Type4
gcdfo:Type4 rdf:type owl:NamedIndividual ,
                     skos:Concept ;
            rdfs:isDefinedBy <https://w3id.org/gcdfo/salmon> ;
            skos:broader gcdfo:EstimateType ;
            skos:definition "Low to moderate effort (1-4 trips), known survey method. Simple analysis by known methods. Reliable resolution of between year differences >200% (in relative units)."@en ;
            skos:inScheme gcdfo:EstimateTypeScheme ;
            skos:prefLabel "Type-4, Relative Abundance, medium resolution"@en ;
            gcdfo:theme gcdfo:DataModelProvenanceTheme ,
                        gcdfo:StockAssessmentTheme .


###  https://w3id.org/gcdfo/salmon#Type5
gcdfo:Type5 rdf:type owl:NamedIndividual ,
                     skos:Concept ;
            rdfs:isDefinedBy <https://w3id.org/gcdfo/salmon> ;
            skos:broader gcdfo:EstimateType ;
            skos:definition "Low effort (e.g. 1 trip), use of vaguely defined, inconsistent or poorly executed methods. Unknown to ill defined; inconsistent or poorly executed. Uncertain numeric comparisons, but high reliability for presence or absence."@en ;
            skos:inScheme gcdfo:EstimateTypeScheme ;
            skos:prefLabel "Type-5, Relative Abundance, low resolution"@en ;
            gcdfo:theme gcdfo:DataModelProvenanceTheme ,
                        gcdfo:StockAssessmentTheme .


###  https://w3id.org/gcdfo/salmon#Type6
gcdfo:Type6 rdf:type owl:NamedIndividual ,
                     skos:Concept ;
            rdfs:isDefinedBy <https://w3id.org/gcdfo/salmon> ;
            skos:altLabel "Presence/Not Detected"@en ;
            skos:broader gcdfo:EstimateType ;
            skos:definition "Non-numeric, year-specific record of presence/not detected (i.e., present/absent without estimating a count), tied to an explicit time and location, with reliable species identification. Underlying field methods may be highly variable; analysis is not required."@en ;
            skos:inScheme gcdfo:EstimateTypeScheme ;
            skos:prefLabel "Type-6, Presence or Absence"@en ;
            gcdfo:theme gcdfo:DataModelProvenanceTheme ,
                        gcdfo:StockAssessmentTheme .


###  https://w3id.org/gcdfo/salmon#UnrankedIndexQuality
gcdfo:UnrankedIndexQuality rdf:type owl:NamedIndividual ,
                                    skos:Concept ;
                           <http://purl.obolibrary.org/obo/IAO_0000115> "A data quality category indicating that no spawner-abundance estimate classification / index quality rating was assigned for the record (i.e., an 'Unknown' estimate classification with no quality rating)."@en ;
                           <http://purl.obolibrary.org/obo/IAO_0000119> "Fisheries and Oceans Canada. 2020. 2020 summary of abundance data for Chinook salmon (Oncorhynchus tshawytscha) in southern British Columbia, Canada (nuSEDS Estimate Classification includes 'Unknown: no quality rating')."@en ;
                           dcterms:source <https://waves-vagues.dfo-mpo.gc.ca/Library/40890041.pdf> ;
                           rdfs:isDefinedBy <https://w3id.org/gcdfo/salmon> ;
                           skos:broader gcdfo:EstimateType ;
                           skos:definition "A data quality category indicating that no spawner-abundance estimate classification / index quality rating was assigned for the record (i.e., an 'Unknown' estimate classification with no quality rating)."@en ;
                           skos:inScheme gcdfo:EstimateTypeScheme ;
                           skos:prefLabel "Unranked index quality"@en ;
                           gcdfo:theme gcdfo:DataModelProvenanceTheme ,
                                       gcdfo:StockAssessmentTheme .


###  https://w3id.org/gcdfo/salmon#UpperBenchmark
gcdfo:UpperBenchmark rdf:type owl:NamedIndividual ,
                              skos:Concept ;
                     rdfs:isDefinedBy <https://w3id.org/gcdfo/salmon> ;
                     skos:definition "An upper-threshold benchmark value, typically delineating the boundary between Amber and Green status zones."@en ;
                     skos:inScheme gcdfo:BenchmarkLevelScheme ;
                     skos:prefLabel "Upper benchmark"@en ;
                     gcdfo:theme gcdfo:StockAssessmentTheme ,
                                 gcdfo:WildSalmonPolicyTheme .


###  https://w3id.org/gcdfo/salmon#Uptime
gcdfo:Uptime rdf:type owl:NamedIndividual ,
                      skos:Concept ;
             rdfs:comment "Limits to Type 2 maximum"@en ;
             rdfs:isDefinedBy <https://w3id.org/gcdfo/salmon> ;
             skos:broader gcdfo:DowngradeCriteria ;
             skos:definition "Counting/device uptime < 95% (or <90% with interpolation)"@en ;
             skos:inScheme gcdfo:DowngradeCriteriaScheme ;
             skos:prefLabel "Uptime"@en ;
             gcdfo:theme gcdfo:DataModelProvenanceTheme ,
                         gcdfo:StockAssessmentTheme .


###  https://w3id.org/gcdfo/salmon#Visibility
gcdfo:Visibility rdf:type owl:NamedIndividual ,
                          skos:Concept ;
                 rdfs:comment "Limits to Type 3 maximum"@en ;
                 rdfs:isDefinedBy <https://w3id.org/gcdfo/salmon> ;
                 skos:broader gcdfo:DowngradeCriteria ;
                 skos:definition "Poor visibility conditions"@en ;
                 skos:inScheme gcdfo:DowngradeCriteriaScheme ;
                 skos:prefLabel "Visibility"@en ;
                 gcdfo:theme gcdfo:DataModelProvenanceTheme ,
                             gcdfo:StockAssessmentTheme .


###  https://w3id.org/gcdfo/salmon#VisualGroundCount
gcdfo:VisualGroundCount rdf:type owl:NamedIndividual ,
                                 skos:Concept ;
                        rdfs:comment "Legacy methods: Stream Walk, Ground count, Bank Walk"@en ;
                        rdfs:isDefinedBy <https://w3id.org/gcdfo/salmon> ;
                        skos:broader gcdfo:EnumerationMethod ;
                        skos:definition "Visual surveys conducted by stream/bank walk with documented visit schedule, reach coverage, timing, and visibility conditions."@en ;
                        skos:inScheme gcdfo:EnumerationMethodScheme ;
                        skos:prefLabel "Visual Ground Count"@en ;
                        gcdfo:theme gcdfo:MonitoringFieldWorkTheme ,
                                    gcdfo:StockAssessmentTheme .


###  https://w3id.org/gcdfo/salmon#VisualSnorkelCount
gcdfo:VisualSnorkelCount rdf:type owl:NamedIndividual ,
                                  skos:Concept ;
                         rdfs:comment "Legacy methods: Snorkel, Snorkel Swim"@en ;
                         rdfs:isDefinedBy <https://w3id.org/gcdfo/salmon> ;
                         skos:broader gcdfo:EnumerationMethod ;
                         skos:definition "Two or more trained snorkelers conduct standardized passes within defined segments, tallying live/dead by species. Field forms capture visibility class, segment boundaries, and repeat-visit schedule; counts are aggregated across observers/passes."@en ;
                         skos:inScheme gcdfo:EnumerationMethodScheme ;
                         skos:prefLabel "Visual Snorkel Count"@en ;
                         gcdfo:theme gcdfo:MonitoringFieldWorkTheme ,
                                     gcdfo:StockAssessmentTheme .


###  https://w3id.org/gcdfo/salmon#WSPBiologicalStatusZone
gcdfo:WSPBiologicalStatusZone rdf:type owl:NamedIndividual ,
                                       skos:Concept .


###  https://w3id.org/gcdfo/salmon#WSPBiologicalStatusZoneScheme
gcdfo:WSPBiologicalStatusZoneScheme rdf:type owl:NamedIndividual ,
                                             skos:ConceptScheme ;
                                    rdfs:isDefinedBy <https://w3id.org/gcdfo/salmon> ;
                                    skos:definition "Controlled vocabulary for biological status zones under the Wild Salmon Policy."@en ;
                                    skos:hasTopConcept gcdfo:WSPBiologicalStatusZone ;
                                    skos:prefLabel "Wild Salmon Policy Status Zone"@en ;
                                    gcdfo:theme gcdfo:PolicyGovernanceTheme ,
                                                gcdfo:StockAssessmentTheme ,
                                                gcdfo:WildSalmonPolicyTheme .


###  https://w3id.org/gcdfo/salmon#WildSalmonPolicy
gcdfo:WildSalmonPolicy rdf:type owl:NamedIndividual ,
                                skos:Concept ;
                       rdfs:isDefinedBy <https://w3id.org/gcdfo/salmon> ;
                       skos:altLabel "WSP"@en ;
                       skos:broader gcdfo:PolicyFramework ;
                       skos:definition "Canada's Wild Salmon Policy framework for conserving and managing wild Pacific salmon, including integrated status assessments and biological benchmarks for Conservation Units."@en ;
                       skos:inScheme gcdfo:PolicyFrameworkScheme ;
                       skos:prefLabel "Wild Salmon Policy"@en ;
                       gcdfo:theme gcdfo:PolicyGovernanceTheme ,
                                   gcdfo:StockAssessmentTheme ,
                                   gcdfo:WildSalmonPolicyTheme .


###  https://w3id.org/gcdfo/salmon#WildSalmonPolicyTheme
gcdfo:WildSalmonPolicyTheme rdf:type owl:NamedIndividual ,
                                     skos:Concept ;
                            rdfs:isDefinedBy <https://w3id.org/gcdfo/salmon> ;
                            skos:definition "Conservation Unit based stock assessment methods, metrics, and metadata"@en ;
                            skos:inScheme gcdfo:ThemeScheme ;
                            skos:prefLabel "Wild Salmon Policy"@en ;
                            gcdfo:theme gcdfo:DataModelProvenanceTheme .


#################################################################
#    Annotations
#################################################################

gcdfo:ConfidenceCategory rdfs:isDefinedBy <https://w3id.org/gcdfo/salmon> ;
                         skos:definition "Categorical confidence rating (High, Medium, Low) for stock assessment metrics."@en ;
                         skos:inScheme gcdfo:RapidStatusConfidenceScheme ;
                         skos:prefLabel "Confidence category"@en ;
                         gcdfo:theme gcdfo:StockAssessmentTheme ,
                                     gcdfo:WildSalmonPolicyTheme .


gcdfo:WSPBiologicalStatusZone <http://purl.obolibrary.org/obo/IAO_0000119> "Fisheries and Oceans Canada. Wild Salmon Policy 2018-2022 Implementation Plan. https://waves-vagues.dfo-mpo.gc.ca/library-bibliotheque/40728109.pdf."@en ;
                              dcterms:source <https://waves-vagues.dfo-mpo.gc.ca/library-bibliotheque/40728109.pdf> ;
                              rdfs:isDefinedBy <https://w3id.org/gcdfo/salmon> ;
                              skos:definition "The biological status of a Conservation Unit (CU) will normally be based on the abundance and distribution of spawners in the unit, or proxies thereof. For each CU, higher and lower benchmarks will be defined that will delimit three status zones: Green, Amber, and Red. As spawner abundance decreases, a CU moves towards the lower status zone, and the extent of management intervention for conservation purposes will increase."@en ;
                              skos:inScheme gcdfo:WSPBiologicalStatusZoneScheme ;
                              skos:prefLabel "Wild Salmon Policy biological status zone"@en ;
                              gcdfo:theme gcdfo:PolicyGovernanceTheme ,
                                          gcdfo:StockAssessmentTheme ,
                                          gcdfo:WildSalmonPolicyTheme .


###  Generated by the OWL API (version 4.5.29) https://github.com/owlcs/owlapi
