<?xml version="1.0"?>
<rdf:RDF xmlns="https://w3id.org/gcdfo/salmon#"
     xml:base="https://w3id.org/gcdfo/salmon"
     xmlns:oa="http://www.w3.org/ns/oa#"
     xmlns:bfo="http://purl.obolibrary.org/obo/BFO_"
     xmlns:dqv="http://www.w3.org/ns/dqv#"
     xmlns:dwc="http://rs.tdwg.org/dwc/terms/"
     xmlns:iao="http://purl.obolibrary.org/obo/IAO_"
     xmlns:obo="http://purl.obolibrary.org/obo/"
     xmlns:odo="http://purl.dataone.org/odo/"
     xmlns:org="http://www.w3.org/ns/org#"
     xmlns:owl="http://www.w3.org/2002/07/owl#"
     xmlns:rdf="http://www.w3.org/1999/02/22-rdf-syntax-ns#"
     xmlns:xml="http://www.w3.org/XML/1998/namespace"
     xmlns:xsd="http://www.w3.org/2001/XMLSchema#"
     xmlns:envo="http://purl.obolibrary.org/obo/ENVO_"
     xmlns:prov="http://www.w3.org/ns/prov#"
     xmlns:qudt="http://qudt.org/schema/qudt/"
     xmlns:rdfs="http://www.w3.org/2000/01/rdf-schema#"
     xmlns:skos="http://www.w3.org/2004/02/skos/core#"
     xmlns:vann="http://purl.org/vocab/vann/"
     xmlns:gcdfo="https://w3id.org/gcdfo/salmon#"
     xmlns:dwciri="http://rs.tdwg.org/dwc/iri/"
     xmlns:schema="https://schema.org/"
     xmlns:dcterms="http://purl.org/dc/terms/"
     xmlns:qudtunit="http://qudt.org/vocab/unit/">
    <owl:Ontology rdf:about="https://w3id.org/gcdfo/salmon">
        <owl:versionIRI rdf:resource="https://w3id.org/gcdfo/salmon/0.0.6-alpha"/>
        <obo:IAO_0000115 xml:lang="en">Hybrid OWL+SKOS ontology for DFO salmon data. Uses SKOS for controlled vocabularies (methods, criteria) and OWL for formal relationships and events.</obo:IAO_0000115>
        <dcterms:contributor xml:lang="en">Brett Johnson</dcterms:contributor>
        <dcterms:contributor xml:lang="en">Melissa K. Morrison</dcterms:contributor>
        <dcterms:created rdf:datatype="http://www.w3.org/2001/XMLSchema#date">2025-09-06</dcterms:created>
        <dcterms:creator xml:lang="en">Fishery &amp; Assessment Data Section (FADS) Data Stewardship Unit</dcterms:creator>
        <dcterms:description xml:lang="en">OWL + SKOS ontology for DFO salmon data: stocks/CUs/MUs, survey events, escapement measurements, and GSI constructs; aligns to DwC via rdfs:subClassOf; hybrid approach with SKOS for methods and OWL for events.</dcterms:description>
        <dcterms:license rdf:resource="https://creativecommons.org/licenses/by/4.0/"/>
        <dcterms:modified rdf:datatype="http://www.w3.org/2001/XMLSchema#date">2026-02-24</dcterms:modified>
        <dcterms:publisher xml:lang="en">Fisheries and Oceans Canada (DFO) Pacific Region Science Branch</dcterms:publisher>
        <dcterms:title xml:lang="en">DFO Salmon Ontology</dcterms:title>
        <vann:preferredNamespacePrefix>gcdfo</vann:preferredNamespacePrefix>
        <vann:preferredNamespaceUri>https://w3id.org/gcdfo/salmon#</vann:preferredNamespaceUri>
        <rdfs:seeAlso rdf:resource="https://github.com/dfo-pacific-science/dfo-salmon-ontology"/>
        <owl:priorVersion rdf:resource="https://w3id.org/gcdfo/salmon/0.0.2"/>
        <owl:versionInfo>0.0.6-alpha (integrated pre-release review branch)</owl:versionInfo>
        <schema:codeRepository rdf:resource="https://github.com/dfo-pacific-science/dfo-salmon-ontology"/>
    </owl:Ontology>
    


    <!-- 
    ///////////////////////////////////////////////////////////////////////////////////////
    //
    // Annotation properties
    //
    ///////////////////////////////////////////////////////////////////////////////////////
     -->

    


    <!-- http://purl.obolibrary.org/obo/IAO_0000115 -->

    <owl:AnnotationProperty rdf:about="http://purl.obolibrary.org/obo/IAO_0000115">
        <rdfs:isDefinedBy rdf:resource="http://purl.obolibrary.org/obo/iao.owl"/>
        <rdfs:label xml:lang="en">definition</rdfs:label>
    </owl:AnnotationProperty>
    


    <!-- http://purl.obolibrary.org/obo/IAO_0000119 -->

    <owl:AnnotationProperty rdf:about="http://purl.obolibrary.org/obo/IAO_0000119">
        <rdfs:isDefinedBy rdf:resource="http://purl.obolibrary.org/obo/iao.owl"/>
        <rdfs:label xml:lang="en">definition source</rdfs:label>
    </owl:AnnotationProperty>
    


    <!-- http://purl.org/dc/terms/contributor -->

    <owl:AnnotationProperty rdf:about="http://purl.org/dc/terms/contributor"/>
    


    <!-- http://purl.org/dc/terms/created -->

    <owl:AnnotationProperty rdf:about="http://purl.org/dc/terms/created"/>
    


    <!-- http://purl.org/dc/terms/creator -->

    <owl:AnnotationProperty rdf:about="http://purl.org/dc/terms/creator"/>
    


    <!-- http://purl.org/dc/terms/description -->

    <owl:AnnotationProperty rdf:about="http://purl.org/dc/terms/description"/>
    


    <!-- http://purl.org/dc/terms/identifier -->

    <owl:AnnotationProperty rdf:about="http://purl.org/dc/terms/identifier"/>
    


    <!-- http://purl.org/dc/terms/isPartOf -->

    <owl:AnnotationProperty rdf:about="http://purl.org/dc/terms/isPartOf"/>
    


    <!-- http://purl.org/dc/terms/isVersionOf -->

    <owl:AnnotationProperty rdf:about="http://purl.org/dc/terms/isVersionOf"/>
    


    <!-- http://purl.org/dc/terms/license -->

    <owl:AnnotationProperty rdf:about="http://purl.org/dc/terms/license"/>
    


    <!-- http://purl.org/dc/terms/modified -->

    <owl:AnnotationProperty rdf:about="http://purl.org/dc/terms/modified"/>
    


    <!-- http://purl.org/dc/terms/publisher -->

    <owl:AnnotationProperty rdf:about="http://purl.org/dc/terms/publisher"/>
    


    <!-- http://purl.org/dc/terms/source -->

    <owl:AnnotationProperty rdf:about="http://purl.org/dc/terms/source"/>
    


    <!-- http://purl.org/dc/terms/title -->

    <owl:AnnotationProperty rdf:about="http://purl.org/dc/terms/title"/>
    


    <!-- http://purl.org/vocab/vann/preferredNamespacePrefix -->

    <owl:AnnotationProperty rdf:about="http://purl.org/vocab/vann/preferredNamespacePrefix"/>
    


    <!-- http://purl.org/vocab/vann/preferredNamespaceUri -->

    <owl:AnnotationProperty rdf:about="http://purl.org/vocab/vann/preferredNamespaceUri"/>
    


    <!-- http://www.w3.org/2004/02/skos/core#altLabel -->

    <owl:AnnotationProperty rdf:about="http://www.w3.org/2004/02/skos/core#altLabel"/>
    


    <!-- http://www.w3.org/2004/02/skos/core#broader -->

    <owl:AnnotationProperty rdf:about="http://www.w3.org/2004/02/skos/core#broader"/>
    


    <!-- http://www.w3.org/2004/02/skos/core#closeMatch -->

    <owl:AnnotationProperty rdf:about="http://www.w3.org/2004/02/skos/core#closeMatch"/>
    


    <!-- http://www.w3.org/2004/02/skos/core#definition -->

    <owl:AnnotationProperty rdf:about="http://www.w3.org/2004/02/skos/core#definition"/>
    


    <!-- http://www.w3.org/2004/02/skos/core#exactMatch -->

    <owl:AnnotationProperty rdf:about="http://www.w3.org/2004/02/skos/core#exactMatch"/>
    


    <!-- http://www.w3.org/2004/02/skos/core#hasTopConcept -->

    <owl:AnnotationProperty rdf:about="http://www.w3.org/2004/02/skos/core#hasTopConcept"/>
    


    <!-- http://www.w3.org/2004/02/skos/core#inScheme -->

    <owl:AnnotationProperty rdf:about="http://www.w3.org/2004/02/skos/core#inScheme"/>
    


    <!-- http://www.w3.org/2004/02/skos/core#notation -->

    <owl:AnnotationProperty rdf:about="http://www.w3.org/2004/02/skos/core#notation"/>
    


    <!-- http://www.w3.org/2004/02/skos/core#prefLabel -->

    <owl:AnnotationProperty rdf:about="http://www.w3.org/2004/02/skos/core#prefLabel"/>
    


    <!-- http://www.w3.org/2004/02/skos/core#scopeNote -->

    <owl:AnnotationProperty rdf:about="http://www.w3.org/2004/02/skos/core#scopeNote"/>
    


    <!-- https://schema.org/codeRepository -->

    <owl:AnnotationProperty rdf:about="https://schema.org/codeRepository"/>
    


    <!-- https://w3id.org/gcdfo/salmon#theme -->

    <owl:AnnotationProperty rdf:about="https://w3id.org/gcdfo/salmon#theme">
        <rdfs:comment xml:lang="en">Associates OWL classes and SKOS concepts with high-level thematic concept schemes (e.g., Stock Assessment, GSI, Policy).</rdfs:comment>
        <rdfs:isDefinedBy rdf:resource="https://w3id.org/gcdfo/salmon"/>
        <rdfs:label xml:lang="en">theme</rdfs:label>
        <theme rdf:resource="https://w3id.org/gcdfo/salmon#DataModelProvenanceTheme"/>
    </owl:AnnotationProperty>
    


    <!-- 
    ///////////////////////////////////////////////////////////////////////////////////////
    //
    // Datatypes
    //
    ///////////////////////////////////////////////////////////////////////////////////////
     -->

    


    <!-- http://www.w3.org/2001/XMLSchema#anyURI -->

    <rdfs:Datatype rdf:about="http://www.w3.org/2001/XMLSchema#anyURI"/>
    


    <!-- http://www.w3.org/2001/XMLSchema#boolean -->

    <rdfs:Datatype rdf:about="http://www.w3.org/2001/XMLSchema#boolean"/>
    


    <!-- http://www.w3.org/2001/XMLSchema#date -->

    <rdfs:Datatype rdf:about="http://www.w3.org/2001/XMLSchema#date"/>
    


    <!-- http://www.w3.org/2001/XMLSchema#dateTime -->

    <rdfs:Datatype rdf:about="http://www.w3.org/2001/XMLSchema#dateTime"/>
    


    <!-- http://www.w3.org/2001/XMLSchema#decimal -->

    <rdfs:Datatype rdf:about="http://www.w3.org/2001/XMLSchema#decimal"/>
    


    <!-- http://www.w3.org/2001/XMLSchema#gYear -->

    <rdfs:Datatype rdf:about="http://www.w3.org/2001/XMLSchema#gYear"/>
    


    <!-- http://www.w3.org/2001/XMLSchema#integer -->

    <rdfs:Datatype rdf:about="http://www.w3.org/2001/XMLSchema#integer"/>
    


    <!-- http://www.w3.org/2001/XMLSchema#string -->

    <rdfs:Datatype rdf:about="http://www.w3.org/2001/XMLSchema#string"/>
    


    <!-- 
    ///////////////////////////////////////////////////////////////////////////////////////
    //
    // Object Properties
    //
    ///////////////////////////////////////////////////////////////////////////////////////
     -->

    


    <!-- http://www.w3.org/ns/dqv#inDimension -->

    <owl:ObjectProperty rdf:about="http://www.w3.org/ns/dqv#inDimension">
        <obo:IAO_0000115 xml:lang="en">Represents the dimensions a quality metric, certificate and annotation allow a measurement of.</obo:IAO_0000115>
        <obo:IAO_0000119 rdf:resource="https://www.w3.org/TR/vocab-dqv/"/>
        <rdfs:comment xml:lang="en">Dimensions are meant to systematically organize metrics, quality certificates and quality annotations. The Data Quality Vocabulary defines no specific cardinality constraints for dqv:inDimension, since distinct quality frameworks might have different perspectives over a metric. A metric may therefore be associated to more than one dimension. However, those who define new quality metrics should try to avoid this as much as possible and assign only one dimension to the metrics they define. More than one dimension can be indicated for each quality annotation or certificate.</rdfs:comment>
        <rdfs:isDefinedBy rdf:resource="http://www.w3.org/ns/dqv#"/>
        <rdfs:label xml:lang="en">in dimension</rdfs:label>
    </owl:ObjectProperty>
    


    <!-- https://w3id.org/gcdfo/salmon#conservationUnitOf -->

    <owl:ObjectProperty rdf:about="https://w3id.org/gcdfo/salmon#conservationUnitOf">
        <owl:inverseOf rdf:resource="https://w3id.org/gcdfo/salmon#hasConservationUnit"/>
        <rdfs:domain rdf:resource="https://w3id.org/gcdfo/salmon#ConservationUnit"/>
        <rdfs:range rdf:resource="https://w3id.org/gcdfo/salmon#StockManagementUnit"/>
        <obo:IAO_0000115 xml:lang="en">Relates a Conservation Unit to the Stock Management Unit it belongs to.</obo:IAO_0000115>
        <rdfs:isDefinedBy rdf:resource="https://w3id.org/gcdfo/salmon"/>
        <rdfs:label xml:lang="en">Conservation Unit of</rdfs:label>
        <theme rdf:resource="https://w3id.org/gcdfo/salmon#FisheriesManagementTheme"/>
        <theme rdf:resource="https://w3id.org/gcdfo/salmon#PolicyGovernanceTheme"/>
        <theme rdf:resource="https://w3id.org/gcdfo/salmon#WildSalmonPolicyTheme"/>
    </owl:ObjectProperty>
    


    <!-- https://w3id.org/gcdfo/salmon#demeOf -->

    <owl:ObjectProperty rdf:about="https://w3id.org/gcdfo/salmon#demeOf">
        <owl:inverseOf rdf:resource="https://w3id.org/gcdfo/salmon#hasDeme"/>
        <rdfs:domain rdf:resource="https://w3id.org/gcdfo/salmon#Deme"/>
        <rdfs:range rdf:resource="https://w3id.org/gcdfo/salmon#Population"/>
        <obo:IAO_0000115 xml:lang="en">Relates a deme to the population it belongs to.</obo:IAO_0000115>
        <rdfs:isDefinedBy rdf:resource="https://w3id.org/gcdfo/salmon"/>
        <rdfs:label xml:lang="en">deme of</rdfs:label>
        <theme rdf:resource="https://w3id.org/gcdfo/salmon#GeneticsStockCompositionTheme"/>
        <theme rdf:resource="https://w3id.org/gcdfo/salmon#WildSalmonPolicyTheme"/>
    </owl:ObjectProperty>
    


    <!-- https://w3id.org/gcdfo/salmon#hasConservationUnit -->

    <owl:ObjectProperty rdf:about="https://w3id.org/gcdfo/salmon#hasConservationUnit">
        <rdfs:domain rdf:resource="https://w3id.org/gcdfo/salmon#StockManagementUnit"/>
        <rdfs:range rdf:resource="https://w3id.org/gcdfo/salmon#ConservationUnit"/>
        <obo:IAO_0000115 xml:lang="en">Relates a Stock Management Unit to one of its constituent Conservation Units.</obo:IAO_0000115>
        <rdfs:isDefinedBy rdf:resource="https://w3id.org/gcdfo/salmon"/>
        <rdfs:label xml:lang="en">has Conservation Unit</rdfs:label>
        <theme rdf:resource="https://w3id.org/gcdfo/salmon#FisheriesManagementTheme"/>
        <theme rdf:resource="https://w3id.org/gcdfo/salmon#PolicyGovernanceTheme"/>
        <theme rdf:resource="https://w3id.org/gcdfo/salmon#WildSalmonPolicyTheme"/>
    </owl:ObjectProperty>
    


    <!-- https://w3id.org/gcdfo/salmon#hasDeme -->

    <owl:ObjectProperty rdf:about="https://w3id.org/gcdfo/salmon#hasDeme">
        <rdfs:domain rdf:resource="https://w3id.org/gcdfo/salmon#Population"/>
        <rdfs:range rdf:resource="https://w3id.org/gcdfo/salmon#Deme"/>
        <obo:IAO_0000115 xml:lang="en">Relates a population to one of its constituent demes.</obo:IAO_0000115>
        <rdfs:isDefinedBy rdf:resource="https://w3id.org/gcdfo/salmon"/>
        <rdfs:label xml:lang="en">has deme</rdfs:label>
        <theme rdf:resource="https://w3id.org/gcdfo/salmon#GeneticsStockCompositionTheme"/>
        <theme rdf:resource="https://w3id.org/gcdfo/salmon#WildSalmonPolicyTheme"/>
    </owl:ObjectProperty>
    


    <!-- https://w3id.org/gcdfo/salmon#hasPopulation -->

    <owl:ObjectProperty rdf:about="https://w3id.org/gcdfo/salmon#hasPopulation">
        <owl:inverseOf rdf:resource="https://w3id.org/gcdfo/salmon#populationOf"/>
        <rdfs:domain rdf:resource="https://w3id.org/gcdfo/salmon#ConservationUnit"/>
        <rdfs:range rdf:resource="https://w3id.org/gcdfo/salmon#Population"/>
        <obo:IAO_0000115 xml:lang="en">Relates a Conservation Unit to one of its constituent populations.</obo:IAO_0000115>
        <rdfs:isDefinedBy rdf:resource="https://w3id.org/gcdfo/salmon"/>
        <rdfs:label xml:lang="en">has population</rdfs:label>
        <theme rdf:resource="https://w3id.org/gcdfo/salmon#StockAssessmentTheme"/>
        <theme rdf:resource="https://w3id.org/gcdfo/salmon#WildSalmonPolicyTheme"/>
    </owl:ObjectProperty>
    


    <!-- https://w3id.org/gcdfo/salmon#hasTargetOrLimitExploitationRate -->

    <owl:ObjectProperty rdf:about="https://w3id.org/gcdfo/salmon#hasTargetOrLimitExploitationRate">
        <owl:inverseOf rdf:resource="https://w3id.org/gcdfo/salmon#isTargetOrLimitForObservedExploitationRate"/>
        <rdfs:domain rdf:resource="https://w3id.org/gcdfo/salmon#ObservedExploitationRate"/>
        <rdfs:range rdf:resource="https://w3id.org/gcdfo/salmon#TargetOrLimitExploitationRate"/>
        <obo:IAO_0000115 xml:lang="en">Relates an observed exploitation-rate estimate to the target, threshold, or limit exploitation-rate value used to evaluate it.</obo:IAO_0000115>
        <rdfs:isDefinedBy rdf:resource="https://w3id.org/gcdfo/salmon"/>
        <rdfs:label xml:lang="en">has target or limit exploitation rate</rdfs:label>
        <theme rdf:resource="https://w3id.org/gcdfo/salmon#FisheriesManagementTheme"/>
        <theme rdf:resource="https://w3id.org/gcdfo/salmon#PolicyGovernanceTheme"/>
        <theme rdf:resource="https://w3id.org/gcdfo/salmon#StockAssessmentTheme"/>
    </owl:ObjectProperty>
    


    <!-- https://w3id.org/gcdfo/salmon#hasYearBasis -->

    <owl:ObjectProperty rdf:about="https://w3id.org/gcdfo/salmon#hasYearBasis">
        <rdfs:domain>
            <owl:Class>
                <owl:unionOf rdf:parseType="Collection">
                    <rdf:Description rdf:about="https://w3id.org/gcdfo/salmon#EscapementMeasurement"/>
                    <rdf:Description rdf:about="https://w3id.org/gcdfo/salmon#ExploitationRate"/>
                    <rdf:Description rdf:about="https://w3id.org/gcdfo/salmon#ObservedExploitationRate"/>
                    <rdf:Description rdf:about="https://w3id.org/gcdfo/salmon#SpawnerAbundance"/>
                    <rdf:Description rdf:about="https://w3id.org/gcdfo/salmon#TargetOrLimitExploitationRate"/>
                    <rdf:Description rdf:about="https://w3id.org/gcdfo/salmon#TotalExploitationRate"/>
                </owl:unionOf>
            </owl:Class>
        </rdfs:domain>
        <rdfs:range>
            <owl:Class>
                <owl:unionOf rdf:parseType="Collection">
                    <rdf:Description rdf:about="https://w3id.org/gcdfo/salmon#BroodYear"/>
                    <rdf:Description rdf:about="https://w3id.org/gcdfo/salmon#CatchYear"/>
                    <rdf:Description rdf:about="https://w3id.org/gcdfo/salmon#ReturnYear"/>
                </owl:unionOf>
            </owl:Class>
        </rdfs:range>
        <obo:IAO_0000115 xml:lang="en">Links a measurement or rate to the year basis (e.g., brood year, catch year, or return year) it is reported against.</obo:IAO_0000115>
        <rdfs:isDefinedBy rdf:resource="https://w3id.org/gcdfo/salmon"/>
        <rdfs:label xml:lang="en">has year basis</rdfs:label>
        <theme rdf:resource="https://w3id.org/gcdfo/salmon#DataModelProvenanceTheme"/>
        <theme rdf:resource="https://w3id.org/gcdfo/salmon#StockAssessmentTheme"/>
    </owl:ObjectProperty>
    


    <!-- https://w3id.org/gcdfo/salmon#isTargetOrLimitForObservedExploitationRate -->

    <owl:ObjectProperty rdf:about="https://w3id.org/gcdfo/salmon#isTargetOrLimitForObservedExploitationRate">
        <rdfs:domain rdf:resource="https://w3id.org/gcdfo/salmon#TargetOrLimitExploitationRate"/>
        <rdfs:range rdf:resource="https://w3id.org/gcdfo/salmon#ObservedExploitationRate"/>
        <obo:IAO_0000115 xml:lang="en">Relates a target, threshold, or limit exploitation-rate value to the observed exploitation-rate estimate it evaluates.</obo:IAO_0000115>
        <rdfs:isDefinedBy rdf:resource="https://w3id.org/gcdfo/salmon"/>
        <rdfs:label xml:lang="en">is target or limit for observed exploitation rate</rdfs:label>
        <theme rdf:resource="https://w3id.org/gcdfo/salmon#FisheriesManagementTheme"/>
        <theme rdf:resource="https://w3id.org/gcdfo/salmon#PolicyGovernanceTheme"/>
        <theme rdf:resource="https://w3id.org/gcdfo/salmon#StockAssessmentTheme"/>
    </owl:ObjectProperty>
    


    <!-- https://w3id.org/gcdfo/salmon#populationOf -->

    <owl:ObjectProperty rdf:about="https://w3id.org/gcdfo/salmon#populationOf">
        <rdfs:domain rdf:resource="https://w3id.org/gcdfo/salmon#Population"/>
        <rdfs:range rdf:resource="https://w3id.org/gcdfo/salmon#ConservationUnit"/>
        <obo:IAO_0000115 xml:lang="en">Relates a population to the Conservation Unit it belongs to.</obo:IAO_0000115>
        <rdfs:isDefinedBy rdf:resource="https://w3id.org/gcdfo/salmon"/>
        <rdfs:label xml:lang="en">population of</rdfs:label>
        <theme rdf:resource="https://w3id.org/gcdfo/salmon#StockAssessmentTheme"/>
        <theme rdf:resource="https://w3id.org/gcdfo/salmon#WildSalmonPolicyTheme"/>
    </owl:ObjectProperty>
    


    <!-- 
    ///////////////////////////////////////////////////////////////////////////////////////
    //
    // Classes
    //
    ///////////////////////////////////////////////////////////////////////////////////////
     -->

    


    <!-- http://purl.dataone.org/odo/ECSO_00002050 -->

    <owl:Class rdf:about="http://purl.dataone.org/odo/ECSO_00002050">
        <rdfs:subClassOf rdf:resource="http://purl.obolibrary.org/obo/IAO_0000109"/>
        <obo:IAO_0000115 xml:lang="en">year of measurement</obo:IAO_0000115>
        <rdfs:isDefinedBy rdf:resource="http://purl.dataone.org/odo/"/>
        <rdfs:label xml:lang="en">year of measurement</rdfs:label>
    </owl:Class>
    


    <!-- http://purl.dataone.org/odo/SALMON_00000137 -->

    <owl:Class rdf:about="http://purl.dataone.org/odo/SALMON_00000137">
        <rdfs:subClassOf rdf:resource="http://purl.obolibrary.org/obo/BFO_0000040"/>
        <obo:IAO_0000115 xml:lang="en">The Food and Agriculture Organization of the United Nations (FAO) defines a fishery as &apos;...an activity leading to harvesting of fish. It may involve capture of wild fish or raising of fish through aquaculture.&apos;</obo:IAO_0000115>
        <rdfs:isDefinedBy rdf:resource="http://purl.dataone.org/odo/"/>
        <rdfs:label xml:lang="en">Fishery type</rdfs:label>
    </owl:Class>
    


    <!-- http://purl.dataone.org/odo/SALMON_00000167 -->

    <owl:Class rdf:about="http://purl.dataone.org/odo/SALMON_00000167">
        <rdfs:subClassOf rdf:resource="http://purl.obolibrary.org/obo/IAO_0000030"/>
        <obo:IAO_0000115 xml:lang="en">A measurement type taken of some physical, biological, or ecological aspect of a fish or fishes.</obo:IAO_0000115>
        <rdfs:isDefinedBy rdf:resource="http://purl.dataone.org/odo/"/>
        <rdfs:label xml:lang="en">Fish measurement type</rdfs:label>
    </owl:Class>
    


    <!-- http://purl.dataone.org/odo/SALMON_00000479 -->

    <owl:Class rdf:about="http://purl.dataone.org/odo/SALMON_00000479">
        <rdfs:subClassOf rdf:resource="http://purl.obolibrary.org/obo/IAO_0000109"/>
        <obo:IAO_0000115 xml:lang="en">The number of salmon which do not get caught by commercial or recreational fisheries and return to their freshwater spawning habitat.</obo:IAO_0000115>
        <rdfs:isDefinedBy rdf:resource="http://purl.dataone.org/odo/"/>
        <rdfs:label xml:lang="en">Salmon escapement count</rdfs:label>
    </owl:Class>
    


    <!-- http://purl.dataone.org/odo/SALMON_00000639 -->

    <owl:Class rdf:about="http://purl.dataone.org/odo/SALMON_00000639">
        <rdfs:subClassOf rdf:resource="http://purl.obolibrary.org/obo/BFO_0000040"/>
        <obo:IAO_0000115 xml:lang="en">Group of individuals of a species which can be regarded as an entity for management or assessment purposes; a separate breeding population of a species; term used to identify a management unit of fishery species. A distinct genetic population, a population defined by movement pattern, part of a population potentially harvestable, or a quantity of fish from a given area. May be a total or a spawning stock.</obo:IAO_0000115>
        <rdfs:isDefinedBy rdf:resource="http://purl.dataone.org/odo/"/>
        <rdfs:label xml:lang="en">Fish stock type</rdfs:label>
    </owl:Class>
    


    <!-- http://purl.obolibrary.org/obo/BFO_0000015 -->

    <owl:Class rdf:about="http://purl.obolibrary.org/obo/BFO_0000015">
        <obo:IAO_0000115 xml:lang="en">An occurrent that has temporal parts and for some time t, p s-depends_on some material entity at t.</obo:IAO_0000115>
        <rdfs:isDefinedBy rdf:resource="http://purl.obolibrary.org/obo/bfo.owl"/>
        <rdfs:label xml:lang="en">process</rdfs:label>
    </owl:Class>
    


    <!-- http://purl.obolibrary.org/obo/BFO_0000020 -->

    <owl:Class rdf:about="http://purl.obolibrary.org/obo/BFO_0000020">
        <obo:IAO_0000115 xml:lang="en">b is a specifically dependent continuant = Def. b is a continuant &amp; there is some independent continuant c which is not a spatial region and which is such that b s-depends_on c at every time t during the course of b’s existence. (axiom label in BFO2 Reference: [050-003])</obo:IAO_0000115>
        <rdfs:isDefinedBy rdf:resource="http://purl.obolibrary.org/obo/bfo.owl"/>
        <rdfs:label xml:lang="en">specifically dependent continuant</rdfs:label>
    </owl:Class>
    


    <!-- http://purl.obolibrary.org/obo/BFO_0000031 -->

    <owl:Class rdf:about="http://purl.obolibrary.org/obo/BFO_0000031">
        <obo:IAO_0000115 xml:lang="en">A continuant that is dependent on one or more independent continuants and whose instances can be multiply instantiated.</obo:IAO_0000115>
        <rdfs:isDefinedBy rdf:resource="http://purl.obolibrary.org/obo/bfo.owl"/>
        <rdfs:label xml:lang="en">generically dependent continuant</rdfs:label>
    </owl:Class>
    


    <!-- http://purl.obolibrary.org/obo/BFO_0000040 -->

    <owl:Class rdf:about="http://purl.obolibrary.org/obo/BFO_0000040">
        <obo:IAO_0000115 xml:lang="en">An independent continuant that is spatially extended whose identity is independent of that of other entities and can be maintained through time.</obo:IAO_0000115>
        <rdfs:isDefinedBy rdf:resource="http://purl.obolibrary.org/obo/bfo.owl"/>
        <rdfs:label xml:lang="en">material entity</rdfs:label>
    </owl:Class>
    


    <!-- http://purl.obolibrary.org/obo/ENVO_00000020 -->

    <owl:Class rdf:about="http://purl.obolibrary.org/obo/ENVO_00000020">
        <rdfs:subClassOf rdf:resource="http://purl.obolibrary.org/obo/ENVO_01000617"/>
        <obo:IAO_0000115 xml:lang="en">A body of water or other liquid of considerable size contained in a depression on a landmass.</obo:IAO_0000115>
        <rdfs:isDefinedBy rdf:resource="http://purl.obolibrary.org/obo/envo.owl"/>
        <rdfs:label xml:lang="en">lake</rdfs:label>
    </owl:Class>
    


    <!-- http://purl.obolibrary.org/obo/ENVO_00000022 -->

    <owl:Class rdf:about="http://purl.obolibrary.org/obo/ENVO_00000022">
        <rdfs:subClassOf rdf:resource="http://purl.obolibrary.org/obo/ENVO_01000618"/>
        <obo:IAO_0000115 xml:lang="en">A stream which, through permanent or seasonal flow processes, moves from elevated land towards lower elevations through a definite channel and empties either into a sea, lake, or another river or ends on land as bed seepage and evapotranspiration exceed water supply.</obo:IAO_0000115>
        <rdfs:isDefinedBy rdf:resource="http://purl.obolibrary.org/obo/envo.owl"/>
        <rdfs:label xml:lang="en">river</rdfs:label>
    </owl:Class>
    


    <!-- http://purl.obolibrary.org/obo/ENVO_00000023 -->

    <owl:Class rdf:about="http://purl.obolibrary.org/obo/ENVO_00000023">
        <rdfs:subClassOf rdf:resource="http://purl.obolibrary.org/obo/ENVO_01000618"/>
        <obo:IAO_0000115 xml:lang="en">A watercourse which is linear and flows across the solid portion of a planetary surface.</obo:IAO_0000115>
        <rdfs:comment xml:lang="en">A creek is typically smaller than a stream.</rdfs:comment>
        <rdfs:isDefinedBy rdf:resource="http://purl.obolibrary.org/obo/envo.owl"/>
        <rdfs:label xml:lang="en">stream</rdfs:label>
        <skos:altLabel xml:lang="en">creek</skos:altLabel>
    </owl:Class>
    


    <!-- http://purl.obolibrary.org/obo/ENVO_00000033 -->

    <owl:Class rdf:about="http://purl.obolibrary.org/obo/ENVO_00000033">
        <rdfs:subClassOf rdf:resource="http://purl.obolibrary.org/obo/ENVO_01000617"/>
        <obo:IAO_0000115 xml:lang="en">A body of water, usually of smaller size than a lake.</obo:IAO_0000115>
        <rdfs:isDefinedBy rdf:resource="http://purl.obolibrary.org/obo/envo.owl"/>
        <rdfs:label xml:lang="en">pond</rdfs:label>
    </owl:Class>
    


    <!-- http://purl.obolibrary.org/obo/ENVO_00000063 -->

    <owl:Class rdf:about="http://purl.obolibrary.org/obo/ENVO_00000063">
        <rdfs:subClassOf rdf:resource="http://purl.obolibrary.org/obo/BFO_0000040"/>
        <rdfs:isDefinedBy rdf:resource="http://purl.obolibrary.org/obo/envo.owl"/>
        <rdfs:label xml:lang="en">water body</rdfs:label>
    </owl:Class>
    


    <!-- http://purl.obolibrary.org/obo/ENVO_00000234 -->

    <owl:Class rdf:about="http://purl.obolibrary.org/obo/ENVO_00000234">
        <rdfs:subClassOf rdf:resource="http://purl.obolibrary.org/obo/ENVO_00000023"/>
        <obo:IAO_0000115 xml:lang="en">A small, slow-moving stream or creek; usually located in low-lying areas.</obo:IAO_0000115>
        <rdfs:isDefinedBy rdf:resource="http://purl.obolibrary.org/obo/envo.owl"/>
        <rdfs:label xml:lang="en">bayou</rdfs:label>
        <skos:altLabel xml:lang="en">slough</skos:altLabel>
        <skos:prefLabel xml:lang="en">slough</skos:prefLabel>
    </owl:Class>
    


    <!-- http://purl.obolibrary.org/obo/ENVO_01000617 -->

    <owl:Class rdf:about="http://purl.obolibrary.org/obo/ENVO_01000617">
        <rdfs:subClassOf rdf:resource="http://purl.obolibrary.org/obo/ENVO_00000063"/>
        <obo:IAO_0000115 xml:lang="en">A lentic water body is a water body in which the accumulated water, in its totality, has very little to no directed flow.</obo:IAO_0000115>
        <rdfs:isDefinedBy rdf:resource="http://purl.obolibrary.org/obo/envo.owl"/>
        <rdfs:label xml:lang="en">lentic water body</rdfs:label>
    </owl:Class>
    


    <!-- http://purl.obolibrary.org/obo/ENVO_01000618 -->

    <owl:Class rdf:about="http://purl.obolibrary.org/obo/ENVO_01000618">
        <rdfs:subClassOf rdf:resource="http://purl.obolibrary.org/obo/ENVO_00000063"/>
        <obo:IAO_0000115 xml:lang="en">A lotic water body is a water body in which the accumulated water, in its totality, is flowing.</obo:IAO_0000115>
        <rdfs:isDefinedBy rdf:resource="http://purl.obolibrary.org/obo/envo.owl"/>
        <rdfs:label xml:lang="en">lotic water body</rdfs:label>
    </owl:Class>
    


    <!-- http://purl.obolibrary.org/obo/IAO_0000030 -->

    <owl:Class rdf:about="http://purl.obolibrary.org/obo/IAO_0000030">
        <rdfs:subClassOf rdf:resource="http://purl.obolibrary.org/obo/BFO_0000031"/>
        <obo:IAO_0000115 xml:lang="en">A generically dependent continuant that is about some thing.</obo:IAO_0000115>
        <rdfs:isDefinedBy rdf:resource="http://purl.obolibrary.org/obo/iao.owl"/>
        <rdfs:label xml:lang="en">information content entity</rdfs:label>
    </owl:Class>
    


    <!-- http://purl.obolibrary.org/obo/IAO_0000033 -->

    <owl:Class rdf:about="http://purl.obolibrary.org/obo/IAO_0000033">
        <rdfs:subClassOf rdf:resource="http://purl.obolibrary.org/obo/IAO_0000030"/>
        <obo:IAO_0000115 xml:lang="en">An information content entity whose concretizations indicate to their bearer how to realize them in a process.</obo:IAO_0000115>
        <rdfs:isDefinedBy rdf:resource="http://purl.obolibrary.org/obo/iao.owl"/>
        <rdfs:label xml:lang="en">directive information entity</rdfs:label>
    </owl:Class>
    


    <!-- http://purl.obolibrary.org/obo/IAO_0000104 -->

    <owl:Class rdf:about="http://purl.obolibrary.org/obo/IAO_0000104">
        <rdfs:subClassOf rdf:resource="http://purl.obolibrary.org/obo/IAO_0000030"/>
        <obo:IAO_0000115 xml:lang="en">A directive information entity with action specifications and objective specifications as parts, and that may be concretized as a realizable entity that, if realized, is realized in a process in which the bearer tries to achieve the objectives by taking the actions specified.</obo:IAO_0000115>
        <rdfs:isDefinedBy rdf:resource="http://purl.obolibrary.org/obo/iao.owl"/>
        <rdfs:label xml:lang="en">plan specification</rdfs:label>
    </owl:Class>
    


    <!-- http://purl.obolibrary.org/obo/IAO_0000109 -->

    <owl:Class rdf:about="http://purl.obolibrary.org/obo/IAO_0000109">
        <rdfs:subClassOf rdf:resource="http://purl.obolibrary.org/obo/IAO_0000030"/>
        <obo:IAO_0000115 xml:lang="en">A measurement datum is an information content entity that is a recording of the output of a measurement such as produced by a device.</obo:IAO_0000115>
        <rdfs:isDefinedBy rdf:resource="http://purl.obolibrary.org/obo/iao.owl"/>
        <rdfs:label xml:lang="en">measurement datum</rdfs:label>
    </owl:Class>
    


    <!-- http://purl.obolibrary.org/obo/IAO_0000310 -->

    <owl:Class rdf:about="http://purl.obolibrary.org/obo/IAO_0000310">
        <rdfs:subClassOf rdf:resource="http://purl.obolibrary.org/obo/IAO_0000030"/>
        <obo:IAO_0000115 xml:lang="en">A collection of information content entities intended to be understood together as a whole.</obo:IAO_0000115>
        <rdfs:isDefinedBy rdf:resource="http://purl.obolibrary.org/obo/iao.owl"/>
        <rdfs:label xml:lang="en">document</rdfs:label>
    </owl:Class>
    


    <!-- http://rs.tdwg.org/dwc/terms/Event -->

    <owl:Class rdf:about="http://rs.tdwg.org/dwc/terms/Event">
        <rdfs:subClassOf rdf:resource="http://purl.obolibrary.org/obo/BFO_0000015"/>
        <obo:IAO_0000115 xml:lang="en">An action that occurs at some location during some time.</obo:IAO_0000115>
        <obo:IAO_0000119 rdf:resource="https://dwc.tdwg.org/list/"/>
        <rdfs:isDefinedBy rdf:resource="http://rs.tdwg.org/dwc/terms/"/>
        <rdfs:label xml:lang="en">Event</rdfs:label>
    </owl:Class>
    


    <!-- http://rs.tdwg.org/dwc/terms/Identification -->

    <owl:Class rdf:about="http://rs.tdwg.org/dwc/terms/Identification">
        <rdfs:subClassOf rdf:resource="http://purl.obolibrary.org/obo/BFO_0000015"/>
        <obo:IAO_0000115 xml:lang="en">A taxonomic determination (e.g., the assignment to a dwc:Taxon).</obo:IAO_0000115>
        <obo:IAO_0000119 rdf:resource="https://dwc.tdwg.org/list/"/>
        <rdfs:isDefinedBy rdf:resource="http://rs.tdwg.org/dwc/terms/"/>
        <rdfs:label xml:lang="en">Identification</rdfs:label>
    </owl:Class>
    


    <!-- http://rs.tdwg.org/dwc/terms/MaterialEntity -->

    <owl:Class rdf:about="http://rs.tdwg.org/dwc/terms/MaterialEntity">
        <rdfs:subClassOf rdf:resource="http://purl.obolibrary.org/obo/BFO_0000040"/>
        <obo:IAO_0000115 xml:lang="en">An entity that can be identified, exists for some period of time, and consists in whole or in part of physical matter while it exists.</obo:IAO_0000115>
        <obo:IAO_0000119 rdf:resource="https://dwc.tdwg.org/list/"/>
        <rdfs:isDefinedBy rdf:resource="http://rs.tdwg.org/dwc/terms/"/>
        <rdfs:label xml:lang="en">Material Entity</rdfs:label>
    </owl:Class>
    


    <!-- http://rs.tdwg.org/dwc/terms/Occurrence -->

    <owl:Class rdf:about="http://rs.tdwg.org/dwc/terms/Occurrence">
        <rdfs:subClassOf rdf:resource="http://purl.obolibrary.org/obo/BFO_0000015"/>
        <obo:IAO_0000115 xml:lang="en">An existence of a dwc:Organism at a particular place at a particular time.</obo:IAO_0000115>
        <obo:IAO_0000119 rdf:resource="https://dwc.tdwg.org/list/"/>
        <rdfs:isDefinedBy rdf:resource="http://rs.tdwg.org/dwc/terms/"/>
        <rdfs:label xml:lang="en">Occurrence</rdfs:label>
    </owl:Class>
    


    <!-- http://rs.tdwg.org/dwc/terms/Organism -->

    <owl:Class rdf:about="http://rs.tdwg.org/dwc/terms/Organism">
        <rdfs:subClassOf rdf:resource="http://purl.obolibrary.org/obo/BFO_0000040"/>
        <obo:IAO_0000115 xml:lang="en">A particular organism or defined group of organisms considered to be taxonomically homogeneous.</obo:IAO_0000115>
        <obo:IAO_0000119 rdf:resource="https://dwc.tdwg.org/list/"/>
        <rdfs:isDefinedBy rdf:resource="http://rs.tdwg.org/dwc/terms/"/>
        <rdfs:label xml:lang="en">Organism</rdfs:label>
    </owl:Class>
    


    <!-- http://www.w3.org/2004/02/skos/core#Concept -->

    <owl:Class rdf:about="http://www.w3.org/2004/02/skos/core#Concept"/>
    


    <!-- http://www.w3.org/2004/02/skos/core#ConceptScheme -->

    <owl:Class rdf:about="http://www.w3.org/2004/02/skos/core#ConceptScheme"/>
    


    <!-- http://www.w3.org/ns/dqv#Dimension -->

    <owl:Class rdf:about="http://www.w3.org/ns/dqv#Dimension">
        <rdfs:subClassOf rdf:resource="http://www.w3.org/2004/02/skos/core#Concept"/>
        <obo:IAO_0000115 xml:lang="en">Represents criteria relevant for assessing quality. Each quality dimension must have one or more metric to measure it. A dimension is linked with a category using the dqv:inCategory property.</obo:IAO_0000115>
        <obo:IAO_0000119 rdf:resource="https://www.w3.org/TR/vocab-dqv/"/>
        <rdfs:isDefinedBy rdf:resource="http://www.w3.org/ns/dqv#"/>
        <rdfs:label xml:lang="en">Dimension</rdfs:label>
    </owl:Class>
    


    <!-- http://www.w3.org/ns/dqv#QualityAnnotation -->

    <owl:Class rdf:about="http://www.w3.org/ns/dqv#QualityAnnotation">
        <rdfs:subClassOf rdf:resource="http://www.w3.org/ns/oa#Annotation"/>
        <obo:IAO_0000115 xml:lang="en">Represents quality annotations, including ratings, quality certificates or feedback that can be associated to datasets or distributions. Quality annotations must have one oa:motivatedBy statement with an instance of oa:Motivation (and skos:Concept) that reflects a quality assessment purpose. We define this instance as dqv:qualityAssessment.</obo:IAO_0000115>
        <obo:IAO_0000119 rdf:resource="https://www.w3.org/TR/vocab-dqv/"/>
        <rdfs:isDefinedBy rdf:resource="http://www.w3.org/ns/dqv#"/>
        <rdfs:label xml:lang="en">Quality Annotation</rdfs:label>
    </owl:Class>
    


    <!-- http://www.w3.org/ns/oa#Annotation -->

    <owl:Class rdf:about="http://www.w3.org/ns/oa#Annotation">
        <rdfs:subClassOf rdf:resource="http://purl.obolibrary.org/obo/IAO_0000030"/>
        <obo:IAO_0000115 xml:lang="en">The class for Web Annotations.</obo:IAO_0000115>
        <obo:IAO_0000119 rdf:resource="http://www.w3.org/ns/oa#Annotation"/>
        <rdfs:isDefinedBy rdf:resource="http://www.w3.org/ns/oa#"/>
        <rdfs:label xml:lang="en">Annotation</rdfs:label>
    </owl:Class>
    


    <!-- https://w3id.org/gcdfo/salmon#AbundancePercentileMetric -->

    <owl:Class rdf:about="https://w3id.org/gcdfo/salmon#AbundancePercentileMetric">
        <rdfs:subClassOf rdf:resource="https://w3id.org/gcdfo/salmon#ObservedRateOrAbundance"/>
        <obo:IAO_0000115 xml:lang="en">An abundance percentile metric giving the percentile rank of the current generational average spawner abundance relative to a historical reference distribution.</obo:IAO_0000115>
        <obo:IAO_0000119 xml:lang="en">Fisheries and Oceans Canada. 2024. Rapid Status Approximations for Pacific Salmon Derived from Integrated Expert Assessments under DFO’s Wild Salmon Policy. CSAS Pacific Region Science Response 2024/004.</obo:IAO_0000119>
        <dcterms:source rdf:resource="https://waves-vagues.dfo-mpo.gc.ca/library-bibliotheque/41225260.pdf"/>
        <rdfs:isDefinedBy rdf:resource="https://w3id.org/gcdfo/salmon"/>
        <rdfs:label xml:lang="en">Abundance percentile metric</rdfs:label>
        <theme rdf:resource="https://w3id.org/gcdfo/salmon#DataModelProvenanceTheme"/>
        <theme rdf:resource="https://w3id.org/gcdfo/salmon#StockAssessmentTheme"/>
        <theme rdf:resource="https://w3id.org/gcdfo/salmon#WildSalmonPolicyTheme"/>
    </owl:Class>
    


    <!-- https://w3id.org/gcdfo/salmon#BenchmarkRatioMetric -->

    <owl:Class rdf:about="https://w3id.org/gcdfo/salmon#BenchmarkRatioMetric">
        <rdfs:subClassOf rdf:resource="https://w3id.org/gcdfo/salmon#ObservedRateOrAbundance"/>
        <obo:IAO_0000115 xml:lang="en">A benchmark-ratio metric equal to the ratio of current generational average spawner abundance to a specified benchmark (lower or upper benchmark), where 1.0 indicates equality to that benchmark.</obo:IAO_0000115>
        <obo:IAO_0000119 xml:lang="en">Fisheries and Oceans Canada. 2024. Rapid Status Approximations for Pacific Salmon Derived from Integrated Expert Assessments under DFO’s Wild Salmon Policy. CSAS Pacific Region Science Response 2024/004.</obo:IAO_0000119>
        <dcterms:source rdf:resource="https://waves-vagues.dfo-mpo.gc.ca/library-bibliotheque/41225260.pdf"/>
        <rdfs:isDefinedBy rdf:resource="https://w3id.org/gcdfo/salmon"/>
        <rdfs:label xml:lang="en">Benchmark ratio metric</rdfs:label>
        <theme rdf:resource="https://w3id.org/gcdfo/salmon#DataModelProvenanceTheme"/>
        <theme rdf:resource="https://w3id.org/gcdfo/salmon#StockAssessmentTheme"/>
        <theme rdf:resource="https://w3id.org/gcdfo/salmon#WildSalmonPolicyTheme"/>
    </owl:Class>
    


    <!-- https://w3id.org/gcdfo/salmon#BroodYear -->

    <owl:Class rdf:about="https://w3id.org/gcdfo/salmon#BroodYear">
        <rdfs:subClassOf rdf:resource="https://w3id.org/gcdfo/salmon#YearBasis"/>
        <obo:IAO_0000115 xml:lang="en">The parental year for a group of returning salmon, i.e. the calendar year when the majority of parents of these fish spawned.</obo:IAO_0000115>
        <obo:IAO_0000119 xml:lang="en">Fisheries and Oceans Canada. Pacific Salmon - Glossary (Pacific Region). https://www.pac.dfo-mpo.gc.ca/fm-gp/salmon-saumon/gloss-eng.html.</obo:IAO_0000119>
        <dcterms:source rdf:resource="https://www.pac.dfo-mpo.gc.ca/fm-gp/salmon-saumon/gloss-eng.html"/>
        <rdfs:isDefinedBy rdf:resource="https://w3id.org/gcdfo/salmon"/>
        <rdfs:label xml:lang="en">Brood year</rdfs:label>
        <skos:closeMatch rdf:resource="http://purl.dataone.org/odo/SALMON_00000520"/>
        <theme rdf:resource="https://w3id.org/gcdfo/salmon#StockAssessmentTheme"/>
    </owl:Class>
    


    <!-- https://w3id.org/gcdfo/salmon#CWTMarineSurvivalRate -->

    <owl:Class rdf:about="https://w3id.org/gcdfo/salmon#CWTMarineSurvivalRate">
        <rdfs:subClassOf rdf:resource="https://w3id.org/gcdfo/salmon#ObservedRateOrAbundance"/>
        <obo:IAO_0000115 xml:lang="en">A marine survival proportion estimated for a coded-wire-tag (CWT) release group, defined as the portion of tagged smolts that survive to be caught in marine fisheries or return to freshwater as adults.</obo:IAO_0000115>
        <obo:IAO_0000119 xml:lang="en">Fisheries and Oceans Canada. 2021. Marine Survival Forecast of Southern British Columbia Coho (defines marine survival as (Catch+Escapement)/Release for coded-wire-tag smolt releases).</obo:IAO_0000119>
        <dcterms:source rdf:resource="https://waves-vagues.dfo-mpo.gc.ca/Library/40978680.pdf"/>
        <rdfs:isDefinedBy rdf:resource="https://w3id.org/gcdfo/salmon"/>
        <rdfs:label xml:lang="en">CWT marine survival rate</rdfs:label>
        <skos:altLabel xml:lang="en">Coded-wire-tag marine survival rate</skos:altLabel>
        <theme rdf:resource="https://w3id.org/gcdfo/salmon#MonitoringFieldWorkTheme"/>
        <theme rdf:resource="https://w3id.org/gcdfo/salmon#StockAssessmentTheme"/>
    </owl:Class>
    


    <!-- https://w3id.org/gcdfo/salmon#CatchYear -->

    <owl:Class rdf:about="https://w3id.org/gcdfo/salmon#CatchYear">
        <rdfs:subClassOf rdf:resource="https://w3id.org/gcdfo/salmon#YearBasis"/>
        <obo:IAO_0000115 xml:lang="en">The calendar year in which returning salmon are caught in fisheries (as opposed to the brood year in which the cohort was spawned).</obo:IAO_0000115>
        <rdfs:isDefinedBy rdf:resource="https://w3id.org/gcdfo/salmon"/>
        <rdfs:label xml:lang="en">Catch year</rdfs:label>
        <theme rdf:resource="https://w3id.org/gcdfo/salmon#StockAssessmentTheme"/>
    </owl:Class>
    


    <!-- https://w3id.org/gcdfo/salmon#ConfidenceCategory -->

    <owl:Class rdf:about="https://w3id.org/gcdfo/salmon#ConfidenceCategory"/>
    


    <!-- https://w3id.org/gcdfo/salmon#ConservationUnit -->

    <owl:Class rdf:about="https://w3id.org/gcdfo/salmon#ConservationUnit">
        <rdfs:subClassOf rdf:resource="https://w3id.org/gcdfo/salmon#ReportingOrManagementStratum"/>
        <obo:IAO_0000115 xml:lang="en">A group of fish sufficiently isolated from other groups that, if extirpated, is very unlikely to recolonize naturally within an acceptable timeframe.</obo:IAO_0000115>
        <obo:IAO_0000119 xml:lang="en">Fisheries and Oceans Canada. 2005. Canada&apos;s Policy for Conservation of Wild Pacific Salmon. https://waves-vagues.dfo-mpo.gc.ca/library-bibliotheque/315577.pdf.</obo:IAO_0000119>
        <obo:IAO_0000119 xml:lang="en">Fisheries and Oceans Canada. Canada&apos;s Policy for Conservation of Wild Pacific Salmon - Glossary. https://www.pac.dfo-mpo.gc.ca/fm-gp/salmon-saumon/wsp-pss/policy-politique-eng.html#glossary.</obo:IAO_0000119>
        <dcterms:isPartOf rdf:resource="urn:ISBN:0662405382"/>
        <dcterms:source rdf:resource="https://waves-vagues.dfo-mpo.gc.ca/library-bibliotheque/315577.pdf"/>
        <dcterms:source rdf:resource="https://www.pac.dfo-mpo.gc.ca/fm-gp/salmon-saumon/wsp-pss/policy-politique-eng.html#glossary"/>
        <rdfs:isDefinedBy rdf:resource="https://w3id.org/gcdfo/salmon"/>
        <rdfs:label xml:lang="en">Conservation Unit</rdfs:label>
        <theme rdf:resource="https://w3id.org/gcdfo/salmon#PolicyGovernanceTheme"/>
        <theme rdf:resource="https://w3id.org/gcdfo/salmon#SalmonEnhancementHatcheriesTheme"/>
        <theme rdf:resource="https://w3id.org/gcdfo/salmon#WildSalmonPolicyTheme"/>
    </owl:Class>
    


    <!-- https://w3id.org/gcdfo/salmon#Deme -->

    <owl:Class rdf:about="https://w3id.org/gcdfo/salmon#Deme">
        <rdfs:subClassOf rdf:resource="http://rs.tdwg.org/dwc/terms/Organism"/>
        <obo:IAO_0000115 xml:lang="en">A local interbreeding group of organisms within a species. In salmon, a deme typically corresponds to a spawning population at a specific site. Demes are the finest biological unit and make up populations.</obo:IAO_0000115>
        <rdfs:isDefinedBy rdf:resource="https://w3id.org/gcdfo/salmon"/>
        <rdfs:label xml:lang="en">Deme</rdfs:label>
        <theme rdf:resource="https://w3id.org/gcdfo/salmon#GeneticsStockCompositionTheme"/>
        <theme rdf:resource="https://w3id.org/gcdfo/salmon#StockAssessmentTheme"/>
        <theme rdf:resource="https://w3id.org/gcdfo/salmon#WildSalmonPolicyTheme"/>
    </owl:Class>
    


    <!-- https://w3id.org/gcdfo/salmon#Escapement -->

    <owl:Class rdf:about="https://w3id.org/gcdfo/salmon#Escapement">
        <rdfs:subClassOf rdf:resource="http://purl.obolibrary.org/obo/BFO_0000015"/>
        <obo:IAO_0000115 xml:lang="en">The number of mature salmon that pass through (or escape) fisheries and return to fresh water to spawn.</obo:IAO_0000115>
        <obo:IAO_0000119 xml:lang="en">Fisheries and Oceans Canada. 2005. Canada&apos;s Policy for Conservation of Wild Pacific Salmon. https://waves-vagues.dfo-mpo.gc.ca/library-bibliotheque/315577.pdf.</obo:IAO_0000119>
        <dcterms:source rdf:resource="https://waves-vagues.dfo-mpo.gc.ca/library-bibliotheque/315577.pdf"/>
        <rdfs:isDefinedBy rdf:resource="https://w3id.org/gcdfo/salmon"/>
        <rdfs:label xml:lang="en">Escapement</rdfs:label>
        <skos:closeMatch rdf:resource="http://purl.dataone.org/odo/SALMON_00000479"/>
        <theme rdf:resource="https://w3id.org/gcdfo/salmon#MonitoringFieldWorkTheme"/>
        <theme rdf:resource="https://w3id.org/gcdfo/salmon#StockAssessmentTheme"/>
    </owl:Class>
    


    <!-- https://w3id.org/gcdfo/salmon#EscapementMeasurement -->

    <owl:Class rdf:about="https://w3id.org/gcdfo/salmon#EscapementMeasurement">
        <rdfs:subClassOf rdf:resource="http://purl.obolibrary.org/obo/IAO_0000109"/>
        <obo:IAO_0000115 xml:lang="en">A measurement or estimate of escapement tied to a stock and a survey event.</obo:IAO_0000115>
        <rdfs:isDefinedBy rdf:resource="https://w3id.org/gcdfo/salmon"/>
        <rdfs:label xml:lang="en">Escapement measurement</rdfs:label>
        <theme rdf:resource="https://w3id.org/gcdfo/salmon#MonitoringFieldWorkTheme"/>
        <theme rdf:resource="https://w3id.org/gcdfo/salmon#StockAssessmentTheme"/>
    </owl:Class>
    


    <!-- https://w3id.org/gcdfo/salmon#EscapementSurveyEvent -->

    <owl:Class rdf:about="https://w3id.org/gcdfo/salmon#EscapementSurveyEvent">
        <rdfs:subClassOf rdf:resource="https://w3id.org/gcdfo/salmon#SurveyEvent"/>
        <obo:IAO_0000115 xml:lang="en">A survey event specifically for estimating escapement.</obo:IAO_0000115>
        <rdfs:isDefinedBy rdf:resource="https://w3id.org/gcdfo/salmon"/>
        <rdfs:label xml:lang="en">Escapement Survey Event</rdfs:label>
        <skos:prefLabel xml:lang="en">Escapement Survey Event</skos:prefLabel>
        <theme rdf:resource="https://w3id.org/gcdfo/salmon#MonitoringFieldWorkTheme"/>
        <theme rdf:resource="https://w3id.org/gcdfo/salmon#StockAssessmentTheme"/>
    </owl:Class>
    


    <!-- https://w3id.org/gcdfo/salmon#ExploitationRate -->

    <owl:Class rdf:about="https://w3id.org/gcdfo/salmon#ExploitationRate">
        <rdfs:subClassOf rdf:resource="http://purl.obolibrary.org/obo/IAO_0000109"/>
        <obo:IAO_0000115 xml:lang="en">A fishing mortality rate expressed as the proportion of the total return removed by fishing over a specified assessment period.</obo:IAO_0000115>
        <obo:IAO_0000119 xml:lang="en">Fisheries and Oceans Canada. Pacific Salmon - Glossary (Pacific Region). https://www.pac.dfo-mpo.gc.ca/fm-gp/salmon-saumon/gloss-eng.html.</obo:IAO_0000119>
        <dcterms:source rdf:resource="https://www.pac.dfo-mpo.gc.ca/fm-gp/salmon-saumon/gloss-eng.html"/>
        <rdfs:isDefinedBy rdf:resource="https://w3id.org/gcdfo/salmon"/>
        <rdfs:label xml:lang="en">Exploitation rate</rdfs:label>
        <theme rdf:resource="https://w3id.org/gcdfo/salmon#FisheriesManagementTheme"/>
        <theme rdf:resource="https://w3id.org/gcdfo/salmon#StockAssessmentTheme"/>
    </owl:Class>
    


    <!-- https://w3id.org/gcdfo/salmon#FisheriesReferencePointLower -->

    <owl:Class rdf:about="https://w3id.org/gcdfo/salmon#FisheriesReferencePointLower">
        <rdfs:subClassOf rdf:resource="https://w3id.org/gcdfo/salmon#LimitReferencePoint"/>
        <obo:IAO_0000115 xml:lang="en">A lower fisheries-management reference point defined for Stock Management Units (SMUs) and related fishery decision frameworks. It may be informed by Conservation Unit (CU) lower biological benchmarks, but is not identical to CU-level lower biological benchmarks used to delineate Wild Salmon Policy biological status zones.</obo:IAO_0000115>
        <obo:IAO_0000119 xml:lang="en">Fisheries and Oceans Canada. (2022). Methodologies and Guidelines for Defining Limit Reference Points for Pacific Salmon. DFO Can. Sci. Advis. Sec. Sci. Advis. Rep. 2022/030. (Erratum: December 2022).</obo:IAO_0000119>
        <rdfs:isDefinedBy rdf:resource="https://w3id.org/gcdfo/salmon"/>
        <rdfs:label xml:lang="en">Fisheries Reference Point - Lower</rdfs:label>
        <skos:altLabel xml:lang="en">FRP-L</skos:altLabel>
        <theme rdf:resource="https://w3id.org/gcdfo/salmon#FisheriesManagementTheme"/>
        <theme rdf:resource="https://w3id.org/gcdfo/salmon#PolicyGovernanceTheme"/>
        <theme rdf:resource="https://w3id.org/gcdfo/salmon#StockAssessmentTheme"/>
    </owl:Class>
    


    <!-- https://w3id.org/gcdfo/salmon#GenerationalAverageAbundance -->

    <owl:Class rdf:about="https://w3id.org/gcdfo/salmon#GenerationalAverageAbundance">
        <rdfs:subClassOf rdf:resource="https://w3id.org/gcdfo/salmon#ObservedRateOrAbundance"/>
        <obo:IAO_0000115 xml:lang="en">The generational average of spawner abundance, calculated as a geometric mean across the number of years corresponding to the most common age at return (generation length), optionally after smoothing depending on CU group.</obo:IAO_0000115>
        <obo:IAO_0000119 xml:lang="en">Fisheries and Oceans Canada. 2024. Rapid Status Approximations for Pacific Salmon Derived from Integrated Expert Assessments under DFO’s Wild Salmon Policy. CSAS Pacific Region Science Response 2024/004.</obo:IAO_0000119>
        <dcterms:source rdf:resource="https://waves-vagues.dfo-mpo.gc.ca/library-bibliotheque/41225260.pdf"/>
        <rdfs:isDefinedBy rdf:resource="https://w3id.org/gcdfo/salmon"/>
        <rdfs:label xml:lang="en">Generational average abundance</rdfs:label>
        <theme rdf:resource="https://w3id.org/gcdfo/salmon#DataModelProvenanceTheme"/>
        <theme rdf:resource="https://w3id.org/gcdfo/salmon#StockAssessmentTheme"/>
        <theme rdf:resource="https://w3id.org/gcdfo/salmon#WildSalmonPolicyTheme"/>
    </owl:Class>
    


    <!-- https://w3id.org/gcdfo/salmon#InRiverMortalityRate -->

    <owl:Class rdf:about="https://w3id.org/gcdfo/salmon#InRiverMortalityRate">
        <rdfs:subClassOf rdf:resource="https://w3id.org/gcdfo/salmon#ObservedRateOrAbundance"/>
        <obo:IAO_0000115 xml:lang="en">The proportion of fish in a defined population/cohort that die during freshwater migration in-river on the way to spawning areas during a specified assessment interval, excluding landed catch (fishery removals) where those are accounted separately.</obo:IAO_0000115>
        <obo:IAO_0000119 xml:lang="en">Fisheries and Oceans Canada. 2025. Stock-Specific Fraser River Sockeye Salmon Run Size Determination. CSAS Pacific Region Science Advisory Report 2025/021 (en route mortality excluding landed catch). COSEWIC. 2017. Sockeye Salmon (Oncorhynchus nerka) assessment and status report (en-route loss is fish that perished in the river en-route to spawning grounds for reasons other than fishing).</obo:IAO_0000119>
        <dcterms:source rdf:resource="https://waves-vagues.dfo-mpo.gc.ca/library-bibliotheque/41294622.pdf"/>
        <dcterms:source rdf:resource="https://www.canada.ca/en/environment-climate-change/services/species-risk-public-registry/cosewic-assessments-status-reports/sockeye-salmon-2017.html"/>
        <rdfs:isDefinedBy rdf:resource="https://w3id.org/gcdfo/salmon"/>
        <rdfs:label xml:lang="en">In-river mortality rate</rdfs:label>
        <theme rdf:resource="https://w3id.org/gcdfo/salmon#StockAssessmentTheme"/>
    </owl:Class>
    


    <!-- https://w3id.org/gcdfo/salmon#IndicatorRiver -->

    <owl:Class rdf:about="https://w3id.org/gcdfo/salmon#IndicatorRiver">
        <rdfs:subClassOf rdf:resource="https://w3id.org/gcdfo/salmon#ReportingOrManagementStratum"/>
        <obo:IAO_0000115 xml:lang="en">A reporting and assessment stratum identifying monitored indicator streams that provide representative indices of spawner abundance for nearby streams.</obo:IAO_0000115>
        <dcterms:source rdf:resource="https://www.salmonexplorer.ca/methods/glossary.html"/>
        <rdfs:isDefinedBy rdf:resource="https://w3id.org/gcdfo/salmon"/>
        <rdfs:label xml:lang="en">Indicator river</rdfs:label>
        <skos:altLabel xml:lang="en">Indicator stream</skos:altLabel>
        <theme rdf:resource="https://w3id.org/gcdfo/salmon#MonitoringFieldWorkTheme"/>
        <theme rdf:resource="https://w3id.org/gcdfo/salmon#PolicyGovernanceTheme"/>
        <theme rdf:resource="https://w3id.org/gcdfo/salmon#StockAssessmentTheme"/>
    </owl:Class>
    


    <!-- https://w3id.org/gcdfo/salmon#LimitReferencePoint -->

    <owl:Class rdf:about="https://w3id.org/gcdfo/salmon#LimitReferencePoint">
        <rdfs:subClassOf rdf:resource="https://w3id.org/gcdfo/salmon#ReferencePoint"/>
        <obo:IAO_0000115 xml:lang="en">A fish stock experiencing serious harm may be depleted to the point where it has impaired productivity or reproductive capacity. As a result, the stock would be less resilient to fishing and could not easily rebuild. Serious harm may be irreversible, or only slowly reversible over the long-term, and can be due to fishing, other human-induced impacts, or natural causes. Under the Precautionary Approach policy and the Fish Stocks Provisions (FSPs), breaching the LRP is a trigger for a rebuilding plan.</obo:IAO_0000115>
        <obo:IAO_0000119 xml:lang="en">Fisheries and Oceans Canada. Introduction to Stock Assessment - Glossary. https://www.dfo-mpo.gc.ca/science/species-especes/fisheries-halieutiques/assessment-evaluation/glossary-glossaire/index-eng.html.</obo:IAO_0000119>
        <dcterms:source rdf:resource="https://www.dfo-mpo.gc.ca/science/species-especes/fisheries-halieutiques/assessment-evaluation/glossary-glossaire/index-eng.html"/>
        <rdfs:isDefinedBy rdf:resource="https://w3id.org/gcdfo/salmon"/>
        <rdfs:label xml:lang="en">Limit reference point</rdfs:label>
        <skos:altLabel xml:lang="en">LRP</skos:altLabel>
        <theme rdf:resource="https://w3id.org/gcdfo/salmon#FisheriesManagementTheme"/>
        <theme rdf:resource="https://w3id.org/gcdfo/salmon#PolicyGovernanceTheme"/>
        <theme rdf:resource="https://w3id.org/gcdfo/salmon#StockAssessmentTheme"/>
    </owl:Class>
    


    <!-- https://w3id.org/gcdfo/salmon#LongTermTrendMetric -->

    <owl:Class rdf:about="https://w3id.org/gcdfo/salmon#LongTermTrendMetric">
        <rdfs:subClassOf rdf:resource="https://w3id.org/gcdfo/salmon#ObservedRateOrAbundance"/>
        <obo:IAO_0000115 xml:lang="en">A long-term trend metric comparing the current generational average (geometric mean) spawner abundance to the long-term average (geometric mean) spawner abundance for an assessed time series.</obo:IAO_0000115>
        <obo:IAO_0000119 xml:lang="en">Fisheries and Oceans Canada. 2024. Rapid Status Approximations for Pacific Salmon Derived from Integrated Expert Assessments under DFO’s Wild Salmon Policy. CSAS Pacific Region Science Response 2024/004.</obo:IAO_0000119>
        <dcterms:source rdf:resource="https://waves-vagues.dfo-mpo.gc.ca/library-bibliotheque/41225260.pdf"/>
        <rdfs:isDefinedBy rdf:resource="https://w3id.org/gcdfo/salmon"/>
        <rdfs:label xml:lang="en">Long-term trend metric</rdfs:label>
        <theme rdf:resource="https://w3id.org/gcdfo/salmon#DataModelProvenanceTheme"/>
        <theme rdf:resource="https://w3id.org/gcdfo/salmon#StockAssessmentTheme"/>
        <theme rdf:resource="https://w3id.org/gcdfo/salmon#WildSalmonPolicyTheme"/>
    </owl:Class>
    


    <!-- https://w3id.org/gcdfo/salmon#LowerBiologicalBenchmark -->

    <owl:Class rdf:about="https://w3id.org/gcdfo/salmon#LowerBiologicalBenchmark">
        <rdfs:subClassOf rdf:resource="https://w3id.org/gcdfo/salmon#MetricBenchmark"/>
        <obo:IAO_0000115 xml:lang="en">Lower benchmark value for a Conservation Unit (CU) metric used to delineate Wild Salmon Policy status zones (typically the boundary between Red and Amber zones). This CU-level biological benchmark is distinct from SMU-level fisheries management lower reference points such as FRP-L.</obo:IAO_0000115>
        <obo:IAO_0000119 xml:lang="en">Fisheries and Oceans Canada. (2021). Wild Salmon Policy 2018-2022 Implementation Plan. Available at https://waves-vagues.dfo-mpo.gc.ca/library-bibliotheque/40728109.pdf.</obo:IAO_0000119>
        <dcterms:source rdf:resource="https://waves-vagues.dfo-mpo.gc.ca/library-bibliotheque/40728109.pdf"/>
        <rdfs:isDefinedBy rdf:resource="https://w3id.org/gcdfo/salmon"/>
        <rdfs:label xml:lang="en">Lower biological benchmark</rdfs:label>
        <theme rdf:resource="https://w3id.org/gcdfo/salmon#PolicyGovernanceTheme"/>
        <theme rdf:resource="https://w3id.org/gcdfo/salmon#StockAssessmentTheme"/>
        <theme rdf:resource="https://w3id.org/gcdfo/salmon#WildSalmonPolicyTheme"/>
    </owl:Class>
    


    <!-- https://w3id.org/gcdfo/salmon#MainstemMortalityRate -->

    <owl:Class rdf:about="https://w3id.org/gcdfo/salmon#MainstemMortalityRate">
        <rdfs:subClassOf rdf:resource="https://w3id.org/gcdfo/salmon#ObservedRateOrAbundance"/>
        <obo:IAO_0000115 xml:lang="en">The proportion of fish that die while migrating through the freshwater mainstem portion of a river system (as operationally delimited by the assessment workflow), over a specified interval or between specified mainstem reference points.</obo:IAO_0000115>
        <obo:IAO_0000119 xml:lang="en">LGL Limited. Migration and Survival of Late-run Fraser Sockeye (radio-telemetry methods; fish detected at Mission are classified as survivors, fishery-related mortalities, or in-river mortalities; fixed-station tracking is conducted at strategic locations including mainstem confluences).</obo:IAO_0000119>
        <dcterms:source rdf:resource="https://waves-vagues.dfo-mpo.gc.ca/library-bibliotheque/341440.pdf"/>
        <rdfs:isDefinedBy rdf:resource="https://w3id.org/gcdfo/salmon"/>
        <rdfs:label xml:lang="en">Mainstem mortality rate</rdfs:label>
        <theme rdf:resource="https://w3id.org/gcdfo/salmon#StockAssessmentTheme"/>
    </owl:Class>
    


    <!-- https://w3id.org/gcdfo/salmon#MarineSurvivalIndex -->

    <owl:Class rdf:about="https://w3id.org/gcdfo/salmon#MarineSurvivalIndex">
        <rdfs:subClassOf rdf:resource="https://w3id.org/gcdfo/salmon#ObservedRateOrAbundance"/>
        <obo:IAO_0000115 xml:lang="en">A dimensionless index or covariate representing marine survival conditions or relative marine survival outcomes (not necessarily a survival proportion).</obo:IAO_0000115>
        <obo:IAO_0000119 xml:lang="en">Fisheries and Oceans Canada. 2021. Marine Survival Forecast of Southern British Columbia Coho (uses climate indicators correlated with marine survival; supports index-like predictors for survival conditions).</obo:IAO_0000119>
        <dcterms:source rdf:resource="https://waves-vagues.dfo-mpo.gc.ca/Library/40978680.pdf"/>
        <rdfs:isDefinedBy rdf:resource="https://w3id.org/gcdfo/salmon"/>
        <rdfs:label xml:lang="en">Marine survival index</rdfs:label>
        <theme rdf:resource="https://w3id.org/gcdfo/salmon#HabitatEcosystemClimateTheme"/>
        <theme rdf:resource="https://w3id.org/gcdfo/salmon#StockAssessmentTheme"/>
    </owl:Class>
    


    <!-- https://w3id.org/gcdfo/salmon#MetricBenchmark -->

    <owl:Class rdf:about="https://w3id.org/gcdfo/salmon#MetricBenchmark">
        <rdfs:subClassOf rdf:resource="http://purl.obolibrary.org/obo/IAO_0000030"/>
        <obo:IAO_0000115 xml:lang="en">Benchmark value for a metric that helps delineate status zones (for example, the limit reference point for absolute abundance).</obo:IAO_0000115>
        <obo:IAO_0000119 xml:lang="en">Pestal, G., MacDonald, B.L., Grant, S.C.H., and Holt, C.A. 2023. State of the salmon: rapid status assessment approach for Pacific salmon under Canada&apos;s Wild Salmon Policy. Canadian Technical Report of Fisheries and Aquatic Sciences 3570.</obo:IAO_0000119>
        <dcterms:source rdf:resource="https://publications.gc.ca/site/eng/9.928944/publication.html"/>
        <rdfs:isDefinedBy rdf:resource="https://w3id.org/gcdfo/salmon"/>
        <rdfs:label xml:lang="en">Metric benchmark</rdfs:label>
        <theme rdf:resource="https://w3id.org/gcdfo/salmon#StockAssessmentTheme"/>
        <theme rdf:resource="https://w3id.org/gcdfo/salmon#WildSalmonPolicyTheme"/>
    </owl:Class>
    


    <!-- https://w3id.org/gcdfo/salmon#ObservedExploitationRate -->

    <owl:Class rdf:about="https://w3id.org/gcdfo/salmon#ObservedExploitationRate">
        <rdfs:subClassOf rdf:resource="https://w3id.org/gcdfo/salmon#ExploitationRate"/>
        <rdfs:subClassOf rdf:resource="https://w3id.org/gcdfo/salmon#ObservedRateOrAbundance"/>
        <obo:IAO_0000115 xml:lang="en">An empirically estimated exploitation rate derived from observed or reconstructed catches/removals and returns/escapement for a specified stock and period.</obo:IAO_0000115>
        <obo:IAO_0000119 xml:lang="en">Fisheries and Oceans Canada. Pacific Salmon - Glossary (Pacific Region). https://www.pac.dfo-mpo.gc.ca/fm-gp/salmon-saumon/gloss-eng.html.</obo:IAO_0000119>
        <dcterms:source rdf:resource="https://www.pac.dfo-mpo.gc.ca/fm-gp/salmon-saumon/gloss-eng.html"/>
        <rdfs:isDefinedBy rdf:resource="https://w3id.org/gcdfo/salmon"/>
        <rdfs:label xml:lang="en">Observed exploitation rate</rdfs:label>
        <theme rdf:resource="https://w3id.org/gcdfo/salmon#DataModelProvenanceTheme"/>
        <theme rdf:resource="https://w3id.org/gcdfo/salmon#FisheriesManagementTheme"/>
        <theme rdf:resource="https://w3id.org/gcdfo/salmon#StockAssessmentTheme"/>
    </owl:Class>
    


    <!-- https://w3id.org/gcdfo/salmon#ObservedRateOrAbundance -->

    <owl:Class rdf:about="https://w3id.org/gcdfo/salmon#ObservedRateOrAbundance">
        <rdfs:subClassOf rdf:resource="http://purl.obolibrary.org/obo/IAO_0000109"/>
        <obo:IAO_0000115 xml:lang="en">A measurement datum representing an empirically observed rate, count, or abundance derived from monitoring or survey data.</obo:IAO_0000115>
        <rdfs:isDefinedBy rdf:resource="https://w3id.org/gcdfo/salmon"/>
        <rdfs:label xml:lang="en">Observed rate or abundance</rdfs:label>
        <theme rdf:resource="https://w3id.org/gcdfo/salmon#DataModelProvenanceTheme"/>
        <theme rdf:resource="https://w3id.org/gcdfo/salmon#StockAssessmentTheme"/>
    </owl:Class>
    


    <!-- https://w3id.org/gcdfo/salmon#OceanMortalityRate -->

    <owl:Class rdf:about="https://w3id.org/gcdfo/salmon#OceanMortalityRate">
        <rdfs:subClassOf rdf:resource="https://w3id.org/gcdfo/salmon#ObservedRateOrAbundance"/>
        <obo:IAO_0000115 xml:lang="en">The proportion of fish that die during the ocean (marine) life-history phase for a defined population/cohort and interval; when a marine survival proportion is available, ocean mortality may be represented as its complement under the assessment’s accounting conventions.</obo:IAO_0000115>
        <obo:IAO_0000119 xml:lang="en">COSEWIC. 2017. Sockeye Salmon (Oncorhynchus nerka) assessment and status report (marine survival index described and interpreted in a Pacific salmon assessment context).</obo:IAO_0000119>
        <dcterms:source rdf:resource="https://www.canada.ca/en/environment-climate-change/services/species-risk-public-registry/cosewic-assessments-status-reports/sockeye-salmon-2017.html"/>
        <rdfs:isDefinedBy rdf:resource="https://w3id.org/gcdfo/salmon"/>
        <rdfs:label xml:lang="en">Ocean mortality rate</rdfs:label>
        <theme rdf:resource="https://w3id.org/gcdfo/salmon#StockAssessmentTheme"/>
    </owl:Class>
    


    <!-- https://w3id.org/gcdfo/salmon#PercentChangeMetric -->

    <owl:Class rdf:about="https://w3id.org/gcdfo/salmon#PercentChangeMetric">
        <rdfs:subClassOf rdf:resource="https://w3id.org/gcdfo/salmon#ObservedRateOrAbundance"/>
        <obo:IAO_0000115 xml:lang="en">A short-term trend metric quantifying the percent (linear) change in spawner abundance over the most recent three generations.</obo:IAO_0000115>
        <obo:IAO_0000119 xml:lang="en">Fisheries and Oceans Canada. 2024. Rapid Status Approximations for Pacific Salmon Derived from Integrated Expert Assessments under DFO’s Wild Salmon Policy. CSAS Pacific Region Science Response 2024/004.</obo:IAO_0000119>
        <dcterms:source rdf:resource="https://waves-vagues.dfo-mpo.gc.ca/library-bibliotheque/41225260.pdf"/>
        <rdfs:isDefinedBy rdf:resource="https://w3id.org/gcdfo/salmon"/>
        <rdfs:label xml:lang="en">Percent change metric</rdfs:label>
        <skos:altLabel xml:lang="en">Rapid-status percent change metric</skos:altLabel>
        <theme rdf:resource="https://w3id.org/gcdfo/salmon#DataModelProvenanceTheme"/>
        <theme rdf:resource="https://w3id.org/gcdfo/salmon#StockAssessmentTheme"/>
        <theme rdf:resource="https://w3id.org/gcdfo/salmon#WildSalmonPolicyTheme"/>
    </owl:Class>
    


    <!-- https://w3id.org/gcdfo/salmon#Population -->

    <owl:Class rdf:about="https://w3id.org/gcdfo/salmon#Population">
        <rdfs:subClassOf rdf:resource="http://rs.tdwg.org/dwc/terms/Organism"/>
        <obo:IAO_0000115 xml:lang="en">A group of organisms of the same species occupying a defined area that interbreed and share a gene pool. In salmon, populations are composed of one or more demes and form the biological basis for Conservation Units.</obo:IAO_0000115>
        <rdfs:isDefinedBy rdf:resource="https://w3id.org/gcdfo/salmon"/>
        <rdfs:label xml:lang="en">Population</rdfs:label>
        <theme rdf:resource="https://w3id.org/gcdfo/salmon#GeneticsStockCompositionTheme"/>
        <theme rdf:resource="https://w3id.org/gcdfo/salmon#StockAssessmentTheme"/>
        <theme rdf:resource="https://w3id.org/gcdfo/salmon#WildSalmonPolicyTheme"/>
    </owl:Class>
    


    <!-- https://w3id.org/gcdfo/salmon#ProbabilityDeclineBelowLowerBenchmarkMetric -->

    <owl:Class rdf:about="https://w3id.org/gcdfo/salmon#ProbabilityDeclineBelowLowerBenchmarkMetric">
        <rdfs:subClassOf rdf:resource="https://w3id.org/gcdfo/salmon#ObservedRateOrAbundance"/>
        <obo:IAO_0000115 xml:lang="en">A probability metric estimating the risk that spawner abundance will be below the lower benchmark, given uncertainty in benchmark estimates and/or abundance estimates, for a defined forecast or assessment horizon.</obo:IAO_0000115>
        <obo:IAO_0000119 xml:lang="en">Fisheries and Oceans Canada. 2024. Rapid Status Approximations for Pacific Salmon Derived from Integrated Expert Assessments under DFO’s Wild Salmon Policy. CSAS Pacific Region Science Response 2024/004.</obo:IAO_0000119>
        <dcterms:source rdf:resource="https://waves-vagues.dfo-mpo.gc.ca/library-bibliotheque/41225260.pdf"/>
        <rdfs:isDefinedBy rdf:resource="https://w3id.org/gcdfo/salmon"/>
        <rdfs:label xml:lang="en">Probability of decline below lower benchmark metric</rdfs:label>
        <theme rdf:resource="https://w3id.org/gcdfo/salmon#DataModelProvenanceTheme"/>
        <theme rdf:resource="https://w3id.org/gcdfo/salmon#StockAssessmentTheme"/>
        <theme rdf:resource="https://w3id.org/gcdfo/salmon#WildSalmonPolicyTheme"/>
    </owl:Class>
    


    <!-- https://w3id.org/gcdfo/salmon#ProportionHatcheryOriginSpawners -->

    <owl:Class rdf:about="https://w3id.org/gcdfo/salmon#ProportionHatcheryOriginSpawners">
        <rdfs:subClassOf rdf:resource="https://w3id.org/gcdfo/salmon#ObservedRateOrAbundance"/>
        <obo:IAO_0000115 xml:lang="en">The proportion of spawners in a population-year that are hatchery-origin (hatchery-origin spawners divided by total spawners).</obo:IAO_0000115>
        <obo:IAO_0000119 xml:lang="en">Derived for SPSR term coverage (Issue #33 term request scope); ‘hatchery-origin’ is defined in the Salmon Origin scheme and operational marking is described in the DFO Coded Wire Tag Program page.</obo:IAO_0000119>
        <dcterms:source rdf:resource="https://www.pac.dfo-mpo.gc.ca/pacific-smon-pacifique/science/research-recherche/cwt-mmc-eng.html"/>
        <rdfs:isDefinedBy rdf:resource="https://w3id.org/gcdfo/salmon"/>
        <rdfs:label xml:lang="en">Proportion of hatchery-origin spawners</rdfs:label>
        <skos:altLabel xml:lang="en">pHOS</skos:altLabel>
        <theme rdf:resource="https://w3id.org/gcdfo/salmon#SalmonEnhancementHatcheriesTheme"/>
        <theme rdf:resource="https://w3id.org/gcdfo/salmon#StockAssessmentTheme"/>
    </owl:Class>
    


    <!-- https://w3id.org/gcdfo/salmon#RapidStatusScoreMetric -->

    <owl:Class rdf:about="https://w3id.org/gcdfo/salmon#RapidStatusScoreMetric">
        <rdfs:subClassOf rdf:resource="https://w3id.org/gcdfo/salmon#ObservedRateOrAbundance"/>
        <obo:IAO_0000115 xml:lang="en">A numeric score produced by a rapid-status algorithm used to represent an ordered status outcome and/or decision-rule position.</obo:IAO_0000115>
        <obo:IAO_0000119 xml:lang="en">Fisheries and Oceans Canada. 2024. Rapid Status Approximations for Pacific Salmon Derived from Integrated Expert Assessments under DFO’s Wild Salmon Policy. CSAS Pacific Region Science Response 2024/004.</obo:IAO_0000119>
        <dcterms:source rdf:resource="https://waves-vagues.dfo-mpo.gc.ca/library-bibliotheque/41225260.pdf"/>
        <rdfs:isDefinedBy rdf:resource="https://w3id.org/gcdfo/salmon"/>
        <rdfs:label xml:lang="en">Rapid status score metric</rdfs:label>
        <theme rdf:resource="https://w3id.org/gcdfo/salmon#DataModelProvenanceTheme"/>
        <theme rdf:resource="https://w3id.org/gcdfo/salmon#StockAssessmentTheme"/>
        <theme rdf:resource="https://w3id.org/gcdfo/salmon#WildSalmonPolicyTheme"/>
    </owl:Class>
    


    <!-- https://w3id.org/gcdfo/salmon#ReferencePoint -->

    <owl:Class rdf:about="https://w3id.org/gcdfo/salmon#ReferencePoint">
        <rdfs:subClassOf rdf:resource="http://purl.obolibrary.org/obo/IAO_0000030"/>
        <obo:IAO_0000115 xml:lang="en">Reference points are used as targets to achieve or as limits to avoid.</obo:IAO_0000115>
        <obo:IAO_0000119 xml:lang="en">Fisheries and Oceans Canada. Introduction to Stock Assessment - Glossary. https://www.dfo-mpo.gc.ca/science/species-especes/fisheries-halieutiques/assessment-evaluation/glossary-glossaire/index-eng.html.</obo:IAO_0000119>
        <dcterms:source rdf:resource="https://www.dfo-mpo.gc.ca/science/species-especes/fisheries-halieutiques/assessment-evaluation/glossary-glossaire/index-eng.html"/>
        <rdfs:isDefinedBy rdf:resource="https://w3id.org/gcdfo/salmon"/>
        <rdfs:label xml:lang="en">Reference point</rdfs:label>
        <theme rdf:resource="https://w3id.org/gcdfo/salmon#FisheriesManagementTheme"/>
        <theme rdf:resource="https://w3id.org/gcdfo/salmon#PolicyGovernanceTheme"/>
        <theme rdf:resource="https://w3id.org/gcdfo/salmon#StockAssessmentTheme"/>
    </owl:Class>
    


    <!-- https://w3id.org/gcdfo/salmon#RelativeHatcherySpawnerAbundance -->

    <owl:Class rdf:about="https://w3id.org/gcdfo/salmon#RelativeHatcherySpawnerAbundance">
        <rdfs:subClassOf rdf:resource="https://w3id.org/gcdfo/salmon#RelativeSpawnerAbundance"/>
        <obo:IAO_0000115 xml:lang="en">Hatchery-origin spawner abundance expressed as a relative (dimensionless) abundance metric to a defined reference (commonly benchmarks), for within-series comparison; in rapid-status workflows, relative abundance is computed using the current generational average (geometric mean) divided by CU-specific lower and/or upper benchmarks.</obo:IAO_0000115>
        <obo:IAO_0000119 xml:lang="en">Fisheries and Oceans Canada. 2024. Rapid Status Approximations for Pacific Salmon… CSAS Pacific Region Science Response 2024/004 (relative abundance metric definition and computation). Holt et al. 2009. Indicators of Status and Benchmarks… CSAS Res. Doc. 2009/058 (discusses hatchery/wild considerations for status assessments).</obo:IAO_0000119>
        <dcterms:source rdf:resource="https://waves-vagues.dfo-mpo.gc.ca/library-bibliotheque/339096.pdf"/>
        <dcterms:source rdf:resource="https://waves-vagues.dfo-mpo.gc.ca/library-bibliotheque/41225260.pdf"/>
        <rdfs:isDefinedBy rdf:resource="https://w3id.org/gcdfo/salmon"/>
        <rdfs:label xml:lang="en">Relative hatchery spawner abundance</rdfs:label>
        <theme rdf:resource="https://w3id.org/gcdfo/salmon#SalmonEnhancementHatcheriesTheme"/>
        <theme rdf:resource="https://w3id.org/gcdfo/salmon#StockAssessmentTheme"/>
    </owl:Class>
    


    <!-- https://w3id.org/gcdfo/salmon#RelativeHatcherySpawnerAbundanceChange -->

    <owl:Class rdf:about="https://w3id.org/gcdfo/salmon#RelativeHatcherySpawnerAbundanceChange">
        <rdfs:subClassOf rdf:resource="https://w3id.org/gcdfo/salmon#RelativeSpawnerAbundanceChange"/>
        <obo:IAO_0000115 xml:lang="en">A change metric (delta or percent change, as defined by the workflow) computed from relative hatchery-origin spawner abundance values over time; in rapid-status workflows, percent change is derived from log-transformed series and quantified over the most recent three generations.</obo:IAO_0000115>
        <obo:IAO_0000119 xml:lang="en">Fisheries and Oceans Canada. 2024. Rapid Status Approximations for Pacific Salmon… CSAS Pacific Region Science Response 2024/004 (definition and computation notes for percent change as a short-term trend over three generations).</obo:IAO_0000119>
        <dcterms:source rdf:resource="https://waves-vagues.dfo-mpo.gc.ca/library-bibliotheque/41225260.pdf"/>
        <rdfs:isDefinedBy rdf:resource="https://w3id.org/gcdfo/salmon"/>
        <rdfs:label xml:lang="en">Relative hatchery spawner abundance change</rdfs:label>
        <theme rdf:resource="https://w3id.org/gcdfo/salmon#SalmonEnhancementHatcheriesTheme"/>
        <theme rdf:resource="https://w3id.org/gcdfo/salmon#StockAssessmentTheme"/>
    </owl:Class>
    


    <!-- https://w3id.org/gcdfo/salmon#RelativeHatcherySpawnerAbundancePercentile -->

    <owl:Class rdf:about="https://w3id.org/gcdfo/salmon#RelativeHatcherySpawnerAbundancePercentile">
        <rdfs:subClassOf rdf:resource="https://w3id.org/gcdfo/salmon#RelativeSpawnerAbundancePercentile"/>
        <obo:IAO_0000115 xml:lang="en">The percentile rank of relative hatchery-origin spawner abundance against a defined historical reference distribution.</obo:IAO_0000115>
        <obo:IAO_0000119 xml:lang="en">Fisheries and Oceans Canada. 2024. Rapid Status Approximations… CSAS Science Response 2024/004 (percentile benchmarks discussion).</obo:IAO_0000119>
        <dcterms:source rdf:resource="https://waves-vagues.dfo-mpo.gc.ca/library-bibliotheque/41225260.pdf"/>
        <rdfs:isDefinedBy rdf:resource="https://w3id.org/gcdfo/salmon"/>
        <rdfs:label xml:lang="en">Relative hatchery spawner abundance percentile</rdfs:label>
        <theme rdf:resource="https://w3id.org/gcdfo/salmon#SalmonEnhancementHatcheriesTheme"/>
        <theme rdf:resource="https://w3id.org/gcdfo/salmon#StockAssessmentTheme"/>
    </owl:Class>
    


    <!-- https://w3id.org/gcdfo/salmon#RelativeHatcherySpawnerAbundanceTrend -->

    <owl:Class rdf:about="https://w3id.org/gcdfo/salmon#RelativeHatcherySpawnerAbundanceTrend">
        <rdfs:subClassOf rdf:resource="https://w3id.org/gcdfo/salmon#RelativeSpawnerAbundanceTrend"/>
        <obo:IAO_0000115 xml:lang="en">A trend metric computed from relative hatchery-origin spawner abundance using a defined trend method; in rapid-status workflows, long-term trend is the ratio of current generational average (geometric mean) abundance to long-term average (geometric mean).</obo:IAO_0000115>
        <obo:IAO_0000119 xml:lang="en">Fisheries and Oceans Canada. 2024. Rapid Status Approximations for Pacific Salmon… CSAS Pacific Region Science Response 2024/004 (long-term trend in abundance metric definition).</obo:IAO_0000119>
        <dcterms:source rdf:resource="https://waves-vagues.dfo-mpo.gc.ca/library-bibliotheque/41225260.pdf"/>
        <rdfs:isDefinedBy rdf:resource="https://w3id.org/gcdfo/salmon"/>
        <rdfs:label xml:lang="en">Relative hatchery spawner abundance trend</rdfs:label>
        <theme rdf:resource="https://w3id.org/gcdfo/salmon#SalmonEnhancementHatcheriesTheme"/>
        <theme rdf:resource="https://w3id.org/gcdfo/salmon#StockAssessmentTheme"/>
    </owl:Class>
    


    <!-- https://w3id.org/gcdfo/salmon#RelativeSpawnerAbundance -->

    <owl:Class rdf:about="https://w3id.org/gcdfo/salmon#RelativeSpawnerAbundance">
        <rdfs:subClassOf rdf:resource="https://w3id.org/gcdfo/salmon#SpawnerAbundance"/>
        <obo:IAO_0000115 xml:lang="en">Spawner abundance expressed as a relative (dimensionless) abundance metric to a defined reference (commonly benchmarks), for within-series comparison; in rapid-status workflows, relative abundance is computed using the current generational average (geometric mean) divided by CU-specific lower and/or upper benchmarks.</obo:IAO_0000115>
        <obo:IAO_0000119 xml:lang="en">Fisheries and Oceans Canada. 2024. Rapid Status Approximations for Pacific Salmon Derived from Integrated Expert Assessments under Fisheries and Oceans Canada Wild Salmon Policy. CSAS Pacific Region Science Response 2024/004 (relative abundance metric definition and computation).</obo:IAO_0000119>
        <dcterms:source rdf:resource="https://waves-vagues.dfo-mpo.gc.ca/library-bibliotheque/41225260.pdf"/>
        <rdfs:isDefinedBy rdf:resource="https://w3id.org/gcdfo/salmon"/>
        <rdfs:label xml:lang="en">Relative spawner abundance</rdfs:label>
        <theme rdf:resource="https://w3id.org/gcdfo/salmon#StockAssessmentTheme"/>
        <theme rdf:resource="https://w3id.org/gcdfo/salmon#WildSalmonPolicyTheme"/>
    </owl:Class>
    


    <!-- https://w3id.org/gcdfo/salmon#RelativeSpawnerAbundanceChange -->

    <owl:Class rdf:about="https://w3id.org/gcdfo/salmon#RelativeSpawnerAbundanceChange">
        <rdfs:subClassOf rdf:resource="https://w3id.org/gcdfo/salmon#SpawnerAbundanceChange"/>
        <obo:IAO_0000115 xml:lang="en">A change metric (delta or percent change, as defined by the workflow) computed from relative spawner abundance values over time; where rapid-status percent-change approaches are used, it represents change in abundance over the most recent three generations after log transformation (and smoothing where applicable).</obo:IAO_0000115>
        <obo:IAO_0000119 xml:lang="en">Fisheries and Oceans Canada. 2024. Rapid Status Approximations for Pacific Salmon… CSAS Pacific Region Science Response 2024/004 (definition and computation notes for percent change as a short-term trend over three generations).</obo:IAO_0000119>
        <dcterms:source rdf:resource="https://waves-vagues.dfo-mpo.gc.ca/library-bibliotheque/41225260.pdf"/>
        <rdfs:isDefinedBy rdf:resource="https://w3id.org/gcdfo/salmon"/>
        <rdfs:label xml:lang="en">Relative spawner abundance change</rdfs:label>
        <theme rdf:resource="https://w3id.org/gcdfo/salmon#StockAssessmentTheme"/>
        <theme rdf:resource="https://w3id.org/gcdfo/salmon#WildSalmonPolicyTheme"/>
    </owl:Class>
    


    <!-- https://w3id.org/gcdfo/salmon#RelativeSpawnerAbundancePercentile -->

    <owl:Class rdf:about="https://w3id.org/gcdfo/salmon#RelativeSpawnerAbundancePercentile">
        <rdfs:subClassOf rdf:resource="https://w3id.org/gcdfo/salmon#SpawnerAbundancePercentile"/>
        <obo:IAO_0000115 xml:lang="en">The percentile rank of relative spawner abundance against a defined historical reference distribution.</obo:IAO_0000115>
        <obo:IAO_0000119 xml:lang="en">Fisheries and Oceans Canada. 2024. Rapid Status Approximations… CSAS Science Response 2024/004 (percentile benchmarks discussion).</obo:IAO_0000119>
        <dcterms:source rdf:resource="https://waves-vagues.dfo-mpo.gc.ca/library-bibliotheque/41225260.pdf"/>
        <rdfs:isDefinedBy rdf:resource="https://w3id.org/gcdfo/salmon"/>
        <rdfs:label xml:lang="en">Relative spawner abundance percentile</rdfs:label>
        <theme rdf:resource="https://w3id.org/gcdfo/salmon#StockAssessmentTheme"/>
        <theme rdf:resource="https://w3id.org/gcdfo/salmon#WildSalmonPolicyTheme"/>
    </owl:Class>
    


    <!-- https://w3id.org/gcdfo/salmon#RelativeSpawnerAbundanceTrend -->

    <owl:Class rdf:about="https://w3id.org/gcdfo/salmon#RelativeSpawnerAbundanceTrend">
        <rdfs:subClassOf rdf:resource="https://w3id.org/gcdfo/salmon#SpawnerAbundanceTrend"/>
        <obo:IAO_0000115 xml:lang="en">A long-term trend metric expressed as the ratio of the current generational average (geometric mean) spawner abundance to the long-term average (geometric mean), yielding a dimensionless measure of relative abundance through time.</obo:IAO_0000115>
        <obo:IAO_0000119 xml:lang="en">Fisheries and Oceans Canada. 2024. Rapid Status Approximations for Pacific Salmon… CSAS Pacific Region Science Response 2024/004 (long-term trend in abundance defined as ratio of current generational average to long-term average).</obo:IAO_0000119>
        <dcterms:source rdf:resource="https://waves-vagues.dfo-mpo.gc.ca/library-bibliotheque/41225260.pdf"/>
        <rdfs:isDefinedBy rdf:resource="https://w3id.org/gcdfo/salmon"/>
        <rdfs:label xml:lang="en">Relative spawner abundance trend</rdfs:label>
        <theme rdf:resource="https://w3id.org/gcdfo/salmon#StockAssessmentTheme"/>
        <theme rdf:resource="https://w3id.org/gcdfo/salmon#WildSalmonPolicyTheme"/>
    </owl:Class>
    


    <!-- https://w3id.org/gcdfo/salmon#RelativeWildSpawnerAbundance -->

    <owl:Class rdf:about="https://w3id.org/gcdfo/salmon#RelativeWildSpawnerAbundance">
        <rdfs:subClassOf rdf:resource="https://w3id.org/gcdfo/salmon#RelativeSpawnerAbundance"/>
        <obo:IAO_0000115 xml:lang="en">Natural-origin (wild) spawner abundance expressed as a relative (dimensionless) abundance metric to a defined reference (commonly benchmarks), for within-series comparison; where WSP-style relative abundance is used, it is computed using current generational averages (geometric mean) relative to CU-specific benchmarks.</obo:IAO_0000115>
        <obo:IAO_0000119 xml:lang="en">Fisheries and Oceans Canada. 2024. Rapid Status Approximations for Pacific Salmon… CSAS Pacific Region Science Response 2024/004 (relative abundance metric definition). Holt et al. 2009. Indicators of Status and Benchmarks for Conservation Units in Canada&apos;s Wild Salmon Policy. CSAS Res. Doc. 2009/058 (wild vs hatchery-origin considerations in spawner series context).</obo:IAO_0000119>
        <dcterms:source rdf:resource="https://waves-vagues.dfo-mpo.gc.ca/library-bibliotheque/339096.pdf"/>
        <dcterms:source rdf:resource="https://waves-vagues.dfo-mpo.gc.ca/library-bibliotheque/41225260.pdf"/>
        <rdfs:isDefinedBy rdf:resource="https://w3id.org/gcdfo/salmon"/>
        <rdfs:label xml:lang="en">Relative wild spawner abundance</rdfs:label>
        <theme rdf:resource="https://w3id.org/gcdfo/salmon#StockAssessmentTheme"/>
        <theme rdf:resource="https://w3id.org/gcdfo/salmon#WildSalmonPolicyTheme"/>
    </owl:Class>
    


    <!-- https://w3id.org/gcdfo/salmon#RelativeWildSpawnerAbundanceChange -->

    <owl:Class rdf:about="https://w3id.org/gcdfo/salmon#RelativeWildSpawnerAbundanceChange">
        <rdfs:subClassOf rdf:resource="https://w3id.org/gcdfo/salmon#RelativeSpawnerAbundanceChange"/>
        <obo:IAO_0000115 xml:lang="en">A change metric (delta or percent change, as defined by the workflow) computed from relative natural-origin spawner abundance values over time; in rapid-status workflows, percent change is defined over the most recent three generations using log-transformed abundance series.</obo:IAO_0000115>
        <obo:IAO_0000119 xml:lang="en">Fisheries and Oceans Canada. 2024. Rapid Status Approximations for Pacific Salmon… CSAS Pacific Region Science Response 2024/004 (definition and computation notes for percent change over the most recent three generations).</obo:IAO_0000119>
        <dcterms:source rdf:resource="https://waves-vagues.dfo-mpo.gc.ca/library-bibliotheque/41225260.pdf"/>
        <rdfs:isDefinedBy rdf:resource="https://w3id.org/gcdfo/salmon"/>
        <rdfs:label xml:lang="en">Relative wild spawner abundance change</rdfs:label>
        <theme rdf:resource="https://w3id.org/gcdfo/salmon#StockAssessmentTheme"/>
        <theme rdf:resource="https://w3id.org/gcdfo/salmon#WildSalmonPolicyTheme"/>
    </owl:Class>
    


    <!-- https://w3id.org/gcdfo/salmon#RelativeWildSpawnerAbundancePercentile -->

    <owl:Class rdf:about="https://w3id.org/gcdfo/salmon#RelativeWildSpawnerAbundancePercentile">
        <rdfs:subClassOf rdf:resource="https://w3id.org/gcdfo/salmon#RelativeSpawnerAbundancePercentile"/>
        <obo:IAO_0000115 xml:lang="en">The percentile rank of relative natural-origin spawner abundance against a defined historical reference distribution.</obo:IAO_0000115>
        <obo:IAO_0000119 xml:lang="en">Fisheries and Oceans Canada. 2024. Rapid Status Approximations… CSAS Science Response 2024/004 (percentile benchmarks discussion).</obo:IAO_0000119>
        <dcterms:source rdf:resource="https://waves-vagues.dfo-mpo.gc.ca/library-bibliotheque/41225260.pdf"/>
        <rdfs:isDefinedBy rdf:resource="https://w3id.org/gcdfo/salmon"/>
        <rdfs:label xml:lang="en">Relative wild spawner abundance percentile</rdfs:label>
        <theme rdf:resource="https://w3id.org/gcdfo/salmon#StockAssessmentTheme"/>
        <theme rdf:resource="https://w3id.org/gcdfo/salmon#WildSalmonPolicyTheme"/>
    </owl:Class>
    


    <!-- https://w3id.org/gcdfo/salmon#RelativeWildSpawnerAbundanceTrend -->

    <owl:Class rdf:about="https://w3id.org/gcdfo/salmon#RelativeWildSpawnerAbundanceTrend">
        <rdfs:subClassOf rdf:resource="https://w3id.org/gcdfo/salmon#RelativeSpawnerAbundanceTrend"/>
        <obo:IAO_0000115 xml:lang="en">A trend metric computed from relative natural-origin spawner abundance using a defined trend method; in rapid-status workflows, long-term trend is the ratio of current generational average (geometric mean) abundance to long-term average (geometric mean).</obo:IAO_0000115>
        <obo:IAO_0000119 xml:lang="en">Fisheries and Oceans Canada. 2024. Rapid Status Approximations for Pacific Salmon… CSAS Pacific Region Science Response 2024/004 (long-term trend in abundance metric definition).</obo:IAO_0000119>
        <dcterms:source rdf:resource="https://waves-vagues.dfo-mpo.gc.ca/library-bibliotheque/41225260.pdf"/>
        <rdfs:isDefinedBy rdf:resource="https://w3id.org/gcdfo/salmon"/>
        <rdfs:label xml:lang="en">Relative wild spawner abundance trend</rdfs:label>
        <theme rdf:resource="https://w3id.org/gcdfo/salmon#StockAssessmentTheme"/>
        <theme rdf:resource="https://w3id.org/gcdfo/salmon#WildSalmonPolicyTheme"/>
    </owl:Class>
    


    <!-- https://w3id.org/gcdfo/salmon#ReportingOrManagementStratum -->

    <owl:Class rdf:about="https://w3id.org/gcdfo/salmon#ReportingOrManagementStratum">
        <rdfs:subClassOf rdf:resource="http://purl.obolibrary.org/obo/IAO_0000030"/>
        <obo:IAO_0000115 xml:lang="en">An information-defined grouping of fish populations used for reporting, conservation assessment, or management purposes. Examples include Conservation Units (CUs), Stock Management Units (MUs), and Designatable Units (DUs).</obo:IAO_0000115>
        <rdfs:isDefinedBy rdf:resource="https://w3id.org/gcdfo/salmon"/>
        <rdfs:label xml:lang="en">Reporting or management stratum</rdfs:label>
        <theme rdf:resource="https://w3id.org/gcdfo/salmon#PolicyGovernanceTheme"/>
        <theme rdf:resource="https://w3id.org/gcdfo/salmon#StockAssessmentTheme"/>
    </owl:Class>
    


    <!-- https://w3id.org/gcdfo/salmon#ReturnYear -->

    <owl:Class rdf:about="https://w3id.org/gcdfo/salmon#ReturnYear">
        <rdfs:subClassOf rdf:resource="https://w3id.org/gcdfo/salmon#YearBasis"/>
        <obo:IAO_0000115 xml:lang="en">The calendar year in which adult salmon return from the ocean to freshwater systems (a year basis used to contextualize run/return-related measurements).</obo:IAO_0000115>
        <obo:IAO_0000119 xml:lang="en">Fisheries and Oceans Canada. Pacific Salmon Glossary (Pacific Region web page).</obo:IAO_0000119>
        <dcterms:source rdf:resource="https://www.pac.dfo-mpo.gc.ca/fm-gp/salmon-saumon/gloss-eng.html"/>
        <rdfs:isDefinedBy rdf:resource="https://w3id.org/gcdfo/salmon"/>
        <rdfs:label xml:lang="en">Return year</rdfs:label>
        <theme rdf:resource="https://w3id.org/gcdfo/salmon#FisheriesManagementTheme"/>
        <theme rdf:resource="https://w3id.org/gcdfo/salmon#StockAssessmentTheme"/>
        <theme rdf:resource="https://w3id.org/gcdfo/salmon#WildSalmonPolicyTheme"/>
    </owl:Class>
    


    <!-- https://w3id.org/gcdfo/salmon#SpawnerAbundance -->

    <owl:Class rdf:about="https://w3id.org/gcdfo/salmon#SpawnerAbundance">
        <rdfs:subClassOf rdf:resource="https://w3id.org/gcdfo/salmon#ObservedRateOrAbundance"/>
        <obo:IAO_0000115 xml:lang="en">The abundance (count) of adult salmon that reach spawning grounds in a given system and time period (often operationalized as escapement/spawning escapement).</obo:IAO_0000115>
        <obo:IAO_0000119 xml:lang="en">Fisheries and Oceans Canada. Pacific Salmon Glossary (defines escapement/spawning escapement as the number of salmon returning to the spawning grounds).</obo:IAO_0000119>
        <dcterms:source rdf:resource="https://www.pac.dfo-mpo.gc.ca/fm-gp/salmon-saumon/gloss-eng.html"/>
        <rdfs:isDefinedBy rdf:resource="https://w3id.org/gcdfo/salmon"/>
        <rdfs:label xml:lang="en">Spawner abundance</rdfs:label>
        <skos:altLabel xml:lang="en">Escapement (count)</skos:altLabel>
        <skos:closeMatch rdf:resource="http://purl.dataone.org/odo/SALMON_00000479"/>
        <theme rdf:resource="https://w3id.org/gcdfo/salmon#StockAssessmentTheme"/>
        <theme rdf:resource="https://w3id.org/gcdfo/salmon#WildSalmonPolicyTheme"/>
    </owl:Class>
    


    <!-- https://w3id.org/gcdfo/salmon#SpawnerAbundanceChange -->

    <owl:Class rdf:about="https://w3id.org/gcdfo/salmon#SpawnerAbundanceChange">
        <rdfs:subClassOf rdf:resource="https://w3id.org/gcdfo/salmon#ObservedRateOrAbundance"/>
        <obo:IAO_0000115 xml:lang="en">A change metric (delta or percent change, as defined by the workflow) computed from spawner abundance values over time; in rapid-status workflows, percent change is quantified as a linear change in log-transformed abundance over the most recent three generations.</obo:IAO_0000115>
        <obo:IAO_0000119 xml:lang="en">Fisheries and Oceans Canada. 2024. Rapid Status Approximations for Pacific Salmon… CSAS Pacific Region Science Response 2024/004 (percent change definition and computation notes). COSEWIC. 2017. Sockeye Salmon assessment and status report (log-linear rate-of-change model and percent-change derivation over three generations).</obo:IAO_0000119>
        <dcterms:source rdf:resource="https://waves-vagues.dfo-mpo.gc.ca/library-bibliotheque/41225260.pdf"/>
        <dcterms:source rdf:resource="https://www.canada.ca/en/environment-climate-change/services/species-risk-public-registry/cosewic-assessments-status-reports/sockeye-salmon-2017.html"/>
        <rdfs:isDefinedBy rdf:resource="https://w3id.org/gcdfo/salmon"/>
        <rdfs:label xml:lang="en">Spawner abundance change</rdfs:label>
        <theme rdf:resource="https://w3id.org/gcdfo/salmon#StockAssessmentTheme"/>
        <theme rdf:resource="https://w3id.org/gcdfo/salmon#WildSalmonPolicyTheme"/>
    </owl:Class>
    


    <!-- https://w3id.org/gcdfo/salmon#SpawnerAbundancePercentile -->

    <owl:Class rdf:about="https://w3id.org/gcdfo/salmon#SpawnerAbundancePercentile">
        <rdfs:subClassOf rdf:resource="https://w3id.org/gcdfo/salmon#ObservedRateOrAbundance"/>
        <obo:IAO_0000115 xml:lang="en">The percentile rank of a spawner abundance value (annual or period-specific) against a defined historical reference distribution.</obo:IAO_0000115>
        <obo:IAO_0000119 xml:lang="en">Fisheries and Oceans Canada. 2024. Rapid Status Approximations… CSAS Science Response 2024/004 (percentile benchmarks discussion).</obo:IAO_0000119>
        <dcterms:source rdf:resource="https://waves-vagues.dfo-mpo.gc.ca/library-bibliotheque/41225260.pdf"/>
        <rdfs:isDefinedBy rdf:resource="https://w3id.org/gcdfo/salmon"/>
        <rdfs:label xml:lang="en">Spawner abundance percentile</rdfs:label>
        <theme rdf:resource="https://w3id.org/gcdfo/salmon#StockAssessmentTheme"/>
        <theme rdf:resource="https://w3id.org/gcdfo/salmon#WildSalmonPolicyTheme"/>
    </owl:Class>
    


    <!-- https://w3id.org/gcdfo/salmon#SpawnerAbundanceTrend -->

    <owl:Class rdf:about="https://w3id.org/gcdfo/salmon#SpawnerAbundanceTrend">
        <rdfs:subClassOf rdf:resource="https://w3id.org/gcdfo/salmon#ObservedRateOrAbundance"/>
        <obo:IAO_0000115 xml:lang="en">A trend metric computed from spawner abundance over time using a defined trend method (e.g., slope over a specified window).</obo:IAO_0000115>
        <obo:IAO_0000119 xml:lang="en">Derived for SPSR term coverage; distinct from gcdfo:LongTermTrendMetric (current generational average vs long-term average) in CSAS Science Response 2024/004.</obo:IAO_0000119>
        <dcterms:source rdf:resource="https://waves-vagues.dfo-mpo.gc.ca/library-bibliotheque/41225260.pdf"/>
        <rdfs:isDefinedBy rdf:resource="https://w3id.org/gcdfo/salmon"/>
        <rdfs:label xml:lang="en">Spawner abundance trend</rdfs:label>
        <theme rdf:resource="https://w3id.org/gcdfo/salmon#StockAssessmentTheme"/>
        <theme rdf:resource="https://w3id.org/gcdfo/salmon#WildSalmonPolicyTheme"/>
    </owl:Class>
    


    <!-- https://w3id.org/gcdfo/salmon#Stock -->

    <owl:Class rdf:about="https://w3id.org/gcdfo/salmon#Stock">
        <rdfs:subClassOf rdf:resource="https://w3id.org/gcdfo/salmon#ReportingOrManagementStratum"/>
        <obo:IAO_0000115 xml:lang="en">An operationally-defined grouping of salmon used for assessment and management purposes. A stock is a management unit or reporting stratum, not a biological organism.</obo:IAO_0000115>
        <obo:IAO_0000119 xml:lang="en">Fisheries and Oceans Canada. Introduction to Stock Assessment - Glossary. https://www.dfo-mpo.gc.ca/science/species-especes/fisheries-halieutiques/assessment-evaluation/glossary-glossaire/index-eng.html.</obo:IAO_0000119>
        <dcterms:source rdf:resource="https://www.dfo-mpo.gc.ca/science/species-especes/fisheries-halieutiques/assessment-evaluation/glossary-glossaire/index-eng.html"/>
        <rdfs:isDefinedBy rdf:resource="https://w3id.org/gcdfo/salmon"/>
        <rdfs:label xml:lang="en">Stock</rdfs:label>
        <skos:altLabel xml:lang="en">Fish stock</skos:altLabel>
        <theme rdf:resource="https://w3id.org/gcdfo/salmon#FisheriesManagementTheme"/>
        <theme rdf:resource="https://w3id.org/gcdfo/salmon#PolicyGovernanceTheme"/>
        <theme rdf:resource="https://w3id.org/gcdfo/salmon#StockAssessmentTheme"/>
    </owl:Class>
    


    <!-- https://w3id.org/gcdfo/salmon#StockAssessment -->

    <owl:Class rdf:about="https://w3id.org/gcdfo/salmon#StockAssessment">
        <rdfs:subClassOf rdf:resource="http://purl.obolibrary.org/obo/BFO_0000015"/>
        <obo:IAO_0000115 xml:lang="en">The scientific process of analyzing data to estimate the abundance and productivity of fish stocks in the past, present, and future. It is the backbone of successful science-based fisheries management</obo:IAO_0000115>
        <obo:IAO_0000119 xml:lang="en">Fisheries and Oceans Canada. Introduction to Stock Assessment. https://www.dfo-mpo.gc.ca/science/species-especes/fisheries-halieutiques/assessment-evaluation/module-1/09-eng.html.</obo:IAO_0000119>
        <dcterms:source rdf:resource="https://www.dfo-mpo.gc.ca/science/species-especes/fisheries-halieutiques/assessment-evaluation/module-1/09-eng.html"/>
        <rdfs:isDefinedBy rdf:resource="https://w3id.org/gcdfo/salmon"/>
        <rdfs:label xml:lang="en">Stock assessment</rdfs:label>
        <theme rdf:resource="https://w3id.org/gcdfo/salmon#StockAssessmentTheme"/>
    </owl:Class>
    


    <!-- https://w3id.org/gcdfo/salmon#StockManagementUnit -->

    <owl:Class rdf:about="https://w3id.org/gcdfo/salmon#StockManagementUnit">
        <rdfs:subClassOf rdf:resource="https://w3id.org/gcdfo/salmon#ReportingOrManagementStratum"/>
        <obo:IAO_0000115 xml:lang="en">A collection of stocks that are managed together with a joint stock status.</obo:IAO_0000115>
        <obo:IAO_0000119 xml:lang="en">Fisheries and Oceans Canada. Introduction to Stock Assessment - Glossary. https://www.dfo-mpo.gc.ca/science/species-especes/fisheries-halieutiques/assessment-evaluation/glossary-glossaire/index-eng.html.</obo:IAO_0000119>
        <dcterms:source rdf:resource="https://www.dfo-mpo.gc.ca/science/species-especes/fisheries-halieutiques/assessment-evaluation/glossary-glossaire/index-eng.html"/>
        <rdfs:isDefinedBy rdf:resource="https://w3id.org/gcdfo/salmon"/>
        <rdfs:label xml:lang="en">Stock Management Unit</rdfs:label>
        <skos:altLabel xml:lang="en">SMU</skos:altLabel>
        <theme rdf:resource="https://w3id.org/gcdfo/salmon#FisheriesManagementTheme"/>
        <theme rdf:resource="https://w3id.org/gcdfo/salmon#PolicyGovernanceTheme"/>
        <theme rdf:resource="https://w3id.org/gcdfo/salmon#StockAssessmentTheme"/>
    </owl:Class>
    


    <!-- https://w3id.org/gcdfo/salmon#SurveyEvent -->

    <owl:Class rdf:about="https://w3id.org/gcdfo/salmon#SurveyEvent">
        <rdfs:subClassOf rdf:resource="http://rs.tdwg.org/dwc/terms/Event"/>
        <obo:IAO_0000115 xml:lang="en">A field event that collects information about key fish stocks to track their status, and track progress to implement fishery policies and measures for these stocks.</obo:IAO_0000115>
        <obo:IAO_0000119 xml:lang="en">Fisheries and Oceans Canada. About the Sustainability Survey for Fisheries. https://www.dfo-mpo.gc.ca/reports-rapports/regs/sff-cpd/survey-sondage/about-propos-en.html.</obo:IAO_0000119>
        <dcterms:source rdf:resource="https://www.dfo-mpo.gc.ca/reports-rapports/regs/sff-cpd/survey-sondage/about-propos-en.html"/>
        <rdfs:isDefinedBy rdf:resource="https://w3id.org/gcdfo/salmon"/>
        <rdfs:label xml:lang="en">Survey event</rdfs:label>
        <theme rdf:resource="https://w3id.org/gcdfo/salmon#MonitoringFieldWorkTheme"/>
        <theme rdf:resource="https://w3id.org/gcdfo/salmon#StockAssessmentTheme"/>
    </owl:Class>
    


    <!-- https://w3id.org/gcdfo/salmon#TargetOrLimitExploitationRate -->

    <owl:Class rdf:about="https://w3id.org/gcdfo/salmon#TargetOrLimitExploitationRate">
        <rdfs:subClassOf rdf:resource="https://w3id.org/gcdfo/salmon#ExploitationRate"/>
        <rdfs:subClassOf rdf:resource="https://w3id.org/gcdfo/salmon#TargetOrLimitRateOrAbundance"/>
        <obo:IAO_0000115 xml:lang="en">A policy- or management-defined exploitation-rate value used as a target, threshold, or limit reference in decision rules.</obo:IAO_0000115>
        <obo:IAO_0000119 xml:lang="en">Fisheries and Oceans Canada. Introduction to Stock Assessment - Glossary. https://www.dfo-mpo.gc.ca/science/species-especes/fisheries-halieutiques/assessment-evaluation/glossary-glossaire/index-eng.html.</obo:IAO_0000119>
        <dcterms:source rdf:resource="https://www.dfo-mpo.gc.ca/science/species-especes/fisheries-halieutiques/assessment-evaluation/glossary-glossaire/index-eng.html"/>
        <rdfs:isDefinedBy rdf:resource="https://w3id.org/gcdfo/salmon"/>
        <rdfs:label xml:lang="en">Target or limit exploitation rate</rdfs:label>
        <theme rdf:resource="https://w3id.org/gcdfo/salmon#FisheriesManagementTheme"/>
        <theme rdf:resource="https://w3id.org/gcdfo/salmon#PolicyGovernanceTheme"/>
        <theme rdf:resource="https://w3id.org/gcdfo/salmon#StockAssessmentTheme"/>
    </owl:Class>
    


    <!-- https://w3id.org/gcdfo/salmon#TargetOrLimitRateOrAbundance -->

    <owl:Class rdf:about="https://w3id.org/gcdfo/salmon#TargetOrLimitRateOrAbundance">
        <rdfs:subClassOf rdf:resource="http://purl.obolibrary.org/obo/IAO_0000109"/>
        <obo:IAO_0000115 xml:lang="en">A value specification representing a policy- or model-defined target or limit, such as TAC or UMSY.</obo:IAO_0000115>
        <rdfs:isDefinedBy rdf:resource="https://w3id.org/gcdfo/salmon"/>
        <rdfs:label xml:lang="en">Target or limit rate or abundance</rdfs:label>
        <theme rdf:resource="https://w3id.org/gcdfo/salmon#DataModelProvenanceTheme"/>
        <theme rdf:resource="https://w3id.org/gcdfo/salmon#PolicyGovernanceTheme"/>
        <theme rdf:resource="https://w3id.org/gcdfo/salmon#StockAssessmentTheme"/>
    </owl:Class>
    


    <!-- https://w3id.org/gcdfo/salmon#TerminalMortalityRate -->

    <owl:Class rdf:about="https://w3id.org/gcdfo/salmon#TerminalMortalityRate">
        <rdfs:subClassOf rdf:resource="https://w3id.org/gcdfo/salmon#ObservedRateOrAbundance"/>
        <obo:IAO_0000115 xml:lang="en">The proportion of fish that die after reaching terminal spawning areas (or immediate vicinity) but before successfully spawning, as defined by the assessment workflow (i.e., pre-spawn mortality in terminal areas).</obo:IAO_0000115>
        <obo:IAO_0000119 xml:lang="en">COSEWIC. 2017. Sockeye Salmon (Oncorhynchus nerka) assessment and status report (pre-spawn mortality includes fish that made it to spawning grounds but did not successfully spawn). LGL Limited. Migration and Survival of Late-run Fraser Sockeye (operational identification of pre-spawn mortalities from spawning-area detections).</obo:IAO_0000119>
        <dcterms:source rdf:resource="https://waves-vagues.dfo-mpo.gc.ca/library-bibliotheque/341440.pdf"/>
        <dcterms:source rdf:resource="https://www.canada.ca/en/environment-climate-change/services/species-risk-public-registry/cosewic-assessments-status-reports/sockeye-salmon-2017.html"/>
        <rdfs:isDefinedBy rdf:resource="https://w3id.org/gcdfo/salmon"/>
        <rdfs:label xml:lang="en">Terminal mortality rate</rdfs:label>
        <theme rdf:resource="https://w3id.org/gcdfo/salmon#StockAssessmentTheme"/>
    </owl:Class>
    


    <!-- https://w3id.org/gcdfo/salmon#TotalExploitationRate -->

    <owl:Class rdf:about="https://w3id.org/gcdfo/salmon#TotalExploitationRate">
        <rdfs:subClassOf rdf:resource="https://w3id.org/gcdfo/salmon#ObservedExploitationRate"/>
        <obo:IAO_0000115 xml:lang="en">The overall proportion of the total return of adult salmon removed by all fisheries over a defined period, aggregating across gear or fishery components.</obo:IAO_0000115>
        <rdfs:isDefinedBy rdf:resource="https://w3id.org/gcdfo/salmon"/>
        <rdfs:label xml:lang="en">Total exploitation rate</rdfs:label>
        <theme rdf:resource="https://w3id.org/gcdfo/salmon#FisheriesManagementTheme"/>
        <theme rdf:resource="https://w3id.org/gcdfo/salmon#StockAssessmentTheme"/>
    </owl:Class>
    


    <!-- https://w3id.org/gcdfo/salmon#TotalMortalityRate -->

    <owl:Class rdf:about="https://w3id.org/gcdfo/salmon#TotalMortalityRate">
        <rdfs:subClassOf rdf:resource="https://w3id.org/gcdfo/salmon#ObservedRateOrAbundance"/>
        <obo:IAO_0000115 xml:lang="en">The overall proportion of fish in a defined cohort that die over the full assessment interval across all included phases and mortality sources, consistent with the workflow’s accounting (e.g., catch vs escapement vs migration losses where relevant).</obo:IAO_0000115>
        <obo:IAO_0000119 xml:lang="en">Fisheries and Oceans Canada. 2025. Stock-Specific Fraser River Sockeye Salmon Run Size Determination. CSAS Pacific Region Science Advisory Report 2025/021 (run size components include catch, spawning escapement, and en route mortality; other Pacific salmon run sizes typically sum catch + escapement). COSEWIC. 2017. Sockeye Salmon assessment and status report (uses catch, escapement, and en-route loss as distinct accounting components).</obo:IAO_0000119>
        <dcterms:source rdf:resource="https://waves-vagues.dfo-mpo.gc.ca/library-bibliotheque/41294622.pdf"/>
        <dcterms:source rdf:resource="https://www.canada.ca/en/environment-climate-change/services/species-risk-public-registry/cosewic-assessments-status-reports/sockeye-salmon-2017.html"/>
        <rdfs:isDefinedBy rdf:resource="https://w3id.org/gcdfo/salmon"/>
        <rdfs:label xml:lang="en">Total mortality rate</rdfs:label>
        <theme rdf:resource="https://w3id.org/gcdfo/salmon#StockAssessmentTheme"/>
    </owl:Class>
    


    <!-- https://w3id.org/gcdfo/salmon#UpperBiologicalBenchmark -->

    <owl:Class rdf:about="https://w3id.org/gcdfo/salmon#UpperBiologicalBenchmark">
        <rdfs:subClassOf rdf:resource="https://w3id.org/gcdfo/salmon#MetricBenchmark"/>
        <obo:IAO_0000115 xml:lang="en">Upper benchmark value for a metric used to delineate Wild Salmon Policy status zones (typically the boundary between Amber and Green zones).</obo:IAO_0000115>
        <obo:IAO_0000119 xml:lang="en">Fisheries and Oceans Canada. Wild Salmon Policy 2018-2022 Implementation Plan. https://waves-vagues.dfo-mpo.gc.ca/library-bibliotheque/40728109.pdf.</obo:IAO_0000119>
        <dcterms:source rdf:resource="https://waves-vagues.dfo-mpo.gc.ca/library-bibliotheque/40728109.pdf"/>
        <rdfs:isDefinedBy rdf:resource="https://w3id.org/gcdfo/salmon"/>
        <rdfs:label xml:lang="en">Upper biological benchmark</rdfs:label>
        <theme rdf:resource="https://w3id.org/gcdfo/salmon#PolicyGovernanceTheme"/>
        <theme rdf:resource="https://w3id.org/gcdfo/salmon#StockAssessmentTheme"/>
        <theme rdf:resource="https://w3id.org/gcdfo/salmon#WildSalmonPolicyTheme"/>
    </owl:Class>
    


    <!-- https://w3id.org/gcdfo/salmon#UpperStockReferencePoint -->

    <owl:Class rdf:about="https://w3id.org/gcdfo/salmon#UpperStockReferencePoint">
        <rdfs:subClassOf rdf:resource="https://w3id.org/gcdfo/salmon#ReferencePoint"/>
        <obo:IAO_0000115 xml:lang="en">A threshold below which fishing must be reduced to avoid reaching the LRP. The USR must be set at an appropriate distance above the LRP to provide sufficient opportunity for managers to recognize a declining stock status and sufficient time for management actions to take effect. </obo:IAO_0000115>
        <obo:IAO_0000119 xml:lang="en">Fisheries and Oceans Canada. Introduction to Stock Assessment - Glossary. https://www.dfo-mpo.gc.ca/science/species-especes/fisheries-halieutiques/assessment-evaluation/glossary-glossaire/index-eng.html.</obo:IAO_0000119>
        <dcterms:source rdf:resource="https://www.dfo-mpo.gc.ca/science/species-especes/fisheries-halieutiques/assessment-evaluation/glossary-glossaire/index-eng.html"/>
        <rdfs:isDefinedBy rdf:resource="https://w3id.org/gcdfo/salmon"/>
        <rdfs:label xml:lang="en">Upper stock reference</rdfs:label>
        <skos:altLabel xml:lang="en">USR</skos:altLabel>
        <theme rdf:resource="https://w3id.org/gcdfo/salmon#FisheriesManagementTheme"/>
        <theme rdf:resource="https://w3id.org/gcdfo/salmon#PolicyGovernanceTheme"/>
        <theme rdf:resource="https://w3id.org/gcdfo/salmon#StockAssessmentTheme"/>
    </owl:Class>
    


    <!-- https://w3id.org/gcdfo/salmon#WSPBiologicalStatusZone -->

    <owl:Class rdf:about="https://w3id.org/gcdfo/salmon#WSPBiologicalStatusZone"/>
    


    <!-- https://w3id.org/gcdfo/salmon#WSPRapidStatus -->

    <owl:Class rdf:about="https://w3id.org/gcdfo/salmon#WSPRapidStatus">
        <rdfs:subClassOf rdf:resource="http://purl.obolibrary.org/obo/IAO_0000030"/>
        <obo:IAO_0000115 xml:lang="en">The WSP rapid status assessment approach builds on previously completed WSP integrated status assessments. The WSP rapid status approach ensures statuses are scientifically objective, consistent, and comparable across BC/Yukon CUs. This approach is also relatively easy to implement, applicable to data rich and data poor CUs, and can be updated annually.</obo:IAO_0000115>
        <obo:IAO_0000119 xml:lang="en">Pestal, G., MacDonald, B.L., Grant, S.C.H., and Holt, C.A. 2023. State of the salmon: rapid status assessment approach for Pacific salmon under Canada&apos;s Wild Salmon Policy. Canadian Technical Report of Fisheries and Aquatic Sciences 3570.</obo:IAO_0000119>
        <dcterms:source rdf:resource="https://publications.gc.ca/site/eng/9.928944/publication.html"/>
        <rdfs:isDefinedBy rdf:resource="https://w3id.org/gcdfo/salmon"/>
        <rdfs:label xml:lang="en">WSP rapid status</rdfs:label>
        <theme rdf:resource="https://w3id.org/gcdfo/salmon#PolicyGovernanceTheme"/>
        <theme rdf:resource="https://w3id.org/gcdfo/salmon#StockAssessmentTheme"/>
        <theme rdf:resource="https://w3id.org/gcdfo/salmon#WildSalmonPolicyTheme"/>
    </owl:Class>
    


    <!-- https://w3id.org/gcdfo/salmon#WSPRapidStatusAlgorithmThreshold -->

    <owl:Class rdf:about="https://w3id.org/gcdfo/salmon#WSPRapidStatusAlgorithmThreshold">
        <rdfs:subClassOf rdf:resource="http://purl.obolibrary.org/obo/IAO_0000030"/>
        <obo:IAO_0000115 xml:lang="en">Threshold value used by the rapid-status algorithm that may differ from expert-defined benchmarks to incorporate precautionary buffers.</obo:IAO_0000115>
        <obo:IAO_0000119 xml:lang="en">Fisheries and Oceans Canada. 2024. Rapid Status Approximations for Pacific Salmon Derived from Integrated Expert Assessments under Fisheries and Oceans Canada Wild Salmon Policy. DFO Canadian Science Advisory Secretariat Science Response 2024/004.</obo:IAO_0000119>
        <dcterms:source rdf:resource="https://www.dfo-mpo.gc.ca/csas-sccs/Publications/ScR-RS/2024/2024_004-eng.html"/>
        <rdfs:isDefinedBy rdf:resource="https://w3id.org/gcdfo/salmon"/>
        <rdfs:label xml:lang="en">Rapid-status algorithm threshold</rdfs:label>
        <theme rdf:resource="https://w3id.org/gcdfo/salmon#StockAssessmentTheme"/>
        <theme rdf:resource="https://w3id.org/gcdfo/salmon#WildSalmonPolicyTheme"/>
    </owl:Class>
    


    <!-- https://w3id.org/gcdfo/salmon#YearBasis -->

    <owl:Class rdf:about="https://w3id.org/gcdfo/salmon#YearBasis">
        <rdfs:subClassOf rdf:resource="http://purl.obolibrary.org/obo/IAO_0000030"/>
        <obo:IAO_0000115 xml:lang="en">A year-based temporal reference used to contextualize measurements or rates (e.g., brood year, catch year, or return year).</obo:IAO_0000115>
        <rdfs:isDefinedBy rdf:resource="https://w3id.org/gcdfo/salmon"/>
        <rdfs:label xml:lang="en">Year basis</rdfs:label>
        <theme rdf:resource="https://w3id.org/gcdfo/salmon#StockAssessmentTheme"/>
    </owl:Class>
    


    <!-- 
    ///////////////////////////////////////////////////////////////////////////////////////
    //
    // Individuals
    //
    ///////////////////////////////////////////////////////////////////////////////////////
     -->

    


    <!-- https://w3id.org/gcdfo/salmon#AbundanceDataType -->

    <owl:NamedIndividual rdf:about="https://w3id.org/gcdfo/salmon#AbundanceDataType">
        <rdf:type rdf:resource="http://www.w3.org/2004/02/skos/core#Concept"/>
        <obo:IAO_0000115 xml:lang="en">A categorical attribute indicating whether an abundance time series is recorded as absolute abundance or as a relative index (used by rapid-status workflows).</obo:IAO_0000115>
        <obo:IAO_0000119 xml:lang="en">Fisheries and Oceans Canada. 2024. Rapid Status Approximations for Pacific Salmon Derived from Integrated Expert Assessments under DFO’s Wild Salmon Policy. CSAS Pacific Region Science Response 2024/004.</obo:IAO_0000119>
        <dcterms:source rdf:resource="https://waves-vagues.dfo-mpo.gc.ca/library-bibliotheque/41225260.pdf"/>
        <rdfs:isDefinedBy rdf:resource="https://w3id.org/gcdfo/salmon"/>
        <skos:broader rdf:resource="https://w3id.org/gcdfo/salmon#MeasurementContext"/>
        <skos:definition xml:lang="en">A categorical attribute indicating whether an abundance time series is recorded as absolute abundance or as a relative index (used by rapid-status workflows).</skos:definition>
        <skos:inScheme rdf:resource="https://w3id.org/gcdfo/salmon#MeasurementContextScheme"/>
        <skos:prefLabel xml:lang="en">Abundance data type</skos:prefLabel>
        <skos:scopeNote xml:lang="en">In SPSR rapid-status workflows, this field distinguishes absolute abundance vs relative index inputs (often abbreviated in code as &apos;Abs_Abd&apos; and &apos;RelIdx&apos;).</skos:scopeNote>
        <theme rdf:resource="https://w3id.org/gcdfo/salmon#DataModelProvenanceTheme"/>
        <theme rdf:resource="https://w3id.org/gcdfo/salmon#StockAssessmentTheme"/>
        <theme rdf:resource="https://w3id.org/gcdfo/salmon#WildSalmonPolicyTheme"/>
    </owl:NamedIndividual>
    


    <!-- https://w3id.org/gcdfo/salmon#AerialSurveyCount -->

    <owl:NamedIndividual rdf:about="https://w3id.org/gcdfo/salmon#AerialSurveyCount">
        <rdf:type rdf:resource="http://www.w3.org/2004/02/skos/core#Concept"/>
        <rdfs:comment xml:lang="en">Legacy methods: Helicopter, Fixed Wing Aircraft, Aerial, Drone, UAS, UAV</rdfs:comment>
        <rdfs:isDefinedBy rdf:resource="https://w3id.org/gcdfo/salmon"/>
        <skos:broader rdf:resource="https://w3id.org/gcdfo/salmon#EnumerationMethod"/>
        <skos:definition xml:lang="en">Overflights (helicopter, fixed wing, or drone) with documented flight lines, coverage, visibility, and sensor settings. Imagery may be reviewed post-flight.</skos:definition>
        <skos:inScheme rdf:resource="https://w3id.org/gcdfo/salmon#EnumerationMethodScheme"/>
        <skos:prefLabel xml:lang="en">Aerial Survey Count</skos:prefLabel>
        <theme rdf:resource="https://w3id.org/gcdfo/salmon#MonitoringFieldWorkTheme"/>
        <theme rdf:resource="https://w3id.org/gcdfo/salmon#StockAssessmentTheme"/>
    </owl:NamedIndividual>
    


    <!-- https://w3id.org/gcdfo/salmon#Age1YearClass -->

    <owl:NamedIndividual rdf:about="https://w3id.org/gcdfo/salmon#Age1YearClass">
        <rdf:type rdf:resource="http://www.w3.org/2004/02/skos/core#Concept"/>
        <rdfs:isDefinedBy rdf:resource="https://w3id.org/gcdfo/salmon"/>
        <skos:broader rdf:resource="https://w3id.org/gcdfo/salmon#AgeClassValue"/>
        <skos:definition xml:lang="en">Age class value 1 year.</skos:definition>
        <skos:inScheme rdf:resource="https://w3id.org/gcdfo/salmon#AgeClassValueScheme"/>
        <skos:notation rdf:datatype="http://www.w3.org/2001/XMLSchema#integer">1</skos:notation>
        <skos:prefLabel xml:lang="en">Age 1 year class</skos:prefLabel>
        <theme rdf:resource="https://w3id.org/gcdfo/salmon#StockAssessmentTheme"/>
    </owl:NamedIndividual>
    


    <!-- https://w3id.org/gcdfo/salmon#Age2YearClass -->

    <owl:NamedIndividual rdf:about="https://w3id.org/gcdfo/salmon#Age2YearClass">
        <rdf:type rdf:resource="http://www.w3.org/2004/02/skos/core#Concept"/>
        <rdfs:isDefinedBy rdf:resource="https://w3id.org/gcdfo/salmon"/>
        <skos:broader rdf:resource="https://w3id.org/gcdfo/salmon#AgeClassValue"/>
        <skos:definition xml:lang="en">Age class value 2 years.</skos:definition>
        <skos:inScheme rdf:resource="https://w3id.org/gcdfo/salmon#AgeClassValueScheme"/>
        <skos:notation rdf:datatype="http://www.w3.org/2001/XMLSchema#integer">2</skos:notation>
        <skos:prefLabel xml:lang="en">Age 2 year class</skos:prefLabel>
        <theme rdf:resource="https://w3id.org/gcdfo/salmon#StockAssessmentTheme"/>
    </owl:NamedIndividual>
    


    <!-- https://w3id.org/gcdfo/salmon#Age3YearClass -->

    <owl:NamedIndividual rdf:about="https://w3id.org/gcdfo/salmon#Age3YearClass">
        <rdf:type rdf:resource="http://www.w3.org/2004/02/skos/core#Concept"/>
        <rdfs:isDefinedBy rdf:resource="https://w3id.org/gcdfo/salmon"/>
        <skos:broader rdf:resource="https://w3id.org/gcdfo/salmon#AgeClassValue"/>
        <skos:definition xml:lang="en">Age class value 3 years.</skos:definition>
        <skos:inScheme rdf:resource="https://w3id.org/gcdfo/salmon#AgeClassValueScheme"/>
        <skos:notation rdf:datatype="http://www.w3.org/2001/XMLSchema#integer">3</skos:notation>
        <skos:prefLabel xml:lang="en">Age 3 year class</skos:prefLabel>
        <theme rdf:resource="https://w3id.org/gcdfo/salmon#StockAssessmentTheme"/>
    </owl:NamedIndividual>
    


    <!-- https://w3id.org/gcdfo/salmon#Age4YearClass -->

    <owl:NamedIndividual rdf:about="https://w3id.org/gcdfo/salmon#Age4YearClass">
        <rdf:type rdf:resource="http://www.w3.org/2004/02/skos/core#Concept"/>
        <rdfs:isDefinedBy rdf:resource="https://w3id.org/gcdfo/salmon"/>
        <skos:broader rdf:resource="https://w3id.org/gcdfo/salmon#AgeClassValue"/>
        <skos:definition xml:lang="en">Age class value 4 years.</skos:definition>
        <skos:inScheme rdf:resource="https://w3id.org/gcdfo/salmon#AgeClassValueScheme"/>
        <skos:notation rdf:datatype="http://www.w3.org/2001/XMLSchema#integer">4</skos:notation>
        <skos:prefLabel xml:lang="en">Age 4 year class</skos:prefLabel>
        <theme rdf:resource="https://w3id.org/gcdfo/salmon#StockAssessmentTheme"/>
    </owl:NamedIndividual>
    


    <!-- https://w3id.org/gcdfo/salmon#Age5YearClass -->

    <owl:NamedIndividual rdf:about="https://w3id.org/gcdfo/salmon#Age5YearClass">
        <rdf:type rdf:resource="http://www.w3.org/2004/02/skos/core#Concept"/>
        <rdfs:isDefinedBy rdf:resource="https://w3id.org/gcdfo/salmon"/>
        <skos:broader rdf:resource="https://w3id.org/gcdfo/salmon#AgeClassValue"/>
        <skos:definition xml:lang="en">Age class value 5 years.</skos:definition>
        <skos:inScheme rdf:resource="https://w3id.org/gcdfo/salmon#AgeClassValueScheme"/>
        <skos:notation rdf:datatype="http://www.w3.org/2001/XMLSchema#integer">5</skos:notation>
        <skos:prefLabel xml:lang="en">Age 5 year class</skos:prefLabel>
        <theme rdf:resource="https://w3id.org/gcdfo/salmon#StockAssessmentTheme"/>
    </owl:NamedIndividual>
    


    <!-- https://w3id.org/gcdfo/salmon#Age6YearClass -->

    <owl:NamedIndividual rdf:about="https://w3id.org/gcdfo/salmon#Age6YearClass">
        <rdf:type rdf:resource="http://www.w3.org/2004/02/skos/core#Concept"/>
        <rdfs:isDefinedBy rdf:resource="https://w3id.org/gcdfo/salmon"/>
        <skos:broader rdf:resource="https://w3id.org/gcdfo/salmon#AgeClassValue"/>
        <skos:definition xml:lang="en">Age class value 6 years.</skos:definition>
        <skos:inScheme rdf:resource="https://w3id.org/gcdfo/salmon#AgeClassValueScheme"/>
        <skos:notation rdf:datatype="http://www.w3.org/2001/XMLSchema#integer">6</skos:notation>
        <skos:prefLabel xml:lang="en">Age 6 year class</skos:prefLabel>
        <theme rdf:resource="https://w3id.org/gcdfo/salmon#StockAssessmentTheme"/>
    </owl:NamedIndividual>
    


    <!-- https://w3id.org/gcdfo/salmon#Age7YearClass -->

    <owl:NamedIndividual rdf:about="https://w3id.org/gcdfo/salmon#Age7YearClass">
        <rdf:type rdf:resource="http://www.w3.org/2004/02/skos/core#Concept"/>
        <rdfs:isDefinedBy rdf:resource="https://w3id.org/gcdfo/salmon"/>
        <skos:broader rdf:resource="https://w3id.org/gcdfo/salmon#AgeClassValue"/>
        <skos:definition xml:lang="en">Age class value 7 years.</skos:definition>
        <skos:inScheme rdf:resource="https://w3id.org/gcdfo/salmon#AgeClassValueScheme"/>
        <skos:notation rdf:datatype="http://www.w3.org/2001/XMLSchema#integer">7</skos:notation>
        <skos:prefLabel xml:lang="en">Age 7 year class</skos:prefLabel>
        <theme rdf:resource="https://w3id.org/gcdfo/salmon#StockAssessmentTheme"/>
    </owl:NamedIndividual>
    


    <!-- https://w3id.org/gcdfo/salmon#AgeAtMaturityBasis -->

    <owl:NamedIndividual rdf:about="https://w3id.org/gcdfo/salmon#AgeAtMaturityBasis">
        <rdf:type rdf:resource="http://www.w3.org/2004/02/skos/core#Concept"/>
        <rdfs:isDefinedBy rdf:resource="https://w3id.org/gcdfo/salmon"/>
        <skos:broader rdf:resource="https://w3id.org/gcdfo/salmon#AgeBasis"/>
        <skos:definition xml:lang="en">Age measured at maturity.</skos:definition>
        <skos:inScheme rdf:resource="https://w3id.org/gcdfo/salmon#AgeBasisScheme"/>
        <skos:prefLabel xml:lang="en">Age at maturity basis</skos:prefLabel>
        <theme rdf:resource="https://w3id.org/gcdfo/salmon#DataModelProvenanceTheme"/>
        <theme rdf:resource="https://w3id.org/gcdfo/salmon#StockAssessmentTheme"/>
    </owl:NamedIndividual>
    


    <!-- https://w3id.org/gcdfo/salmon#AgeAtReturnBasis -->

    <owl:NamedIndividual rdf:about="https://w3id.org/gcdfo/salmon#AgeAtReturnBasis">
        <rdf:type rdf:resource="http://www.w3.org/2004/02/skos/core#Concept"/>
        <rdfs:isDefinedBy rdf:resource="https://w3id.org/gcdfo/salmon"/>
        <skos:broader rdf:resource="https://w3id.org/gcdfo/salmon#AgeBasis"/>
        <skos:definition xml:lang="en">Age measured at return migration (adult return timing).</skos:definition>
        <skos:inScheme rdf:resource="https://w3id.org/gcdfo/salmon#AgeBasisScheme"/>
        <skos:prefLabel xml:lang="en">Age at return basis</skos:prefLabel>
        <theme rdf:resource="https://w3id.org/gcdfo/salmon#DataModelProvenanceTheme"/>
        <theme rdf:resource="https://w3id.org/gcdfo/salmon#StockAssessmentTheme"/>
    </owl:NamedIndividual>
    


    <!-- https://w3id.org/gcdfo/salmon#AgeAtSamplingBasis -->

    <owl:NamedIndividual rdf:about="https://w3id.org/gcdfo/salmon#AgeAtSamplingBasis">
        <rdf:type rdf:resource="http://www.w3.org/2004/02/skos/core#Concept"/>
        <rdfs:isDefinedBy rdf:resource="https://w3id.org/gcdfo/salmon"/>
        <skos:broader rdf:resource="https://w3id.org/gcdfo/salmon#AgeBasis"/>
        <skos:definition xml:lang="en">Age measured at the time of sampling or observation.</skos:definition>
        <skos:inScheme rdf:resource="https://w3id.org/gcdfo/salmon#AgeBasisScheme"/>
        <skos:prefLabel xml:lang="en">Age at sampling basis</skos:prefLabel>
        <theme rdf:resource="https://w3id.org/gcdfo/salmon#DataModelProvenanceTheme"/>
        <theme rdf:resource="https://w3id.org/gcdfo/salmon#StockAssessmentTheme"/>
    </owl:NamedIndividual>
    


    <!-- https://w3id.org/gcdfo/salmon#AgeBasis -->

    <owl:NamedIndividual rdf:about="https://w3id.org/gcdfo/salmon#AgeBasis">
        <rdf:type rdf:resource="http://www.w3.org/2004/02/skos/core#Concept"/>
        <rdfs:isDefinedBy rdf:resource="https://w3id.org/gcdfo/salmon"/>
        <skos:definition xml:lang="en">The reference event or life-history point that an age value is measured against.</skos:definition>
        <skos:inScheme rdf:resource="https://w3id.org/gcdfo/salmon#AgeBasisScheme"/>
        <skos:prefLabel xml:lang="en">Age basis</skos:prefLabel>
        <theme rdf:resource="https://w3id.org/gcdfo/salmon#DataModelProvenanceTheme"/>
        <theme rdf:resource="https://w3id.org/gcdfo/salmon#StockAssessmentTheme"/>
    </owl:NamedIndividual>
    


    <!-- https://w3id.org/gcdfo/salmon#AgeBasisScheme -->

    <owl:NamedIndividual rdf:about="https://w3id.org/gcdfo/salmon#AgeBasisScheme">
        <rdf:type rdf:resource="http://www.w3.org/2004/02/skos/core#ConceptScheme"/>
        <rdfs:isDefinedBy rdf:resource="https://w3id.org/gcdfo/salmon"/>
        <skos:definition xml:lang="en">Controlled vocabulary for the reference event used by an age value (for example, age at return).</skos:definition>
        <skos:hasTopConcept rdf:resource="https://w3id.org/gcdfo/salmon#AgeBasis"/>
        <skos:prefLabel xml:lang="en">Age basis scheme</skos:prefLabel>
        <theme rdf:resource="https://w3id.org/gcdfo/salmon#DataModelProvenanceTheme"/>
        <theme rdf:resource="https://w3id.org/gcdfo/salmon#StockAssessmentTheme"/>
    </owl:NamedIndividual>
    


    <!-- https://w3id.org/gcdfo/salmon#AgeClassValue -->

    <owl:NamedIndividual rdf:about="https://w3id.org/gcdfo/salmon#AgeClassValue">
        <rdf:type rdf:resource="http://www.w3.org/2004/02/skos/core#Concept"/>
        <rdfs:isDefinedBy rdf:resource="https://w3id.org/gcdfo/salmon"/>
        <skos:definition xml:lang="en">An integer-like age class value used as a compositional constraint in salmon measurements.</skos:definition>
        <skos:inScheme rdf:resource="https://w3id.org/gcdfo/salmon#AgeClassValueScheme"/>
        <skos:prefLabel xml:lang="en">Age class value</skos:prefLabel>
        <theme rdf:resource="https://w3id.org/gcdfo/salmon#StockAssessmentTheme"/>
    </owl:NamedIndividual>
    


    <!-- https://w3id.org/gcdfo/salmon#AgeClassValueScheme -->

    <owl:NamedIndividual rdf:about="https://w3id.org/gcdfo/salmon#AgeClassValueScheme">
        <rdf:type rdf:resource="http://www.w3.org/2004/02/skos/core#ConceptScheme"/>
        <rdfs:isDefinedBy rdf:resource="https://w3id.org/gcdfo/salmon"/>
        <skos:definition xml:lang="en">Controlled vocabulary for integer-like age class values used as constraints on salmon measurements.</skos:definition>
        <skos:hasTopConcept rdf:resource="https://w3id.org/gcdfo/salmon#AgeClassValue"/>
        <skos:prefLabel xml:lang="en">Age class value scheme</skos:prefLabel>
        <theme rdf:resource="https://w3id.org/gcdfo/salmon#StockAssessmentTheme"/>
    </owl:NamedIndividual>
    


    <!-- https://w3id.org/gcdfo/salmon#AgeDimension -->

    <owl:NamedIndividual rdf:about="https://w3id.org/gcdfo/salmon#AgeDimension">
        <rdf:type rdf:resource="http://www.w3.org/2004/02/skos/core#Concept"/>
        <rdfs:isDefinedBy rdf:resource="https://w3id.org/gcdfo/salmon"/>
        <skos:definition xml:lang="en">The age component represented by a value (total age, freshwater years, or ocean years).</skos:definition>
        <skos:inScheme rdf:resource="https://w3id.org/gcdfo/salmon#AgeDimensionScheme"/>
        <skos:prefLabel xml:lang="en">Age dimension</skos:prefLabel>
        <theme rdf:resource="https://w3id.org/gcdfo/salmon#StockAssessmentTheme"/>
    </owl:NamedIndividual>
    


    <!-- https://w3id.org/gcdfo/salmon#AgeDimensionScheme -->

    <owl:NamedIndividual rdf:about="https://w3id.org/gcdfo/salmon#AgeDimensionScheme">
        <rdf:type rdf:resource="http://www.w3.org/2004/02/skos/core#ConceptScheme"/>
        <rdfs:isDefinedBy rdf:resource="https://w3id.org/gcdfo/salmon"/>
        <skos:definition xml:lang="en">Controlled vocabulary for which age component is represented (total age, freshwater years, or ocean years).</skos:definition>
        <skos:hasTopConcept rdf:resource="https://w3id.org/gcdfo/salmon#AgeDimension"/>
        <skos:prefLabel xml:lang="en">Age dimension scheme</skos:prefLabel>
        <theme rdf:resource="https://w3id.org/gcdfo/salmon#StockAssessmentTheme"/>
    </owl:NamedIndividual>
    


    <!-- https://w3id.org/gcdfo/salmon#AgeNotation -->

    <owl:NamedIndividual rdf:about="https://w3id.org/gcdfo/salmon#AgeNotation">
        <rdf:type rdf:resource="http://www.w3.org/2004/02/skos/core#Concept"/>
        <rdfs:isDefinedBy rdf:resource="https://w3id.org/gcdfo/salmon"/>
        <skos:definition xml:lang="en">A notation system used to encode salmon age values in stock assessment data.</skos:definition>
        <skos:inScheme rdf:resource="https://w3id.org/gcdfo/salmon#AgeNotationScheme"/>
        <skos:prefLabel xml:lang="en">Age notation</skos:prefLabel>
        <theme rdf:resource="https://w3id.org/gcdfo/salmon#DataModelProvenanceTheme"/>
        <theme rdf:resource="https://w3id.org/gcdfo/salmon#StockAssessmentTheme"/>
    </owl:NamedIndividual>
    


    <!-- https://w3id.org/gcdfo/salmon#AgeNotationScheme -->

    <owl:NamedIndividual rdf:about="https://w3id.org/gcdfo/salmon#AgeNotationScheme">
        <rdf:type rdf:resource="http://www.w3.org/2004/02/skos/core#ConceptScheme"/>
        <rdfs:isDefinedBy rdf:resource="https://w3id.org/gcdfo/salmon"/>
        <skos:definition xml:lang="en">Controlled vocabulary for salmon age notation systems (for example, Gilbert-Rich and European notation).</skos:definition>
        <skos:hasTopConcept rdf:resource="https://w3id.org/gcdfo/salmon#AgeNotation"/>
        <skos:prefLabel xml:lang="en">Age notation scheme</skos:prefLabel>
        <theme rdf:resource="https://w3id.org/gcdfo/salmon#DataModelProvenanceTheme"/>
        <theme rdf:resource="https://w3id.org/gcdfo/salmon#StockAssessmentTheme"/>
    </owl:NamedIndividual>
    


    <!-- https://w3id.org/gcdfo/salmon#AmberZone -->

    <owl:NamedIndividual rdf:about="https://w3id.org/gcdfo/salmon#AmberZone">
        <rdf:type rdf:resource="http://www.w3.org/2004/02/skos/core#Concept"/>
        <rdf:type rdf:resource="https://w3id.org/gcdfo/salmon#WSPBiologicalStatusZone"/>
        <obo:IAO_0000119 xml:lang="en">Fisheries and Oceans Canada. Wild Salmon Policy 2018-2022 Implementation Plan. https://waves-vagues.dfo-mpo.gc.ca/library-bibliotheque/40728109.pdf.</obo:IAO_0000119>
        <dcterms:source rdf:resource="https://waves-vagues.dfo-mpo.gc.ca/library-bibliotheque/40728109.pdf"/>
        <rdfs:isDefinedBy rdf:resource="https://w3id.org/gcdfo/salmon"/>
        <skos:definition xml:lang="en">Amber status implies caution in the management of the Conservation Unit. While a CU in the Amber zone should be at a low risk of loss, there will be a degree of lost production. Decisions about the conservation of CUs in the Amber zone will involve broader consideration of biological, social, and economic issues. </skos:definition>
        <skos:inScheme rdf:resource="https://w3id.org/gcdfo/salmon#WSPBiologicalStatusZoneScheme"/>
        <skos:prefLabel xml:lang="en">Amber zone</skos:prefLabel>
        <theme rdf:resource="https://w3id.org/gcdfo/salmon#StockAssessmentTheme"/>
        <theme rdf:resource="https://w3id.org/gcdfo/salmon#WildSalmonPolicyTheme"/>
    </owl:NamedIndividual>
    


    <!-- https://w3id.org/gcdfo/salmon#AreaUnderTheCurve -->

    <owl:NamedIndividual rdf:about="https://w3id.org/gcdfo/salmon#AreaUnderTheCurve">
        <rdf:type rdf:resource="http://www.w3.org/2004/02/skos/core#Concept"/>
        <rdfs:isDefinedBy rdf:resource="https://w3id.org/gcdfo/salmon"/>
        <skos:altLabel xml:lang="en">AUC</skos:altLabel>
        <skos:broader rdf:resource="https://w3id.org/gcdfo/salmon#EstimateMethod"/>
        <skos:definition xml:lang="en">Integrates serial counts over time using a survey-life parameter; may apply observer efficiency.</skos:definition>
        <skos:inScheme rdf:resource="https://w3id.org/gcdfo/salmon#EstimateMethodScheme"/>
        <skos:prefLabel xml:lang="en">Area Under the Curve</skos:prefLabel>
        <theme rdf:resource="https://w3id.org/gcdfo/salmon#MonitoringFieldWorkTheme"/>
        <theme rdf:resource="https://w3id.org/gcdfo/salmon#StockAssessmentTheme"/>
    </owl:NamedIndividual>
    


    <!-- https://w3id.org/gcdfo/salmon#BenchmarkLevelScheme -->

    <owl:NamedIndividual rdf:about="https://w3id.org/gcdfo/salmon#BenchmarkLevelScheme">
        <rdf:type rdf:resource="http://www.w3.org/2004/02/skos/core#ConceptScheme"/>
        <rdfs:isDefinedBy rdf:resource="https://w3id.org/gcdfo/salmon"/>
        <skos:definition xml:lang="en">Controlled vocabulary for generic benchmark-level qualifiers usable as I-ADOPT constraint values attached to benchmark variables or values.</skos:definition>
        <skos:prefLabel xml:lang="en">Benchmark Level Scheme</skos:prefLabel>
        <theme rdf:resource="https://w3id.org/gcdfo/salmon#StockAssessmentTheme"/>
        <theme rdf:resource="https://w3id.org/gcdfo/salmon#WildSalmonPolicyTheme"/>
    </owl:NamedIndividual>
    


    <!-- https://w3id.org/gcdfo/salmon#BiologicalBenchmarkAndIndicatorScheme -->

    <owl:NamedIndividual rdf:about="https://w3id.org/gcdfo/salmon#BiologicalBenchmarkAndIndicatorScheme">
        <rdf:type rdf:resource="http://www.w3.org/2004/02/skos/core#ConceptScheme"/>
        <rdfs:isDefinedBy rdf:resource="https://w3id.org/gcdfo/salmon"/>
        <skos:definition xml:lang="en">Controlled vocabulary for key biological benchmarks, performance indicators, and reference points used in salmon stock assessment and management (e.g., SMSY, Sgen, spawner abundance).</skos:definition>
        <skos:hasTopConcept rdf:resource="https://w3id.org/gcdfo/salmon#TargetOrLimitRateOrAbundance"/>
        <skos:prefLabel xml:lang="en">Biological Benchmark and Indicator Scheme</skos:prefLabel>
        <theme rdf:resource="https://w3id.org/gcdfo/salmon#StockAssessmentTheme"/>
        <theme rdf:resource="https://w3id.org/gcdfo/salmon#WildSalmonPolicyTheme"/>
    </owl:NamedIndividual>
    


    <!-- https://w3id.org/gcdfo/salmon#BreachBypass -->

    <owl:NamedIndividual rdf:about="https://w3id.org/gcdfo/salmon#BreachBypass">
        <rdf:type rdf:resource="http://www.w3.org/2004/02/skos/core#Concept"/>
        <rdfs:comment xml:lang="en">Limits to Type 2 maximum</rdfs:comment>
        <rdfs:isDefinedBy rdf:resource="https://w3id.org/gcdfo/salmon"/>
        <skos:broader rdf:resource="https://w3id.org/gcdfo/salmon#DowngradeCriteria"/>
        <skos:definition xml:lang="en">Bypass or breach risks not monitored and verified negligible</skos:definition>
        <skos:inScheme rdf:resource="https://w3id.org/gcdfo/salmon#DowngradeCriteriaScheme"/>
        <skos:prefLabel xml:lang="en">Bypass/Breach Risk</skos:prefLabel>
        <theme rdf:resource="https://w3id.org/gcdfo/salmon#DataModelProvenanceTheme"/>
        <theme rdf:resource="https://w3id.org/gcdfo/salmon#StockAssessmentTheme"/>
    </owl:NamedIndividual>
    


    <!-- https://w3id.org/gcdfo/salmon#COSEWICStatusScheme -->

    <owl:NamedIndividual rdf:about="https://w3id.org/gcdfo/salmon#COSEWICStatusScheme">
        <rdf:type rdf:resource="http://www.w3.org/2004/02/skos/core#ConceptScheme"/>
        <rdfs:isDefinedBy rdf:resource="https://w3id.org/gcdfo/salmon"/>
        <skos:definition xml:lang="en">Controlled vocabulary for COSEWIC statuses</skos:definition>
        <skos:hasTopConcept rdf:resource="https://w3id.org/gcdfo/salmon#COSEWICStatusCategory"/>
        <skos:prefLabel xml:lang="en">COSEWIC Status Scheme</skos:prefLabel>
        <theme rdf:resource="https://w3id.org/gcdfo/salmon#PolicyGovernanceTheme"/>
        <theme rdf:resource="https://w3id.org/gcdfo/salmon#SpeciesAtRiskRecoveryTheme"/>
        <theme rdf:resource="https://w3id.org/gcdfo/salmon#StockAssessmentTheme"/>
    </owl:NamedIndividual>
    


    <!-- https://w3id.org/gcdfo/salmon#CalibratedTimeSeries -->

    <owl:NamedIndividual rdf:about="https://w3id.org/gcdfo/salmon#CalibratedTimeSeries">
        <rdf:type rdf:resource="http://www.w3.org/2004/02/skos/core#Concept"/>
        <rdfs:comment xml:lang="en">Document calibration source years, transferability, diagnostics. Type-2 when calibration robust and applicable; else Type-3.</rdfs:comment>
        <rdfs:isDefinedBy rdf:resource="https://w3id.org/gcdfo/salmon"/>
        <skos:broader rdf:resource="https://w3id.org/gcdfo/salmon#EstimateMethod"/>
        <skos:definition xml:lang="en">Regression/state-space model calibrated to a Type-1/2 series converts a lower-precision index to abundance.</skos:definition>
        <skos:inScheme rdf:resource="https://w3id.org/gcdfo/salmon#EstimateMethodScheme"/>
        <skos:prefLabel xml:lang="en">Calibrated Time Series</skos:prefLabel>
        <theme rdf:resource="https://w3id.org/gcdfo/salmon#MonitoringFieldWorkTheme"/>
        <theme rdf:resource="https://w3id.org/gcdfo/salmon#StockAssessmentTheme"/>
    </owl:NamedIndividual>
    


    <!-- https://w3id.org/gcdfo/salmon#CatchContext -->

    <owl:NamedIndividual rdf:about="https://w3id.org/gcdfo/salmon#CatchContext">
        <rdf:type rdf:resource="http://www.w3.org/2004/02/skos/core#Concept"/>
        <rdfs:isDefinedBy rdf:resource="https://w3id.org/gcdfo/salmon"/>
        <skos:broader rdf:resource="https://w3id.org/gcdfo/salmon#MeasurementContext"/>
        <skos:definition xml:lang="en">Measurement context indicating values refer to fishery catch.</skos:definition>
        <skos:inScheme rdf:resource="https://w3id.org/gcdfo/salmon#MeasurementContextScheme"/>
        <skos:prefLabel xml:lang="en">Catch context</skos:prefLabel>
        <theme rdf:resource="https://w3id.org/gcdfo/salmon#StockAssessmentTheme"/>
    </owl:NamedIndividual>
    


    <!-- https://w3id.org/gcdfo/salmon#Classification -->

    <owl:NamedIndividual rdf:about="https://w3id.org/gcdfo/salmon#Classification">
        <rdf:type rdf:resource="http://www.w3.org/2004/02/skos/core#Concept"/>
        <rdfs:comment xml:lang="en">Limits to Type 3 maximum</rdfs:comment>
        <rdfs:isDefinedBy rdf:resource="https://w3id.org/gcdfo/salmon"/>
        <skos:broader rdf:resource="https://w3id.org/gcdfo/salmon#DowngradeCriteria"/>
        <skos:definition xml:lang="en">Classification/attribution not documented</skos:definition>
        <skos:inScheme rdf:resource="https://w3id.org/gcdfo/salmon#DowngradeCriteriaScheme"/>
        <skos:prefLabel xml:lang="en">Classification</skos:prefLabel>
        <theme rdf:resource="https://w3id.org/gcdfo/salmon#DataModelProvenanceTheme"/>
        <theme rdf:resource="https://w3id.org/gcdfo/salmon#StockAssessmentTheme"/>
    </owl:NamedIndividual>
    


    <!-- https://w3id.org/gcdfo/salmon#ConfidenceCategory -->

    <owl:NamedIndividual rdf:about="https://w3id.org/gcdfo/salmon#ConfidenceCategory">
        <rdf:type rdf:resource="http://www.w3.org/2004/02/skos/core#Concept"/>
    </owl:NamedIndividual>
    


    <!-- https://w3id.org/gcdfo/salmon#CrossSectionCoverage -->

    <owl:NamedIndividual rdf:about="https://w3id.org/gcdfo/salmon#CrossSectionCoverage">
        <rdf:type rdf:resource="http://www.w3.org/2004/02/skos/core#Concept"/>
        <rdfs:comment xml:lang="en">Limits to Type 2 maximum</rdfs:comment>
        <rdfs:isDefinedBy rdf:resource="https://w3id.org/gcdfo/salmon"/>
        <skos:broader rdf:resource="https://w3id.org/gcdfo/salmon#DowngradeCriteria"/>
        <skos:definition xml:lang="en">Incomplete cross-section coverage</skos:definition>
        <skos:inScheme rdf:resource="https://w3id.org/gcdfo/salmon#DowngradeCriteriaScheme"/>
        <skos:prefLabel xml:lang="en">Cross-section Coverage</skos:prefLabel>
        <theme rdf:resource="https://w3id.org/gcdfo/salmon#DataModelProvenanceTheme"/>
        <theme rdf:resource="https://w3id.org/gcdfo/salmon#StockAssessmentTheme"/>
    </owl:NamedIndividual>
    


    <!-- https://w3id.org/gcdfo/salmon#DataModelProvenanceTheme -->

    <owl:NamedIndividual rdf:about="https://w3id.org/gcdfo/salmon#DataModelProvenanceTheme">
        <rdf:type rdf:resource="http://www.w3.org/2004/02/skos/core#Concept"/>
        <rdfs:isDefinedBy rdf:resource="https://w3id.org/gcdfo/salmon"/>
        <skos:definition xml:lang="en">Data models, analytical workflows, provenance, quality dimensions, and metadata supporting salmon science.</skos:definition>
        <skos:inScheme rdf:resource="https://w3id.org/gcdfo/salmon#ThemeScheme"/>
        <skos:prefLabel xml:lang="en">Data, Models, and Provenance</skos:prefLabel>
        <theme rdf:resource="https://w3id.org/gcdfo/salmon#DataModelProvenanceTheme"/>
    </owl:NamedIndividual>
    


    <!-- https://w3id.org/gcdfo/salmon#DataQualityRatingContext -->

    <owl:NamedIndividual rdf:about="https://w3id.org/gcdfo/salmon#DataQualityRatingContext">
        <rdf:type rdf:resource="http://www.w3.org/2004/02/skos/core#Concept"/>
        <rdfs:isDefinedBy rdf:resource="https://w3id.org/gcdfo/salmon"/>
        <skos:broader rdf:resource="https://w3id.org/gcdfo/salmon#MeasurementContext"/>
        <skos:definition xml:lang="en">Measurement context indicating categorical or ordinal quality ratings.</skos:definition>
        <skos:inScheme rdf:resource="https://w3id.org/gcdfo/salmon#MeasurementContextScheme"/>
        <skos:prefLabel xml:lang="en">Data quality rating context</skos:prefLabel>
        <theme rdf:resource="https://w3id.org/gcdfo/salmon#DataModelProvenanceTheme"/>
    </owl:NamedIndividual>
    


    <!-- https://w3id.org/gcdfo/salmon#Detectability -->

    <owl:NamedIndividual rdf:about="https://w3id.org/gcdfo/salmon#Detectability">
        <rdf:type rdf:resource="http://www.w3.org/2004/02/skos/core#Concept"/>
        <rdfs:comment xml:lang="en">Limits to Type 3 maximum</rdfs:comment>
        <rdfs:isDefinedBy rdf:resource="https://w3id.org/gcdfo/salmon"/>
        <skos:broader rdf:resource="https://w3id.org/gcdfo/salmon#DowngradeCriteria"/>
        <skos:definition xml:lang="en">Detectability factors not validated</skos:definition>
        <skos:inScheme rdf:resource="https://w3id.org/gcdfo/salmon#DowngradeCriteriaScheme"/>
        <skos:prefLabel xml:lang="en">Detectability</skos:prefLabel>
        <theme rdf:resource="https://w3id.org/gcdfo/salmon#DataModelProvenanceTheme"/>
        <theme rdf:resource="https://w3id.org/gcdfo/salmon#StockAssessmentTheme"/>
    </owl:NamedIndividual>
    


    <!-- https://w3id.org/gcdfo/salmon#DeviceConfiguration -->

    <owl:NamedIndividual rdf:about="https://w3id.org/gcdfo/salmon#DeviceConfiguration">
        <rdf:type rdf:resource="http://www.w3.org/2004/02/skos/core#Concept"/>
        <rdfs:comment xml:lang="en">Limits to Type 2 maximum</rdfs:comment>
        <rdfs:isDefinedBy rdf:resource="https://w3id.org/gcdfo/salmon"/>
        <skos:broader rdf:resource="https://w3id.org/gcdfo/salmon#DowngradeCriteria"/>
        <skos:definition xml:lang="en">Device not within operational specifications</skos:definition>
        <skos:inScheme rdf:resource="https://w3id.org/gcdfo/salmon#DowngradeCriteriaScheme"/>
        <skos:prefLabel xml:lang="en">Device Configuration</skos:prefLabel>
        <theme rdf:resource="https://w3id.org/gcdfo/salmon#DataModelProvenanceTheme"/>
        <theme rdf:resource="https://w3id.org/gcdfo/salmon#StockAssessmentTheme"/>
    </owl:NamedIndividual>
    


    <!-- https://w3id.org/gcdfo/salmon#Documentation -->

    <owl:NamedIndividual rdf:about="https://w3id.org/gcdfo/salmon#Documentation">
        <rdf:type rdf:resource="http://www.w3.org/2004/02/skos/core#Concept"/>
        <rdfs:comment xml:lang="en">Downgrades Type 1/2 by one level</rdfs:comment>
        <rdfs:isDefinedBy rdf:resource="https://w3id.org/gcdfo/salmon"/>
        <skos:broader rdf:resource="https://w3id.org/gcdfo/salmon#DowngradeCriteria"/>
        <skos:definition xml:lang="en">Missing SIL/SEN logs or QA/methods report</skos:definition>
        <skos:inScheme rdf:resource="https://w3id.org/gcdfo/salmon#DowngradeCriteriaScheme"/>
        <skos:prefLabel xml:lang="en">Documentation</skos:prefLabel>
        <theme rdf:resource="https://w3id.org/gcdfo/salmon#DataModelProvenanceTheme"/>
        <theme rdf:resource="https://w3id.org/gcdfo/salmon#StockAssessmentTheme"/>
    </owl:NamedIndividual>
    


    <!-- https://w3id.org/gcdfo/salmon#DowngradeCriteria -->

    <owl:NamedIndividual rdf:about="https://w3id.org/gcdfo/salmon#DowngradeCriteria">
        <rdf:type rdf:resource="http://www.w3.org/2004/02/skos/core#Concept"/>
        <rdfs:isDefinedBy rdf:resource="https://w3id.org/gcdfo/salmon"/>
        <skos:definition xml:lang="en">Criteria that may result in downgrading an escapement estimate type classification</skos:definition>
        <skos:inScheme rdf:resource="https://w3id.org/gcdfo/salmon#DowngradeCriteriaScheme"/>
        <skos:prefLabel xml:lang="en">Downgrade Criteria</skos:prefLabel>
        <theme rdf:resource="https://w3id.org/gcdfo/salmon#DataModelProvenanceTheme"/>
        <theme rdf:resource="https://w3id.org/gcdfo/salmon#StockAssessmentTheme"/>
    </owl:NamedIndividual>
    


    <!-- https://w3id.org/gcdfo/salmon#DowngradeCriteriaScheme -->

    <owl:NamedIndividual rdf:about="https://w3id.org/gcdfo/salmon#DowngradeCriteriaScheme">
        <rdf:type rdf:resource="http://www.w3.org/2004/02/skos/core#ConceptScheme"/>
        <rdfs:isDefinedBy rdf:resource="https://w3id.org/gcdfo/salmon"/>
        <skos:definition xml:lang="en">Controlled vocabulary for estimate type downgrade criteria</skos:definition>
        <skos:hasTopConcept rdf:resource="https://w3id.org/gcdfo/salmon#DowngradeCriteria"/>
        <skos:prefLabel xml:lang="en">Downgrade Criteria Scheme</skos:prefLabel>
        <theme rdf:resource="https://w3id.org/gcdfo/salmon#StockAssessmentTheme"/>
    </owl:NamedIndividual>
    


    <!-- https://w3id.org/gcdfo/salmon#EffortStandardization -->

    <owl:NamedIndividual rdf:about="https://w3id.org/gcdfo/salmon#EffortStandardization">
        <rdf:type rdf:resource="http://www.w3.org/2004/02/skos/core#Concept"/>
        <rdfs:comment xml:lang="en">Limits to Type 4 maximum</rdfs:comment>
        <rdfs:isDefinedBy rdf:resource="https://w3id.org/gcdfo/salmon"/>
        <skos:broader rdf:resource="https://w3id.org/gcdfo/salmon#DowngradeCriteria"/>
        <skos:definition xml:lang="en">Effort not standardized</skos:definition>
        <skos:inScheme rdf:resource="https://w3id.org/gcdfo/salmon#DowngradeCriteriaScheme"/>
        <skos:prefLabel xml:lang="en">Effort Standardization</skos:prefLabel>
        <theme rdf:resource="https://w3id.org/gcdfo/salmon#DataModelProvenanceTheme"/>
        <theme rdf:resource="https://w3id.org/gcdfo/salmon#StockAssessmentTheme"/>
    </owl:NamedIndividual>
    


    <!-- https://w3id.org/gcdfo/salmon#ElectrofishingCount -->

    <owl:NamedIndividual rdf:about="https://w3id.org/gcdfo/salmon#ElectrofishingCount">
        <rdf:type rdf:resource="http://www.w3.org/2004/02/skos/core#Concept"/>
        <rdfs:comment xml:lang="en">Legacy methods: Electrofishing, Electroshocking</rdfs:comment>
        <rdfs:isDefinedBy rdf:resource="https://w3id.org/gcdfo/salmon"/>
        <skos:broader rdf:resource="https://w3id.org/gcdfo/salmon#EnumerationMethod"/>
        <skos:definition xml:lang="en">Effort-standardized electrofishing passes used to generate catch-per-unit-effort (CPUE) indices.</skos:definition>
        <skos:inScheme rdf:resource="https://w3id.org/gcdfo/salmon#EnumerationMethodScheme"/>
        <skos:prefLabel xml:lang="en">Electrofishing Count</skos:prefLabel>
        <theme rdf:resource="https://w3id.org/gcdfo/salmon#MonitoringFieldWorkTheme"/>
        <theme rdf:resource="https://w3id.org/gcdfo/salmon#StockAssessmentTheme"/>
    </owl:NamedIndividual>
    


    <!-- https://w3id.org/gcdfo/salmon#EnumerationMethod -->

    <owl:NamedIndividual rdf:about="https://w3id.org/gcdfo/salmon#EnumerationMethod">
        <rdf:type rdf:resource="http://www.w3.org/2004/02/skos/core#Concept"/>
        <rdfs:isDefinedBy rdf:resource="https://w3id.org/gcdfo/salmon"/>
        <skos:definition xml:lang="en">A method used to enumerate or count salmon in the field</skos:definition>
        <skos:inScheme rdf:resource="https://w3id.org/gcdfo/salmon#EnumerationMethodScheme"/>
        <skos:prefLabel xml:lang="en">Enumeration Method</skos:prefLabel>
        <theme rdf:resource="https://w3id.org/gcdfo/salmon#MonitoringFieldWorkTheme"/>
        <theme rdf:resource="https://w3id.org/gcdfo/salmon#StockAssessmentTheme"/>
    </owl:NamedIndividual>
    


    <!-- https://w3id.org/gcdfo/salmon#EnumerationMethodScheme -->

    <owl:NamedIndividual rdf:about="https://w3id.org/gcdfo/salmon#EnumerationMethodScheme">
        <rdf:type rdf:resource="http://www.w3.org/2004/02/skos/core#ConceptScheme"/>
        <rdfs:isDefinedBy rdf:resource="https://w3id.org/gcdfo/salmon"/>
        <skos:definition xml:lang="en">Controlled vocabulary for salmon enumeration methods</skos:definition>
        <skos:hasTopConcept rdf:resource="https://w3id.org/gcdfo/salmon#EnumerationMethod"/>
        <skos:prefLabel xml:lang="en">Escapement Enumeration Method Scheme</skos:prefLabel>
        <theme rdf:resource="https://w3id.org/gcdfo/salmon#StockAssessmentTheme"/>
    </owl:NamedIndividual>
    


    <!-- https://w3id.org/gcdfo/salmon#EnvironmentalConditions -->

    <owl:NamedIndividual rdf:about="https://w3id.org/gcdfo/salmon#EnvironmentalConditions">
        <rdf:type rdf:resource="http://www.w3.org/2004/02/skos/core#Concept"/>
        <rdfs:comment xml:lang="en">Limits to Type 2 maximum</rdfs:comment>
        <rdfs:isDefinedBy rdf:resource="https://w3id.org/gcdfo/salmon"/>
        <skos:broader rdf:resource="https://w3id.org/gcdfo/salmon#DowngradeCriteria"/>
        <skos:definition xml:lang="en">Environmental conditions outside specifications</skos:definition>
        <skos:inScheme rdf:resource="https://w3id.org/gcdfo/salmon#DowngradeCriteriaScheme"/>
        <skos:prefLabel xml:lang="en">Environmental Conditions</skos:prefLabel>
        <theme rdf:resource="https://w3id.org/gcdfo/salmon#DataModelProvenanceTheme"/>
        <theme rdf:resource="https://w3id.org/gcdfo/salmon#StockAssessmentTheme"/>
    </owl:NamedIndividual>
    


    <!-- https://w3id.org/gcdfo/salmon#EstimateMethod -->

    <owl:NamedIndividual rdf:about="https://w3id.org/gcdfo/salmon#EstimateMethod">
        <rdf:type rdf:resource="http://www.w3.org/2004/02/skos/core#Concept"/>
        <rdfs:isDefinedBy rdf:resource="https://w3id.org/gcdfo/salmon"/>
        <skos:definition xml:lang="en">A method used to analyze and estimate salmon abundance from enumeration data</skos:definition>
        <skos:inScheme rdf:resource="https://w3id.org/gcdfo/salmon#EstimateMethodScheme"/>
        <skos:prefLabel xml:lang="en">Estimate Method</skos:prefLabel>
        <theme rdf:resource="https://w3id.org/gcdfo/salmon#MonitoringFieldWorkTheme"/>
        <theme rdf:resource="https://w3id.org/gcdfo/salmon#StockAssessmentTheme"/>
    </owl:NamedIndividual>
    


    <!-- https://w3id.org/gcdfo/salmon#EstimateMethodScheme -->

    <owl:NamedIndividual rdf:about="https://w3id.org/gcdfo/salmon#EstimateMethodScheme">
        <rdf:type rdf:resource="http://www.w3.org/2004/02/skos/core#ConceptScheme"/>
        <rdfs:isDefinedBy rdf:resource="https://w3id.org/gcdfo/salmon"/>
        <skos:definition xml:lang="en">Controlled vocabulary for salmon estimate methods</skos:definition>
        <skos:hasTopConcept rdf:resource="https://w3id.org/gcdfo/salmon#EstimateMethod"/>
        <skos:prefLabel xml:lang="en">Escapement Estimate Method Scheme</skos:prefLabel>
        <theme rdf:resource="https://w3id.org/gcdfo/salmon#StockAssessmentTheme"/>
    </owl:NamedIndividual>
    


    <!-- https://w3id.org/gcdfo/salmon#EstimateType -->

    <owl:NamedIndividual rdf:about="https://w3id.org/gcdfo/salmon#EstimateType">
        <rdf:type rdf:resource="http://www.w3.org/2004/02/skos/core#Concept"/>
        <rdfs:isDefinedBy rdf:resource="https://w3id.org/gcdfo/salmon"/>
        <skos:definition xml:lang="en">Classification of escapement estimate quality based on Hyatt 1997 framework</skos:definition>
        <skos:inScheme rdf:resource="https://w3id.org/gcdfo/salmon#EstimateTypeScheme"/>
        <skos:prefLabel xml:lang="en">Estimate Type</skos:prefLabel>
        <theme rdf:resource="https://w3id.org/gcdfo/salmon#DataModelProvenanceTheme"/>
        <theme rdf:resource="https://w3id.org/gcdfo/salmon#StockAssessmentTheme"/>
    </owl:NamedIndividual>
    


    <!-- https://w3id.org/gcdfo/salmon#EstimateTypeScheme -->

    <owl:NamedIndividual rdf:about="https://w3id.org/gcdfo/salmon#EstimateTypeScheme">
        <rdf:type rdf:resource="http://www.w3.org/2004/02/skos/core#ConceptScheme"/>
        <rdfs:isDefinedBy rdf:resource="https://w3id.org/gcdfo/salmon"/>
        <skos:definition xml:lang="en">Controlled vocabulary for Hyatt 1997 estimate types</skos:definition>
        <skos:hasTopConcept rdf:resource="https://w3id.org/gcdfo/salmon#EstimateType"/>
        <skos:prefLabel xml:lang="en">Escapement Estimate Type Scheme</skos:prefLabel>
        <theme rdf:resource="https://w3id.org/gcdfo/salmon#StockAssessmentTheme"/>
    </owl:NamedIndividual>
    


    <!-- https://w3id.org/gcdfo/salmon#EuropeanAgeNotation -->

    <owl:NamedIndividual rdf:about="https://w3id.org/gcdfo/salmon#EuropeanAgeNotation">
        <rdf:type rdf:resource="http://www.w3.org/2004/02/skos/core#Concept"/>
        <dcterms:source rdf:resource="https://www.pac.dfo-mpo.gc.ca/fm-gp/fraser/docs/archiv-reports-rapports/indigenous-autochtone/2010FrasRvrChkInformDoc.htm"/>
        <rdfs:isDefinedBy rdf:resource="https://w3id.org/gcdfo/salmon"/>
        <skos:broader rdf:resource="https://w3id.org/gcdfo/salmon#AgeNotation"/>
        <skos:definition xml:lang="en">Salmon age notation that records freshwater years followed by ocean years (for example, 1.2).</skos:definition>
        <skos:inScheme rdf:resource="https://w3id.org/gcdfo/salmon#AgeNotationScheme"/>
        <skos:notation>European</skos:notation>
        <skos:prefLabel xml:lang="en">European age notation</skos:prefLabel>
        <theme rdf:resource="https://w3id.org/gcdfo/salmon#DataModelProvenanceTheme"/>
        <theme rdf:resource="https://w3id.org/gcdfo/salmon#StockAssessmentTheme"/>
    </owl:NamedIndividual>
    


    <!-- https://w3id.org/gcdfo/salmon#ExpansionFactor -->

    <owl:NamedIndividual rdf:about="https://w3id.org/gcdfo/salmon#ExpansionFactor">
        <rdf:type rdf:resource="http://www.w3.org/2004/02/skos/core#Concept"/>
        <obo:IAO_0000115 xml:lang="en">A multiplicative factor used to expand observed counts or detections from a sampled subset (e.g., indicator sites, PIT detections) to an estimated total abundance or escapement.</obo:IAO_0000115>
        <obo:IAO_0000119 xml:lang="en">Fisheries and Oceans Canada. 2021. Marine Survival Forecast of Southern British Columbia Coho (describes applying expansion factors to PIT detections to estimate total escapement).</obo:IAO_0000119>
        <dcterms:source rdf:resource="https://waves-vagues.dfo-mpo.gc.ca/Library/40978680.pdf"/>
        <rdfs:isDefinedBy rdf:resource="https://w3id.org/gcdfo/salmon"/>
        <skos:broader rdf:resource="https://w3id.org/gcdfo/salmon#ExpansionMathematicalOperations"/>
        <skos:definition xml:lang="en">A multiplicative factor used to expand observed counts or detections from a sampled subset (e.g., indicator sites, PIT detections) to an estimated total abundance or escapement.</skos:definition>
        <skos:inScheme rdf:resource="https://w3id.org/gcdfo/salmon#EstimateMethodScheme"/>
        <skos:prefLabel xml:lang="en">Expansion factor</skos:prefLabel>
        <theme rdf:resource="https://w3id.org/gcdfo/salmon#DataModelProvenanceTheme"/>
        <theme rdf:resource="https://w3id.org/gcdfo/salmon#StockAssessmentTheme"/>
    </owl:NamedIndividual>
    


    <!-- https://w3id.org/gcdfo/salmon#ExpansionMathematicalOperations -->

    <owl:NamedIndividual rdf:about="https://w3id.org/gcdfo/salmon#ExpansionMathematicalOperations">
        <rdf:type rdf:resource="http://www.w3.org/2004/02/skos/core#Concept"/>
        <rdfs:comment xml:lang="en">Legacy methods: Lake Expansion, Redd Expansion, Peak×Factor, (Peak+CumDead)×Factor, Addition/Subtraction, Multiplication/Division. Inherits base method&apos;s Type; weak provenance = downgrade one Type.</rdfs:comment>
        <rdfs:isDefinedBy rdf:resource="https://w3id.org/gcdfo/salmon"/>
        <skos:broader rdf:resource="https://w3id.org/gcdfo/salmon#EstimateMethod"/>
        <skos:definition xml:lang="en">Applies expansion factors or arithmetic transforms to a base count/index.</skos:definition>
        <skos:inScheme rdf:resource="https://w3id.org/gcdfo/salmon#EstimateMethodScheme"/>
        <skos:prefLabel xml:lang="en">Expansion/Mathematical Operations</skos:prefLabel>
        <theme rdf:resource="https://w3id.org/gcdfo/salmon#MonitoringFieldWorkTheme"/>
        <theme rdf:resource="https://w3id.org/gcdfo/salmon#StockAssessmentTheme"/>
    </owl:NamedIndividual>
    


    <!-- https://w3id.org/gcdfo/salmon#FishStockProvisions -->

    <owl:NamedIndividual rdf:about="https://w3id.org/gcdfo/salmon#FishStockProvisions">
        <rdf:type rdf:resource="http://www.w3.org/2004/02/skos/core#Concept"/>
        <rdfs:isDefinedBy rdf:resource="https://w3id.org/gcdfo/salmon"/>
        <skos:altLabel xml:lang="en">FSP</skos:altLabel>
        <skos:broader rdf:resource="https://w3id.org/gcdfo/salmon#PolicyFramework"/>
        <skos:definition xml:lang="en">Legal provisions in Canada&apos;s Fisheries Act and regulations related to maintaining and rebuilding fish stocks, including obligations triggered when reference points are breached.</skos:definition>
        <skos:inScheme rdf:resource="https://w3id.org/gcdfo/salmon#PolicyFrameworkScheme"/>
        <skos:prefLabel xml:lang="en">Fish Stocks Provisions</skos:prefLabel>
        <theme rdf:resource="https://w3id.org/gcdfo/salmon#FisheriesManagementTheme"/>
        <theme rdf:resource="https://w3id.org/gcdfo/salmon#PolicyGovernanceTheme"/>
        <theme rdf:resource="https://w3id.org/gcdfo/salmon#StockAssessmentTheme"/>
    </owl:NamedIndividual>
    


    <!-- https://w3id.org/gcdfo/salmon#FisheriesManagementTheme -->

    <owl:NamedIndividual rdf:about="https://w3id.org/gcdfo/salmon#FisheriesManagementTheme">
        <rdf:type rdf:resource="http://www.w3.org/2004/02/skos/core#Concept"/>
        <rdfs:isDefinedBy rdf:resource="https://w3id.org/gcdfo/salmon"/>
        <skos:definition xml:lang="en">Fishery openings, harvest control rules, catch/effort measures, and exploitation monitoring for salmon fisheries.</skos:definition>
        <skos:inScheme rdf:resource="https://w3id.org/gcdfo/salmon#ThemeScheme"/>
        <skos:prefLabel xml:lang="en">Fisheries Management</skos:prefLabel>
        <theme rdf:resource="https://w3id.org/gcdfo/salmon#DataModelProvenanceTheme"/>
    </owl:NamedIndividual>
    


    <!-- https://w3id.org/gcdfo/salmon#FixedSiteCensusElectronic -->

    <owl:NamedIndividual rdf:about="https://w3id.org/gcdfo/salmon#FixedSiteCensusElectronic">
        <rdf:type rdf:resource="http://www.w3.org/2004/02/skos/core#Concept"/>
        <rdfs:comment xml:lang="en">Legacy methods: Electronic/Optical counter, Resistivity Counter, Video/Camera counter</rdfs:comment>
        <rdfs:isDefinedBy rdf:resource="https://w3id.org/gcdfo/salmon"/>
        <skos:broader rdf:resource="https://w3id.org/gcdfo/salmon#EnumerationMethod"/>
        <skos:definition xml:lang="en">Automated counting at a constrained opening using electronic/optical counters, resistivity counters, or video/camera systems. QA review of automated events, cross-section coverage, and uptime/coverage are documented.</skos:definition>
        <skos:inScheme rdf:resource="https://w3id.org/gcdfo/salmon#EnumerationMethodScheme"/>
        <skos:prefLabel xml:lang="en">Fixed Site Census (Electronic)</skos:prefLabel>
        <theme rdf:resource="https://w3id.org/gcdfo/salmon#MonitoringFieldWorkTheme"/>
        <theme rdf:resource="https://w3id.org/gcdfo/salmon#StockAssessmentTheme"/>
    </owl:NamedIndividual>
    


    <!-- https://w3id.org/gcdfo/salmon#FixedSiteCensusManual -->

    <owl:NamedIndividual rdf:about="https://w3id.org/gcdfo/salmon#FixedSiteCensusManual">
        <rdf:type rdf:resource="http://www.w3.org/2004/02/skos/core#Concept"/>
        <rdfs:comment xml:lang="en">Legacy methods: Fence, Weir, Fixed Site Census (manual)</rdfs:comment>
        <rdfs:isDefinedBy rdf:resource="https://w3id.org/gcdfo/salmon"/>
        <skos:broader rdf:resource="https://w3id.org/gcdfo/salmon#EnumerationMethod"/>
        <skos:definition xml:lang="en">Salmon are guided through a controlled opening in a fence/weir where trained observers visually tally each passage event on a continuous or daily schedule. Counting chambers/windows and SIL/SEN daily logs document coverage; bypass routes are monitored and closed where possible.</skos:definition>
        <skos:inScheme rdf:resource="https://w3id.org/gcdfo/salmon#EnumerationMethodScheme"/>
        <skos:prefLabel xml:lang="en">Fixed Site Census (Manual)</skos:prefLabel>
        <theme rdf:resource="https://w3id.org/gcdfo/salmon#MonitoringFieldWorkTheme"/>
        <theme rdf:resource="https://w3id.org/gcdfo/salmon#StockAssessmentTheme"/>
    </owl:NamedIndividual>
    


    <!-- https://w3id.org/gcdfo/salmon#FixedStationTally -->

    <owl:NamedIndividual rdf:about="https://w3id.org/gcdfo/salmon#FixedStationTally">
        <rdf:type rdf:resource="http://www.w3.org/2004/02/skos/core#Concept"/>
        <rdfs:isDefinedBy rdf:resource="https://w3id.org/gcdfo/salmon"/>
        <skos:broader rdf:resource="https://w3id.org/gcdfo/salmon#EstimateMethod"/>
        <skos:definition xml:lang="en">Seasonal total = roll‑up of daily/continuous counts from a fixed (non‑sonar) station; simple arithmetic with documented coverage.</skos:definition>
        <skos:inScheme rdf:resource="https://w3id.org/gcdfo/salmon#EstimateMethodScheme"/>
        <skos:prefLabel xml:lang="en">Fixed‑Station Tally</skos:prefLabel>
        <theme rdf:resource="https://w3id.org/gcdfo/salmon#MonitoringFieldWorkTheme"/>
        <theme rdf:resource="https://w3id.org/gcdfo/salmon#StockAssessmentTheme"/>
    </owl:NamedIndividual>
    


    <!-- https://w3id.org/gcdfo/salmon#FreshwaterAgeDimension -->

    <owl:NamedIndividual rdf:about="https://w3id.org/gcdfo/salmon#FreshwaterAgeDimension">
        <rdf:type rdf:resource="http://www.w3.org/2004/02/skos/core#Concept"/>
        <rdfs:isDefinedBy rdf:resource="https://w3id.org/gcdfo/salmon"/>
        <skos:broader rdf:resource="https://w3id.org/gcdfo/salmon#AgeDimension"/>
        <skos:definition xml:lang="en">Age value represents years spent in freshwater.</skos:definition>
        <skos:inScheme rdf:resource="https://w3id.org/gcdfo/salmon#AgeDimensionScheme"/>
        <skos:prefLabel xml:lang="en">Freshwater age dimension</skos:prefLabel>
        <theme rdf:resource="https://w3id.org/gcdfo/salmon#StockAssessmentTheme"/>
    </owl:NamedIndividual>
    


    <!-- https://w3id.org/gcdfo/salmon#GeneticsStockCompositionTheme -->

    <owl:NamedIndividual rdf:about="https://w3id.org/gcdfo/salmon#GeneticsStockCompositionTheme">
        <rdf:type rdf:resource="http://www.w3.org/2004/02/skos/core#Concept"/>
        <rdfs:isDefinedBy rdf:resource="https://w3id.org/gcdfo/salmon"/>
        <skos:definition xml:lang="en">Genetic markers, assays, and analyses used to infer stock composition, parentage, and population structure.</skos:definition>
        <skos:inScheme rdf:resource="https://w3id.org/gcdfo/salmon#ThemeScheme"/>
        <skos:prefLabel xml:lang="en">Genetics and Stock Composition</skos:prefLabel>
        <theme rdf:resource="https://w3id.org/gcdfo/salmon#DataModelProvenanceTheme"/>
    </owl:NamedIndividual>
    


    <!-- https://w3id.org/gcdfo/salmon#GilbertRichAgeNotation -->

    <owl:NamedIndividual rdf:about="https://w3id.org/gcdfo/salmon#GilbertRichAgeNotation">
        <rdf:type rdf:resource="http://www.w3.org/2004/02/skos/core#Concept"/>
        <dcterms:source rdf:resource="https://www.pac.dfo-mpo.gc.ca/fm-gp/fraser/docs/archiv-reports-rapports/indigenous-autochtone/2010FrasRvrChkInformDoc.htm"/>
        <rdfs:isDefinedBy rdf:resource="https://w3id.org/gcdfo/salmon"/>
        <skos:altLabel xml:lang="en">GR age notation</skos:altLabel>
        <skos:broader rdf:resource="https://w3id.org/gcdfo/salmon#AgeNotation"/>
        <skos:definition xml:lang="en">Salmon age notation where total age is annotated with freshwater years as a subscript-like suffix (for example, 4_2 for total age 4 with 2 freshwater years).</skos:definition>
        <skos:inScheme rdf:resource="https://w3id.org/gcdfo/salmon#AgeNotationScheme"/>
        <skos:notation>Gilbert-Rich</skos:notation>
        <skos:prefLabel xml:lang="en">Gilbert-Rich age notation</skos:prefLabel>
        <theme rdf:resource="https://w3id.org/gcdfo/salmon#DataModelProvenanceTheme"/>
        <theme rdf:resource="https://w3id.org/gcdfo/salmon#StockAssessmentTheme"/>
    </owl:NamedIndividual>
    


    <!-- https://w3id.org/gcdfo/salmon#GreenZone -->

    <owl:NamedIndividual rdf:about="https://w3id.org/gcdfo/salmon#GreenZone">
        <rdf:type rdf:resource="http://www.w3.org/2004/02/skos/core#Concept"/>
        <rdf:type rdf:resource="https://w3id.org/gcdfo/salmon#WSPBiologicalStatusZone"/>
        <obo:IAO_0000119 xml:lang="en">Fisheries and Oceans Canada. Wild Salmon Policy 2018-2022 Implementation Plan. https://waves-vagues.dfo-mpo.gc.ca/library-bibliotheque/40728109.pdf.</obo:IAO_0000119>
        <dcterms:source rdf:resource="https://waves-vagues.dfo-mpo.gc.ca/library-bibliotheque/40728109.pdf"/>
        <rdfs:isDefinedBy rdf:resource="https://w3id.org/gcdfo/salmon"/>
        <skos:definition xml:lang="en">Social and economic considerations will tend to be the primary drivers for the management of Conservation Units in the Green zone, though ecosystem or other non-consumptive use values could also be considered.</skos:definition>
        <skos:inScheme rdf:resource="https://w3id.org/gcdfo/salmon#WSPBiologicalStatusZoneScheme"/>
        <skos:prefLabel xml:lang="en">Green zone</skos:prefLabel>
        <theme rdf:resource="https://w3id.org/gcdfo/salmon#PolicyGovernanceTheme"/>
        <theme rdf:resource="https://w3id.org/gcdfo/salmon#WildSalmonPolicyTheme"/>
    </owl:NamedIndividual>
    


    <!-- https://w3id.org/gcdfo/salmon#HabitatEcosystemClimateTheme -->

    <owl:NamedIndividual rdf:about="https://w3id.org/gcdfo/salmon#HabitatEcosystemClimateTheme">
        <rdf:type rdf:resource="http://www.w3.org/2004/02/skos/core#Concept"/>
        <rdfs:isDefinedBy rdf:resource="https://w3id.org/gcdfo/salmon"/>
        <skos:definition xml:lang="en">Habitat attributes, ecosystem conditions, and climate or environmental stressors affecting salmon.</skos:definition>
        <skos:inScheme rdf:resource="https://w3id.org/gcdfo/salmon#ThemeScheme"/>
        <skos:prefLabel xml:lang="en">Habitat, Ecosystem, and Climate Pressures</skos:prefLabel>
        <theme rdf:resource="https://w3id.org/gcdfo/salmon#DataModelProvenanceTheme"/>
    </owl:NamedIndividual>
    


    <!-- https://w3id.org/gcdfo/salmon#HatcheryOrigin -->

    <owl:NamedIndividual rdf:about="https://w3id.org/gcdfo/salmon#HatcheryOrigin">
        <rdf:type rdf:resource="http://www.w3.org/2004/02/skos/core#Concept"/>
        <obo:IAO_0000119 xml:lang="en">Fisheries and Oceans Canada. 2018. Review of genetically based targets for enhanced contributions to Canadian Pacific Chinook Salmon populations. DFO Canadian Science Advisory Secretariat Science Advisory Report 2018/001 (Erratum: October 2023).</obo:IAO_0000119>
        <dcterms:source rdf:resource="https://www.dfo-mpo.gc.ca/csas-sccs/Publications/SAR-AS/2018/2018_001-eng.html"/>
        <rdfs:isDefinedBy rdf:resource="https://w3id.org/gcdfo/salmon"/>
        <skos:broader rdf:resource="https://w3id.org/gcdfo/salmon#SalmonOrigin"/>
        <skos:definition xml:lang="en">Individuals that were born or reared in a hatchery facility.</skos:definition>
        <skos:inScheme rdf:resource="https://w3id.org/gcdfo/salmon#SalmonOriginScheme"/>
        <skos:prefLabel xml:lang="en">Hatchery-origin</skos:prefLabel>
        <theme rdf:resource="https://w3id.org/gcdfo/salmon#GeneticsStockCompositionTheme"/>
        <theme rdf:resource="https://w3id.org/gcdfo/salmon#SalmonEnhancementHatcheriesTheme"/>
        <theme rdf:resource="https://w3id.org/gcdfo/salmon#StockAssessmentTheme"/>
    </owl:NamedIndividual>
    


    <!-- https://w3id.org/gcdfo/salmon#HydroacousticModelling -->

    <owl:NamedIndividual rdf:about="https://w3id.org/gcdfo/salmon#HydroacousticModelling">
        <rdf:type rdf:resource="http://www.w3.org/2004/02/skos/core#Concept"/>
        <rdfs:comment xml:lang="en">Legacy methods: Hydroacoustics, Sonar (ARIS/DIDSON). Not Type-1 under Hyatt; interpolation and classification error are central downgrades.</rdfs:comment>
        <rdfs:isDefinedBy rdf:resource="https://w3id.org/gcdfo/salmon"/>
        <skos:broader rdf:resource="https://w3id.org/gcdfo/salmon#EstimateMethod"/>
        <skos:definition xml:lang="en">Model pipeline converts sonar detections to passage totals; sets range/angle/blind zones; species/size attribution rules documented.</skos:definition>
        <skos:inScheme rdf:resource="https://w3id.org/gcdfo/salmon#EstimateMethodScheme"/>
        <skos:prefLabel xml:lang="en">Hydroacoustic Modelling</skos:prefLabel>
        <theme rdf:resource="https://w3id.org/gcdfo/salmon#MonitoringFieldWorkTheme"/>
        <theme rdf:resource="https://w3id.org/gcdfo/salmon#StockAssessmentTheme"/>
    </owl:NamedIndividual>
    


    <!-- https://w3id.org/gcdfo/salmon#HydroacousticSonarCount -->

    <owl:NamedIndividual rdf:about="https://w3id.org/gcdfo/salmon#HydroacousticSonarCount">
        <rdf:type rdf:resource="http://www.w3.org/2004/02/skos/core#Concept"/>
        <rdfs:comment xml:lang="en">Legacy methods: Sonar-ARIS, Sonar-DIDSON, Hydroacoustic</rdfs:comment>
        <rdfs:isDefinedBy rdf:resource="https://w3id.org/gcdfo/salmon"/>
        <skos:broader rdf:resource="https://w3id.org/gcdfo/salmon#EnumerationMethod"/>
        <skos:definition xml:lang="en">Sonar detections (ARIS, DIDSON, or other hydroacoustic systems) with documented coverage, visibility/noise conditions, and uptime. Raw detections require processing through a modelling/classification pipeline.</skos:definition>
        <skos:inScheme rdf:resource="https://w3id.org/gcdfo/salmon#EnumerationMethodScheme"/>
        <skos:prefLabel xml:lang="en">Hydroacoustic Sonar Count</skos:prefLabel>
        <theme rdf:resource="https://w3id.org/gcdfo/salmon#MonitoringFieldWorkTheme"/>
        <theme rdf:resource="https://w3id.org/gcdfo/salmon#StockAssessmentTheme"/>
    </owl:NamedIndividual>
    


    <!-- https://w3id.org/gcdfo/salmon#InRiverPhase -->

    <owl:NamedIndividual rdf:about="https://w3id.org/gcdfo/salmon#InRiverPhase">
        <rdf:type rdf:resource="http://www.w3.org/2004/02/skos/core#Concept"/>
        <rdfs:isDefinedBy rdf:resource="https://w3id.org/gcdfo/salmon"/>
        <skos:altLabel xml:lang="en">Freshwater phase</skos:altLabel>
        <skos:broader rdf:resource="https://w3id.org/gcdfo/salmon#LifePhase"/>
        <skos:definition xml:lang="en">Freshwater in-river phase (migration and/or residence) outside the marine environment.</skos:definition>
        <skos:inScheme rdf:resource="https://w3id.org/gcdfo/salmon#LifePhaseScheme"/>
        <skos:prefLabel xml:lang="en">In-river phase</skos:prefLabel>
        <theme rdf:resource="https://w3id.org/gcdfo/salmon#StockAssessmentTheme"/>
    </owl:NamedIndividual>
    


    <!-- https://w3id.org/gcdfo/salmon#InfillMethod -->

    <owl:NamedIndividual rdf:about="https://w3id.org/gcdfo/salmon#InfillMethod">
        <rdf:type rdf:resource="http://www.w3.org/2004/02/skos/core#Concept"/>
        <rdfs:comment xml:lang="en">Limits to Type 2 maximum</rdfs:comment>
        <rdfs:isDefinedBy rdf:resource="https://w3id.org/gcdfo/salmon"/>
        <skos:broader rdf:resource="https://w3id.org/gcdfo/salmon#DowngradeCriteria"/>
        <skos:definition xml:lang="en">Interpolation used for missing data; defensibility must be documented</skos:definition>
        <skos:inScheme rdf:resource="https://w3id.org/gcdfo/salmon#DowngradeCriteriaScheme"/>
        <skos:prefLabel xml:lang="en">Infill Method</skos:prefLabel>
        <theme rdf:resource="https://w3id.org/gcdfo/salmon#DataModelProvenanceTheme"/>
        <theme rdf:resource="https://w3id.org/gcdfo/salmon#StockAssessmentTheme"/>
    </owl:NamedIndividual>
    


    <!-- https://w3id.org/gcdfo/salmon#LifePhase -->

    <owl:NamedIndividual rdf:about="https://w3id.org/gcdfo/salmon#LifePhase">
        <rdf:type rdf:resource="http://www.w3.org/2004/02/skos/core#Concept"/>
        <rdfs:isDefinedBy rdf:resource="https://w3id.org/gcdfo/salmon"/>
        <skos:definition xml:lang="en">A phase or segment used to stratify salmon measurements by where or when they apply (e.g., ocean phase, terminal phase).</skos:definition>
        <skos:inScheme rdf:resource="https://w3id.org/gcdfo/salmon#LifePhaseScheme"/>
        <skos:prefLabel xml:lang="en">Life phase</skos:prefLabel>
        <theme rdf:resource="https://w3id.org/gcdfo/salmon#StockAssessmentTheme"/>
    </owl:NamedIndividual>
    


    <!-- https://w3id.org/gcdfo/salmon#LifePhaseScheme -->

    <owl:NamedIndividual rdf:about="https://w3id.org/gcdfo/salmon#LifePhaseScheme">
        <rdf:type rdf:resource="http://www.w3.org/2004/02/skos/core#ConceptScheme"/>
        <rdfs:isDefinedBy rdf:resource="https://w3id.org/gcdfo/salmon"/>
        <skos:definition xml:lang="en">Controlled vocabulary for life-phase or fishery/migration segment qualifiers used to stratify measurements (e.g., ocean, terminal, mainstem).</skos:definition>
        <skos:hasTopConcept rdf:resource="https://w3id.org/gcdfo/salmon#LifePhase"/>
        <skos:prefLabel xml:lang="en">Life phase scheme</skos:prefLabel>
        <theme rdf:resource="https://w3id.org/gcdfo/salmon#StockAssessmentTheme"/>
    </owl:NamedIndividual>
    


    <!-- https://w3id.org/gcdfo/salmon#LowerBenchmark -->

    <owl:NamedIndividual rdf:about="https://w3id.org/gcdfo/salmon#LowerBenchmark">
        <rdf:type rdf:resource="http://www.w3.org/2004/02/skos/core#Concept"/>
        <rdfs:isDefinedBy rdf:resource="https://w3id.org/gcdfo/salmon"/>
        <skos:definition xml:lang="en">A lower-threshold benchmark value, typically delineating the boundary between Red and Amber status zones.</skos:definition>
        <skos:inScheme rdf:resource="https://w3id.org/gcdfo/salmon#BenchmarkLevelScheme"/>
        <skos:prefLabel xml:lang="en">Lower benchmark</skos:prefLabel>
        <theme rdf:resource="https://w3id.org/gcdfo/salmon#StockAssessmentTheme"/>
        <theme rdf:resource="https://w3id.org/gcdfo/salmon#WildSalmonPolicyTheme"/>
    </owl:NamedIndividual>
    


    <!-- https://w3id.org/gcdfo/salmon#MainstemPhase -->

    <owl:NamedIndividual rdf:about="https://w3id.org/gcdfo/salmon#MainstemPhase">
        <rdf:type rdf:resource="http://www.w3.org/2004/02/skos/core#Concept"/>
        <rdfs:isDefinedBy rdf:resource="https://w3id.org/gcdfo/salmon"/>
        <skos:broader rdf:resource="https://w3id.org/gcdfo/salmon#LifePhase"/>
        <skos:definition xml:lang="en">Freshwater mainstem migration phase in a river system (often corresponding to mainstem in-river fisheries or monitoring segments).</skos:definition>
        <skos:inScheme rdf:resource="https://w3id.org/gcdfo/salmon#LifePhaseScheme"/>
        <skos:prefLabel xml:lang="en">Mainstem phase</skos:prefLabel>
        <theme rdf:resource="https://w3id.org/gcdfo/salmon#StockAssessmentTheme"/>
    </owl:NamedIndividual>
    


    <!-- https://w3id.org/gcdfo/salmon#ManagementReferenceContext -->

    <owl:NamedIndividual rdf:about="https://w3id.org/gcdfo/salmon#ManagementReferenceContext">
        <rdf:type rdf:resource="http://www.w3.org/2004/02/skos/core#Concept"/>
        <rdfs:isDefinedBy rdf:resource="https://w3id.org/gcdfo/salmon"/>
        <skos:broader rdf:resource="https://w3id.org/gcdfo/salmon#MeasurementContext"/>
        <skos:definition xml:lang="en">Measurement context indicating values are management benchmarks or reference-oriented metrics.</skos:definition>
        <skos:inScheme rdf:resource="https://w3id.org/gcdfo/salmon#MeasurementContextScheme"/>
        <skos:prefLabel xml:lang="en">Management reference context</skos:prefLabel>
        <theme rdf:resource="https://w3id.org/gcdfo/salmon#PolicyGovernanceTheme"/>
        <theme rdf:resource="https://w3id.org/gcdfo/salmon#StockAssessmentTheme"/>
    </owl:NamedIndividual>
    


    <!-- https://w3id.org/gcdfo/salmon#MarkRecaptureAnalysis -->

    <owl:NamedIndividual rdf:about="https://w3id.org/gcdfo/salmon#MarkRecaptureAnalysis">
        <rdf:type rdf:resource="http://www.w3.org/2004/02/skos/core#Concept"/>
        <rdfs:comment xml:lang="en">Legacy methods: Petersen, Jolly-Seber, Open model, Bayesian MR. Store uncertainty (e.g., CV) when available; note tag loss/recovery protocols.</rdfs:comment>
        <rdfs:isDefinedBy rdf:resource="https://w3id.org/gcdfo/salmon"/>
        <skos:broader rdf:resource="https://w3id.org/gcdfo/salmon#EstimateMethod"/>
        <skos:definition xml:lang="en">Capture-recapture estimators (Petersen, Jolly-Seber, open/Bayesian models) applied to field marks/recoveries.</skos:definition>
        <skos:inScheme rdf:resource="https://w3id.org/gcdfo/salmon#EstimateMethodScheme"/>
        <skos:prefLabel xml:lang="en">Mark-Recapture Analysis</skos:prefLabel>
        <theme rdf:resource="https://w3id.org/gcdfo/salmon#MonitoringFieldWorkTheme"/>
        <theme rdf:resource="https://w3id.org/gcdfo/salmon#StockAssessmentTheme"/>
    </owl:NamedIndividual>
    


    <!-- https://w3id.org/gcdfo/salmon#MarkRecaptureAssumptions -->

    <owl:NamedIndividual rdf:about="https://w3id.org/gcdfo/salmon#MarkRecaptureAssumptions">
        <rdf:type rdf:resource="http://www.w3.org/2004/02/skos/core#Concept"/>
        <rdfs:comment xml:lang="en">Limits to Type 3 maximum</rdfs:comment>
        <rdfs:isDefinedBy rdf:resource="https://w3id.org/gcdfo/salmon"/>
        <skos:broader rdf:resource="https://w3id.org/gcdfo/salmon#DowngradeCriteria"/>
        <skos:definition xml:lang="en">MR assumptions not evaluated</skos:definition>
        <skos:inScheme rdf:resource="https://w3id.org/gcdfo/salmon#DowngradeCriteriaScheme"/>
        <skos:prefLabel xml:lang="en">Mark-Recapture Assumptions</skos:prefLabel>
        <theme rdf:resource="https://w3id.org/gcdfo/salmon#DataModelProvenanceTheme"/>
        <theme rdf:resource="https://w3id.org/gcdfo/salmon#StockAssessmentTheme"/>
    </owl:NamedIndividual>
    


    <!-- https://w3id.org/gcdfo/salmon#MarkRecaptureFieldProgram -->

    <owl:NamedIndividual rdf:about="https://w3id.org/gcdfo/salmon#MarkRecaptureFieldProgram">
        <rdf:type rdf:resource="http://www.w3.org/2004/02/skos/core#Concept"/>
        <rdfs:comment xml:lang="en">Legacy methods: Tag Recovery</rdfs:comment>
        <rdfs:isDefinedBy rdf:resource="https://w3id.org/gcdfo/salmon"/>
        <skos:broader rdf:resource="https://w3id.org/gcdfo/salmon#EnumerationMethod"/>
        <skos:definition xml:lang="en">Field program involving marking and subsequent recapture/recovery of tagged fish with documented assumptions and recovery coverage.</skos:definition>
        <skos:inScheme rdf:resource="https://w3id.org/gcdfo/salmon#EnumerationMethodScheme"/>
        <skos:prefLabel xml:lang="en">Mark-Recapture Field Program</skos:prefLabel>
        <theme rdf:resource="https://w3id.org/gcdfo/salmon#MonitoringFieldWorkTheme"/>
        <theme rdf:resource="https://w3id.org/gcdfo/salmon#StockAssessmentTheme"/>
    </owl:NamedIndividual>
    


    <!-- https://w3id.org/gcdfo/salmon#MeasurementContext -->

    <owl:NamedIndividual rdf:about="https://w3id.org/gcdfo/salmon#MeasurementContext">
        <rdf:type rdf:resource="http://www.w3.org/2004/02/skos/core#Concept"/>
        <rdfs:isDefinedBy rdf:resource="https://w3id.org/gcdfo/salmon"/>
        <skos:definition xml:lang="en">A context qualifier used to disambiguate the interpretation of a measurement column.</skos:definition>
        <skos:inScheme rdf:resource="https://w3id.org/gcdfo/salmon#MeasurementContextScheme"/>
        <skos:prefLabel xml:lang="en">Measurement context</skos:prefLabel>
        <theme rdf:resource="https://w3id.org/gcdfo/salmon#DataModelProvenanceTheme"/>
        <theme rdf:resource="https://w3id.org/gcdfo/salmon#StockAssessmentTheme"/>
    </owl:NamedIndividual>
    


    <!-- https://w3id.org/gcdfo/salmon#MeasurementContextScheme -->

    <owl:NamedIndividual rdf:about="https://w3id.org/gcdfo/salmon#MeasurementContextScheme">
        <rdf:type rdf:resource="http://www.w3.org/2004/02/skos/core#ConceptScheme"/>
        <rdfs:isDefinedBy rdf:resource="https://w3id.org/gcdfo/salmon"/>
        <skos:definition xml:lang="en">Controlled vocabulary for compositional measurement context qualifiers (for example, catch context, run context).</skos:definition>
        <skos:hasTopConcept rdf:resource="https://w3id.org/gcdfo/salmon#MeasurementContext"/>
        <skos:prefLabel xml:lang="en">Measurement context scheme</skos:prefLabel>
        <theme rdf:resource="https://w3id.org/gcdfo/salmon#DataModelProvenanceTheme"/>
        <theme rdf:resource="https://w3id.org/gcdfo/salmon#StockAssessmentTheme"/>
    </owl:NamedIndividual>
    


    <!-- https://w3id.org/gcdfo/salmon#MethodUnknown -->

    <owl:NamedIndividual rdf:about="https://w3id.org/gcdfo/salmon#MethodUnknown">
        <rdf:type rdf:resource="http://www.w3.org/2004/02/skos/core#Concept"/>
        <rdfs:comment xml:lang="en">Limits to Type 5 maximum</rdfs:comment>
        <rdfs:isDefinedBy rdf:resource="https://w3id.org/gcdfo/salmon"/>
        <skos:broader rdf:resource="https://w3id.org/gcdfo/salmon#DowngradeCriteria"/>
        <skos:definition xml:lang="en">Survey/analytical methods not adequately identified/consistent</skos:definition>
        <skos:inScheme rdf:resource="https://w3id.org/gcdfo/salmon#DowngradeCriteriaScheme"/>
        <skos:prefLabel xml:lang="en">Method Unknown/Inconsistent</skos:prefLabel>
        <theme rdf:resource="https://w3id.org/gcdfo/salmon#DataModelProvenanceTheme"/>
        <theme rdf:resource="https://w3id.org/gcdfo/salmon#StockAssessmentTheme"/>
    </owl:NamedIndividual>
    


    <!-- https://w3id.org/gcdfo/salmon#MonitoringFieldWorkTheme -->

    <owl:NamedIndividual rdf:about="https://w3id.org/gcdfo/salmon#MonitoringFieldWorkTheme">
        <rdf:type rdf:resource="http://www.w3.org/2004/02/skos/core#Concept"/>
        <rdfs:isDefinedBy rdf:resource="https://w3id.org/gcdfo/salmon"/>
        <skos:definition xml:lang="en">Field observations, sampling protocols, survey events, gear, and measurement methods used to collect salmon data.</skos:definition>
        <skos:inScheme rdf:resource="https://w3id.org/gcdfo/salmon#ThemeScheme"/>
        <skos:prefLabel xml:lang="en">Monitoring and Field Work</skos:prefLabel>
        <theme rdf:resource="https://w3id.org/gcdfo/salmon#DataModelProvenanceTheme"/>
    </owl:NamedIndividual>
    


    <!-- https://w3id.org/gcdfo/salmon#NaturalOrigin -->

    <owl:NamedIndividual rdf:about="https://w3id.org/gcdfo/salmon#NaturalOrigin">
        <rdf:type rdf:resource="http://www.w3.org/2004/02/skos/core#Concept"/>
        <obo:IAO_0000119 xml:lang="en">Fisheries and Oceans Canada. 2018. Review of genetically based targets for enhanced contributions to Canadian Pacific Chinook Salmon populations. DFO Canadian Science Advisory Secretariat Science Advisory Report 2018/001 (Erratum: October 2023).</obo:IAO_0000119>
        <dcterms:source rdf:resource="https://www.dfo-mpo.gc.ca/csas-sccs/Publications/SAR-AS/2018/2018_001-eng.html"/>
        <rdfs:isDefinedBy rdf:resource="https://w3id.org/gcdfo/salmon"/>
        <skos:broader rdf:resource="https://w3id.org/gcdfo/salmon#SalmonOrigin"/>
        <skos:definition xml:lang="en">Individuals that are born and reared in the wild (natural environment).</skos:definition>
        <skos:inScheme rdf:resource="https://w3id.org/gcdfo/salmon#SalmonOriginScheme"/>
        <skos:prefLabel xml:lang="en">Natural-origin</skos:prefLabel>
        <theme rdf:resource="https://w3id.org/gcdfo/salmon#GeneticsStockCompositionTheme"/>
        <theme rdf:resource="https://w3id.org/gcdfo/salmon#StockAssessmentTheme"/>
        <theme rdf:resource="https://w3id.org/gcdfo/salmon#WildSalmonPolicyTheme"/>
    </owl:NamedIndividual>
    


    <!-- https://w3id.org/gcdfo/salmon#NumberOfVisits -->

    <owl:NamedIndividual rdf:about="https://w3id.org/gcdfo/salmon#NumberOfVisits">
        <rdf:type rdf:resource="http://www.w3.org/2004/02/skos/core#Concept"/>
        <rdfs:comment xml:lang="en">Limits to Type 4 maximum</rdfs:comment>
        <rdfs:isDefinedBy rdf:resource="https://w3id.org/gcdfo/salmon"/>
        <skos:broader rdf:resource="https://w3id.org/gcdfo/salmon#DowngradeCriteria"/>
        <skos:definition xml:lang="en">Insufficient number of survey visits</skos:definition>
        <skos:inScheme rdf:resource="https://w3id.org/gcdfo/salmon#DowngradeCriteriaScheme"/>
        <skos:prefLabel xml:lang="en">Number of Visits</skos:prefLabel>
        <theme rdf:resource="https://w3id.org/gcdfo/salmon#DataModelProvenanceTheme"/>
        <theme rdf:resource="https://w3id.org/gcdfo/salmon#StockAssessmentTheme"/>
    </owl:NamedIndividual>
    


    <!-- https://w3id.org/gcdfo/salmon#OceanAgeDimension -->

    <owl:NamedIndividual rdf:about="https://w3id.org/gcdfo/salmon#OceanAgeDimension">
        <rdf:type rdf:resource="http://www.w3.org/2004/02/skos/core#Concept"/>
        <rdfs:isDefinedBy rdf:resource="https://w3id.org/gcdfo/salmon"/>
        <skos:altLabel xml:lang="en">Marine age dimension</skos:altLabel>
        <skos:broader rdf:resource="https://w3id.org/gcdfo/salmon#AgeDimension"/>
        <skos:definition xml:lang="en">Age value represents years spent in the marine environment.</skos:definition>
        <skos:inScheme rdf:resource="https://w3id.org/gcdfo/salmon#AgeDimensionScheme"/>
        <skos:prefLabel xml:lang="en">Ocean age dimension</skos:prefLabel>
        <theme rdf:resource="https://w3id.org/gcdfo/salmon#StockAssessmentTheme"/>
    </owl:NamedIndividual>
    


    <!-- https://w3id.org/gcdfo/salmon#OceanPhase -->

    <owl:NamedIndividual rdf:about="https://w3id.org/gcdfo/salmon#OceanPhase">
        <rdf:type rdf:resource="http://www.w3.org/2004/02/skos/core#Concept"/>
        <rdfs:isDefinedBy rdf:resource="https://w3id.org/gcdfo/salmon"/>
        <skos:altLabel xml:lang="en">Marine phase</skos:altLabel>
        <skos:broader rdf:resource="https://w3id.org/gcdfo/salmon#LifePhase"/>
        <skos:definition xml:lang="en">Phase of the salmon life cycle or assessment period occurring in the marine environment.</skos:definition>
        <skos:inScheme rdf:resource="https://w3id.org/gcdfo/salmon#LifePhaseScheme"/>
        <skos:prefLabel xml:lang="en">Ocean phase</skos:prefLabel>
        <theme rdf:resource="https://w3id.org/gcdfo/salmon#StockAssessmentTheme"/>
    </owl:NamedIndividual>
    


    <!-- https://w3id.org/gcdfo/salmon#PeakCountAnalysis -->

    <owl:NamedIndividual rdf:about="https://w3id.org/gcdfo/salmon#PeakCountAnalysis">
        <rdf:type rdf:resource="http://www.w3.org/2004/02/skos/core#Concept"/>
        <rdfs:comment xml:lang="en">Legacy methods: Peak Live, Peak Live + Dead, Peak + Cumulative Dead, Cumulative New</rdfs:comment>
        <rdfs:isDefinedBy rdf:resource="https://w3id.org/gcdfo/salmon"/>
        <skos:broader rdf:resource="https://w3id.org/gcdfo/salmon#EstimateMethod"/>
        <skos:definition xml:lang="en">Uses the peak survey (live ± dead variants) as the season estimate/index.</skos:definition>
        <skos:inScheme rdf:resource="https://w3id.org/gcdfo/salmon#EstimateMethodScheme"/>
        <skos:prefLabel xml:lang="en">Peak Count Analysis</skos:prefLabel>
        <theme rdf:resource="https://w3id.org/gcdfo/salmon#MonitoringFieldWorkTheme"/>
        <theme rdf:resource="https://w3id.org/gcdfo/salmon#StockAssessmentTheme"/>
    </owl:NamedIndividual>
    


    <!-- https://w3id.org/gcdfo/salmon#PolicyFramework -->

    <owl:NamedIndividual rdf:about="https://w3id.org/gcdfo/salmon#PolicyFramework">
        <rdf:type rdf:resource="http://www.w3.org/2004/02/skos/core#Concept"/>
        <rdfs:isDefinedBy rdf:resource="https://w3id.org/gcdfo/salmon"/>
        <skos:definition xml:lang="en">A policy, legal, or governance framework that defines how salmon status metrics, benchmarks, or reference points are set and interpreted.</skos:definition>
        <skos:inScheme rdf:resource="https://w3id.org/gcdfo/salmon#PolicyFrameworkScheme"/>
        <skos:prefLabel xml:lang="en">Policy framework</skos:prefLabel>
        <theme rdf:resource="https://w3id.org/gcdfo/salmon#PolicyGovernanceTheme"/>
        <theme rdf:resource="https://w3id.org/gcdfo/salmon#StockAssessmentTheme"/>
        <theme rdf:resource="https://w3id.org/gcdfo/salmon#WildSalmonPolicyTheme"/>
    </owl:NamedIndividual>
    


    <!-- https://w3id.org/gcdfo/salmon#PolicyFrameworkScheme -->

    <owl:NamedIndividual rdf:about="https://w3id.org/gcdfo/salmon#PolicyFrameworkScheme">
        <rdf:type rdf:resource="http://www.w3.org/2004/02/skos/core#ConceptScheme"/>
        <rdfs:isDefinedBy rdf:resource="https://w3id.org/gcdfo/salmon"/>
        <skos:definition xml:lang="en">Controlled vocabulary for policy and governance frameworks referenced by salmon assessment metrics and benchmarks (e.g., WSP, PA).</skos:definition>
        <skos:hasTopConcept rdf:resource="https://w3id.org/gcdfo/salmon#PolicyFramework"/>
        <skos:prefLabel xml:lang="en">Policy framework scheme</skos:prefLabel>
        <theme rdf:resource="https://w3id.org/gcdfo/salmon#PolicyGovernanceTheme"/>
        <theme rdf:resource="https://w3id.org/gcdfo/salmon#StockAssessmentTheme"/>
        <theme rdf:resource="https://w3id.org/gcdfo/salmon#WildSalmonPolicyTheme"/>
    </owl:NamedIndividual>
    


    <!-- https://w3id.org/gcdfo/salmon#PolicyGovernanceTheme -->

    <owl:NamedIndividual rdf:about="https://w3id.org/gcdfo/salmon#PolicyGovernanceTheme">
        <rdf:type rdf:resource="http://www.w3.org/2004/02/skos/core#Concept"/>
        <rdfs:isDefinedBy rdf:resource="https://w3id.org/gcdfo/salmon"/>
        <skos:definition xml:lang="en">DFO policy frameworks, governance, regulations, and organizational structure relevant to salmon management.</skos:definition>
        <skos:inScheme rdf:resource="https://w3id.org/gcdfo/salmon#ThemeScheme"/>
        <skos:prefLabel xml:lang="en">Policy, Governance, and Organizational Structure</skos:prefLabel>
        <theme rdf:resource="https://w3id.org/gcdfo/salmon#DataModelProvenanceTheme"/>
    </owl:NamedIndividual>
    


    <!-- https://w3id.org/gcdfo/salmon#PrecautionaryApproach -->

    <owl:NamedIndividual rdf:about="https://w3id.org/gcdfo/salmon#PrecautionaryApproach">
        <rdf:type rdf:resource="http://www.w3.org/2004/02/skos/core#Concept"/>
        <rdfs:isDefinedBy rdf:resource="https://w3id.org/gcdfo/salmon"/>
        <skos:altLabel xml:lang="en">PA</skos:altLabel>
        <skos:broader rdf:resource="https://w3id.org/gcdfo/salmon#PolicyFramework"/>
        <skos:definition xml:lang="en">DFO policy framework for applying precaution in fisheries decision-making, including use of reference points and stock status zones.</skos:definition>
        <skos:inScheme rdf:resource="https://w3id.org/gcdfo/salmon#PolicyFrameworkScheme"/>
        <skos:prefLabel xml:lang="en">Precautionary Approach</skos:prefLabel>
        <theme rdf:resource="https://w3id.org/gcdfo/salmon#FisheriesManagementTheme"/>
        <theme rdf:resource="https://w3id.org/gcdfo/salmon#PolicyGovernanceTheme"/>
        <theme rdf:resource="https://w3id.org/gcdfo/salmon#StockAssessmentTheme"/>
    </owl:NamedIndividual>
    


    <!-- https://w3id.org/gcdfo/salmon#PrecisionAccuracy -->

    <owl:NamedIndividual rdf:about="https://w3id.org/gcdfo/salmon#PrecisionAccuracy">
        <rdf:type rdf:resource="http://www.w3.org/2004/02/skos/core#Concept"/>
        <rdfs:comment xml:lang="en">Downgrades by one level</rdfs:comment>
        <rdfs:isDefinedBy rdf:resource="https://w3id.org/gcdfo/salmon"/>
        <skos:broader rdf:resource="https://w3id.org/gcdfo/salmon#DowngradeCriteria"/>
        <skos:definition xml:lang="en">Precision/accuracy weaker than expected for type</skos:definition>
        <skos:inScheme rdf:resource="https://w3id.org/gcdfo/salmon#DowngradeCriteriaScheme"/>
        <skos:prefLabel xml:lang="en">Precision/Accuracy</skos:prefLabel>
        <theme rdf:resource="https://w3id.org/gcdfo/salmon#DataModelProvenanceTheme"/>
        <theme rdf:resource="https://w3id.org/gcdfo/salmon#StockAssessmentTheme"/>
    </owl:NamedIndividual>
    


    <!-- https://w3id.org/gcdfo/salmon#RapidStatusConfidenceHigh -->

    <owl:NamedIndividual rdf:about="https://w3id.org/gcdfo/salmon#RapidStatusConfidenceHigh">
        <rdf:type rdf:resource="http://www.w3.org/2004/02/skos/core#Concept"/>
        <rdf:type rdf:resource="https://w3id.org/gcdfo/salmon#ConfidenceCategory"/>
        <obo:IAO_0000115 xml:lang="en">Rapid status confidence category indicating that high-quality abundance metrics support the result.</obo:IAO_0000115>
        <rdfs:isDefinedBy rdf:resource="https://w3id.org/gcdfo/salmon"/>
        <rdfs:label xml:lang="en">High rapid-status confidence</rdfs:label>
        <skos:inScheme rdf:resource="https://w3id.org/gcdfo/salmon#RapidStatusConfidenceScheme"/>
        <skos:prefLabel xml:lang="en">High confidence</skos:prefLabel>
        <theme rdf:resource="https://w3id.org/gcdfo/salmon#StockAssessmentTheme"/>
        <theme rdf:resource="https://w3id.org/gcdfo/salmon#WildSalmonPolicyTheme"/>
    </owl:NamedIndividual>
    


    <!-- https://w3id.org/gcdfo/salmon#RapidStatusConfidenceLow -->

    <owl:NamedIndividual rdf:about="https://w3id.org/gcdfo/salmon#RapidStatusConfidenceLow">
        <rdf:type rdf:resource="http://www.w3.org/2004/02/skos/core#Concept"/>
        <rdf:type rdf:resource="https://w3id.org/gcdfo/salmon#ConfidenceCategory"/>
        <obo:IAO_0000115 xml:lang="en">Rapid status confidence category indicating limited supporting data (for example, derived from trend metrics alone).</obo:IAO_0000115>
        <rdfs:isDefinedBy rdf:resource="https://w3id.org/gcdfo/salmon"/>
        <rdfs:label xml:lang="en">Low rapid-status confidence</rdfs:label>
        <skos:inScheme rdf:resource="https://w3id.org/gcdfo/salmon#RapidStatusConfidenceScheme"/>
        <skos:prefLabel xml:lang="en">Low confidence</skos:prefLabel>
        <theme rdf:resource="https://w3id.org/gcdfo/salmon#StockAssessmentTheme"/>
        <theme rdf:resource="https://w3id.org/gcdfo/salmon#WildSalmonPolicyTheme"/>
    </owl:NamedIndividual>
    


    <!-- https://w3id.org/gcdfo/salmon#RapidStatusConfidenceMedium -->

    <owl:NamedIndividual rdf:about="https://w3id.org/gcdfo/salmon#RapidStatusConfidenceMedium">
        <rdf:type rdf:resource="http://www.w3.org/2004/02/skos/core#Concept"/>
        <rdf:type rdf:resource="https://w3id.org/gcdfo/salmon#ConfidenceCategory"/>
        <obo:IAO_0000115 xml:lang="en">Rapid status confidence category indicating mixed evidence or reliance on trend metrics supplemented by some abundance information.</obo:IAO_0000115>
        <rdfs:isDefinedBy rdf:resource="https://w3id.org/gcdfo/salmon"/>
        <rdfs:label xml:lang="en">Medium rapid-status confidence</rdfs:label>
        <skos:inScheme rdf:resource="https://w3id.org/gcdfo/salmon#RapidStatusConfidenceScheme"/>
        <skos:prefLabel xml:lang="en">Medium confidence</skos:prefLabel>
        <theme rdf:resource="https://w3id.org/gcdfo/salmon#StockAssessmentTheme"/>
        <theme rdf:resource="https://w3id.org/gcdfo/salmon#WildSalmonPolicyTheme"/>
    </owl:NamedIndividual>
    


    <!-- https://w3id.org/gcdfo/salmon#RapidStatusConfidenceScheme -->

    <owl:NamedIndividual rdf:about="https://w3id.org/gcdfo/salmon#RapidStatusConfidenceScheme">
        <rdf:type rdf:resource="http://www.w3.org/2004/02/skos/core#ConceptScheme"/>
        <rdfs:isDefinedBy rdf:resource="https://w3id.org/gcdfo/salmon"/>
        <skos:definition xml:lang="en">Controlled vocabulary for categorical confidence ratings attached to rapid status assessments.</skos:definition>
        <skos:hasTopConcept rdf:resource="https://w3id.org/gcdfo/salmon#ConfidenceCategory"/>
        <skos:prefLabel xml:lang="en">Rapid status confidence scheme</skos:prefLabel>
        <theme rdf:resource="https://w3id.org/gcdfo/salmon#StockAssessmentTheme"/>
        <theme rdf:resource="https://w3id.org/gcdfo/salmon#WildSalmonPolicyTheme"/>
    </owl:NamedIndividual>
    


    <!-- https://w3id.org/gcdfo/salmon#ReachCoverage -->

    <owl:NamedIndividual rdf:about="https://w3id.org/gcdfo/salmon#ReachCoverage">
        <rdf:type rdf:resource="http://www.w3.org/2004/02/skos/core#Concept"/>
        <rdfs:comment xml:lang="en">Limits to Type 3 maximum</rdfs:comment>
        <rdfs:isDefinedBy rdf:resource="https://w3id.org/gcdfo/salmon"/>
        <skos:broader rdf:resource="https://w3id.org/gcdfo/salmon#DowngradeCriteria"/>
        <skos:definition xml:lang="en">Insufficient reach coverage</skos:definition>
        <skos:inScheme rdf:resource="https://w3id.org/gcdfo/salmon#DowngradeCriteriaScheme"/>
        <skos:prefLabel xml:lang="en">Reach Coverage</skos:prefLabel>
        <theme rdf:resource="https://w3id.org/gcdfo/salmon#DataModelProvenanceTheme"/>
        <theme rdf:resource="https://w3id.org/gcdfo/salmon#StockAssessmentTheme"/>
    </owl:NamedIndividual>
    


    <!-- https://w3id.org/gcdfo/salmon#RecruitStageContext -->

    <owl:NamedIndividual rdf:about="https://w3id.org/gcdfo/salmon#RecruitStageContext">
        <rdf:type rdf:resource="http://www.w3.org/2004/02/skos/core#Concept"/>
        <rdfs:isDefinedBy rdf:resource="https://w3id.org/gcdfo/salmon"/>
        <skos:broader rdf:resource="https://w3id.org/gcdfo/salmon#MeasurementContext"/>
        <skos:definition xml:lang="en">Measurement context indicating values refer to recruits.</skos:definition>
        <skos:inScheme rdf:resource="https://w3id.org/gcdfo/salmon#MeasurementContextScheme"/>
        <skos:prefLabel xml:lang="en">Recruit stage context</skos:prefLabel>
        <theme rdf:resource="https://w3id.org/gcdfo/salmon#StockAssessmentTheme"/>
    </owl:NamedIndividual>
    


    <!-- https://w3id.org/gcdfo/salmon#RedZone -->

    <owl:NamedIndividual rdf:about="https://w3id.org/gcdfo/salmon#RedZone">
        <rdf:type rdf:resource="http://www.w3.org/2004/02/skos/core#Concept"/>
        <rdf:type rdf:resource="https://w3id.org/gcdfo/salmon#WSPBiologicalStatusZone"/>
        <obo:IAO_0000119 xml:lang="en">Fisheries and Oceans Canada. Wild Salmon Policy 2018-2022 Implementation Plan. https://waves-vagues.dfo-mpo.gc.ca/library-bibliotheque/40728109.pdf.</obo:IAO_0000119>
        <dcterms:source rdf:resource="https://waves-vagues.dfo-mpo.gc.ca/library-bibliotheque/40728109.pdf"/>
        <rdfs:isDefinedBy rdf:resource="https://w3id.org/gcdfo/salmon"/>
        <skos:definition xml:lang="en">A Conservation Unit in the Red zone is undesirable because of the risk of extirpation, and the loss of ecological benefits and salmon production. Changes in status will trigger management actions that will vary depending on species, geographic regions, and cause of the decline.</skos:definition>
        <skos:inScheme rdf:resource="https://w3id.org/gcdfo/salmon#WSPBiologicalStatusZoneScheme"/>
        <skos:prefLabel xml:lang="en">Red zone</skos:prefLabel>
        <theme rdf:resource="https://w3id.org/gcdfo/salmon#StockAssessmentTheme"/>
        <theme rdf:resource="https://w3id.org/gcdfo/salmon#WildSalmonPolicyTheme"/>
    </owl:NamedIndividual>
    


    <!-- https://w3id.org/gcdfo/salmon#ReddCount -->

    <owl:NamedIndividual rdf:about="https://w3id.org/gcdfo/salmon#ReddCount">
        <rdf:type rdf:resource="http://www.w3.org/2004/02/skos/core#Concept"/>
        <rdfs:comment xml:lang="en">Legacy methods: Redd Counts</rdfs:comment>
        <rdfs:isDefinedBy rdf:resource="https://w3id.org/gcdfo/salmon"/>
        <skos:broader rdf:resource="https://w3id.org/gcdfo/salmon#EnumerationMethod"/>
        <skos:definition xml:lang="en">Redd counts with documentation of detectability, timing, and reach coverage. Conversion to spawner estimates requires spawners-per-redd factors handled in analysis.</skos:definition>
        <skos:inScheme rdf:resource="https://w3id.org/gcdfo/salmon#EnumerationMethodScheme"/>
        <skos:prefLabel xml:lang="en">Redd Count</skos:prefLabel>
        <theme rdf:resource="https://w3id.org/gcdfo/salmon#MonitoringFieldWorkTheme"/>
        <theme rdf:resource="https://w3id.org/gcdfo/salmon#StockAssessmentTheme"/>
    </owl:NamedIndividual>
    


    <!-- https://w3id.org/gcdfo/salmon#ReddExpansionAnalysis -->

    <owl:NamedIndividual rdf:about="https://w3id.org/gcdfo/salmon#ReddExpansionAnalysis">
        <rdf:type rdf:resource="http://www.w3.org/2004/02/skos/core#Concept"/>
        <rdfs:comment xml:lang="en">Requires validated spawners-per-redd factor and documentation of detectability assumptions.</rdfs:comment>
        <rdfs:isDefinedBy rdf:resource="https://w3id.org/gcdfo/salmon"/>
        <skos:broader rdf:resource="https://w3id.org/gcdfo/salmon#EstimateMethod"/>
        <skos:definition xml:lang="en">Converts redd counts to spawner estimates using spawners-per-redd expansion factors.</skos:definition>
        <skos:inScheme rdf:resource="https://w3id.org/gcdfo/salmon#EstimateMethodScheme"/>
        <skos:prefLabel xml:lang="en">Redd Expansion Analysis</skos:prefLabel>
        <theme rdf:resource="https://w3id.org/gcdfo/salmon#MonitoringFieldWorkTheme"/>
        <theme rdf:resource="https://w3id.org/gcdfo/salmon#StockAssessmentTheme"/>
    </owl:NamedIndividual>
    


    <!-- https://w3id.org/gcdfo/salmon#ReviewQA -->

    <owl:NamedIndividual rdf:about="https://w3id.org/gcdfo/salmon#ReviewQA">
        <rdf:type rdf:resource="http://www.w3.org/2004/02/skos/core#Concept"/>
        <rdfs:comment xml:lang="en">Limits to Type 2 maximum</rdfs:comment>
        <rdfs:isDefinedBy rdf:resource="https://w3id.org/gcdfo/salmon"/>
        <skos:broader rdf:resource="https://w3id.org/gcdfo/salmon#DowngradeCriteria"/>
        <skos:definition xml:lang="en">Insufficient QA review of automated events</skos:definition>
        <skos:inScheme rdf:resource="https://w3id.org/gcdfo/salmon#DowngradeCriteriaScheme"/>
        <skos:prefLabel xml:lang="en">Review/QA</skos:prefLabel>
        <theme rdf:resource="https://w3id.org/gcdfo/salmon#DataModelProvenanceTheme"/>
        <theme rdf:resource="https://w3id.org/gcdfo/salmon#StockAssessmentTheme"/>
    </owl:NamedIndividual>
    


    <!-- https://w3id.org/gcdfo/salmon#RunContext -->

    <owl:NamedIndividual rdf:about="https://w3id.org/gcdfo/salmon#RunContext">
        <rdf:type rdf:resource="http://www.w3.org/2004/02/skos/core#Concept"/>
        <rdfs:isDefinedBy rdf:resource="https://w3id.org/gcdfo/salmon"/>
        <skos:broader rdf:resource="https://w3id.org/gcdfo/salmon#MeasurementContext"/>
        <skos:definition xml:lang="en">Measurement context indicating values refer to run size or returning run composition.</skos:definition>
        <skos:inScheme rdf:resource="https://w3id.org/gcdfo/salmon#MeasurementContextScheme"/>
        <skos:prefLabel xml:lang="en">Run context</skos:prefLabel>
        <theme rdf:resource="https://w3id.org/gcdfo/salmon#StockAssessmentTheme"/>
    </owl:NamedIndividual>
    


    <!-- https://w3id.org/gcdfo/salmon#RunCoverage -->

    <owl:NamedIndividual rdf:about="https://w3id.org/gcdfo/salmon#RunCoverage">
        <rdf:type rdf:resource="http://www.w3.org/2004/02/skos/core#Concept"/>
        <rdfs:comment xml:lang="en">Limits to Type 2 maximum</rdfs:comment>
        <rdfs:isDefinedBy rdf:resource="https://w3id.org/gcdfo/salmon"/>
        <skos:broader rdf:resource="https://w3id.org/gcdfo/salmon#DowngradeCriteria"/>
        <skos:definition xml:lang="en">Run-window coverage &lt; 95% of season days</skos:definition>
        <skos:inScheme rdf:resource="https://w3id.org/gcdfo/salmon#DowngradeCriteriaScheme"/>
        <skos:prefLabel xml:lang="en">Run Coverage</skos:prefLabel>
        <theme rdf:resource="https://w3id.org/gcdfo/salmon#DataModelProvenanceTheme"/>
        <theme rdf:resource="https://w3id.org/gcdfo/salmon#StockAssessmentTheme"/>
    </owl:NamedIndividual>
    


    <!-- https://w3id.org/gcdfo/salmon#SalmonEnhancementHatcheriesTheme -->

    <owl:NamedIndividual rdf:about="https://w3id.org/gcdfo/salmon#SalmonEnhancementHatcheriesTheme">
        <rdf:type rdf:resource="http://www.w3.org/2004/02/skos/core#Concept"/>
        <rdfs:isDefinedBy rdf:resource="https://w3id.org/gcdfo/salmon"/>
        <skos:definition xml:lang="en">Hatchery production, broodstock management, releases, and enhancement program practices for salmon.</skos:definition>
        <skos:inScheme rdf:resource="https://w3id.org/gcdfo/salmon#ThemeScheme"/>
        <skos:prefLabel xml:lang="en">Salmon Enhancement and Hatcheries</skos:prefLabel>
        <theme rdf:resource="https://w3id.org/gcdfo/salmon#DataModelProvenanceTheme"/>
    </owl:NamedIndividual>
    


    <!-- https://w3id.org/gcdfo/salmon#SalmonOrigin -->

    <owl:NamedIndividual rdf:about="https://w3id.org/gcdfo/salmon#SalmonOrigin">
        <rdf:type rdf:resource="http://www.w3.org/2004/02/skos/core#Concept"/>
        <rdfs:isDefinedBy rdf:resource="https://w3id.org/gcdfo/salmon"/>
        <skos:definition xml:lang="en">Origin category describing whether salmon are naturally produced, hatchery produced, or mixed-origin.</skos:definition>
        <skos:inScheme rdf:resource="https://w3id.org/gcdfo/salmon#SalmonOriginScheme"/>
        <skos:prefLabel xml:lang="en">Salmon origin</skos:prefLabel>
        <theme rdf:resource="https://w3id.org/gcdfo/salmon#SalmonEnhancementHatcheriesTheme"/>
        <theme rdf:resource="https://w3id.org/gcdfo/salmon#StockAssessmentTheme"/>
    </owl:NamedIndividual>
    


    <!-- https://w3id.org/gcdfo/salmon#SalmonOriginScheme -->

    <owl:NamedIndividual rdf:about="https://w3id.org/gcdfo/salmon#SalmonOriginScheme">
        <rdf:type rdf:resource="http://www.w3.org/2004/02/skos/core#ConceptScheme"/>
        <rdfs:isDefinedBy rdf:resource="https://w3id.org/gcdfo/salmon"/>
        <skos:definition xml:lang="en">Controlled vocabulary for describing the origin of individual salmon (e.g., natural-origin, hatchery-origin, mixed-origin).</skos:definition>
        <skos:hasTopConcept rdf:resource="https://w3id.org/gcdfo/salmon#SalmonOrigin"/>
        <skos:prefLabel xml:lang="en">Salmon Origin Scheme</skos:prefLabel>
        <theme rdf:resource="https://w3id.org/gcdfo/salmon#GeneticsStockCompositionTheme"/>
        <theme rdf:resource="https://w3id.org/gcdfo/salmon#SalmonEnhancementHatcheriesTheme"/>
        <theme rdf:resource="https://w3id.org/gcdfo/salmon#StockAssessmentTheme"/>
    </owl:NamedIndividual>
    


    <!-- https://w3id.org/gcdfo/salmon#SpawnerStageContext -->

    <owl:NamedIndividual rdf:about="https://w3id.org/gcdfo/salmon#SpawnerStageContext">
        <rdf:type rdf:resource="http://www.w3.org/2004/02/skos/core#Concept"/>
        <rdfs:isDefinedBy rdf:resource="https://w3id.org/gcdfo/salmon"/>
        <skos:broader rdf:resource="https://w3id.org/gcdfo/salmon#MeasurementContext"/>
        <skos:definition xml:lang="en">Measurement context indicating values refer to spawners or spawning-stage fish.</skos:definition>
        <skos:inScheme rdf:resource="https://w3id.org/gcdfo/salmon#MeasurementContextScheme"/>
        <skos:prefLabel xml:lang="en">Spawner stage context</skos:prefLabel>
        <theme rdf:resource="https://w3id.org/gcdfo/salmon#StockAssessmentTheme"/>
    </owl:NamedIndividual>
    


    <!-- https://w3id.org/gcdfo/salmon#SpeciesAtRiskRecoveryTheme -->

    <owl:NamedIndividual rdf:about="https://w3id.org/gcdfo/salmon#SpeciesAtRiskRecoveryTheme">
        <rdf:type rdf:resource="http://www.w3.org/2004/02/skos/core#Concept"/>
        <rdfs:isDefinedBy rdf:resource="https://w3id.org/gcdfo/salmon"/>
        <skos:definition xml:lang="en">COSEWIC/SARA recovery planning, critical habitat, threats, and status assessments for species of conservation concern.</skos:definition>
        <skos:inScheme rdf:resource="https://w3id.org/gcdfo/salmon#ThemeScheme"/>
        <skos:prefLabel xml:lang="en">Species at Risk and Recovery</skos:prefLabel>
        <theme rdf:resource="https://w3id.org/gcdfo/salmon#DataModelProvenanceTheme"/>
    </owl:NamedIndividual>
    


    <!-- https://w3id.org/gcdfo/salmon#StockAssessmentTheme -->

    <owl:NamedIndividual rdf:about="https://w3id.org/gcdfo/salmon#StockAssessmentTheme">
        <rdf:type rdf:resource="http://www.w3.org/2004/02/skos/core#Concept"/>
        <rdfs:isDefinedBy rdf:resource="https://w3id.org/gcdfo/salmon"/>
        <skos:definition xml:lang="en">Stock assessment models, benchmarks, status determinations, and performance metrics for salmon units.</skos:definition>
        <skos:inScheme rdf:resource="https://w3id.org/gcdfo/salmon#ThemeScheme"/>
        <skos:prefLabel xml:lang="en">Stock Assessment</skos:prefLabel>
        <theme rdf:resource="https://w3id.org/gcdfo/salmon#DataModelProvenanceTheme"/>
    </owl:NamedIndividual>
    


    <!-- https://w3id.org/gcdfo/salmon#StockStatusZoneScheme -->

    <owl:NamedIndividual rdf:about="https://w3id.org/gcdfo/salmon#StockStatusZoneScheme">
        <rdf:type rdf:resource="http://www.w3.org/2004/02/skos/core#ConceptScheme"/>
        <rdfs:isDefinedBy rdf:resource="https://w3id.org/gcdfo/salmon"/>
        <skos:altLabel xml:lang="en">Stock Status Zone Scheme</skos:altLabel>
        <skos:definition xml:lang="en">Legacy alias scheme for stock status zones. Use :WSPBiologicalStatusZoneScheme as the canonical scheme for Red/Amber/Green Wild Salmon Policy biological status zones.</skos:definition>
        <skos:exactMatch rdf:resource="https://w3id.org/gcdfo/salmon#WSPBiologicalStatusZoneScheme"/>
        <skos:hasTopConcept rdf:resource="https://w3id.org/gcdfo/salmon#WSPBiologicalStatusZone"/>
        <skos:prefLabel xml:lang="en">Stock Status Zone Scheme (legacy alias)</skos:prefLabel>
        <theme rdf:resource="https://w3id.org/gcdfo/salmon#FisheriesManagementTheme"/>
        <theme rdf:resource="https://w3id.org/gcdfo/salmon#StockAssessmentTheme"/>
        <theme rdf:resource="https://w3id.org/gcdfo/salmon#WildSalmonPolicyTheme"/>
    </owl:NamedIndividual>
    


    <!-- https://w3id.org/gcdfo/salmon#SurvivalOrMortalityContext -->

    <owl:NamedIndividual rdf:about="https://w3id.org/gcdfo/salmon#SurvivalOrMortalityContext">
        <rdf:type rdf:resource="http://www.w3.org/2004/02/skos/core#Concept"/>
        <rdfs:isDefinedBy rdf:resource="https://w3id.org/gcdfo/salmon"/>
        <skos:broader rdf:resource="https://w3id.org/gcdfo/salmon#MeasurementContext"/>
        <skos:definition xml:lang="en">Measurement context indicating values represent survival, mortality, or related rates.</skos:definition>
        <skos:inScheme rdf:resource="https://w3id.org/gcdfo/salmon#MeasurementContextScheme"/>
        <skos:prefLabel xml:lang="en">Survival or mortality context</skos:prefLabel>
        <theme rdf:resource="https://w3id.org/gcdfo/salmon#StockAssessmentTheme"/>
    </owl:NamedIndividual>
    


    <!-- https://w3id.org/gcdfo/salmon#TerminalPhase -->

    <owl:NamedIndividual rdf:about="https://w3id.org/gcdfo/salmon#TerminalPhase">
        <rdf:type rdf:resource="http://www.w3.org/2004/02/skos/core#Concept"/>
        <rdfs:isDefinedBy rdf:resource="https://w3id.org/gcdfo/salmon"/>
        <skos:broader rdf:resource="https://w3id.org/gcdfo/salmon#LifePhase"/>
        <skos:definition xml:lang="en">Phase occurring in terminal areas near river mouths or spawning areas (often including terminal fisheries and local migration to spawning sites).</skos:definition>
        <skos:inScheme rdf:resource="https://w3id.org/gcdfo/salmon#LifePhaseScheme"/>
        <skos:prefLabel xml:lang="en">Terminal phase</skos:prefLabel>
        <theme rdf:resource="https://w3id.org/gcdfo/salmon#StockAssessmentTheme"/>
    </owl:NamedIndividual>
    


    <!-- https://w3id.org/gcdfo/salmon#ThemeScheme -->

    <owl:NamedIndividual rdf:about="https://w3id.org/gcdfo/salmon#ThemeScheme">
        <rdf:type rdf:resource="http://www.w3.org/2004/02/skos/core#ConceptScheme"/>
        <rdfs:isDefinedBy rdf:resource="https://w3id.org/gcdfo/salmon"/>
        <skos:definition xml:lang="en">High-level thematic concept scheme for organizing DFO Salmon Ontology classes and concepts.</skos:definition>
        <skos:prefLabel xml:lang="en">Theme Scheme</skos:prefLabel>
        <theme rdf:resource="https://w3id.org/gcdfo/salmon#DataModelProvenanceTheme"/>
    </owl:NamedIndividual>
    


    <!-- https://w3id.org/gcdfo/salmon#Timing -->

    <owl:NamedIndividual rdf:about="https://w3id.org/gcdfo/salmon#Timing">
        <rdf:type rdf:resource="http://www.w3.org/2004/02/skos/core#Concept"/>
        <rdfs:comment xml:lang="en">Limits to Type 3 maximum</rdfs:comment>
        <rdfs:isDefinedBy rdf:resource="https://w3id.org/gcdfo/salmon"/>
        <skos:broader rdf:resource="https://w3id.org/gcdfo/salmon#DowngradeCriteria"/>
        <skos:definition xml:lang="en">Poor timing of surveys</skos:definition>
        <skos:inScheme rdf:resource="https://w3id.org/gcdfo/salmon#DowngradeCriteriaScheme"/>
        <skos:prefLabel xml:lang="en">Timing</skos:prefLabel>
        <theme rdf:resource="https://w3id.org/gcdfo/salmon#DataModelProvenanceTheme"/>
        <theme rdf:resource="https://w3id.org/gcdfo/salmon#StockAssessmentTheme"/>
    </owl:NamedIndividual>
    


    <!-- https://w3id.org/gcdfo/salmon#TotalAgeDimension -->

    <owl:NamedIndividual rdf:about="https://w3id.org/gcdfo/salmon#TotalAgeDimension">
        <rdf:type rdf:resource="http://www.w3.org/2004/02/skos/core#Concept"/>
        <rdfs:isDefinedBy rdf:resource="https://w3id.org/gcdfo/salmon"/>
        <skos:broader rdf:resource="https://w3id.org/gcdfo/salmon#AgeDimension"/>
        <skos:definition xml:lang="en">Age value represents total age in years.</skos:definition>
        <skos:inScheme rdf:resource="https://w3id.org/gcdfo/salmon#AgeDimensionScheme"/>
        <skos:prefLabel xml:lang="en">Total age dimension</skos:prefLabel>
        <theme rdf:resource="https://w3id.org/gcdfo/salmon#StockAssessmentTheme"/>
    </owl:NamedIndividual>
    


    <!-- https://w3id.org/gcdfo/salmon#TrapCount -->

    <owl:NamedIndividual rdf:about="https://w3id.org/gcdfo/salmon#TrapCount">
        <rdf:type rdf:resource="http://www.w3.org/2004/02/skos/core#Concept"/>
        <rdfs:comment xml:lang="en">Legacy methods: Trap, Hatchery Passage Counting</rdfs:comment>
        <rdfs:isDefinedBy rdf:resource="https://w3id.org/gcdfo/salmon"/>
        <skos:broader rdf:resource="https://w3id.org/gcdfo/salmon#EnumerationMethod"/>
        <skos:definition xml:lang="en">Trap-based counts from non-spanning traps with documented emptying schedule, efficiency measurements, and coverage information.</skos:definition>
        <skos:inScheme rdf:resource="https://w3id.org/gcdfo/salmon#EnumerationMethodScheme"/>
        <skos:prefLabel xml:lang="en">Trap Count</skos:prefLabel>
        <theme rdf:resource="https://w3id.org/gcdfo/salmon#MonitoringFieldWorkTheme"/>
        <theme rdf:resource="https://w3id.org/gcdfo/salmon#StockAssessmentTheme"/>
    </owl:NamedIndividual>
    


    <!-- https://w3id.org/gcdfo/salmon#TrapEfficiency -->

    <owl:NamedIndividual rdf:about="https://w3id.org/gcdfo/salmon#TrapEfficiency">
        <rdf:type rdf:resource="http://www.w3.org/2004/02/skos/core#Concept"/>
        <rdfs:comment xml:lang="en">Limits to Type 3 maximum</rdfs:comment>
        <rdfs:isDefinedBy rdf:resource="https://w3id.org/gcdfo/salmon"/>
        <skos:broader rdf:resource="https://w3id.org/gcdfo/salmon#DowngradeCriteria"/>
        <skos:definition xml:lang="en">Trap efficiency not measured/validated</skos:definition>
        <skos:inScheme rdf:resource="https://w3id.org/gcdfo/salmon#DowngradeCriteriaScheme"/>
        <skos:prefLabel xml:lang="en">Trap Efficiency</skos:prefLabel>
        <theme rdf:resource="https://w3id.org/gcdfo/salmon#DataModelProvenanceTheme"/>
        <theme rdf:resource="https://w3id.org/gcdfo/salmon#StockAssessmentTheme"/>
    </owl:NamedIndividual>
    


    <!-- https://w3id.org/gcdfo/salmon#TrapModelAnalysis -->

    <owl:NamedIndividual rdf:about="https://w3id.org/gcdfo/salmon#TrapModelAnalysis">
        <rdf:type rdf:resource="http://www.w3.org/2004/02/skos/core#Concept"/>
        <rdfs:comment xml:lang="en">Requires documented trap efficiency measurements and cross-section coverage factors.</rdfs:comment>
        <rdfs:isDefinedBy rdf:resource="https://w3id.org/gcdfo/salmon"/>
        <skos:broader rdf:resource="https://w3id.org/gcdfo/salmon#EstimateMethod"/>
        <skos:definition xml:lang="en">Trap-based counts adjusted with efficiency/coverage models to estimate total passage.</skos:definition>
        <skos:inScheme rdf:resource="https://w3id.org/gcdfo/salmon#EstimateMethodScheme"/>
        <skos:prefLabel xml:lang="en">Trap Model Analysis</skos:prefLabel>
        <theme rdf:resource="https://w3id.org/gcdfo/salmon#MonitoringFieldWorkTheme"/>
        <theme rdf:resource="https://w3id.org/gcdfo/salmon#StockAssessmentTheme"/>
    </owl:NamedIndividual>
    


    <!-- https://w3id.org/gcdfo/salmon#Type1 -->

    <owl:NamedIndividual rdf:about="https://w3id.org/gcdfo/salmon#Type1">
        <rdf:type rdf:resource="http://www.w3.org/2004/02/skos/core#Concept"/>
        <rdfs:isDefinedBy rdf:resource="https://w3id.org/gcdfo/salmon"/>
        <skos:broader rdf:resource="https://w3id.org/gcdfo/salmon#EstimateType"/>
        <skos:definition xml:lang="en">Total, seasonal counts through fence or fishway; virtually no bypass. Simple, often single step analysis. Reliable resolution of between year differences &gt;10% (in absolute units).</skos:definition>
        <skos:inScheme rdf:resource="https://w3id.org/gcdfo/salmon#EstimateTypeScheme"/>
        <skos:prefLabel xml:lang="en">Type-1, True Abundance, high resolution</skos:prefLabel>
        <theme rdf:resource="https://w3id.org/gcdfo/salmon#DataModelProvenanceTheme"/>
        <theme rdf:resource="https://w3id.org/gcdfo/salmon#StockAssessmentTheme"/>
    </owl:NamedIndividual>
    


    <!-- https://w3id.org/gcdfo/salmon#Type2 -->

    <owl:NamedIndividual rdf:about="https://w3id.org/gcdfo/salmon#Type2">
        <rdf:type rdf:resource="http://www.w3.org/2004/02/skos/core#Concept"/>
        <rdfs:isDefinedBy rdf:resource="https://w3id.org/gcdfo/salmon"/>
        <skos:broader rdf:resource="https://w3id.org/gcdfo/salmon#EstimateType"/>
        <skos:definition xml:lang="en">Indirect estimate of total spawner abundance with qualified accuracy and known precision (i.e., a variance estimate—an explicit quantitative measure of uncertainty around the estimate). Derived from high-effort, standardized methods (e.g., mark-recapture, serial counts for area under the curve) with documented analytical conversions (including interpolation/calibration as needed). Reported in absolute units (estimate ± variance). Reliable resolution of between-year differences &gt;25% (in absolute units).</skos:definition>
        <skos:inScheme rdf:resource="https://w3id.org/gcdfo/salmon#EstimateTypeScheme"/>
        <skos:prefLabel xml:lang="en">Type-2, True Abundance, medium resolution</skos:prefLabel>
        <theme rdf:resource="https://w3id.org/gcdfo/salmon#DataModelProvenanceTheme"/>
        <theme rdf:resource="https://w3id.org/gcdfo/salmon#StockAssessmentTheme"/>
    </owl:NamedIndividual>
    


    <!-- https://w3id.org/gcdfo/salmon#Type3 -->

    <owl:NamedIndividual rdf:about="https://w3id.org/gcdfo/salmon#Type3">
        <rdf:type rdf:resource="http://www.w3.org/2004/02/skos/core#Concept"/>
        <rdfs:isDefinedBy rdf:resource="https://w3id.org/gcdfo/salmon"/>
        <skos:broader rdf:resource="https://w3id.org/gcdfo/salmon#EstimateType"/>
        <skos:definition xml:lang="en">Relative abundance index (i.e., not an absolute count) derived from moderate to high effort surveys (typically 3 or more site visits) using standardized methods applied consistently between and within years (e.g., equal-effort surveys executed by walk, swim, overflight). Accuracy and precision are not fully quantified (i.e., no explicit variance estimate), but are assumed stable enough for within-series comparisons. Reliable resolution of between-year differences &gt;25% (in relative units).</skos:definition>
        <skos:inScheme rdf:resource="https://w3id.org/gcdfo/salmon#EstimateTypeScheme"/>
        <skos:prefLabel xml:lang="en">Type-3, Relative Abundance, high resolution</skos:prefLabel>
        <theme rdf:resource="https://w3id.org/gcdfo/salmon#DataModelProvenanceTheme"/>
        <theme rdf:resource="https://w3id.org/gcdfo/salmon#StockAssessmentTheme"/>
    </owl:NamedIndividual>
    


    <!-- https://w3id.org/gcdfo/salmon#Type4 -->

    <owl:NamedIndividual rdf:about="https://w3id.org/gcdfo/salmon#Type4">
        <rdf:type rdf:resource="http://www.w3.org/2004/02/skos/core#Concept"/>
        <rdfs:isDefinedBy rdf:resource="https://w3id.org/gcdfo/salmon"/>
        <skos:broader rdf:resource="https://w3id.org/gcdfo/salmon#EstimateType"/>
        <skos:definition xml:lang="en">Low to moderate effort (1-4 trips), known survey method. Simple analysis by known methods. Reliable resolution of between year differences &gt;200% (in relative units).</skos:definition>
        <skos:inScheme rdf:resource="https://w3id.org/gcdfo/salmon#EstimateTypeScheme"/>
        <skos:prefLabel xml:lang="en">Type-4, Relative Abundance, medium resolution</skos:prefLabel>
        <theme rdf:resource="https://w3id.org/gcdfo/salmon#DataModelProvenanceTheme"/>
        <theme rdf:resource="https://w3id.org/gcdfo/salmon#StockAssessmentTheme"/>
    </owl:NamedIndividual>
    


    <!-- https://w3id.org/gcdfo/salmon#Type5 -->

    <owl:NamedIndividual rdf:about="https://w3id.org/gcdfo/salmon#Type5">
        <rdf:type rdf:resource="http://www.w3.org/2004/02/skos/core#Concept"/>
        <rdfs:isDefinedBy rdf:resource="https://w3id.org/gcdfo/salmon"/>
        <skos:broader rdf:resource="https://w3id.org/gcdfo/salmon#EstimateType"/>
        <skos:definition xml:lang="en">Low effort (e.g. 1 trip), use of vaguely defined, inconsistent or poorly executed methods. Unknown to ill defined; inconsistent or poorly executed. Uncertain numeric comparisons, but high reliability for presence or absence.</skos:definition>
        <skos:inScheme rdf:resource="https://w3id.org/gcdfo/salmon#EstimateTypeScheme"/>
        <skos:prefLabel xml:lang="en">Type-5, Relative Abundance, low resolution</skos:prefLabel>
        <theme rdf:resource="https://w3id.org/gcdfo/salmon#DataModelProvenanceTheme"/>
        <theme rdf:resource="https://w3id.org/gcdfo/salmon#StockAssessmentTheme"/>
    </owl:NamedIndividual>
    


    <!-- https://w3id.org/gcdfo/salmon#Type6 -->

    <owl:NamedIndividual rdf:about="https://w3id.org/gcdfo/salmon#Type6">
        <rdf:type rdf:resource="http://www.w3.org/2004/02/skos/core#Concept"/>
        <rdfs:isDefinedBy rdf:resource="https://w3id.org/gcdfo/salmon"/>
        <skos:altLabel xml:lang="en">Presence/Not Detected</skos:altLabel>
        <skos:broader rdf:resource="https://w3id.org/gcdfo/salmon#EstimateType"/>
        <skos:definition xml:lang="en">Non-numeric, year-specific record of presence/not detected (i.e., present/absent without estimating a count), tied to an explicit time and location, with reliable species identification. Underlying field methods may be highly variable; analysis is not required.</skos:definition>
        <skos:inScheme rdf:resource="https://w3id.org/gcdfo/salmon#EstimateTypeScheme"/>
        <skos:prefLabel xml:lang="en">Type-6, Presence or Absence</skos:prefLabel>
        <theme rdf:resource="https://w3id.org/gcdfo/salmon#DataModelProvenanceTheme"/>
        <theme rdf:resource="https://w3id.org/gcdfo/salmon#StockAssessmentTheme"/>
    </owl:NamedIndividual>
    


    <!-- https://w3id.org/gcdfo/salmon#UnrankedIndexQuality -->

    <owl:NamedIndividual rdf:about="https://w3id.org/gcdfo/salmon#UnrankedIndexQuality">
        <rdf:type rdf:resource="http://www.w3.org/2004/02/skos/core#Concept"/>
        <obo:IAO_0000115 xml:lang="en">A data quality category indicating that no spawner-abundance estimate classification / index quality rating was assigned for the record (i.e., an &apos;Unknown&apos; estimate classification with no quality rating).</obo:IAO_0000115>
        <obo:IAO_0000119 xml:lang="en">Fisheries and Oceans Canada. 2020. 2020 summary of abundance data for Chinook salmon (Oncorhynchus tshawytscha) in southern British Columbia, Canada (nuSEDS Estimate Classification includes &apos;Unknown: no quality rating&apos;).</obo:IAO_0000119>
        <dcterms:source rdf:resource="https://waves-vagues.dfo-mpo.gc.ca/Library/40890041.pdf"/>
        <rdfs:isDefinedBy rdf:resource="https://w3id.org/gcdfo/salmon"/>
        <skos:broader rdf:resource="https://w3id.org/gcdfo/salmon#EstimateType"/>
        <skos:definition xml:lang="en">A data quality category indicating that no spawner-abundance estimate classification / index quality rating was assigned for the record (i.e., an &apos;Unknown&apos; estimate classification with no quality rating).</skos:definition>
        <skos:inScheme rdf:resource="https://w3id.org/gcdfo/salmon#EstimateTypeScheme"/>
        <skos:prefLabel xml:lang="en">Unranked index quality</skos:prefLabel>
        <theme rdf:resource="https://w3id.org/gcdfo/salmon#DataModelProvenanceTheme"/>
        <theme rdf:resource="https://w3id.org/gcdfo/salmon#StockAssessmentTheme"/>
    </owl:NamedIndividual>
    


    <!-- https://w3id.org/gcdfo/salmon#UpperBenchmark -->

    <owl:NamedIndividual rdf:about="https://w3id.org/gcdfo/salmon#UpperBenchmark">
        <rdf:type rdf:resource="http://www.w3.org/2004/02/skos/core#Concept"/>
        <rdfs:isDefinedBy rdf:resource="https://w3id.org/gcdfo/salmon"/>
        <skos:definition xml:lang="en">An upper-threshold benchmark value, typically delineating the boundary between Amber and Green status zones.</skos:definition>
        <skos:inScheme rdf:resource="https://w3id.org/gcdfo/salmon#BenchmarkLevelScheme"/>
        <skos:prefLabel xml:lang="en">Upper benchmark</skos:prefLabel>
        <theme rdf:resource="https://w3id.org/gcdfo/salmon#StockAssessmentTheme"/>
        <theme rdf:resource="https://w3id.org/gcdfo/salmon#WildSalmonPolicyTheme"/>
    </owl:NamedIndividual>
    


    <!-- https://w3id.org/gcdfo/salmon#Uptime -->

    <owl:NamedIndividual rdf:about="https://w3id.org/gcdfo/salmon#Uptime">
        <rdf:type rdf:resource="http://www.w3.org/2004/02/skos/core#Concept"/>
        <rdfs:comment xml:lang="en">Limits to Type 2 maximum</rdfs:comment>
        <rdfs:isDefinedBy rdf:resource="https://w3id.org/gcdfo/salmon"/>
        <skos:broader rdf:resource="https://w3id.org/gcdfo/salmon#DowngradeCriteria"/>
        <skos:definition xml:lang="en">Counting/device uptime &lt; 95% (or &lt;90% with interpolation)</skos:definition>
        <skos:inScheme rdf:resource="https://w3id.org/gcdfo/salmon#DowngradeCriteriaScheme"/>
        <skos:prefLabel xml:lang="en">Uptime</skos:prefLabel>
        <theme rdf:resource="https://w3id.org/gcdfo/salmon#DataModelProvenanceTheme"/>
        <theme rdf:resource="https://w3id.org/gcdfo/salmon#StockAssessmentTheme"/>
    </owl:NamedIndividual>
    


    <!-- https://w3id.org/gcdfo/salmon#Visibility -->

    <owl:NamedIndividual rdf:about="https://w3id.org/gcdfo/salmon#Visibility">
        <rdf:type rdf:resource="http://www.w3.org/2004/02/skos/core#Concept"/>
        <rdfs:comment xml:lang="en">Limits to Type 3 maximum</rdfs:comment>
        <rdfs:isDefinedBy rdf:resource="https://w3id.org/gcdfo/salmon"/>
        <skos:broader rdf:resource="https://w3id.org/gcdfo/salmon#DowngradeCriteria"/>
        <skos:definition xml:lang="en">Poor visibility conditions</skos:definition>
        <skos:inScheme rdf:resource="https://w3id.org/gcdfo/salmon#DowngradeCriteriaScheme"/>
        <skos:prefLabel xml:lang="en">Visibility</skos:prefLabel>
        <theme rdf:resource="https://w3id.org/gcdfo/salmon#DataModelProvenanceTheme"/>
        <theme rdf:resource="https://w3id.org/gcdfo/salmon#StockAssessmentTheme"/>
    </owl:NamedIndividual>
    


    <!-- https://w3id.org/gcdfo/salmon#VisualGroundCount -->

    <owl:NamedIndividual rdf:about="https://w3id.org/gcdfo/salmon#VisualGroundCount">
        <rdf:type rdf:resource="http://www.w3.org/2004/02/skos/core#Concept"/>
        <rdfs:comment xml:lang="en">Legacy methods: Stream Walk, Ground count, Bank Walk</rdfs:comment>
        <rdfs:isDefinedBy rdf:resource="https://w3id.org/gcdfo/salmon"/>
        <skos:broader rdf:resource="https://w3id.org/gcdfo/salmon#EnumerationMethod"/>
        <skos:definition xml:lang="en">Visual surveys conducted by stream/bank walk with documented visit schedule, reach coverage, timing, and visibility conditions.</skos:definition>
        <skos:inScheme rdf:resource="https://w3id.org/gcdfo/salmon#EnumerationMethodScheme"/>
        <skos:prefLabel xml:lang="en">Visual Ground Count</skos:prefLabel>
        <theme rdf:resource="https://w3id.org/gcdfo/salmon#MonitoringFieldWorkTheme"/>
        <theme rdf:resource="https://w3id.org/gcdfo/salmon#StockAssessmentTheme"/>
    </owl:NamedIndividual>
    


    <!-- https://w3id.org/gcdfo/salmon#VisualSnorkelCount -->

    <owl:NamedIndividual rdf:about="https://w3id.org/gcdfo/salmon#VisualSnorkelCount">
        <rdf:type rdf:resource="http://www.w3.org/2004/02/skos/core#Concept"/>
        <rdfs:comment xml:lang="en">Legacy methods: Snorkel, Snorkel Swim</rdfs:comment>
        <rdfs:isDefinedBy rdf:resource="https://w3id.org/gcdfo/salmon"/>
        <skos:broader rdf:resource="https://w3id.org/gcdfo/salmon#EnumerationMethod"/>
        <skos:definition xml:lang="en">Two or more trained snorkelers conduct standardized passes within defined segments, tallying live/dead by species. Field forms capture visibility class, segment boundaries, and repeat-visit schedule; counts are aggregated across observers/passes.</skos:definition>
        <skos:inScheme rdf:resource="https://w3id.org/gcdfo/salmon#EnumerationMethodScheme"/>
        <skos:prefLabel xml:lang="en">Visual Snorkel Count</skos:prefLabel>
        <theme rdf:resource="https://w3id.org/gcdfo/salmon#MonitoringFieldWorkTheme"/>
        <theme rdf:resource="https://w3id.org/gcdfo/salmon#StockAssessmentTheme"/>
    </owl:NamedIndividual>
    


    <!-- https://w3id.org/gcdfo/salmon#WSPBiologicalStatusZone -->

    <owl:NamedIndividual rdf:about="https://w3id.org/gcdfo/salmon#WSPBiologicalStatusZone">
        <rdf:type rdf:resource="http://www.w3.org/2004/02/skos/core#Concept"/>
    </owl:NamedIndividual>
    


    <!-- https://w3id.org/gcdfo/salmon#WSPBiologicalStatusZoneScheme -->

    <owl:NamedIndividual rdf:about="https://w3id.org/gcdfo/salmon#WSPBiologicalStatusZoneScheme">
        <rdf:type rdf:resource="http://www.w3.org/2004/02/skos/core#ConceptScheme"/>
        <rdfs:isDefinedBy rdf:resource="https://w3id.org/gcdfo/salmon"/>
        <skos:definition xml:lang="en">Controlled vocabulary for biological status zones under the Wild Salmon Policy.</skos:definition>
        <skos:hasTopConcept rdf:resource="https://w3id.org/gcdfo/salmon#WSPBiologicalStatusZone"/>
        <skos:prefLabel xml:lang="en">Wild Salmon Policy Status Zone</skos:prefLabel>
        <theme rdf:resource="https://w3id.org/gcdfo/salmon#PolicyGovernanceTheme"/>
        <theme rdf:resource="https://w3id.org/gcdfo/salmon#StockAssessmentTheme"/>
        <theme rdf:resource="https://w3id.org/gcdfo/salmon#WildSalmonPolicyTheme"/>
    </owl:NamedIndividual>
    


    <!-- https://w3id.org/gcdfo/salmon#WildSalmonPolicy -->

    <owl:NamedIndividual rdf:about="https://w3id.org/gcdfo/salmon#WildSalmonPolicy">
        <rdf:type rdf:resource="http://www.w3.org/2004/02/skos/core#Concept"/>
        <rdfs:isDefinedBy rdf:resource="https://w3id.org/gcdfo/salmon"/>
        <skos:altLabel xml:lang="en">WSP</skos:altLabel>
        <skos:broader rdf:resource="https://w3id.org/gcdfo/salmon#PolicyFramework"/>
        <skos:definition xml:lang="en">Canada&apos;s Wild Salmon Policy framework for conserving and managing wild Pacific salmon, including integrated status assessments and biological benchmarks for Conservation Units.</skos:definition>
        <skos:inScheme rdf:resource="https://w3id.org/gcdfo/salmon#PolicyFrameworkScheme"/>
        <skos:prefLabel xml:lang="en">Wild Salmon Policy</skos:prefLabel>
        <theme rdf:resource="https://w3id.org/gcdfo/salmon#PolicyGovernanceTheme"/>
        <theme rdf:resource="https://w3id.org/gcdfo/salmon#StockAssessmentTheme"/>
        <theme rdf:resource="https://w3id.org/gcdfo/salmon#WildSalmonPolicyTheme"/>
    </owl:NamedIndividual>
    


    <!-- https://w3id.org/gcdfo/salmon#WildSalmonPolicyTheme -->

    <owl:NamedIndividual rdf:about="https://w3id.org/gcdfo/salmon#WildSalmonPolicyTheme">
        <rdf:type rdf:resource="http://www.w3.org/2004/02/skos/core#Concept"/>
        <rdfs:isDefinedBy rdf:resource="https://w3id.org/gcdfo/salmon"/>
        <skos:definition xml:lang="en">Conservation Unit based stock assessment methods, metrics, and metadata</skos:definition>
        <skos:inScheme rdf:resource="https://w3id.org/gcdfo/salmon#ThemeScheme"/>
        <skos:prefLabel xml:lang="en">Wild Salmon Policy</skos:prefLabel>
        <theme rdf:resource="https://w3id.org/gcdfo/salmon#DataModelProvenanceTheme"/>
    </owl:NamedIndividual>
    


    <!-- 
    ///////////////////////////////////////////////////////////////////////////////////////
    //
    // Annotations
    //
    ///////////////////////////////////////////////////////////////////////////////////////
     -->

    <rdf:Description rdf:about="https://w3id.org/gcdfo/salmon#ConfidenceCategory">
        <rdfs:isDefinedBy rdf:resource="https://w3id.org/gcdfo/salmon"/>
        <skos:definition xml:lang="en">Categorical confidence rating (High, Medium, Low) for stock assessment metrics.</skos:definition>
        <skos:inScheme rdf:resource="https://w3id.org/gcdfo/salmon#RapidStatusConfidenceScheme"/>
        <skos:prefLabel xml:lang="en">Confidence category</skos:prefLabel>
        <theme rdf:resource="https://w3id.org/gcdfo/salmon#StockAssessmentTheme"/>
        <theme rdf:resource="https://w3id.org/gcdfo/salmon#WildSalmonPolicyTheme"/>
    </rdf:Description>
    <rdf:Description rdf:about="https://w3id.org/gcdfo/salmon#WSPBiologicalStatusZone">
        <obo:IAO_0000119 xml:lang="en">Fisheries and Oceans Canada. Wild Salmon Policy 2018-2022 Implementation Plan. https://waves-vagues.dfo-mpo.gc.ca/library-bibliotheque/40728109.pdf.</obo:IAO_0000119>
        <dcterms:source rdf:resource="https://waves-vagues.dfo-mpo.gc.ca/library-bibliotheque/40728109.pdf"/>
        <rdfs:isDefinedBy rdf:resource="https://w3id.org/gcdfo/salmon"/>
        <skos:definition xml:lang="en">The biological status of a Conservation Unit (CU) will normally be based on the abundance and distribution of spawners in the unit, or proxies thereof. For each CU, higher and lower benchmarks will be defined that will delimit three status zones: Green, Amber, and Red. As spawner abundance decreases, a CU moves towards the lower status zone, and the extent of management intervention for conservation purposes will increase.</skos:definition>
        <skos:inScheme rdf:resource="https://w3id.org/gcdfo/salmon#WSPBiologicalStatusZoneScheme"/>
        <skos:prefLabel xml:lang="en">Wild Salmon Policy biological status zone</skos:prefLabel>
        <theme rdf:resource="https://w3id.org/gcdfo/salmon#PolicyGovernanceTheme"/>
        <theme rdf:resource="https://w3id.org/gcdfo/salmon#StockAssessmentTheme"/>
        <theme rdf:resource="https://w3id.org/gcdfo/salmon#WildSalmonPolicyTheme"/>
    </rdf:Description>
</rdf:RDF>



<!-- Generated by the OWL API (version 4.5.29) https://github.com/owlcs/owlapi -->

